<?xml version="1.0"?>
<rdf:RDF xmlns="https://dataforhistory.org/ontology/maritimehistorycontinued#"
     xml:base="https://dataforhistory.org/ontology/maritimehistorycontinued"
     xmlns:owl="http://www.w3.org/2002/07/owl#"
     xmlns:rdf="http://www.w3.org/1999/02/22-rdf-syntax-ns#"
     xmlns:xml="http://www.w3.org/XML/1998/namespace"
     xmlns:xsd="http://www.w3.org/2001/XMLSchema#"
     xmlns:rdfs="http://www.w3.org/2000/01/rdf-schema#"
     xmlns:skos="http://www.w3.org/2004/02/skos/core#">
    <owl:Ontology rdf:about="https://dataforhistory.org/ontology/maritimehistorycontinued">
        <rdfs:comment xml:lang="en">CIDOC CRM version 6.2
Closed version - May 2015.</rdfs:comment>
        <rdfs:comment xml:lang="en">Classes and properties in this namespace extend HistDMI and the CIDOC CRM class types for integrating data about social interactions.
This namespace is ongoing and can be modified at any time.</rdfs:comment>
        <rdfs:comment xml:lang="en">Classes and properties used to model the field of maritime history.</rdfs:comment>
        <rdfs:comment xml:lang="en">This is an extension of the CIDOC CRM extension that integrates high-level classes and properties generally needed in historical research. The general epistemological foundations of this ontology are presented in the description of the root namespace. </rdfs:comment>
        <rdfs:label xml:lang="en">CIDOC CRM Top-Level Extension for Humanities and Social sciences (SDHSS)  – ongoing</rdfs:label>
        <rdfs:label xml:lang="en">CIDOC CRM version 6.2</rdfs:label>
        <rdfs:label xml:lang="en">Maritime history ongoing</rdfs:label>
        <rdfs:label xml:lang="en">Social, legal and economic life (SDHSS) ongoing</rdfs:label>
        <owl:versionInfo rdf:datatype="http://www.w3.org/2001/XMLSchema#string">Exported from OntoME: CIDOC CRM Top-Level Extension for Humanities and Social sciences (SDHSS)  – ongoing</owl:versionInfo>
        <owl:versionInfo rdf:datatype="http://www.w3.org/2001/XMLSchema#string">Exported from OntoME: CIDOC CRM version 6.2</owl:versionInfo>
        <owl:versionInfo rdf:datatype="http://www.w3.org/2001/XMLSchema#string">Exported from OntoME: Maritime history ongoing</owl:versionInfo>
        <owl:versionInfo rdf:datatype="http://www.w3.org/2001/XMLSchema#string">Exported from OntoME: Social, legal and economic life (SDHSS) ongoing</owl:versionInfo>
    </owl:Ontology>
    


    <!-- 
    ///////////////////////////////////////////////////////////////////////////////////////
    //
    // Annotation properties
    //
    ///////////////////////////////////////////////////////////////////////////////////////
     -->

    


    <!-- http://www.w3.org/2004/02/skos/core#notation -->

    <owl:AnnotationProperty rdf:about="http://www.w3.org/2004/02/skos/core#notation"/>
    


    <!-- 
    ///////////////////////////////////////////////////////////////////////////////////////
    //
    // Object Properties
    //
    ///////////////////////////////////////////////////////////////////////////////////////
     -->

    


    <!-- http://dataforhistory.org/histdmi-generic-ongoing/property/P10 -->

    <owl:ObjectProperty rdf:about="http://dataforhistory.org/histdmi-generic-ongoing/property/P10">
        <rdfs:domain rdf:resource="http://www.cidoc-crm.org/cidoc-crm/E1"/>
        <rdfs:range rdf:resource="http://www.cidoc-crm.org/cidoc-crm/E1"/>
        <rdfs:comment xml:lang="en">This high level property is parent or ancestor of all properties that are not time-indexed, i.e. not determined by a variable representing time. These relationships exist as such, in a categorical way and independently from the time flow.
All time-indexed properties should be expressed as a Temporal Entity – E2 using childs or descendants of the  involves – histP1 property for associating Per instances participating in or related to the temporal entity.
 </rdfs:comment>
        <rdfs:label xml:lang="en">time-independent entity association</rdfs:label>
        <skos:notation rdf:datatype="http://www.w3.org/2001/XMLSchema#string">P10</skos:notation>
    </owl:ObjectProperty>
    


    <!-- http://dataforhistory.org/histdmi-generic-ongoing/property/P11 -->

    <owl:ObjectProperty rdf:about="http://dataforhistory.org/histdmi-generic-ongoing/property/P11">
        <rdfs:domain rdf:resource="http://dataforhistory.org/histdmi-generic-ongoing/class/C11"/>
        <rdfs:range rdf:resource="http://www.cidoc-crm.org/cidoc-crm/E1"/>
        <rdfs:comment xml:lang="en">This property associates the Appelation for language to the E1 CRM Entity that it identifies.</rdfs:comment>
        <rdfs:label xml:lang="en">is appellation for language of</rdfs:label>
        <skos:notation rdf:datatype="http://www.w3.org/2001/XMLSchema#string">P11</skos:notation>
    </owl:ObjectProperty>
    


    <!-- http://dataforhistory.org/histdmi-generic-ongoing/property/P12 -->

    <owl:ObjectProperty rdf:about="http://dataforhistory.org/histdmi-generic-ongoing/property/P12">
        <rdfs:domain rdf:resource="http://dataforhistory.org/histdmi-generic-ongoing/class/C11"/>
        <rdfs:range rdf:resource="http://www.cidoc-crm.org/cidoc-crm/E56"/>
        <rdfs:comment xml:lang="en">This property associates the language for which the appellation is a valid identifier of an entity for a given time span</rdfs:comment>
        <rdfs:label xml:lang="en">used in language</rdfs:label>
        <skos:notation rdf:datatype="http://www.w3.org/2001/XMLSchema#string">P12</skos:notation>
    </owl:ObjectProperty>
    


    <!-- http://dataforhistory.org/histdmi-generic-ongoing/property/P13 -->

    <owl:ObjectProperty rdf:about="http://dataforhistory.org/histdmi-generic-ongoing/property/P13">
        <rdfs:domain rdf:resource="http://dataforhistory.org/histdmi-generic-ongoing/class/C11"/>
        <rdfs:range rdf:resource="http://www.cidoc-crm.org/cidoc-crm/E41"/>
        <rdfs:comment xml:lang="en">This property associates the Appelation for language to the E41 Appelation that refers to it.</rdfs:comment>
        <rdfs:label xml:lang="en">refers to name</rdfs:label>
        <skos:notation rdf:datatype="http://www.w3.org/2001/XMLSchema#string">P13</skos:notation>
    </owl:ObjectProperty>
    


    <!-- http://dataforhistory.org/histdmi-generic-ongoing/property/P14 -->

    <owl:ObjectProperty rdf:about="http://dataforhistory.org/histdmi-generic-ongoing/property/P14">
        <rdfs:domain rdf:resource="http://dataforhistory.org/histdmi-generic-ongoing/class/C11"/>
        <rdfs:range rdf:resource="http://dataforhistory.org/histdmi-generic-ongoing/class/C12"/>
        <rdfs:comment xml:lang="en">Associates Appellation for language – histC10 with the type which defines its identity</rdfs:comment>
        <rdfs:label xml:lang="en">has appellation for language type</rdfs:label>
        <skos:notation rdf:datatype="http://www.w3.org/2001/XMLSchema#string">P14</skos:notation>
    </owl:ObjectProperty>
    


    <!-- http://dataforhistory.org/histdmi-generic-ongoing/property/P15 -->

    <owl:ObjectProperty rdf:about="http://dataforhistory.org/histdmi-generic-ongoing/property/P15">
        <rdfs:domain rdf:resource="http://dataforhistory.org/histdmi-generic-ongoing/class/C15"/>
        <rdfs:range rdf:resource="http://dataforhistory.org/histdmi-generic-ongoing/class/C13"/>
        <rdfs:comment xml:lang="en">This property associates the C15 Geographical location with the C13 Geographical place related to it.</rdfs:comment>
        <rdfs:label xml:lang="en">was relative to</rdfs:label>
        <skos:notation rdf:datatype="http://www.w3.org/2001/XMLSchema#string">P15</skos:notation>
    </owl:ObjectProperty>
    


    <!-- http://dataforhistory.org/histdmi-generic-ongoing/property/P16 -->

    <owl:ObjectProperty rdf:about="http://dataforhistory.org/histdmi-generic-ongoing/property/P16">
        <rdfs:domain rdf:resource="http://dataforhistory.org/histdmi-generic-ongoing/class/C15"/>
        <rdfs:range rdf:resource="http://www.cidoc-crm.org/cidoc-crm/E54"/>
        <rdfs:comment xml:lang="en">This property is used to provide the value of the distance between the located object and the reference geographical place</rdfs:comment>
        <rdfs:label xml:lang="en">at distance</rdfs:label>
        <skos:notation rdf:datatype="http://www.w3.org/2001/XMLSchema#string">P16</skos:notation>
    </owl:ObjectProperty>
    


    <!-- http://dataforhistory.org/histdmi-generic-ongoing/property/P17 -->

    <owl:ObjectProperty rdf:about="http://dataforhistory.org/histdmi-generic-ongoing/property/P17">
        <rdfs:domain rdf:resource="http://dataforhistory.org/histdmi-generic-ongoing/class/C15"/>
        <rdfs:range rdf:resource="http://www.cidoc-crm.org/cidoc-crm/E77"/>
        <rdfs:comment xml:lang="en">This property identifies a E77 Persistent Item localized at some place during the given time span of a C15 Geographical Location.</rdfs:comment>
        <rdfs:label xml:lang="en">was location of</rdfs:label>
        <skos:notation rdf:datatype="http://www.w3.org/2001/XMLSchema#string">P17</skos:notation>
    </owl:ObjectProperty>
    


    <!-- http://dataforhistory.org/histdmi-generic-ongoing/property/P18 -->

    <owl:ObjectProperty rdf:about="http://dataforhistory.org/histdmi-generic-ongoing/property/P18">
        <rdfs:domain rdf:resource="http://www.cidoc-crm.org/cidoc-crm/E1"/>
        <rdfs:range rdf:resource="http://www.cidoc-crm.org/cidoc-crm/E1"/>
        <rdfs:comment xml:lang="en">This is an abstract property – do not use it in profiles !
As a high level meta-property the present property expresses the fact that the domain class is an identity defining component of the range class. This means that the identity of the range class instance depends on the associated domain class instance and no alternative instances are allowed for this property against the general rule of CIDOC CRM.
This property is used to characterize subproperties of it. It should be replaced by a property of property associating the concerned property with the boolean value True/False.</rdfs:comment>
        <rdfs:label xml:lang="en">is identifying component of range class</rdfs:label>
        <skos:notation rdf:datatype="http://www.w3.org/2001/XMLSchema#string">P18</skos:notation>
    </owl:ObjectProperty>
    


    <!-- http://dataforhistory.org/histdmi-generic-ongoing/property/P19 -->

    <owl:ObjectProperty rdf:about="http://dataforhistory.org/histdmi-generic-ongoing/property/P19">
        <rdfs:domain rdf:resource="http://dataforhistory.org/histdmi-generic-ongoing/class/C15"/>
        <rdfs:range rdf:resource="http://dataforhistory.org/histdmi-generic-ongoing/class/C16"/>
        <rdfs:comment xml:lang="en">Associates a geographical localisation with the type which defines its identity</rdfs:comment>
        <rdfs:label xml:lang="en">has location type</rdfs:label>
        <skos:notation rdf:datatype="http://www.w3.org/2001/XMLSchema#string">P19</skos:notation>
    </owl:ObjectProperty>
    


    <!-- http://dataforhistory.org/histdmi-generic-ongoing/property/P2 -->

    <owl:ObjectProperty rdf:about="http://dataforhistory.org/histdmi-generic-ongoing/property/P2">
        <rdfs:domain rdf:resource="http://www.cidoc-crm.org/cidoc-crm/E1"/>
        <rdfs:range rdf:resource="http://www.cidoc-crm.org/cidoc-crm/E1"/>
        <rdfs:comment xml:lang="en">This is an abstract property – do not use it in profiles !
As a high level meta-property the present property expresses the fact that the range class is an identity defining component of the domain class This means that the identity of the domain class instance depends on the associated range class instance and no alternative instances are allowed for this property against the general rule of CIDOC CRM.
E.g. in the case of a Birth – E67 there can be no discussion about the person which is P98 brought into life by a specific instance of a birth. A specific instance of a birth is always related to just one person (or a limited range of persons in the case of twins, triplets, etc.). A discussion (and therefore production of alternative property instances) can take place concerning the P97 from father  property or the birth place, but never about the P98 brought into life property. This is necessary to allow data consistency in an information system and avoid considering e.g. the same birth instance as the birth of five different people which makes discussion impossible about the mother, father or birth place of one specific person.
This property has no direct instances but is used to specify the role of the instanciated subproperties as identifying properties for the domain temporal entity.</rdfs:comment>
        <rdfs:label xml:lang="en">domain class has identity defining component</rdfs:label>
        <skos:notation rdf:datatype="http://www.w3.org/2001/XMLSchema#string">P2</skos:notation>
    </owl:ObjectProperty>
    


    <!-- http://dataforhistory.org/histdmi-generic-ongoing/property/P20 -->

    <owl:ObjectProperty rdf:about="http://dataforhistory.org/histdmi-generic-ongoing/property/P20">
        <rdfs:domain rdf:resource="http://dataforhistory.org/histdmi-generic-ongoing/class/C13"/>
        <rdfs:range rdf:resource="http://dataforhistory.org/histdmi-generic-ongoing/class/C14"/>
        <rdfs:comment xml:lang="en">Associates a geographical place with the type which defines its identity</rdfs:comment>
        <rdfs:label xml:lang="en">has geographical place type</rdfs:label>
        <skos:notation rdf:datatype="http://www.w3.org/2001/XMLSchema#string">P20</skos:notation>
    </owl:ObjectProperty>
    


    <!-- http://dataforhistory.org/histdmi-generic-ongoing/property/P21 -->

    <owl:ObjectProperty rdf:about="http://dataforhistory.org/histdmi-generic-ongoing/property/P21">
        <rdfs:domain rdf:resource="http://www.cidoc-crm.org/cidoc-crm/E21"/>
        <rdfs:range rdf:resource="http://dataforhistory.org/histdmi-generic-ongoing/class/C7"/>
        <rdfs:comment xml:lang="en">This property associates the person having a given state of mind</rdfs:comment>
        <rdfs:label xml:lang="en">has state of mind</rdfs:label>
        <skos:notation rdf:datatype="http://www.w3.org/2001/XMLSchema#string">P21</skos:notation>
    </owl:ObjectProperty>
    


    <!-- http://dataforhistory.org/histdmi-generic-ongoing/property/P22 -->

    <owl:ObjectProperty rdf:about="http://dataforhistory.org/histdmi-generic-ongoing/property/P22">
        <rdfs:domain rdf:resource="http://www.cidoc-crm.org/cidoc-crm/E1"/>
        <rdfs:range rdf:resource="http://dataforhistory.org/histdmi-generic-ongoing/class/C28"/>
        <rdfs:comment xml:lang="en">This property associates to an entity a quantifiable quality of it. A quality being inherent in an instance, the domain cardinality is accordingly defined as 1,1 ; not all entities having necessarily quantifiable qualities, and virtually multiple, ther range is defined as 0,n.</rdfs:comment>
        <rdfs:label xml:lang="en">has quality</rdfs:label>
        <skos:notation rdf:datatype="http://www.w3.org/2001/XMLSchema#string">P22</skos:notation>
    </owl:ObjectProperty>
    


    <!-- http://dataforhistory.org/histdmi-generic-ongoing/property/P23 -->

    <owl:ObjectProperty rdf:about="http://dataforhistory.org/histdmi-generic-ongoing/property/P23">
        <rdfs:domain rdf:resource="http://dataforhistory.org/histdmi-generic-ongoing/class/C28"/>
        <rdfs:range rdf:resource="http://dataforhistory.org/histdmi-generic-ongoing/class/C20"/>
        <rdfs:comment xml:lang="en">Associates a Quantifiable Entity Quality with the type which defines its identity.</rdfs:comment>
        <rdfs:label xml:lang="en">has quality type</rdfs:label>
        <skos:notation rdf:datatype="http://www.w3.org/2001/XMLSchema#string">P23</skos:notation>
    </owl:ObjectProperty>
    


    <!-- http://dataforhistory.org/histdmi-generic-ongoing/property/P24 -->

    <owl:ObjectProperty rdf:about="http://dataforhistory.org/histdmi-generic-ongoing/property/P24">
        <rdfs:domain rdf:resource="http://dataforhistory.org/histdmi-generic-ongoing/class/C19"/>
        <rdfs:range rdf:resource="http://www.cidoc-crm.org/cidoc-crm/E63"/>
        <rdfs:comment xml:lang="en">This property associates the event that is situated at the beginning of the existence of a persistent item. The starting event can be a simple or complex one and the quantifier correspondingly restricted to one.</rdfs:comment>
        <rdfs:label xml:lang="en">life was initiated by</rdfs:label>
        <skos:notation rdf:datatype="http://www.w3.org/2001/XMLSchema#string">P24</skos:notation>
    </owl:ObjectProperty>
    


    <!-- http://dataforhistory.org/histdmi-generic-ongoing/property/P25 -->

    <owl:ObjectProperty rdf:about="http://dataforhistory.org/histdmi-generic-ongoing/property/P25">
        <rdfs:domain rdf:resource="http://dataforhistory.org/histdmi-generic-ongoing/class/C19"/>
        <rdfs:range rdf:resource="http://www.cidoc-crm.org/cidoc-crm/E64"/>
        <rdfs:comment xml:lang="en">This property associates the event which is generally considered as the event endig the existence of a persistent item.</rdfs:comment>
        <rdfs:label xml:lang="en">life was terminated by</rdfs:label>
        <skos:notation rdf:datatype="http://www.w3.org/2001/XMLSchema#string">P25</skos:notation>
    </owl:ObjectProperty>
    


    <!-- http://dataforhistory.org/histdmi-generic-ongoing/property/P26 -->

    <owl:ObjectProperty rdf:about="http://dataforhistory.org/histdmi-generic-ongoing/property/P26">
        <rdfs:domain rdf:resource="http://dataforhistory.org/histdmi-generic-ongoing/class/C19"/>
        <rdfs:range rdf:resource="http://www.cidoc-crm.org/cidoc-crm/E77"/>
        <rdfs:comment xml:lang="en">This property associates the persistent item to its life as the collection of events it is involved in during its existence.</rdfs:comment>
        <rdfs:label xml:lang="en">is life of</rdfs:label>
        <skos:notation rdf:datatype="http://www.w3.org/2001/XMLSchema#string">P26</skos:notation>
    </owl:ObjectProperty>
    


    <!-- http://dataforhistory.org/histdmi-generic-ongoing/property/P27 -->

    <owl:ObjectProperty rdf:about="http://dataforhistory.org/histdmi-generic-ongoing/property/P27">
        <rdfs:domain rdf:resource="http://dataforhistory.org/histdmi-generic-ongoing/class/C22"/>
        <rdfs:range rdf:resource="http://www.cidoc-crm.org/cidoc-crm/E18"/>
        <rdfs:comment xml:lang="en">This property associates the main physical entity concerned by the composition, i. e. that has one or more parts.</rdfs:comment>
        <rdfs:label xml:lang="en">concerns</rdfs:label>
        <skos:notation rdf:datatype="http://www.w3.org/2001/XMLSchema#string">P27</skos:notation>
    </owl:ObjectProperty>
    


    <!-- http://dataforhistory.org/histdmi-generic-ongoing/property/P28 -->

    <owl:ObjectProperty rdf:about="http://dataforhistory.org/histdmi-generic-ongoing/property/P28">
        <rdfs:domain rdf:resource="http://dataforhistory.org/histdmi-generic-ongoing/class/C22"/>
        <rdfs:range rdf:resource="http://www.cidoc-crm.org/cidoc-crm/E18"/>
        <rdfs:comment xml:lang="en">This property associates the part of a physical thing that composes it during a limited time-span</rdfs:comment>
        <rdfs:label xml:lang="en">has part</rdfs:label>
        <skos:notation rdf:datatype="http://www.w3.org/2001/XMLSchema#string">P28</skos:notation>
    </owl:ObjectProperty>
    


    <!-- http://dataforhistory.org/histdmi-generic-ongoing/property/P29 -->

    <owl:ObjectProperty rdf:about="http://dataforhistory.org/histdmi-generic-ongoing/property/P29">
        <rdfs:domain rdf:resource="http://dataforhistory.org/histdmi-generic-ongoing/class/C23"/>
        <rdfs:range rdf:resource="http://dataforhistory.org/histdmi-generic-ongoing/class/C24"/>
        <rdfs:comment xml:lang="en"> 

Associates an usewith the type which defines its identity
</rdfs:comment>
        <rdfs:label xml:lang="en">has use type</rdfs:label>
        <skos:notation rdf:datatype="http://www.w3.org/2001/XMLSchema#string">P29</skos:notation>
    </owl:ObjectProperty>
    


    <!-- http://dataforhistory.org/histdmi-generic-ongoing/property/P3 -->

    <owl:ObjectProperty rdf:about="http://dataforhistory.org/histdmi-generic-ongoing/property/P3">
        <rdfs:domain rdf:resource="http://dataforhistory.org/histdmi-generic-ongoing/class/C2"/>
        <rdfs:range rdf:resource="http://dataforhistory.org/histdmi-generic-ongoing/class/C27"/>
        <rdfs:comment xml:lang="en">This property identifies the C27 Collective State of Mind which has been effected or initiated by a C2 Social Event. Different social events can contribute to the origin of the same instance of a collective state of mind and one social event can produce several collective states of mind.</rdfs:comment>
        <rdfs:label xml:lang="en">effected</rdfs:label>
        <skos:notation rdf:datatype="http://www.w3.org/2001/XMLSchema#string">P3</skos:notation>
    </owl:ObjectProperty>
    


    <!-- http://dataforhistory.org/histdmi-generic-ongoing/property/P30 -->

    <owl:ObjectProperty rdf:about="http://dataforhistory.org/histdmi-generic-ongoing/property/P30">
        <rdfs:domain rdf:resource="http://dataforhistory.org/histdmi-generic-ongoing/class/C23"/>
        <rdfs:range rdf:resource="http://www.cidoc-crm.org/cidoc-crm/E39"/>
        <rdfs:comment xml:lang="en">Associates the actor using the persistent item. The actor being identity defining for this class, the maximum cardinality is one.</rdfs:comment>
        <rdfs:label xml:lang="en">is use by actor</rdfs:label>
        <skos:notation rdf:datatype="http://www.w3.org/2001/XMLSchema#string">P30</skos:notation>
    </owl:ObjectProperty>
    


    <!-- http://dataforhistory.org/histdmi-generic-ongoing/property/P31 -->

    <owl:ObjectProperty rdf:about="http://dataforhistory.org/histdmi-generic-ongoing/property/P31">
        <rdfs:domain rdf:resource="http://dataforhistory.org/histdmi-generic-ongoing/class/C23"/>
        <rdfs:range rdf:resource="http://www.cidoc-crm.org/cidoc-crm/E89"/>
        <rdfs:comment xml:lang="en">This property associates a propositional object defining the purpose of the use</rdfs:comment>
        <rdfs:label xml:lang="en">has purpose</rdfs:label>
        <skos:notation rdf:datatype="http://www.w3.org/2001/XMLSchema#string">P31</skos:notation>
    </owl:ObjectProperty>
    


    <!-- http://dataforhistory.org/histdmi-generic-ongoing/property/P32 -->

    <owl:ObjectProperty rdf:about="http://dataforhistory.org/histdmi-generic-ongoing/property/P32">
        <rdfs:domain rdf:resource="http://dataforhistory.org/histdmi-generic-ongoing/class/C23"/>
        <rdfs:range rdf:resource="http://www.cidoc-crm.org/cidoc-crm/E77"/>
        <rdfs:comment xml:lang="en">This property associates the persistent item that is the object of the used. As an identifying property, the maximum cardinality is one, the use concerning just one object.</rdfs:comment>
        <rdfs:label xml:lang="en">is use of</rdfs:label>
        <skos:notation rdf:datatype="http://www.w3.org/2001/XMLSchema#string">P32</skos:notation>
    </owl:ObjectProperty>
    


    <!-- http://dataforhistory.org/histdmi-generic-ongoing/property/P33 -->

    <owl:ObjectProperty rdf:about="http://dataforhistory.org/histdmi-generic-ongoing/property/P33">
        <rdfs:domain rdf:resource="http://dataforhistory.org/histdmi-generic-ongoing/class/C2"/>
        <rdfs:range rdf:resource="http://dataforhistory.org/histdmi-generic-ongoing/class/C26"/>
        <rdfs:comment xml:lang="en">This property associates the social event ( a &apos;&apos;situation&apos;&apos; in the understanding of the DnS ontology) to the portion of social representations (i.e. the &apos;&apos;description&apos;&apos; in the understanding of the DnS ontology) that allows to perceive and recognize the social phenomenon present in the event.</rdfs:comment>
        <rdfs:label xml:lang="en">satisfies</rdfs:label>
        <skos:notation rdf:datatype="http://www.w3.org/2001/XMLSchema#string">P33</skos:notation>
    </owl:ObjectProperty>
    


    <!-- http://dataforhistory.org/histdmi-generic-ongoing/property/P34 -->

    <owl:ObjectProperty rdf:about="http://dataforhistory.org/histdmi-generic-ongoing/property/P34">
        <rdfs:domain rdf:resource="http://dataforhistory.org/histdmi-generic-ongoing/class/C27"/>
        <rdfs:range rdf:resource="http://dataforhistory.org/histdmi-generic-ongoing/class/C26"/>
        <rdfs:comment xml:lang="en">This property associates a time-indexed collective state of mind with the social representation representing its content.</rdfs:comment>
        <rdfs:label xml:lang="en">has content</rdfs:label>
        <skos:notation rdf:datatype="http://www.w3.org/2001/XMLSchema#string">P34</skos:notation>
    </owl:ObjectProperty>
    


    <!-- http://dataforhistory.org/histdmi-generic-ongoing/property/P35 -->

    <owl:ObjectProperty rdf:about="http://dataforhistory.org/histdmi-generic-ongoing/property/P35">
        <rdfs:domain rdf:resource="http://dataforhistory.org/histdmi-generic-ongoing/class/C28"/>
        <rdfs:range rdf:resource="http://www.cidoc-crm.org/cidoc-crm/E54"/>
        <rdfs:comment xml:lang="en">This property associates to a quantifiable quality the dimension of it.</rdfs:comment>
        <rdfs:label xml:lang="en">has quality dimension</rdfs:label>
        <skos:notation rdf:datatype="http://www.w3.org/2001/XMLSchema#string">P35</skos:notation>
    </owl:ObjectProperty>
    


    <!-- http://dataforhistory.org/histdmi-generic-ongoing/property/P36 -->

    <owl:ObjectProperty rdf:about="http://dataforhistory.org/histdmi-generic-ongoing/property/P36">
        <rdfs:domain rdf:resource="http://dataforhistory.org/histdmi-generic-ongoing/class/C25"/>
        <rdfs:range rdf:resource="http://www.cidoc-crm.org/cidoc-crm/E4"/>
        <rdfs:comment xml:lang="en">A crm:E4 Period is a set &quot;of coherent phenomena or cultural manifestations occurring in time and space&quot;. This property associates to a social collective, i.e. a cluster of persons who share the same intentionality, skills or practices, all the events and social/cultural phenomena in which they participate.</rdfs:comment>
        <rdfs:label xml:lang="en">has manifestation in</rdfs:label>
        <skos:notation rdf:datatype="http://www.w3.org/2001/XMLSchema#string">P36</skos:notation>
    </owl:ObjectProperty>
    


    <!-- http://dataforhistory.org/histdmi-generic-ongoing/property/P37 -->

    <owl:ObjectProperty rdf:about="http://dataforhistory.org/histdmi-generic-ongoing/property/P37">
        <rdfs:domain rdf:resource="http://dataforhistory.org/histdmi-generic-ongoing/class/C21"/>
        <rdfs:range rdf:resource="http://dataforhistory.org/histdmi-generic-ongoing/class/C29"/>
        <rdfs:comment xml:lang="en">This property associates to the personal skill the know-how it concerns, i.e. it is about and more or less efficiently realizes.</rdfs:comment>
        <rdfs:label xml:lang="en">concerns</rdfs:label>
        <skos:notation rdf:datatype="http://www.w3.org/2001/XMLSchema#string">P37</skos:notation>
    </owl:ObjectProperty>
    


    <!-- http://dataforhistory.org/histdmi-generic-ongoing/property/P38 -->

    <owl:ObjectProperty rdf:about="http://dataforhistory.org/histdmi-generic-ongoing/property/P38">
        <rdfs:domain rdf:resource="http://www.cidoc-crm.org/cidoc-crm/E21"/>
        <rdfs:range rdf:resource="http://dataforhistory.org/histdmi-generic-ongoing/class/C21"/>
        <rdfs:comment xml:lang="en">This property associates the person with the skill he/she has. A skill being modelled as a quality of a person, it must be retated to one and just one person.</rdfs:comment>
        <rdfs:label xml:lang="en">has skill</rdfs:label>
        <skos:notation rdf:datatype="http://www.w3.org/2001/XMLSchema#string">P38</skos:notation>
    </owl:ObjectProperty>
    


    <!-- http://dataforhistory.org/histdmi-generic-ongoing/property/P39 -->

    <owl:ObjectProperty rdf:about="http://dataforhistory.org/histdmi-generic-ongoing/property/P39">
        <rdfs:domain rdf:resource="http://www.cidoc-crm.org/cidoc-crm/E1"/>
        <rdfs:range rdf:resource="http://dataforhistory.org/histdmi-generic-ongoing/class/C30"/>
        <rdfs:comment xml:lang="en">This property associates the entity that is integrated into specific social representations, i.e. that receives a new connotation and becomes part of them, and in this way acquires a specific social quality.</rdfs:comment>
        <rdfs:label xml:lang="en">has social connotation</rdfs:label>
        <skos:notation rdf:datatype="http://www.w3.org/2001/XMLSchema#string">P39</skos:notation>
    </owl:ObjectProperty>
    


    <!-- http://dataforhistory.org/histdmi-generic-ongoing/property/P4 -->

    <owl:ObjectProperty rdf:about="http://dataforhistory.org/histdmi-generic-ongoing/property/P4">
        <rdfs:domain rdf:resource="http://dataforhistory.org/histdmi-generic-ongoing/class/C2"/>
        <rdfs:range rdf:resource="http://dataforhistory.org/histdmi-generic-ongoing/class/C27"/>
        <rdfs:comment xml:lang="en">
This property associates a Social Situation to the Collective State of Mind that it directly oder indirectly ends. Different social situations can contribute to the end of the same instance of Collective State of Mind and one event can end several Collective states of Minds.
</rdfs:comment>
        <rdfs:label xml:lang="en">ends</rdfs:label>
        <skos:notation rdf:datatype="http://www.w3.org/2001/XMLSchema#string">P4</skos:notation>
    </owl:ObjectProperty>
    


    <!-- http://dataforhistory.org/histdmi-generic-ongoing/property/P40 -->

    <owl:ObjectProperty rdf:about="http://dataforhistory.org/histdmi-generic-ongoing/property/P40">
        <rdfs:domain rdf:resource="http://dataforhistory.org/histdmi-generic-ongoing/class/C27"/>
        <rdfs:range rdf:resource="http://dataforhistory.org/histdmi-generic-ongoing/class/C26"/>
        <rdfs:comment xml:lang="en">This property associates a social connotation or social event to the general social representations&apos;&apos; set in the context of which the concerned social connotation or social event happen. The social representation specific to the connotation or event themselves are associated respectively with the inherited sdt:P34 has content and sdt:P33  satisfies properties.</rdfs:comment>
        <rdfs:label xml:lang="en">has context</rdfs:label>
        <skos:notation rdf:datatype="http://www.w3.org/2001/XMLSchema#string">P40</skos:notation>
    </owl:ObjectProperty>
    


    <!-- http://dataforhistory.org/histdmi-generic-ongoing/property/P41 -->

    <owl:ObjectProperty rdf:about="http://dataforhistory.org/histdmi-generic-ongoing/property/P41">
        <rdfs:domain rdf:resource="http://dataforhistory.org/histdmi-generic-ongoing/class/C2"/>
        <rdfs:range rdf:resource="http://dataforhistory.org/histdmi-generic-ongoing/class/C31"/>
        <rdfs:comment xml:lang="en">Associates a hist:C2 Social Situation with the type which defines its identity.</rdfs:comment>
        <rdfs:label xml:lang="en">has social event type</rdfs:label>
        <skos:notation rdf:datatype="http://www.w3.org/2001/XMLSchema#string">P41</skos:notation>
    </owl:ObjectProperty>
    


    <!-- http://dataforhistory.org/histdmi-generic-ongoing/property/P42 -->

    <owl:ObjectProperty rdf:about="http://dataforhistory.org/histdmi-generic-ongoing/property/P42">
        <rdfs:domain rdf:resource="http://dataforhistory.org/histdmi-generic-ongoing/class/C2"/>
        <rdfs:domain rdf:resource="http://dataforhistory.org/histdmi-generic-ongoing/class/C6"/>
        <rdfs:range rdf:resource="http://dataforhistory.org/histdmi-generic-ongoing/class/C13"/>
        <rdfs:range rdf:resource="http://dataforhistory.org/histdmi-generic-ongoing/class/C26"/>
        <rdfs:comment xml:lang="en">Associates a hist:C31 Social Situation Type instance to the social representations that define it. A social situation type is or was defined in the context of a specific human collective sharing the social representations that gave origin to the specific social situation and associated type. A social situation type can be nevertheless integrated into other social representations, as any other existing entity, and this is modelled with the hist:C30 Social Characterization class.</rdfs:comment>
        <rdfs:comment xml:lang="en">This property is a shortcut of longer paths involving phenomena in time and space (subclasses of crm:E5 Event) that are the setting of the social event and are themselves localized in geographical space. The geographical place associated to the social event corresponds to its maximal extention in space during the whole time-span of the social event. If different locations at different times of the same social event are part of the information, different localized crm:E5 Event (or subclasses) instances should be produced as they represent the different settings of the same social relationship.</rdfs:comment>
        <rdfs:label xml:lang="en">has maximal projection in geographical space</rdfs:label>
        <rdfs:label xml:lang="en">is defined by</rdfs:label>
        <skos:notation rdf:datatype="http://www.w3.org/2001/XMLSchema#string">P42</skos:notation>
    </owl:ObjectProperty>
    


    <!-- http://dataforhistory.org/histdmi-generic-ongoing/property/P43 -->

    <owl:ObjectProperty rdf:about="http://dataforhistory.org/histdmi-generic-ongoing/property/P43">
        <rdfs:domain rdf:resource="http://dataforhistory.org/histdmi-generic-ongoing/class/C2"/>
        <rdfs:range rdf:resource="http://www.cidoc-crm.org/cidoc-crm/E5"/>
        <rdfs:comment xml:lang="en">This property associates to a social event the spatio-temporal phenomena in the context of which it takes place or occurs. A social event is carved out in a set of spatio-temporal events according to a given description, i.e. a corresponding social representation. These events provide the setting for the social event. E.g. the wedding celebration (the event) is the setting of the marriage (the social event) conceived as the transition from being (considered by a community as) single to being (considered as) married.</rdfs:comment>
        <rdfs:label xml:lang="en">has setting</rdfs:label>
        <skos:notation rdf:datatype="http://www.w3.org/2001/XMLSchema#string">P43</skos:notation>
    </owl:ObjectProperty>
    


    <!-- http://dataforhistory.org/histdmi-generic-ongoing/property/P44 -->

    <owl:ObjectProperty rdf:about="http://dataforhistory.org/histdmi-generic-ongoing/property/P44">
        <rdfs:domain rdf:resource="http://dataforhistory.org/histdmi-generic-ongoing/class/C7"/>
        <rdfs:range rdf:resource="http://www.cidoc-crm.org/cidoc-crm/E89"/>
        <rdfs:comment xml:lang="en">This property associates the individual state of mind, modelled as a quality of a person, to its propositional, i.e. intentional content.</rdfs:comment>
        <rdfs:label xml:lang="en">has content</rdfs:label>
        <skos:notation rdf:datatype="http://www.w3.org/2001/XMLSchema#string">P44</skos:notation>
    </owl:ObjectProperty>
    


    <!-- http://dataforhistory.org/histdmi-generic-ongoing/property/P5 -->

    <owl:ObjectProperty rdf:about="http://dataforhistory.org/histdmi-generic-ongoing/property/P5">
        <rdfs:domain rdf:resource="http://www.cidoc-crm.org/cidoc-crm/E2"/>
        <rdfs:range rdf:resource="http://www.cidoc-crm.org/cidoc-crm/E2"/>
        <rdfs:comment xml:lang="en">This property indicates that the domain temporal entity is a part of a more complex range temporal entity, e.g. a simple event (domain) can be a component of a complex one (range), like a process. If the component or child instance belongs to the same class as the parent one, and if some instances of properties are not explicitely provided in the child instance, this means they are identical (i.e. &apos;&apos;inherited&apos;&apos;) from the parent instance.</rdfs:comment>
        <rdfs:label xml:lang="en">is component of</rdfs:label>
        <skos:notation rdf:datatype="http://www.w3.org/2001/XMLSchema#string">P5</skos:notation>
    </owl:ObjectProperty>
    


    <!-- http://dataforhistory.org/histdmi-generic-ongoing/property/P6 -->

    <owl:ObjectProperty rdf:about="http://dataforhistory.org/histdmi-generic-ongoing/property/P6">
        <rdfs:domain rdf:resource="http://www.cidoc-crm.org/cidoc-crm/E4"/>
        <rdfs:range rdf:resource="http://dataforhistory.org/histdmi-generic-ongoing/class/C13"/>
        <rdfs:comment xml:lang="en">This property specifies the geographical place where an instance of E4 Period happened.</rdfs:comment>
        <rdfs:label xml:lang="en">took place at</rdfs:label>
        <skos:notation rdf:datatype="http://www.w3.org/2001/XMLSchema#string">P6</skos:notation>
    </owl:ObjectProperty>
    


    <!-- http://dataforhistory.org/histdmi-generic-ongoing/property/P7 -->

    <owl:ObjectProperty rdf:about="http://dataforhistory.org/histdmi-generic-ongoing/property/P7">
        <rdfs:domain rdf:resource="http://dataforhistory.org/histdmi-generic-ongoing/class/C25"/>
        <rdfs:range rdf:resource="http://dataforhistory.org/histdmi-generic-ongoing/class/C27"/>
        <rdfs:comment xml:lang="en">This property associates the state of mind with the social collective it characterizes. The fact of sharing a state of mind, i.e. social representations, contributes to the existence of a social collective, it is a part of its identity.</rdfs:comment>
        <rdfs:label xml:lang="en">has collective state of mind</rdfs:label>
        <skos:notation rdf:datatype="http://www.w3.org/2001/XMLSchema#string">P7</skos:notation>
    </owl:ObjectProperty>
    


    <!-- http://dataforhistory.org/histdmi-generic-ongoing/property/P8 -->

    <owl:ObjectProperty rdf:about="http://dataforhistory.org/histdmi-generic-ongoing/property/P8">
        <rdfs:domain rdf:resource="http://dataforhistory.org/histdmi-generic-ongoing/class/C33"/>
        <rdfs:domain rdf:resource="http://www.cidoc-crm.org/cidoc-crm/E5"/>
        <rdfs:range rdf:resource="http://dataforhistory.org/histdmi-generic-ongoing/class/C1"/>
        <rdfs:range rdf:resource="http://dataforhistory.org/histdmi-generic-ongoing/class/C34"/>
        <rdfs:comment xml:lang="en">Associates a unitary event (sdh:C33) with the type which defines its identity</rdfs:comment>
        <rdfs:comment xml:lang="en">This property associates an event to the quality that it effects or initiates. Different events can contribute to the origin of the same quality and one event can produce several qualities, in one or more entities.</rdfs:comment>
        <rdfs:label xml:lang="en">effects quality</rdfs:label>
        <rdfs:label xml:lang="en">has event type</rdfs:label>
        <skos:notation rdf:datatype="http://www.w3.org/2001/XMLSchema#string">P8</skos:notation>
    </owl:ObjectProperty>
    


    <!-- http://dataforhistory.org/histdmi-generic-ongoing/property/P9 -->

    <owl:ObjectProperty rdf:about="http://dataforhistory.org/histdmi-generic-ongoing/property/P9">
        <rdfs:domain rdf:resource="http://www.cidoc-crm.org/cidoc-crm/E5"/>
        <rdfs:range rdf:resource="http://dataforhistory.org/histdmi-generic-ongoing/class/C1"/>
        <rdfs:comment xml:lang="en">This property associates an event to the quality that it directly oder indirectly ends. Different events can contribute to the end of the same quality and one event can end several qualities, in one or more entitites.</rdfs:comment>
        <rdfs:label xml:lang="en">ends</rdfs:label>
        <skos:notation rdf:datatype="http://www.w3.org/2001/XMLSchema#string">P9</skos:notation>
    </owl:ObjectProperty>
    


    <!-- http://dataforhistory.org/histsocial-ongoing/property/P1 -->

    <owl:ObjectProperty rdf:about="http://dataforhistory.org/histsocial-ongoing/property/P1">
        <rdfs:domain rdf:resource="http://dataforhistory.org/histsocial-ongoing/class/C5"/>
        <rdfs:range rdf:resource="http://www.cidoc-crm.org/cidoc-crm/E39"/>
        <rdfs:comment xml:lang="en">This property associates to the Temporal Entity the Actor (individual or group) that is member of a group</rdfs:comment>
        <rdfs:label xml:lang="en">was a membership of</rdfs:label>
        <skos:notation rdf:datatype="http://www.w3.org/2001/XMLSchema#string">P1</skos:notation>
    </owl:ObjectProperty>
    


    <!-- http://dataforhistory.org/histsocial-ongoing/property/P10 -->

    <owl:ObjectProperty rdf:about="http://dataforhistory.org/histsocial-ongoing/property/P10">
        <rdfs:domain rdf:resource="http://dataforhistory.org/histsocial-ongoing/class/C15"/>
        <rdfs:range rdf:resource="http://www.cidoc-crm.org/cidoc-crm/E39"/>
        <rdfs:comment xml:lang="en">This property associates the actor (person or group) participating in the event. Only one actor can be added per class instance.</rdfs:comment>
        <rdfs:label xml:lang="en">is participation of</rdfs:label>
        <skos:notation rdf:datatype="http://www.w3.org/2001/XMLSchema#string">P10</skos:notation>
    </owl:ObjectProperty>
    


    <!-- http://dataforhistory.org/histsocial-ongoing/property/P11 -->

    <owl:ObjectProperty rdf:about="http://dataforhistory.org/histsocial-ongoing/property/P11">
        <rdfs:domain rdf:resource="http://dataforhistory.org/histsocial-ongoing/class/C15"/>
        <rdfs:range rdf:resource="http://www.cidoc-crm.org/cidoc-crm/E5"/>
        <rdfs:comment xml:lang="en">This property identifies the event to which the participation is related.</rdfs:comment>
        <rdfs:label xml:lang="en">is participation in</rdfs:label>
        <skos:notation rdf:datatype="http://www.w3.org/2001/XMLSchema#string">P11</skos:notation>
    </owl:ObjectProperty>
    


    <!-- http://dataforhistory.org/histsocial-ongoing/property/P12 -->

    <owl:ObjectProperty rdf:about="http://dataforhistory.org/histsocial-ongoing/property/P12">
        <rdfs:domain rdf:resource="http://dataforhistory.org/histsocial-ongoing/class/C15"/>
        <rdfs:range rdf:resource="http://dataforhistory.org/histsocial-ongoing/class/C2"/>
        <rdfs:comment xml:lang="en">The function exercised or office/rank hold by the actor in the event. More instances per event and actor if this property are possible but the time span must then be the same for all of them. Otherwise different instances of the class Participation should be created.</rdfs:comment>
        <rdfs:label xml:lang="en">is participation with social quality</rdfs:label>
        <skos:notation rdf:datatype="http://www.w3.org/2001/XMLSchema#string">P12</skos:notation>
    </owl:ObjectProperty>
    


    <!-- http://dataforhistory.org/histsocial-ongoing/property/P13 -->

    <owl:ObjectProperty rdf:about="http://dataforhistory.org/histsocial-ongoing/property/P13">
        <rdfs:domain rdf:resource="http://dataforhistory.org/histsocial-ongoing/class/C1"/>
        <rdfs:range rdf:resource="http://www.cidoc-crm.org/cidoc-crm/E39"/>
        <rdfs:comment xml:lang="en">Associates the actor (person or group) concerned by the character</rdfs:comment>
        <rdfs:label xml:lang="en">pertains to</rdfs:label>
        <skos:notation rdf:datatype="http://www.w3.org/2001/XMLSchema#string">P13</skos:notation>
    </owl:ObjectProperty>
    


    <!-- http://dataforhistory.org/histsocial-ongoing/property/P14 -->

    <owl:ObjectProperty rdf:about="http://dataforhistory.org/histsocial-ongoing/property/P14">
        <rdfs:domain rdf:resource="http://dataforhistory.org/histsocial-ongoing/class/C1"/>
        <rdfs:range rdf:resource="http://dataforhistory.org/histsocial-ongoing/class/C2"/>
        <rdfs:comment xml:lang="en">Associates the considered social quality. The maximal cardinality is one for social qualities because each of them has to be associated to the actor separately. This is because no only each quality sould be considered individually, but the time span of each of them is usually different. Therefore it cannot be expressed in just one temporal entity instance</rdfs:comment>
        <rdfs:label xml:lang="en">has social quality</rdfs:label>
        <skos:notation rdf:datatype="http://www.w3.org/2001/XMLSchema#string">P14</skos:notation>
    </owl:ObjectProperty>
    


    <!-- http://dataforhistory.org/histsocial-ongoing/property/P15 -->

    <owl:ObjectProperty rdf:about="http://dataforhistory.org/histsocial-ongoing/property/P15">
        <rdfs:domain rdf:resource="http://dataforhistory.org/histsocial-ongoing/class/C3"/>
        <rdfs:range rdf:resource="http://www.cidoc-crm.org/cidoc-crm/E39"/>
        <rdfs:comment xml:lang="en">Associates to the relationship the persons or groups involved in it.
Each relationship generally involves only two instances of one or more classes. Informal relationships like commercial relations or friendship should be restricted to two persistent items per instance. Therefore, the range quantifiers sould be: 2,2.
Relationships involving more than two partners could be used to express multi-lateral agreements, treaties, etc. although it is preferable to treat structured relationships between several entities as membership in a group. This is mandatory if the duration of the relationship is not the same for all partners.</rdfs:comment>
        <rdfs:label xml:lang="en">involves partner</rdfs:label>
        <skos:notation rdf:datatype="http://www.w3.org/2001/XMLSchema#string">P15</skos:notation>
    </owl:ObjectProperty>
    


    <!-- http://dataforhistory.org/histsocial-ongoing/property/P16 -->

    <owl:ObjectProperty rdf:about="http://dataforhistory.org/histsocial-ongoing/property/P16">
        <rdfs:domain rdf:resource="http://dataforhistory.org/histsocial-ongoing/class/C3"/>
        <rdfs:range rdf:resource="http://dataforhistory.org/histsocial-ongoing/class/C4"/>
        <rdfs:comment xml:lang="en">Associates a social relationship with the type which defines its identity</rdfs:comment>
        <rdfs:label xml:lang="en">has relationship type</rdfs:label>
        <skos:notation rdf:datatype="http://www.w3.org/2001/XMLSchema#string">P16</skos:notation>
    </owl:ObjectProperty>
    


    <!-- http://dataforhistory.org/histsocial-ongoing/property/P17 -->

    <owl:ObjectProperty rdf:about="http://dataforhistory.org/histsocial-ongoing/property/P17">
        <rdfs:domain rdf:resource="http://dataforhistory.org/histsocial-ongoing/class/C3"/>
        <rdfs:range rdf:resource="http://www.cidoc-crm.org/cidoc-crm/E39"/>
        <rdfs:comment xml:lang="en">This property associates to the relationhips the actor being at its source, i.e. the starting vertex in a directed relationship</rdfs:comment>
        <rdfs:label xml:lang="en">has relationship source</rdfs:label>
        <skos:notation rdf:datatype="http://www.w3.org/2001/XMLSchema#string">P17</skos:notation>
    </owl:ObjectProperty>
    


    <!-- http://dataforhistory.org/histsocial-ongoing/property/P18 -->

    <owl:ObjectProperty rdf:about="http://dataforhistory.org/histsocial-ongoing/property/P18">
        <rdfs:domain rdf:resource="http://dataforhistory.org/histsocial-ongoing/class/C3"/>
        <rdfs:range rdf:resource="http://www.cidoc-crm.org/cidoc-crm/E39"/>
        <rdfs:comment xml:lang="en">This property associates to the relationhips the actor being its target, i.e. the vertex at the end of a directed relationship</rdfs:comment>
        <rdfs:label xml:lang="en">has relationship target</rdfs:label>
        <skos:notation rdf:datatype="http://www.w3.org/2001/XMLSchema#string">P18</skos:notation>
    </owl:ObjectProperty>
    


    <!-- http://dataforhistory.org/histsocial-ongoing/property/P19 -->

    <owl:ObjectProperty rdf:about="http://dataforhistory.org/histsocial-ongoing/property/P19">
        <rdfs:domain rdf:resource="http://dataforhistory.org/histsocial-ongoing/class/C13"/>
        <rdfs:range rdf:resource="http://www.cidoc-crm.org/cidoc-crm/E74"/>
        <rdfs:comment xml:lang="en">A social role, conceived as the embodiment of a Social Actor, is generally related to a group that embodies, on its side, the Social Actor for which the social role (as Social Actor) is defined. E.g. a person is elected as National Councillor in the 2019-2023 legislature, i.e. a group of persons embodying during this legislature the Swiss National Council.</rdfs:comment>
        <rdfs:label xml:lang="en">is in relation to</rdfs:label>
        <skos:notation rdf:datatype="http://www.w3.org/2001/XMLSchema#string">P19</skos:notation>
    </owl:ObjectProperty>
    


    <!-- http://dataforhistory.org/histsocial-ongoing/property/P2 -->

    <owl:ObjectProperty rdf:about="http://dataforhistory.org/histsocial-ongoing/property/P2">
        <rdfs:domain rdf:resource="http://dataforhistory.org/histsocial-ongoing/class/C5"/>
        <rdfs:range rdf:resource="http://www.cidoc-crm.org/cidoc-crm/E74"/>
        <rdfs:comment xml:lang="en">This property associates the group concerned by the membership</rdfs:comment>
        <rdfs:label xml:lang="en">was membership in</rdfs:label>
        <skos:notation rdf:datatype="http://www.w3.org/2001/XMLSchema#string">P2</skos:notation>
    </owl:ObjectProperty>
    


    <!-- http://dataforhistory.org/histsocial-ongoing/property/P20 -->

    <owl:ObjectProperty rdf:about="http://dataforhistory.org/histsocial-ongoing/property/P20">
        <rdfs:domain rdf:resource="http://dataforhistory.org/histsocial-ongoing/class/C9"/>
        <rdfs:range rdf:resource="http://www.cidoc-crm.org/cidoc-crm/E21"/>
        <rdfs:comment xml:lang="en">This property associates the two (always two) persons participating to the union</rdfs:comment>
        <rdfs:label xml:lang="en">has partner</rdfs:label>
        <skos:notation rdf:datatype="http://www.w3.org/2001/XMLSchema#string">P20</skos:notation>
    </owl:ObjectProperty>
    


    <!-- http://dataforhistory.org/histsocial-ongoing/property/P21 -->

    <owl:ObjectProperty rdf:about="http://dataforhistory.org/histsocial-ongoing/property/P21">
        <rdfs:domain rdf:resource="http://dataforhistory.org/histsocial-ongoing/class/C9"/>
        <rdfs:range rdf:resource="http://dataforhistory.org/histsocial-ongoing/class/C10"/>
        <rdfs:comment xml:lang="en">Associates a union with the type which defines its identity</rdfs:comment>
        <rdfs:label xml:lang="en">has type of union</rdfs:label>
        <skos:notation rdf:datatype="http://www.w3.org/2001/XMLSchema#string">P21</skos:notation>
    </owl:ObjectProperty>
    


    <!-- http://dataforhistory.org/histsocial-ongoing/property/P22 -->

    <owl:ObjectProperty rdf:about="http://dataforhistory.org/histsocial-ongoing/property/P22">
        <rdfs:domain rdf:resource="http://www.cidoc-crm.org/cidoc-crm/E67"/>
        <rdfs:range rdf:resource="http://dataforhistory.org/histsocial-ongoing/class/C9"/>
        <rdfs:comment xml:lang="en">This property models the biological origin of a birth from the physical union of the parents. This is the common scenario. For more specific situations, like adoption or artificial procreation, a more suitable model should be applied.</rdfs:comment>
        <rdfs:label xml:lang="en">stems from</rdfs:label>
        <skos:notation rdf:datatype="http://www.w3.org/2001/XMLSchema#string">P22</skos:notation>
    </owl:ObjectProperty>
    


    <!-- http://dataforhistory.org/histsocial-ongoing/property/P23 -->

    <owl:ObjectProperty rdf:about="http://dataforhistory.org/histsocial-ongoing/property/P23">
        <rdfs:domain rdf:resource="http://www.cidoc-crm.org/cidoc-crm/E21"/>
        <rdfs:range rdf:resource="http://dataforhistory.org/histsocial-ongoing/class/C11"/>
        <rdfs:comment xml:lang="en">This property associates a person with his/hers gender. Insofar as this property is timeless, it has to be considered as a shortcut for a TeEn expressing the evolution of gender over time (as subclass of Time-related Persistent Item Characteristic – histC1). Also the quantifier on the gender side is open to different possibilities.</rdfs:comment>
        <rdfs:label xml:lang="en">has gender</rdfs:label>
        <skos:notation rdf:datatype="http://www.w3.org/2001/XMLSchema#string">P23</skos:notation>
    </owl:ObjectProperty>
    


    <!-- http://dataforhistory.org/histsocial-ongoing/property/P24 -->

    <owl:ObjectProperty rdf:about="http://dataforhistory.org/histsocial-ongoing/property/P24">
        <rdfs:domain rdf:resource="http://www.cidoc-crm.org/cidoc-crm/E21"/>
        <rdfs:range rdf:resource="http://dataforhistory.org/histdmi-generic-ongoing/class/C13"/>
        <rdfs:comment xml:lang="en">This property associates a person to the geographical region or place he/she comes from, in the sense of unspecified origin. If this place or region is the place where the person was born, it would be preferable to use a E67 Birth event</rdfs:comment>
        <rdfs:label xml:lang="en">has its origins in</rdfs:label>
        <skos:notation rdf:datatype="http://www.w3.org/2001/XMLSchema#string">P24</skos:notation>
    </owl:ObjectProperty>
    


    <!-- http://dataforhistory.org/histsocial-ongoing/property/P25 -->

    <owl:ObjectProperty rdf:about="http://dataforhistory.org/histsocial-ongoing/property/P25">
        <rdfs:domain rdf:resource="http://dataforhistory.org/histsocial-ongoing/class/C25"/>
        <rdfs:range rdf:resource="http://dataforhistory.org/histsocial-ongoing/class/C16"/>
        <rdfs:comment xml:lang="en">Associates the legal individual of which the existence is documented in social representations during a given time-span.</rdfs:comment>
        <rdfs:label xml:lang="en">has legal existence</rdfs:label>
        <skos:notation rdf:datatype="http://www.w3.org/2001/XMLSchema#string">P25</skos:notation>
    </owl:ObjectProperty>
    


    <!-- http://dataforhistory.org/histsocial-ongoing/property/P26 -->

    <owl:ObjectProperty rdf:about="http://dataforhistory.org/histsocial-ongoing/property/P26">
        <rdfs:domain rdf:resource="http://www.cidoc-crm.org/cidoc-crm/E39"/>
        <rdfs:range rdf:resource="http://dataforhistory.org/histsocial-ongoing/class/C13"/>
        <rdfs:comment xml:lang="en">This property associates a person or group to the embodiment of social actor, i.e. the fact of acting in the quality and virtue of being the human actor who realises a social actor, an abstract individual possessing more or less clearly defined rights and duties.</rdfs:comment>
        <rdfs:label xml:lang="en">embodies</rdfs:label>
        <skos:notation rdf:datatype="http://www.w3.org/2001/XMLSchema#string">P26</skos:notation>
    </owl:ObjectProperty>
    


    <!-- http://dataforhistory.org/histsocial-ongoing/property/P27 -->

    <owl:ObjectProperty rdf:about="http://dataforhistory.org/histsocial-ongoing/property/P27">
        <rdfs:domain rdf:resource="http://dataforhistory.org/histsocial-ongoing/class/C25"/>
        <rdfs:range rdf:resource="http://dataforhistory.org/histsocial-ongoing/class/C19"/>
        <rdfs:comment xml:lang="en">This properties associates a legal individual with characterization that define it and can evolve over time, the identity of the legal individual remaining the same</rdfs:comment>
        <rdfs:label xml:lang="en">has characterization</rdfs:label>
        <skos:notation rdf:datatype="http://www.w3.org/2001/XMLSchema#string">P27</skos:notation>
    </owl:ObjectProperty>
    


    <!-- http://dataforhistory.org/histsocial-ongoing/property/P28 -->

    <owl:ObjectProperty rdf:about="http://dataforhistory.org/histsocial-ongoing/property/P28">
        <rdfs:domain rdf:resource="http://dataforhistory.org/histsocial-ongoing/class/C19"/>
        <rdfs:range rdf:resource="http://dataforhistory.org/histsocial-ongoing/class/C17"/>
        <rdfs:comment xml:lang="en">This property associates the right or duty related to a social object during a given time-span</rdfs:comment>
        <rdfs:label xml:lang="en">is defined by</rdfs:label>
        <skos:notation rdf:datatype="http://www.w3.org/2001/XMLSchema#string">P28</skos:notation>
    </owl:ObjectProperty>
    


    <!-- http://dataforhistory.org/histsocial-ongoing/property/P29 -->

    <owl:ObjectProperty rdf:about="http://dataforhistory.org/histsocial-ongoing/property/P29">
        <rdfs:domain rdf:resource="http://dataforhistory.org/histsocial-ongoing/class/C17"/>
        <rdfs:range rdf:resource="http://www.cidoc-crm.org/cidoc-crm/E39"/>
        <rdfs:comment xml:lang="en">This property denotes the subject of law (a person or a group) holding the right.</rdfs:comment>
        <rdfs:label xml:lang="en">right is held by</rdfs:label>
        <skos:notation rdf:datatype="http://www.w3.org/2001/XMLSchema#string">P29</skos:notation>
    </owl:ObjectProperty>
    


    <!-- http://dataforhistory.org/histsocial-ongoing/property/P3 -->

    <owl:ObjectProperty rdf:about="http://dataforhistory.org/histsocial-ongoing/property/P3">
        <rdfs:domain rdf:resource="http://dataforhistory.org/histsocial-ongoing/class/C5"/>
        <rdfs:range rdf:resource="http://dataforhistory.org/histsocial-ongoing/class/C6"/>
        <rdfs:comment xml:lang="en">Associates a membership with the type which defines its identity, making clear the kind of membership that is intended (legal, informal, nationality, etc.).</rdfs:comment>
        <rdfs:label xml:lang="en">has membership type</rdfs:label>
        <skos:notation rdf:datatype="http://www.w3.org/2001/XMLSchema#string">P3</skos:notation>
    </owl:ObjectProperty>
    


    <!-- http://dataforhistory.org/histsocial-ongoing/property/P30 -->

    <owl:ObjectProperty rdf:about="http://dataforhistory.org/histsocial-ongoing/property/P30">
        <rdfs:domain rdf:resource="http://dataforhistory.org/histsocial-ongoing/class/C17"/>
        <rdfs:range rdf:resource="http://dataforhistory.org/histsocial-ongoing/class/C20"/>
        <rdfs:comment xml:lang="en">This property associates to the right or obligation to its temporal quality or validity time-span in collective intentionality.</rdfs:comment>
        <rdfs:label xml:lang="en">has validity</rdfs:label>
        <skos:notation rdf:datatype="http://www.w3.org/2001/XMLSchema#string">P30</skos:notation>
    </owl:ObjectProperty>
    


    <!-- http://dataforhistory.org/histsocial-ongoing/property/P31 -->

    <owl:ObjectProperty rdf:about="http://dataforhistory.org/histsocial-ongoing/property/P31">
        <rdfs:domain rdf:resource="http://dataforhistory.org/histsocial-ongoing/class/C17"/>
        <rdfs:range rdf:resource="http://www.cidoc-crm.org/cidoc-crm/E77"/>
        <rdfs:comment xml:lang="en">This property associates the object with is subject to the right or obligation.</rdfs:comment>
        <rdfs:label xml:lang="en">has subject</rdfs:label>
        <skos:notation rdf:datatype="http://www.w3.org/2001/XMLSchema#string">P31</skos:notation>
    </owl:ObjectProperty>
    


    <!-- http://dataforhistory.org/histsocial-ongoing/property/P32 -->

    <owl:ObjectProperty rdf:about="http://dataforhistory.org/histsocial-ongoing/property/P32">
        <rdfs:domain rdf:resource="http://dataforhistory.org/histsocial-ongoing/class/C17"/>
        <rdfs:range rdf:resource="http://dataforhistory.org/histsocial-ongoing/class/C21"/>
        <rdfs:comment xml:lang="en">Associates a C17 Right or obligation instance with the type which defines its identity.</rdfs:comment>
        <rdfs:label xml:lang="en">has right or obligation type</rdfs:label>
        <skos:notation rdf:datatype="http://www.w3.org/2001/XMLSchema#string">P32</skos:notation>
    </owl:ObjectProperty>
    


    <!-- http://dataforhistory.org/histsocial-ongoing/property/P33 -->

    <owl:ObjectProperty rdf:about="http://dataforhistory.org/histsocial-ongoing/property/P33">
        <rdfs:domain rdf:resource="http://dataforhistory.org/histsocial-ongoing/class/C13"/>
        <rdfs:range rdf:resource="http://dataforhistory.org/histsocial-ongoing/class/C12"/>
        <rdfs:comment xml:lang="en">This property associates the social role of an actor, understood as a time-indexed quality of it, with the instance of the Social Actor class, i.e. with the  abstract individual that the actor (as group or person) embodies.</rdfs:comment>
        <rdfs:label xml:lang="en">embodies</rdfs:label>
        <skos:notation rdf:datatype="http://www.w3.org/2001/XMLSchema#string">P33</skos:notation>
    </owl:ObjectProperty>
    


    <!-- http://dataforhistory.org/histsocial-ongoing/property/P34 -->

    <owl:ObjectProperty rdf:about="http://dataforhistory.org/histsocial-ongoing/property/P34">
        <rdfs:domain rdf:resource="http://dataforhistory.org/histsocial-ongoing/class/C15"/>
        <rdfs:range rdf:resource="http://www.cidoc-crm.org/cidoc-crm/E39"/>
        <rdfs:comment xml:lang="en">This property models the fact that an actor participates in an event on behalf of another actor, be this for representing him or for other reasons. One can represent more then one actor in one and the same event, but in this case the time-span of the representation must be the same for all represented actors. Otherwise, several instances of participation should be produced.</rdfs:comment>
        <rdfs:label xml:lang="en">is participation on behalf of</rdfs:label>
        <skos:notation rdf:datatype="http://www.w3.org/2001/XMLSchema#string">P34</skos:notation>
    </owl:ObjectProperty>
    


    <!-- http://dataforhistory.org/histsocial-ongoing/property/P35 -->

    <owl:ObjectProperty rdf:about="http://dataforhistory.org/histsocial-ongoing/property/P35">
        <rdfs:domain rdf:resource="http://dataforhistory.org/histsocial-ongoing/class/C23"/>
        <rdfs:range rdf:resource="http://dataforhistory.org/histsocial-ongoing/class/C24"/>
        <rdfs:comment xml:lang="en">
Associates a social quality (temporal entity) with the type which defines its identity
</rdfs:comment>
        <rdfs:label xml:lang="en">is defined by</rdfs:label>
        <skos:notation rdf:datatype="http://www.w3.org/2001/XMLSchema#string">P35</skos:notation>
    </owl:ObjectProperty>
    


    <!-- http://dataforhistory.org/histsocial-ongoing/property/P36 -->

    <owl:ObjectProperty rdf:about="http://dataforhistory.org/histsocial-ongoing/property/P36">
        <rdfs:domain rdf:resource="http://dataforhistory.org/histsocial-ongoing/class/C23"/>
        <rdfs:range rdf:resource="http://www.cidoc-crm.org/cidoc-crm/E21"/>
        <rdfs:comment xml:lang="en">This property associates the social event to the spatio-temporal, physical event in which the social event (defined in human collective intentionality but not physical space) happens.</rdfs:comment>
        <rdfs:label xml:lang="en">pertains to</rdfs:label>
        <skos:notation rdf:datatype="http://www.w3.org/2001/XMLSchema#string">P36</skos:notation>
    </owl:ObjectProperty>
    


    <!-- http://dataforhistory.org/histsocial-ongoing/property/P37 -->

    <owl:ObjectProperty rdf:about="http://dataforhistory.org/histsocial-ongoing/property/P37">
        <rdfs:domain rdf:resource="http://dataforhistory.org/histsocial-ongoing/class/C27"/>
        <rdfs:range rdf:resource="http://dataforhistory.org/histsocial-ongoing/class/C26"/>
        <rdfs:comment xml:lang="en">Associates the legal quality of an actor to the temporal validity of it</rdfs:comment>
        <rdfs:label xml:lang="en">has legal quality</rdfs:label>
        <skos:notation rdf:datatype="http://www.w3.org/2001/XMLSchema#string">P37</skos:notation>
    </owl:ObjectProperty>
    


    <!-- http://dataforhistory.org/histsocial-ongoing/property/P38 -->

    <owl:ObjectProperty rdf:about="http://dataforhistory.org/histsocial-ongoing/property/P38">
        <rdfs:domain rdf:resource="http://dataforhistory.org/histsocial-ongoing/class/C27"/>
        <rdfs:range rdf:resource="http://dataforhistory.org/histsocial-ongoing/class/C22"/>
        <rdfs:comment xml:lang="en">Associates a type to a legal connotation.</rdfs:comment>
        <rdfs:label xml:lang="en">has legal connotation type</rdfs:label>
        <skos:notation rdf:datatype="http://www.w3.org/2001/XMLSchema#string">P38</skos:notation>
    </owl:ObjectProperty>
    


    <!-- http://dataforhistory.org/histsocial-ongoing/property/P39 -->

    <owl:ObjectProperty rdf:about="http://dataforhistory.org/histsocial-ongoing/property/P39">
        <rdfs:domain rdf:resource="http://dataforhistory.org/histsocial-ongoing/class/C26"/>
        <rdfs:range rdf:resource="http://dataforhistory.org/histsocial-ongoing/class/C22"/>
        <rdfs:comment xml:lang="en">Associates a legal quality to the type that classifies it.</rdfs:comment>
        <rdfs:label xml:lang="en">has type</rdfs:label>
        <skos:notation rdf:datatype="http://www.w3.org/2001/XMLSchema#string">P39</skos:notation>
    </owl:ObjectProperty>
    


    <!-- http://dataforhistory.org/histsocial-ongoing/property/P4 -->

    <owl:ObjectProperty rdf:about="http://dataforhistory.org/histsocial-ongoing/property/P4">
        <rdfs:domain rdf:resource="http://dataforhistory.org/histsocial-ongoing/class/C8"/>
        <rdfs:range rdf:resource="http://www.cidoc-crm.org/cidoc-crm/E21"/>
        <rdfs:comment xml:lang="en">This property associates the person having the given occupation</rdfs:comment>
        <rdfs:label xml:lang="en">is occupation of</rdfs:label>
        <skos:notation rdf:datatype="http://www.w3.org/2001/XMLSchema#string">P4</skos:notation>
    </owl:ObjectProperty>
    


    <!-- http://dataforhistory.org/histsocial-ongoing/property/P40 -->

    <owl:ObjectProperty rdf:about="http://dataforhistory.org/histsocial-ongoing/property/P40">
        <rdfs:domain rdf:resource="http://dataforhistory.org/histsocial-ongoing/class/C20"/>
        <rdfs:range rdf:resource="http://dataforhistory.org/histdmi-generic-ongoing/class/C13"/>
        <rdfs:comment xml:lang="en">This property associates the geographical domain of validity of a right or obligation</rdfs:comment>
        <rdfs:label xml:lang="en">is valid in</rdfs:label>
        <skos:notation rdf:datatype="http://www.w3.org/2001/XMLSchema#string">P40</skos:notation>
    </owl:ObjectProperty>
    


    <!-- http://dataforhistory.org/histsocial-ongoing/property/P41 -->

    <owl:ObjectProperty rdf:about="http://dataforhistory.org/histsocial-ongoing/property/P41">
        <rdfs:domain rdf:resource="http://dataforhistory.org/histsocial-ongoing/class/C18"/>
        <rdfs:range rdf:resource="http://www.cidoc-crm.org/cidoc-crm/E21"/>
        <rdfs:comment xml:lang="en">This property associates the two or more persons involved in the interaction. If more than two persons are involved in one instance of an interaction, e.g. in the case of a meeting, there must be a unity in time and space for all the participants. If a person joins the interaction at a later moment than the beginning, or leaves before the end, the C15 Participation class can be used.</rdfs:comment>
        <rdfs:label xml:lang="en">is interaction of</rdfs:label>
        <skos:notation rdf:datatype="http://www.w3.org/2001/XMLSchema#string">P41</skos:notation>
    </owl:ObjectProperty>
    


    <!-- http://dataforhistory.org/histsocial-ongoing/property/P5 -->

    <owl:ObjectProperty rdf:about="http://dataforhistory.org/histsocial-ongoing/property/P5">
        <rdfs:domain rdf:resource="http://dataforhistory.org/histsocial-ongoing/class/C8"/>
        <rdfs:range rdf:resource="http://dataforhistory.org/histsocial-ongoing/class/C7"/>
        <rdfs:comment xml:lang="en">Is the type of the time-related occupation of a person</rdfs:comment>
        <rdfs:label xml:lang="en">is about</rdfs:label>
        <skos:notation rdf:datatype="http://www.w3.org/2001/XMLSchema#string">P5</skos:notation>
    </owl:ObjectProperty>
    


    <!-- http://dataforhistory.org/histsocial-ongoing/property/P6 -->

    <owl:ObjectProperty rdf:about="http://dataforhistory.org/histsocial-ongoing/property/P6">
        <rdfs:domain rdf:resource="http://dataforhistory.org/histsocial-ongoing/class/C8"/>
        <rdfs:range rdf:resource="http://dataforhistory.org/histdmi-generic-ongoing/class/C13"/>
        <rdfs:comment xml:lang="en">Associates the geographical place where the whole activity takes place. If the place changes during the activity this property should not be used and different instances of histC2 Time-related geographical localisation should be produced, one per location and time span.</rdfs:comment>
        <rdfs:label xml:lang="en">takes place at</rdfs:label>
        <skos:notation rdf:datatype="http://www.w3.org/2001/XMLSchema#string">P6</skos:notation>
    </owl:ObjectProperty>
    


    <!-- http://dataforhistory.org/histsocial-ongoing/property/P7 -->

    <owl:ObjectProperty rdf:about="http://dataforhistory.org/histsocial-ongoing/property/P7">
        <rdfs:domain rdf:resource="http://dataforhistory.org/histsocial-ongoing/class/C8"/>
        <rdfs:range rdf:resource="http://www.cidoc-crm.org/cidoc-crm/E39"/>
        <rdfs:comment xml:lang="en">The organization within which the occupation is carried out, the person entrusting the occupation, etc. Use properties of properties to clarify, if necessary, the role of the organization or person entrusting the occupation.</rdfs:comment>
        <rdfs:label xml:lang="en">on behalf of</rdfs:label>
        <skos:notation rdf:datatype="http://www.w3.org/2001/XMLSchema#string">P7</skos:notation>
    </owl:ObjectProperty>
    


    <!-- http://dataforhistory.org/histsocial-ongoing/property/P8 -->

    <owl:ObjectProperty rdf:about="http://dataforhistory.org/histsocial-ongoing/property/P8">
        <rdfs:domain rdf:resource="http://www.cidoc-crm.org/cidoc-crm/E77"/>
        <rdfs:range rdf:resource="http://dataforhistory.org/histsocial-ongoing/class/C14"/>
        <rdfs:comment xml:lang="en">This property associates the persistent item to the right subjection it is concerned by</rdfs:comment>
        <rdfs:label xml:lang="en">is subject to</rdfs:label>
        <skos:notation rdf:datatype="http://www.w3.org/2001/XMLSchema#string">P8</skos:notation>
    </owl:ObjectProperty>
    


    <!-- http://dataforhistory.org/histsocial-ongoing/property/P9 -->

    <owl:ObjectProperty rdf:about="http://dataforhistory.org/histsocial-ongoing/property/P9">
        <rdfs:domain rdf:resource="http://dataforhistory.org/histsocial-ongoing/class/C14"/>
        <rdfs:range rdf:resource="http://www.cidoc-crm.org/cidoc-crm/E39"/>
        <rdfs:comment xml:lang="en">This property associates the actor or actors having the right over a given persistent item. If more then one actor is associated, this means they exercise their right on the same persitent item collectively and during the same period of time.</rdfs:comment>
        <rdfs:label xml:lang="en">is right of</rdfs:label>
        <skos:notation rdf:datatype="http://www.w3.org/2001/XMLSchema#string">P9</skos:notation>
    </owl:ObjectProperty>
    


    <!-- http://dataforhistory.org/maritime-history-ongoing/property/P1 -->

    <owl:ObjectProperty rdf:about="http://dataforhistory.org/maritime-history-ongoing/property/P1">
        <rdfs:domain rdf:resource="http://dataforhistory.org/maritime-history-ongoing/class/C1"/>
        <rdfs:range rdf:resource="http://dataforhistory.org/histdmi-generic-ongoing/class/C13"/>
        <rdfs:comment xml:lang="en">This property identifies the C13 Geographical Place which is the departure place of a C1 Ship Voyage.</rdfs:comment>
        <rdfs:label xml:lang="en">had departure place</rdfs:label>
        <skos:notation rdf:datatype="http://www.w3.org/2001/XMLSchema#string">P1</skos:notation>
    </owl:ObjectProperty>
    


    <!-- http://dataforhistory.org/maritime-history-ongoing/property/P10 -->

    <owl:ObjectProperty rdf:about="http://dataforhistory.org/maritime-history-ongoing/property/P10">
        <rdfs:domain rdf:resource="http://dataforhistory.org/maritime-history-ongoing/class/C8"/>
        <rdfs:range rdf:resource="http://dataforhistory.org/maritime-history-ongoing/class/C1"/>
        <rdfs:comment xml:lang="en">To supply a ship with all the equipment, crew, food, etc. </rdfs:comment>
        <rdfs:label xml:lang="en">has set up</rdfs:label>
        <skos:notation rdf:datatype="http://www.w3.org/2001/XMLSchema#string">P10</skos:notation>
    </owl:ObjectProperty>
    


    <!-- http://dataforhistory.org/maritime-history-ongoing/property/P11 -->

    <owl:ObjectProperty rdf:about="http://dataforhistory.org/maritime-history-ongoing/property/P11">
        <rdfs:domain rdf:resource="http://dataforhistory.org/maritime-history-ongoing/class/C6"/>
        <rdfs:range rdf:resource="http://dataforhistory.org/maritime-history-ongoing/class/C5"/>
        <rdfs:comment xml:lang="en">This property associates the transported good</rdfs:comment>
        <rdfs:label xml:lang="en">carried</rdfs:label>
        <skos:notation rdf:datatype="http://www.w3.org/2001/XMLSchema#string">P11</skos:notation>
    </owl:ObjectProperty>
    


    <!-- http://dataforhistory.org/maritime-history-ongoing/property/P12 -->

    <owl:ObjectProperty rdf:about="http://dataforhistory.org/maritime-history-ongoing/property/P12">
        <rdfs:domain rdf:resource="http://www.cidoc-crm.org/cidoc-crm/E21"/>
        <rdfs:range rdf:resource="http://dataforhistory.org/maritime-history-ongoing/class/C1"/>
        <rdfs:comment xml:lang="en">This property is a shortcut for the  Participation – histC25 temporal entity. It just asserts that someone participated in a voyage in some way and for an undefined timespan.</rdfs:comment>
        <rdfs:label xml:lang="en">participated in</rdfs:label>
        <skos:notation rdf:datatype="http://www.w3.org/2001/XMLSchema#string">P12</skos:notation>
    </owl:ObjectProperty>
    


    <!-- http://dataforhistory.org/maritime-history-ongoing/property/P2 -->

    <owl:ObjectProperty rdf:about="http://dataforhistory.org/maritime-history-ongoing/property/P2">
        <rdfs:domain rdf:resource="http://dataforhistory.org/maritime-history-ongoing/class/C1"/>
        <rdfs:range rdf:resource="http://dataforhistory.org/histdmi-generic-ongoing/class/C13"/>
        <rdfs:comment xml:lang="en">This property identifies the C13 Geographical Place which is the final arrival place of a C1 Ship Voyage.</rdfs:comment>
        <rdfs:label xml:lang="en">had arrival place</rdfs:label>
        <skos:notation rdf:datatype="http://www.w3.org/2001/XMLSchema#string">P2</skos:notation>
    </owl:ObjectProperty>
    


    <!-- http://dataforhistory.org/maritime-history-ongoing/property/P3 -->

    <owl:ObjectProperty rdf:about="http://dataforhistory.org/maritime-history-ongoing/property/P3">
        <rdfs:domain rdf:resource="http://dataforhistory.org/maritime-history-ongoing/class/C1"/>
        <rdfs:range rdf:resource="http://dataforhistory.org/maritime-history-ongoing/class/C2"/>
        <rdfs:comment xml:lang="en">This property identifies the C2 Ship by which the C1 Ship Voyage was carried out.</rdfs:comment>
        <rdfs:label xml:lang="en">was carried out by</rdfs:label>
        <skos:notation rdf:datatype="http://www.w3.org/2001/XMLSchema#string">P3</skos:notation>
    </owl:ObjectProperty>
    


    <!-- http://dataforhistory.org/maritime-history-ongoing/property/P4 -->

    <owl:ObjectProperty rdf:about="http://dataforhistory.org/maritime-history-ongoing/property/P4">
        <rdfs:domain rdf:resource="http://dataforhistory.org/maritime-history-ongoing/class/C7"/>
        <rdfs:range rdf:resource="http://dataforhistory.org/histdmi-generic-ongoing/class/C13"/>
        <rdfs:comment xml:lang="en">The place where the stopover takes place</rdfs:comment>
        <rdfs:label xml:lang="en">took place at</rdfs:label>
        <skos:notation rdf:datatype="http://www.w3.org/2001/XMLSchema#string">P4</skos:notation>
    </owl:ObjectProperty>
    


    <!-- http://dataforhistory.org/maritime-history-ongoing/property/P5 -->

    <owl:ObjectProperty rdf:about="http://dataforhistory.org/maritime-history-ongoing/property/P5">
        <rdfs:domain rdf:resource="http://dataforhistory.org/maritime-history-ongoing/class/C7"/>
        <rdfs:range rdf:resource="http://dataforhistory.org/maritime-history-ongoing/class/C1"/>
        <rdfs:comment xml:lang="en">Associates a stopover with the voyage it is part of</rdfs:comment>
        <rdfs:label xml:lang="en">was part of</rdfs:label>
        <skos:notation rdf:datatype="http://www.w3.org/2001/XMLSchema#string">P5</skos:notation>
    </owl:ObjectProperty>
    


    <!-- http://dataforhistory.org/maritime-history-ongoing/property/P6 -->

    <owl:ObjectProperty rdf:about="http://dataforhistory.org/maritime-history-ongoing/property/P6">
        <rdfs:domain rdf:resource="http://dataforhistory.org/maritime-history-ongoing/class/C2"/>
        <rdfs:range rdf:resource="http://dataforhistory.org/maritime-history-ongoing/class/C3"/>
        <rdfs:comment xml:lang="en">Associates a ship with the type which defines its identity</rdfs:comment>
        <rdfs:label xml:lang="en">has ship type</rdfs:label>
        <skos:notation rdf:datatype="http://www.w3.org/2001/XMLSchema#string">P6</skos:notation>
    </owl:ObjectProperty>
    


    <!-- http://dataforhistory.org/maritime-history-ongoing/property/P7 -->

    <owl:ObjectProperty rdf:about="http://dataforhistory.org/maritime-history-ongoing/property/P7">
        <rdfs:domain rdf:resource="http://dataforhistory.org/maritime-history-ongoing/class/C12"/>
        <rdfs:range rdf:resource="http://dataforhistory.org/maritime-history-ongoing/class/C2"/>
        <rdfs:comment xml:lang="en">This property identifies the C2 Ship that came into existence as a result of an C12 Shipbuilding.</rdfs:comment>
        <rdfs:label xml:lang="en">has built</rdfs:label>
        <skos:notation rdf:datatype="http://www.w3.org/2001/XMLSchema#string">P7</skos:notation>
    </owl:ObjectProperty>
    


    <!-- http://dataforhistory.org/maritime-history-ongoing/property/P8 -->

    <owl:ObjectProperty rdf:about="http://dataforhistory.org/maritime-history-ongoing/property/P8">
        <rdfs:domain rdf:resource="http://dataforhistory.org/maritime-history-ongoing/class/C12"/>
        <rdfs:range rdf:resource="http://dataforhistory.org/maritime-history-ongoing/class/C4"/>
        <rdfs:comment xml:lang="en">This property identifies the C4 Shipyard that carried out the C12 Shipbuilding.</rdfs:comment>
        <rdfs:label xml:lang="en">carried out by</rdfs:label>
        <skos:notation rdf:datatype="http://www.w3.org/2001/XMLSchema#string">P8</skos:notation>
    </owl:ObjectProperty>
    


    <!-- http://dataforhistory.org/maritime-history-ongoing/property/P9 -->

    <owl:ObjectProperty rdf:about="http://dataforhistory.org/maritime-history-ongoing/property/P9">
        <rdfs:domain rdf:resource="http://dataforhistory.org/maritime-history-ongoing/class/C6"/>
        <rdfs:range rdf:resource="http://dataforhistory.org/maritime-history-ongoing/class/C1"/>
        <rdfs:comment xml:lang="en">This property associates the transport activity with one or more voyages in which the activity is carried out</rdfs:comment>
        <rdfs:label xml:lang="en">is carried out in the context of</rdfs:label>
        <skos:notation rdf:datatype="http://www.w3.org/2001/XMLSchema#string">P9</skos:notation>
    </owl:ObjectProperty>
    


    <!-- http://www.cidoc-crm.org/cidoc-crm/P1 -->

    <owl:ObjectProperty rdf:about="http://www.cidoc-crm.org/cidoc-crm/P1">
        <rdfs:domain rdf:resource="http://www.cidoc-crm.org/cidoc-crm/E1"/>
        <rdfs:range rdf:resource="http://www.cidoc-crm.org/cidoc-crm/E41"/>
        <rdfs:comment xml:lang="en">This property describes the naming or identification of any real world item by a name or any other identifier. This property is
            intended for identifiers in general use, which form part of the world the model intends to describe, and not merely for internal database
            identifiers which are specific to a technical system, unless these latter also have a more general use outside the technical context. This
            property includes in particular identification by mathematical expressions such as coordinate systems used for the identification of
            instances of E53 Place. The property does not reveal anything about when, where and by whom this identifier was used. A more detailed
            representation can be made using the fully developed (i.e. indirect) path through E15 Identifier Assignment. </rdfs:comment>
        <rdfs:label xml:lang="en">is identified by</rdfs:label>
        <skos:notation rdf:datatype="http://www.w3.org/2001/XMLSchema#string">P1</skos:notation>
    </owl:ObjectProperty>
    


    <!-- http://www.cidoc-crm.org/cidoc-crm/P10 -->

    <owl:ObjectProperty rdf:about="http://www.cidoc-crm.org/cidoc-crm/P10">
        <rdfs:domain rdf:resource="http://www.cidoc-crm.org/cidoc-crm/E92"/>
        <rdfs:range rdf:resource="http://www.cidoc-crm.org/cidoc-crm/E92"/>
        <rdfs:comment xml:lang="en">This property associates an instance of E92 Spacetime Volume with another instance of E92 Spacetime Volume that falls within the
            latter. In other words, all points in the former are also points in the latter. </rdfs:comment>
        <rdfs:label xml:lang="en">falls within</rdfs:label>
        <skos:notation rdf:datatype="http://www.w3.org/2001/XMLSchema#string">P10</skos:notation>
    </owl:ObjectProperty>
    


    <!-- http://www.cidoc-crm.org/cidoc-crm/P100 -->

    <owl:ObjectProperty rdf:about="http://www.cidoc-crm.org/cidoc-crm/P100">
        <rdfs:domain rdf:resource="http://www.cidoc-crm.org/cidoc-crm/E69"/>
        <rdfs:range rdf:resource="http://www.cidoc-crm.org/cidoc-crm/E21"/>
        <rdfs:comment xml:lang="en">This property property links an E69 Death event to the E21 Person that died.</rdfs:comment>
        <rdfs:label xml:lang="en">was death of</rdfs:label>
        <skos:notation rdf:datatype="http://www.w3.org/2001/XMLSchema#string">P100</skos:notation>
    </owl:ObjectProperty>
    


    <!-- http://www.cidoc-crm.org/cidoc-crm/P101 -->

    <owl:ObjectProperty rdf:about="http://www.cidoc-crm.org/cidoc-crm/P101">
        <rdfs:domain rdf:resource="http://www.cidoc-crm.org/cidoc-crm/E70"/>
        <rdfs:range rdf:resource="http://www.cidoc-crm.org/cidoc-crm/E55"/>
        <rdfs:comment xml:lang="en">This property links an instance of E70 Thing to an E55 Type of usage. It allows the relationship between particular things, both
            physical and immaterial, and general methods and techniques of use to be documented. Thus it can be asserted that a baseball bat had a
            general use for sport and a specific use for threatening people during the Great Train Robbery. </rdfs:comment>
        <rdfs:label xml:lang="en">had as general use</rdfs:label>
        <skos:notation rdf:datatype="http://www.w3.org/2001/XMLSchema#string">P101</skos:notation>
    </owl:ObjectProperty>
    


    <!-- http://www.cidoc-crm.org/cidoc-crm/P102 -->

    <owl:ObjectProperty rdf:about="http://www.cidoc-crm.org/cidoc-crm/P102">
        <rdfs:domain rdf:resource="http://www.cidoc-crm.org/cidoc-crm/E71"/>
        <rdfs:range rdf:resource="http://www.cidoc-crm.org/cidoc-crm/E35"/>
        <rdfs:comment xml:lang="en">This property describes the E35 Title applied to an instance of E71 Man-Made Thing. The E55 Type of Title is assigned in a sub
            property. The P102.1 has type property of the P102 has title (is title of) property enables the relationship between the Title and the
            thing to be further clarified, for example, if the Title was a given Title, a supplied Title etc. It allows any man-made material or
            immaterial thing to be given a Title. It is possible to imagine a Title being created without a specific object in mind. </rdfs:comment>
        <rdfs:label xml:lang="en">has title</rdfs:label>
        <skos:notation rdf:datatype="http://www.w3.org/2001/XMLSchema#string">P102</skos:notation>
    </owl:ObjectProperty>
    


    <!-- http://www.cidoc-crm.org/cidoc-crm/P103 -->

    <owl:ObjectProperty rdf:about="http://www.cidoc-crm.org/cidoc-crm/P103">
        <rdfs:domain rdf:resource="http://www.cidoc-crm.org/cidoc-crm/E71"/>
        <rdfs:range rdf:resource="http://www.cidoc-crm.org/cidoc-crm/E55"/>
        <rdfs:comment xml:lang="en">This property links an instance of E71 Man-Made Thing to an E55 Type of usage. It creates a property between specific man-made
            things, both physical and immaterial, to Types of intended methods and techniques of use. Note: A link between specific man-made things
            and a specific use activity should be expressed using P19 was intended use of (was made for).</rdfs:comment>
        <rdfs:label xml:lang="en">was intended for</rdfs:label>
        <skos:notation rdf:datatype="http://www.w3.org/2001/XMLSchema#string">P103</skos:notation>
    </owl:ObjectProperty>
    


    <!-- http://www.cidoc-crm.org/cidoc-crm/P104 -->

    <owl:ObjectProperty rdf:about="http://www.cidoc-crm.org/cidoc-crm/P104">
        <rdfs:domain rdf:resource="http://www.cidoc-crm.org/cidoc-crm/E72"/>
        <rdfs:range rdf:resource="http://www.cidoc-crm.org/cidoc-crm/E30"/>
        <rdfs:comment xml:lang="en">This property links a particular E72 Legal Object to the instances of E30 Right to which it is subject. The Right is held by an
            E39 Actor as described by P75 possesses (is possessed by). </rdfs:comment>
        <rdfs:label xml:lang="en">is subject to</rdfs:label>
        <skos:notation rdf:datatype="http://www.w3.org/2001/XMLSchema#string">P104</skos:notation>
    </owl:ObjectProperty>
    


    <!-- http://www.cidoc-crm.org/cidoc-crm/P105 -->

    <owl:ObjectProperty rdf:about="http://www.cidoc-crm.org/cidoc-crm/P105">
        <rdfs:domain rdf:resource="http://www.cidoc-crm.org/cidoc-crm/E72"/>
        <rdfs:range rdf:resource="http://www.cidoc-crm.org/cidoc-crm/E39"/>
        <rdfs:comment xml:lang="en">This property identifies the E39 Actor who holds the instances of E30 Right to an E72 Legal Object. It is a superproperty of P52
            has current owner (is current owner of) because ownership is a right that is held on the owned object. P105 right held by (has right on)
            is a shortcut of the fully developed path from E72 Legal Object through P104 is subject to (applies to), E30 Right, P75 possesses (is
            possessed by) to E39 Actor. </rdfs:comment>
        <rdfs:label xml:lang="en">right held by</rdfs:label>
        <skos:notation rdf:datatype="http://www.w3.org/2001/XMLSchema#string">P105</skos:notation>
    </owl:ObjectProperty>
    


    <!-- http://www.cidoc-crm.org/cidoc-crm/P106 -->

    <owl:ObjectProperty rdf:about="http://www.cidoc-crm.org/cidoc-crm/P106">
        <rdfs:domain rdf:resource="http://www.cidoc-crm.org/cidoc-crm/E90"/>
        <rdfs:range rdf:resource="http://www.cidoc-crm.org/cidoc-crm/E90"/>
        <rdfs:comment xml:lang="en">This property associates an instance of E90 Symbolic Object with a part of it that is by itself an instance of E90 Symbolic
            Object, such as fragments of texts or clippings from an image. </rdfs:comment>
        <rdfs:label xml:lang="en">is composed of</rdfs:label>
        <skos:notation rdf:datatype="http://www.w3.org/2001/XMLSchema#string">P106</skos:notation>
    </owl:ObjectProperty>
    


    <!-- http://www.cidoc-crm.org/cidoc-crm/P107 -->

    <owl:ObjectProperty rdf:about="http://www.cidoc-crm.org/cidoc-crm/P107">
        <rdfs:domain rdf:resource="http://www.cidoc-crm.org/cidoc-crm/E74"/>
        <rdfs:range rdf:resource="http://www.cidoc-crm.org/cidoc-crm/E39"/>
        <rdfs:comment xml:lang="en">This property relates an E39 Actor to the E74 Group of which that E39 Actor is a member. Groups, Legal Bodies and Persons, may
            all be members of Groups. A Group necessarily consists of more than one member. This property is a shortcut of the more fully developed
            path from E74 Group through P144 joined with (gained member by), E85 Joining, P143 joined (was joined by) to E39 Actor The property P107.1
            kind of member can be used to specify the type of membership or the role the member has in the group. </rdfs:comment>
        <rdfs:label xml:lang="en">has current or former member</rdfs:label>
        <skos:notation rdf:datatype="http://www.w3.org/2001/XMLSchema#string">P107</skos:notation>
    </owl:ObjectProperty>
    


    <!-- http://www.cidoc-crm.org/cidoc-crm/P108 -->

    <owl:ObjectProperty rdf:about="http://www.cidoc-crm.org/cidoc-crm/P108">
        <rdfs:domain rdf:resource="http://www.cidoc-crm.org/cidoc-crm/E12"/>
        <rdfs:range rdf:resource="http://www.cidoc-crm.org/cidoc-crm/E24"/>
        <rdfs:comment xml:lang="en">This property identifies the E24 Physical Man-Made Thing that came into existence as a result of an E12 Production. The identity
            of an instance of E24 Physical Man-Made Thing is not defined by its matter, but by its existence as a subject of documentation. An E12
            Production can result in the creation of multiple instances of E24 Physical Man-Made Thing. </rdfs:comment>
        <rdfs:label xml:lang="en">has produced</rdfs:label>
        <skos:notation rdf:datatype="http://www.w3.org/2001/XMLSchema#string">P108</skos:notation>
    </owl:ObjectProperty>
    


    <!-- http://www.cidoc-crm.org/cidoc-crm/P109 -->

    <owl:ObjectProperty rdf:about="http://www.cidoc-crm.org/cidoc-crm/P109">
        <rdfs:domain rdf:resource="http://www.cidoc-crm.org/cidoc-crm/E78"/>
        <rdfs:range rdf:resource="http://www.cidoc-crm.org/cidoc-crm/E39"/>
        <rdfs:comment xml:lang="en">This property identifies the E39 Actor or Actors who assume or have assumed overall curatorial responsibility for an E78
            Collection. It does not allow a history of curation to be recorded. This would require use of an Event initiating a curator being
            responsible for a Collection. </rdfs:comment>
        <rdfs:label xml:lang="en">has current or former curator</rdfs:label>
        <skos:notation rdf:datatype="http://www.w3.org/2001/XMLSchema#string">P109</skos:notation>
    </owl:ObjectProperty>
    


    <!-- http://www.cidoc-crm.org/cidoc-crm/P11 -->

    <owl:ObjectProperty rdf:about="http://www.cidoc-crm.org/cidoc-crm/P11">
        <rdfs:domain rdf:resource="http://www.cidoc-crm.org/cidoc-crm/E5"/>
        <rdfs:range rdf:resource="http://www.cidoc-crm.org/cidoc-crm/E39"/>
        <rdfs:comment xml:lang="en">This property describes the active or passive participation of instances of E39 Actors in an E5 Event. It connects the life-line
            of the related E39 Actor with the E53 Place and E50 Date of the event. The property implies that the Actor was involved in the event but
            does not imply any causal relationship. The subject of a portrait can be said to have participated in the creation of the portrait. </rdfs:comment>
        <rdfs:label xml:lang="en">had participant</rdfs:label>
        <skos:notation rdf:datatype="http://www.w3.org/2001/XMLSchema#string">P11</skos:notation>
    </owl:ObjectProperty>
    


    <!-- http://www.cidoc-crm.org/cidoc-crm/P110 -->

    <owl:ObjectProperty rdf:about="http://www.cidoc-crm.org/cidoc-crm/P110">
        <rdfs:domain rdf:resource="http://www.cidoc-crm.org/cidoc-crm/E79"/>
        <rdfs:range rdf:resource="http://www.cidoc-crm.org/cidoc-crm/E24"/>
        <rdfs:comment xml:lang="en">This property identifies the E24 Physical Man-Made Thing that is added to (augmented) in an E79 Part Addition. Although a Part
            Addition event normally concerns only one item of Physical Man-Made Thing, it is possible to imagine circumstances under which more than
            one item might be added to (augmented). For example, the artist Jackson Pollock trailing paint onto multiple canvasses. </rdfs:comment>
        <rdfs:label xml:lang="en">augmented</rdfs:label>
        <skos:notation rdf:datatype="http://www.w3.org/2001/XMLSchema#string">P110</skos:notation>
    </owl:ObjectProperty>
    


    <!-- http://www.cidoc-crm.org/cidoc-crm/P111 -->

    <owl:ObjectProperty rdf:about="http://www.cidoc-crm.org/cidoc-crm/P111">
        <rdfs:domain rdf:resource="http://www.cidoc-crm.org/cidoc-crm/E79"/>
        <rdfs:range rdf:resource="http://www.cidoc-crm.org/cidoc-crm/E18"/>
        <rdfs:comment xml:lang="en">This property identifies the E18 Physical Thing that is added during an E79 Part Addition activity </rdfs:comment>
        <rdfs:label xml:lang="en">added</rdfs:label>
        <skos:notation rdf:datatype="http://www.w3.org/2001/XMLSchema#string">P111</skos:notation>
    </owl:ObjectProperty>
    


    <!-- http://www.cidoc-crm.org/cidoc-crm/P112 -->

    <owl:ObjectProperty rdf:about="http://www.cidoc-crm.org/cidoc-crm/P112">
        <rdfs:domain rdf:resource="http://www.cidoc-crm.org/cidoc-crm/E80"/>
        <rdfs:range rdf:resource="http://www.cidoc-crm.org/cidoc-crm/E24"/>
        <rdfs:comment xml:lang="en">This property identifies the E24 Physical Man-Made Thing that was diminished by E80 Part Removal. Although a Part removal
            activity normally concerns only one item of Physical Man-Made Thing, it is possible to imagine circumstances under which more than one
            item might be diminished by a single Part Removal activity. </rdfs:comment>
        <rdfs:label xml:lang="en">diminished</rdfs:label>
        <skos:notation rdf:datatype="http://www.w3.org/2001/XMLSchema#string">P112</skos:notation>
    </owl:ObjectProperty>
    


    <!-- http://www.cidoc-crm.org/cidoc-crm/P113 -->

    <owl:ObjectProperty rdf:about="http://www.cidoc-crm.org/cidoc-crm/P113">
        <rdfs:domain rdf:resource="http://www.cidoc-crm.org/cidoc-crm/E80"/>
        <rdfs:range rdf:resource="http://www.cidoc-crm.org/cidoc-crm/E18"/>
        <rdfs:comment xml:lang="en">This property identifies the E18 Physical Thing that is removed during an E80 Part Removal activity.</rdfs:comment>
        <rdfs:label xml:lang="en">removed</rdfs:label>
        <skos:notation rdf:datatype="http://www.w3.org/2001/XMLSchema#string">P113</skos:notation>
    </owl:ObjectProperty>
    


    <!-- http://www.cidoc-crm.org/cidoc-crm/P114 -->

    <owl:ObjectProperty rdf:about="http://www.cidoc-crm.org/cidoc-crm/P114">
        <rdfs:domain rdf:resource="http://www.cidoc-crm.org/cidoc-crm/E2"/>
        <rdfs:range rdf:resource="http://www.cidoc-crm.org/cidoc-crm/E2"/>
        <rdfs:comment xml:lang="en">This symmetric property allows the instances of E2 Temporal Entity with the same E52 Time-Span to be equated. This property is
            only necessary if the time span is unknown (otherwise the equivalence can be calculated). This property is the same as the &quot;equal&quot;
            relationship of Allen’s temporal logic (Allen, 1983, pp. 832-843). </rdfs:comment>
        <rdfs:label xml:lang="en">is equal in time to</rdfs:label>
        <skos:notation rdf:datatype="http://www.w3.org/2001/XMLSchema#string">P114</skos:notation>
    </owl:ObjectProperty>
    


    <!-- http://www.cidoc-crm.org/cidoc-crm/P115 -->

    <owl:ObjectProperty rdf:about="http://www.cidoc-crm.org/cidoc-crm/P115">
        <rdfs:domain rdf:resource="http://www.cidoc-crm.org/cidoc-crm/E2"/>
        <rdfs:range rdf:resource="http://www.cidoc-crm.org/cidoc-crm/E2"/>
        <rdfs:comment xml:lang="en">This property allows the ending point for a E2 Temporal Entity to be situated by reference to the ending point of another
            temporal entity of longer duration. This property is only necessary if the time span is unknown (otherwise the relationship can be
            calculated). This property is the same as the &quot;finishes / finished-by&quot; relationships of Allen’s temporal logic (Allen, 1983, pp. 832-843). </rdfs:comment>
        <rdfs:label xml:lang="en">finishes</rdfs:label>
        <skos:notation rdf:datatype="http://www.w3.org/2001/XMLSchema#string">P115</skos:notation>
    </owl:ObjectProperty>
    


    <!-- http://www.cidoc-crm.org/cidoc-crm/P116 -->

    <owl:ObjectProperty rdf:about="http://www.cidoc-crm.org/cidoc-crm/P116">
        <rdfs:domain rdf:resource="http://www.cidoc-crm.org/cidoc-crm/E2"/>
        <rdfs:range rdf:resource="http://www.cidoc-crm.org/cidoc-crm/E2"/>
        <rdfs:comment xml:lang="en">This property allows the starting point for a E2 Temporal Entity to be situated by reference to the starting point of another
            temporal entity of longer duration. This property is only necessary if the time span is unknown (otherwise the relationship can be
            calculated). This property is the same as the &quot;starts / started-by&quot; relationships of Allen’s temporal logic (Allen, 1983, pp. 832-843). </rdfs:comment>
        <rdfs:label xml:lang="en">starts</rdfs:label>
        <skos:notation rdf:datatype="http://www.w3.org/2001/XMLSchema#string">P116</skos:notation>
    </owl:ObjectProperty>
    


    <!-- http://www.cidoc-crm.org/cidoc-crm/P117 -->

    <owl:ObjectProperty rdf:about="http://www.cidoc-crm.org/cidoc-crm/P117">
        <rdfs:domain rdf:resource="http://www.cidoc-crm.org/cidoc-crm/E2"/>
        <rdfs:range rdf:resource="http://www.cidoc-crm.org/cidoc-crm/E2"/>
        <rdfs:comment xml:lang="en">This property allows the entire E52 Time-Span of an E2 Temporal Entity to be situated within the Time-Span of another temporal
            entity that starts before and ends after the included temporal entity. This property is only necessary if the time span is unknown
            (otherwise the relationship can be calculated). This property is the same as the &quot;during / includes&quot; relationships of Allen’s temporal
            logic (Allen, 1983, pp. 832-843). </rdfs:comment>
        <rdfs:label xml:lang="en">occurs during</rdfs:label>
        <skos:notation rdf:datatype="http://www.w3.org/2001/XMLSchema#string">P117</skos:notation>
    </owl:ObjectProperty>
    


    <!-- http://www.cidoc-crm.org/cidoc-crm/P118 -->

    <owl:ObjectProperty rdf:about="http://www.cidoc-crm.org/cidoc-crm/P118">
        <rdfs:domain rdf:resource="http://www.cidoc-crm.org/cidoc-crm/E2"/>
        <rdfs:range rdf:resource="http://www.cidoc-crm.org/cidoc-crm/E2"/>
        <rdfs:comment xml:lang="en">This property identifies an overlap between the instances of E52 Time-Span of two instances of E2 Temporal Entity. It implies a
            temporal order between the two entities: if A overlaps in time B, then A must start before B, and B must end after A. This property is
            only necessary if the relevant time spans are unknown (otherwise the relationship can be calculated). This property is the same as the
            &quot;overlaps / overlapped-by&quot; relationships of Allen’s temporal logic (Allen, 1983, pp. 832-843). </rdfs:comment>
        <rdfs:label xml:lang="en">overlaps in time with</rdfs:label>
        <skos:notation rdf:datatype="http://www.w3.org/2001/XMLSchema#string">P118</skos:notation>
    </owl:ObjectProperty>
    


    <!-- http://www.cidoc-crm.org/cidoc-crm/P119 -->

    <owl:ObjectProperty rdf:about="http://www.cidoc-crm.org/cidoc-crm/P119">
        <rdfs:domain rdf:resource="http://www.cidoc-crm.org/cidoc-crm/E2"/>
        <rdfs:range rdf:resource="http://www.cidoc-crm.org/cidoc-crm/E2"/>
        <rdfs:comment xml:lang="en">This property indicates that one E2 Temporal Entity immediately follows another. It implies a particular order between the two
            entities: if A meets in time with B, then A must precede B. This property is only necessary if the relevant time spans are unknown
            (otherwise the relationship can be calculated). This property is the same as the &quot;meets / met-by&quot; relationships of Allen’s temporal logic
            (Allen, 1983, pp. 832-843). </rdfs:comment>
        <rdfs:label xml:lang="en">meets in time with</rdfs:label>
        <skos:notation rdf:datatype="http://www.w3.org/2001/XMLSchema#string">P119</skos:notation>
    </owl:ObjectProperty>
    


    <!-- http://www.cidoc-crm.org/cidoc-crm/P12 -->

    <owl:ObjectProperty rdf:about="http://www.cidoc-crm.org/cidoc-crm/P12">
        <rdfs:domain rdf:resource="http://www.cidoc-crm.org/cidoc-crm/E5"/>
        <rdfs:range rdf:resource="http://www.cidoc-crm.org/cidoc-crm/E77"/>
        <rdfs:comment xml:lang="en">This property describes the active or passive presence of an E77 Persistent Item in an E5 Event without implying any specific
            role. It connects the history of a thing with the E53 Place and E50 Date of an event. For example, an object may be the desk, now in a
            museum on which a treaty was signed. The presence of an immaterial thing implies the presence of at least one of its carriers. </rdfs:comment>
        <rdfs:label xml:lang="en">occurred in the presence of</rdfs:label>
        <skos:notation rdf:datatype="http://www.w3.org/2001/XMLSchema#string">P12</skos:notation>
    </owl:ObjectProperty>
    


    <!-- http://www.cidoc-crm.org/cidoc-crm/P120 -->

    <owl:ObjectProperty rdf:about="http://www.cidoc-crm.org/cidoc-crm/P120">
        <rdfs:domain rdf:resource="http://www.cidoc-crm.org/cidoc-crm/E2"/>
        <rdfs:range rdf:resource="http://www.cidoc-crm.org/cidoc-crm/E2"/>
        <rdfs:comment xml:lang="en">This property identifies the relative chronological sequence of two temporal entities. It implies that a temporal gap exists
            between the end of A and the start of B. This property is only necessary if the relevant time spans are unknown (otherwise the
            relationship can be calculated). This property is the same as the &quot;before / after&quot; relationships of Allen’s temporal logic (Allen, 1983,
            pp. 832-843). </rdfs:comment>
        <rdfs:label xml:lang="en">occurs before</rdfs:label>
        <skos:notation rdf:datatype="http://www.w3.org/2001/XMLSchema#string">P120</skos:notation>
    </owl:ObjectProperty>
    


    <!-- http://www.cidoc-crm.org/cidoc-crm/P121 -->

    <owl:ObjectProperty rdf:about="http://www.cidoc-crm.org/cidoc-crm/P121">
        <rdfs:domain rdf:resource="http://www.cidoc-crm.org/cidoc-crm/E53"/>
        <rdfs:range rdf:resource="http://www.cidoc-crm.org/cidoc-crm/E53"/>
        <rdfs:comment xml:lang="en">This symmetric property allows the instances of E53 Place with overlapping geometric extents to be associated with each other.
            It does not specify anything about the shared area. This property is purely spatial, in contrast to Allen operators, which are purely
            temporal. </rdfs:comment>
        <rdfs:label xml:lang="en">overlaps with</rdfs:label>
        <skos:notation rdf:datatype="http://www.w3.org/2001/XMLSchema#string">P121</skos:notation>
    </owl:ObjectProperty>
    


    <!-- http://www.cidoc-crm.org/cidoc-crm/P122 -->

    <owl:ObjectProperty rdf:about="http://www.cidoc-crm.org/cidoc-crm/P122">
        <rdfs:domain rdf:resource="http://www.cidoc-crm.org/cidoc-crm/E53"/>
        <rdfs:range rdf:resource="http://www.cidoc-crm.org/cidoc-crm/E53"/>
        <rdfs:comment xml:lang="en">This symmetric property allows the instances of E53 Place which share common borders to be related as such. This property is
            purely spatial, in contrast to Allen operators, which are purely temporal. </rdfs:comment>
        <rdfs:label xml:lang="en">borders with</rdfs:label>
        <skos:notation rdf:datatype="http://www.w3.org/2001/XMLSchema#string">P122</skos:notation>
    </owl:ObjectProperty>
    


    <!-- http://www.cidoc-crm.org/cidoc-crm/P123 -->

    <owl:ObjectProperty rdf:about="http://www.cidoc-crm.org/cidoc-crm/P123">
        <rdfs:domain rdf:resource="http://www.cidoc-crm.org/cidoc-crm/E81"/>
        <rdfs:range rdf:resource="http://www.cidoc-crm.org/cidoc-crm/E77"/>
        <rdfs:comment xml:lang="en">This property identifies the E77 Persistent Item or items that are the result of an E81 Transformation. New items replace the
            transformed item or items, which cease to exist as units of documentation. The physical continuity between the old and the new is
            expressed by the link to the common Transformation. </rdfs:comment>
        <rdfs:label xml:lang="en">resulted in</rdfs:label>
        <skos:notation rdf:datatype="http://www.w3.org/2001/XMLSchema#string">P123</skos:notation>
    </owl:ObjectProperty>
    


    <!-- http://www.cidoc-crm.org/cidoc-crm/P124 -->

    <owl:ObjectProperty rdf:about="http://www.cidoc-crm.org/cidoc-crm/P124">
        <rdfs:domain rdf:resource="http://www.cidoc-crm.org/cidoc-crm/E81"/>
        <rdfs:range rdf:resource="http://www.cidoc-crm.org/cidoc-crm/E77"/>
        <rdfs:comment xml:lang="en">This property identifies the E77 Persistent Item or items that cease to exist due to a E81 Transformation. It is replaced by the
            result of the Transformation, which becomes a new unit of documentation. The continuity between both items, the new and the old, is
            expressed by the link to the common Transformation. </rdfs:comment>
        <rdfs:label xml:lang="en">transformed</rdfs:label>
        <skos:notation rdf:datatype="http://www.w3.org/2001/XMLSchema#string">P124</skos:notation>
    </owl:ObjectProperty>
    


    <!-- http://www.cidoc-crm.org/cidoc-crm/P125 -->

    <owl:ObjectProperty rdf:about="http://www.cidoc-crm.org/cidoc-crm/P125">
        <rdfs:domain rdf:resource="http://www.cidoc-crm.org/cidoc-crm/E7"/>
        <rdfs:range rdf:resource="http://www.cidoc-crm.org/cidoc-crm/E55"/>
        <rdfs:comment xml:lang="en">This property defines the kind of objects used in an E7 Activity, when the specific instance is either unknown or not of
            interest, such as use of &quot;a hammer&quot;. </rdfs:comment>
        <rdfs:label xml:lang="en">used object of type</rdfs:label>
        <skos:notation rdf:datatype="http://www.w3.org/2001/XMLSchema#string">P125</skos:notation>
    </owl:ObjectProperty>
    


    <!-- http://www.cidoc-crm.org/cidoc-crm/P126 -->

    <owl:ObjectProperty rdf:about="http://www.cidoc-crm.org/cidoc-crm/P126">
        <rdfs:domain rdf:resource="http://www.cidoc-crm.org/cidoc-crm/E11"/>
        <rdfs:range rdf:resource="http://www.cidoc-crm.org/cidoc-crm/E57"/>
        <rdfs:comment xml:lang="en">This property identifies E57 Material employed in an E11 Modification. The E57 Material used during the E11 Modification does
            not necessarily become incorporated into the E24 Physical Man-Made Thing that forms the subject of the E11 Modification. </rdfs:comment>
        <rdfs:label xml:lang="en">employed</rdfs:label>
        <skos:notation rdf:datatype="http://www.w3.org/2001/XMLSchema#string">P126</skos:notation>
    </owl:ObjectProperty>
    


    <!-- http://www.cidoc-crm.org/cidoc-crm/P127 -->

    <owl:ObjectProperty rdf:about="http://www.cidoc-crm.org/cidoc-crm/P127">
        <rdfs:domain rdf:resource="http://www.cidoc-crm.org/cidoc-crm/E55"/>
        <rdfs:range rdf:resource="http://www.cidoc-crm.org/cidoc-crm/E55"/>
        <rdfs:comment xml:lang="en">This property identifies a super-Type to which an E55 Type is related. It allows Types to be organised into hierarchies. This is
            the sense of &quot;broader term generic (BTG)&quot; as defined in ISO 2788 </rdfs:comment>
        <rdfs:label xml:lang="en">has broader term</rdfs:label>
        <skos:notation rdf:datatype="http://www.w3.org/2001/XMLSchema#string">P127</skos:notation>
    </owl:ObjectProperty>
    


    <!-- http://www.cidoc-crm.org/cidoc-crm/P128 -->

    <owl:ObjectProperty rdf:about="http://www.cidoc-crm.org/cidoc-crm/P128">
        <rdfs:domain rdf:resource="http://www.cidoc-crm.org/cidoc-crm/E18"/>
        <rdfs:range rdf:resource="http://www.cidoc-crm.org/cidoc-crm/E90"/>
        <rdfs:comment xml:lang="en">This property identifies an E90 Symbolic Object carried by an instance of E18 Physical Thing. </rdfs:comment>
        <rdfs:label xml:lang="en">carries</rdfs:label>
        <skos:notation rdf:datatype="http://www.w3.org/2001/XMLSchema#string">P128</skos:notation>
    </owl:ObjectProperty>
    


    <!-- http://www.cidoc-crm.org/cidoc-crm/P129 -->

    <owl:ObjectProperty rdf:about="http://www.cidoc-crm.org/cidoc-crm/P129">
        <rdfs:domain rdf:resource="http://www.cidoc-crm.org/cidoc-crm/E89"/>
        <rdfs:range rdf:resource="http://www.cidoc-crm.org/cidoc-crm/E1"/>
        <rdfs:comment xml:lang="en">This property documents that an E89 Propositional Object has as subject an instance of E1 CRM Entity. </rdfs:comment>
        <rdfs:label xml:lang="en">is about</rdfs:label>
        <skos:notation rdf:datatype="http://www.w3.org/2001/XMLSchema#string">P129</skos:notation>
    </owl:ObjectProperty>
    


    <!-- http://www.cidoc-crm.org/cidoc-crm/P13 -->

    <owl:ObjectProperty rdf:about="http://www.cidoc-crm.org/cidoc-crm/P13">
        <rdfs:domain rdf:resource="http://www.cidoc-crm.org/cidoc-crm/E6"/>
        <rdfs:range rdf:resource="http://www.cidoc-crm.org/cidoc-crm/E18"/>
        <rdfs:comment xml:lang="en">This property allows specific instances of E18 Physical Thing that have been destroyed to be related to a destruction event.
            Destruction implies the end of an item’s life as a subject of cultural documentation – the physical matter of which the item was composed
            may in fact continue to exist. A destruction event may be contiguous with a Production that brings into existence a derived object
            composed partly of matter from the destroyed object. </rdfs:comment>
        <rdfs:label xml:lang="en">destroyed</rdfs:label>
        <skos:notation rdf:datatype="http://www.w3.org/2001/XMLSchema#string">P13</skos:notation>
    </owl:ObjectProperty>
    


    <!-- http://www.cidoc-crm.org/cidoc-crm/P130 -->

    <owl:ObjectProperty rdf:about="http://www.cidoc-crm.org/cidoc-crm/P130">
        <rdfs:domain rdf:resource="http://www.cidoc-crm.org/cidoc-crm/E70"/>
        <rdfs:range rdf:resource="http://www.cidoc-crm.org/cidoc-crm/E70"/>
        <rdfs:comment xml:lang="en">This property generalises the notions of &quot;copy of&quot; and &quot;similar to&quot; into a dynamic, asymmetric relationship, where the domain
            expresses the derivative, if such a direction can be established. Otherwise, the relationship is symmetric. It is a short-cut of P15 was
            influenced by (influenced) in a creation or production, if such a reason for the similarity can be verified. Moreover it expresses
            similarity in cases that can be stated between two objects only, without historical knowledge about its reasons. </rdfs:comment>
        <rdfs:label xml:lang="en">shows features of</rdfs:label>
        <skos:notation rdf:datatype="http://www.w3.org/2001/XMLSchema#string">P130</skos:notation>
    </owl:ObjectProperty>
    


    <!-- http://www.cidoc-crm.org/cidoc-crm/P131 -->

    <owl:ObjectProperty rdf:about="http://www.cidoc-crm.org/cidoc-crm/P131">
        <rdfs:domain rdf:resource="http://www.cidoc-crm.org/cidoc-crm/E39"/>
        <rdfs:range rdf:resource="http://www.cidoc-crm.org/cidoc-crm/E82"/>
        <rdfs:comment xml:lang="en">This property identifies a name used specifically to identify an E39 Actor. This property is a specialisation of P1 is
            identified by (identifies) is identified by. </rdfs:comment>
        <rdfs:label xml:lang="en">is identified by</rdfs:label>
        <skos:notation rdf:datatype="http://www.w3.org/2001/XMLSchema#string">P131</skos:notation>
    </owl:ObjectProperty>
    


    <!-- http://www.cidoc-crm.org/cidoc-crm/P132 -->

    <owl:ObjectProperty rdf:about="http://www.cidoc-crm.org/cidoc-crm/P132">
        <rdfs:domain rdf:resource="http://www.cidoc-crm.org/cidoc-crm/E92"/>
        <rdfs:range rdf:resource="http://www.cidoc-crm.org/cidoc-crm/E92"/>
        <rdfs:comment xml:lang="en">This symmetric property allows instances of E4 Period that overlap both temporally and spatially to be related, i,e. they share
            some spatio-temporal extent. This property does not imply any ordering or sequence between the two periods, either spatial or temporal. </rdfs:comment>
        <rdfs:label xml:lang="en">overlaps with</rdfs:label>
        <skos:notation rdf:datatype="http://www.w3.org/2001/XMLSchema#string">P132</skos:notation>
    </owl:ObjectProperty>
    


    <!-- http://www.cidoc-crm.org/cidoc-crm/P133 -->

    <owl:ObjectProperty rdf:about="http://www.cidoc-crm.org/cidoc-crm/P133">
        <rdfs:domain rdf:resource="http://www.cidoc-crm.org/cidoc-crm/E92"/>
        <rdfs:range rdf:resource="http://www.cidoc-crm.org/cidoc-crm/E92"/>
        <rdfs:comment xml:lang="en">This symmetric property allows instances of E4 Period that do not overlap both temporally and spatially, to be related i,e. they
            do not share any spatio-temporal extent. This property does not imply any ordering or sequence between the two periods either spatial or
            temporal. </rdfs:comment>
        <rdfs:label xml:lang="en">is separated from</rdfs:label>
        <skos:notation rdf:datatype="http://www.w3.org/2001/XMLSchema#string">P133</skos:notation>
    </owl:ObjectProperty>
    


    <!-- http://www.cidoc-crm.org/cidoc-crm/P134 -->

    <owl:ObjectProperty rdf:about="http://www.cidoc-crm.org/cidoc-crm/P134">
        <rdfs:domain rdf:resource="http://www.cidoc-crm.org/cidoc-crm/E7"/>
        <rdfs:range rdf:resource="http://www.cidoc-crm.org/cidoc-crm/E7"/>
        <rdfs:comment xml:lang="en">This property associates two instances of E7 Activity, where the domain is considered as an intentional continuation of the
            range. A continuation of an activity may happen when the continued activity is still ongoing or after the continued activity has
            completely ended. The continuing activity may have started already before it decided to continue the other one. Continuation implies a
            coherence of intentions and outcomes of the involved activities. </rdfs:comment>
        <rdfs:label xml:lang="en">continued</rdfs:label>
        <skos:notation rdf:datatype="http://www.w3.org/2001/XMLSchema#string">P134</skos:notation>
    </owl:ObjectProperty>
    


    <!-- http://www.cidoc-crm.org/cidoc-crm/P135 -->

    <owl:ObjectProperty rdf:about="http://www.cidoc-crm.org/cidoc-crm/P135">
        <rdfs:domain rdf:resource="http://www.cidoc-crm.org/cidoc-crm/E83"/>
        <rdfs:range rdf:resource="http://www.cidoc-crm.org/cidoc-crm/E55"/>
        <rdfs:comment xml:lang="en">This property identifies the E55 Type, which is created in an E83Type Creation activity.</rdfs:comment>
        <rdfs:label xml:lang="en">created type</rdfs:label>
        <skos:notation rdf:datatype="http://www.w3.org/2001/XMLSchema#string">P135</skos:notation>
    </owl:ObjectProperty>
    


    <!-- http://www.cidoc-crm.org/cidoc-crm/P136 -->

    <owl:ObjectProperty rdf:about="http://www.cidoc-crm.org/cidoc-crm/P136">
        <rdfs:domain rdf:resource="http://www.cidoc-crm.org/cidoc-crm/E83"/>
        <rdfs:range rdf:resource="http://www.cidoc-crm.org/cidoc-crm/E1"/>
        <rdfs:comment xml:lang="en">This property identifies one or more items that were used as evidence to declare a new E55 Type. The examination of these items
            is often the only objective way to understand the precise characteristics of a new Type. Such items should be deposited in a museum or
            similar institution for that reason. The taxonomic role renders the specific relationship of each item to the Type, such as &quot;holotype&quot; or
            &quot;original element&quot;. </rdfs:comment>
        <rdfs:label xml:lang="en">was based on</rdfs:label>
        <skos:notation rdf:datatype="http://www.w3.org/2001/XMLSchema#string">P136</skos:notation>
    </owl:ObjectProperty>
    


    <!-- http://www.cidoc-crm.org/cidoc-crm/P137 -->

    <owl:ObjectProperty rdf:about="http://www.cidoc-crm.org/cidoc-crm/P137">
        <rdfs:domain rdf:resource="http://www.cidoc-crm.org/cidoc-crm/E1"/>
        <rdfs:range rdf:resource="http://www.cidoc-crm.org/cidoc-crm/E55"/>
        <rdfs:comment xml:lang="en">This property allows an item to be declared as a particular example of an E55 Type or taxon The P137.1 in the taxonomic role
            property of P137 exemplifies (is exemplified by) allows differentiation of taxonomic roles. The taxonomic role renders the specific
            relationship of this example to the Type, such as &quot;prototypical&quot;, &quot;archetypical&quot;, &quot;lectotype&quot;, etc. The taxonomic role &quot;lectotype&quot; is not
            associated with the Type Creation (E83) itself, but selected in a later phase. </rdfs:comment>
        <rdfs:label xml:lang="en">exemplifies</rdfs:label>
        <skos:notation rdf:datatype="http://www.w3.org/2001/XMLSchema#string">P137</skos:notation>
    </owl:ObjectProperty>
    


    <!-- http://www.cidoc-crm.org/cidoc-crm/P138 -->

    <owl:ObjectProperty rdf:about="http://www.cidoc-crm.org/cidoc-crm/P138">
        <rdfs:domain rdf:resource="http://www.cidoc-crm.org/cidoc-crm/E36"/>
        <rdfs:range rdf:resource="http://www.cidoc-crm.org/cidoc-crm/E1"/>
        <rdfs:comment xml:lang="en">This property establishes the relationship between an E36 Visual Item and the entity that it visually represents. Any entity may
            be represented visually. This property is part of the fully developed path from E24 Physical Man-Made Thing through P65 shows visual item
            (is shown by), E36 Visual Item, P138 represents (has representation) to E1 CRM Entity, which is shortcut by P62depicts (is depicted by).
            P138.1 mode of representation allows the nature of the representation to be refined. This property is also used for the relationship
            between an original and a digitisation of the original by the use of techniques such as digital photography, flatbed or infrared scanning.
            Digitisation is here seen as a process with a mechanical, causal component rendering the spatial distribution of structural and optical
            properties of the original and does not necessarily include any visual similarity identifiable by human observation. </rdfs:comment>
        <rdfs:label xml:lang="en">represents</rdfs:label>
        <skos:notation rdf:datatype="http://www.w3.org/2001/XMLSchema#string">P138</skos:notation>
    </owl:ObjectProperty>
    


    <!-- http://www.cidoc-crm.org/cidoc-crm/P139 -->

    <owl:ObjectProperty rdf:about="http://www.cidoc-crm.org/cidoc-crm/P139">
        <rdfs:domain rdf:resource="http://www.cidoc-crm.org/cidoc-crm/E41"/>
        <rdfs:range rdf:resource="http://www.cidoc-crm.org/cidoc-crm/E41"/>
        <rdfs:comment xml:lang="en">This property establishes a relationship of equivalence between two instances of E41 Appellation independent from any item
            identified by them. It is a dynamic asymmetric relationship, where the range expresses the derivative, if such a direction can be
            established. Otherwise, the relationship is symmetric. The relationship is not transitive. The equivalence applies to all cases of use of
            an instance of E41 Appellation. Multiple names assigned to an object, which are not equivalent for all things identified with a specific
            instance of E41 Appellation, should be modelled as repeated values of P1 is identified by (identifies). P139.1 has type allows the type of
            derivation, such as “transliteration from Latin 1 to ASCII” be refined.. </rdfs:comment>
        <rdfs:label xml:lang="en">has alternative form</rdfs:label>
        <skos:notation rdf:datatype="http://www.w3.org/2001/XMLSchema#string">P139</skos:notation>
    </owl:ObjectProperty>
    


    <!-- http://www.cidoc-crm.org/cidoc-crm/P14 -->

    <owl:ObjectProperty rdf:about="http://www.cidoc-crm.org/cidoc-crm/P14">
        <rdfs:domain rdf:resource="http://www.cidoc-crm.org/cidoc-crm/E7"/>
        <rdfs:range rdf:resource="http://www.cidoc-crm.org/cidoc-crm/E39"/>
        <rdfs:comment xml:lang="en">This property describes the active participation of an E39 Actor in an E7 Activity. It implies causal or legal responsibility.
            The P14.1 in the role of property of the property allows the nature of an Actor’s participation to be specified. </rdfs:comment>
        <rdfs:label xml:lang="en">carried out by</rdfs:label>
        <skos:notation rdf:datatype="http://www.w3.org/2001/XMLSchema#string">P14</skos:notation>
    </owl:ObjectProperty>
    


    <!-- http://www.cidoc-crm.org/cidoc-crm/P140 -->

    <owl:ObjectProperty rdf:about="http://www.cidoc-crm.org/cidoc-crm/P140">
        <rdfs:domain rdf:resource="http://www.cidoc-crm.org/cidoc-crm/E13"/>
        <rdfs:range rdf:resource="http://www.cidoc-crm.org/cidoc-crm/E1"/>
        <rdfs:comment xml:lang="en">This property indicates the item to which an attribute or relation is assigned. </rdfs:comment>
        <rdfs:label xml:lang="en">assigned attribute to</rdfs:label>
        <skos:notation rdf:datatype="http://www.w3.org/2001/XMLSchema#string">P140</skos:notation>
    </owl:ObjectProperty>
    


    <!-- http://www.cidoc-crm.org/cidoc-crm/P141 -->

    <owl:ObjectProperty rdf:about="http://www.cidoc-crm.org/cidoc-crm/P141">
        <rdfs:domain rdf:resource="http://www.cidoc-crm.org/cidoc-crm/E13"/>
        <rdfs:range rdf:resource="http://www.cidoc-crm.org/cidoc-crm/E1"/>
        <rdfs:comment xml:lang="en">This property indicates the attribute that was assigned or the item that was related to the item denoted by a property P140
            assigned attribute to in an Attribute assignment action. </rdfs:comment>
        <rdfs:label xml:lang="en">assigned</rdfs:label>
        <skos:notation rdf:datatype="http://www.w3.org/2001/XMLSchema#string">P141</skos:notation>
    </owl:ObjectProperty>
    


    <!-- http://www.cidoc-crm.org/cidoc-crm/P142 -->

    <owl:ObjectProperty rdf:about="http://www.cidoc-crm.org/cidoc-crm/P142">
        <rdfs:domain rdf:resource="http://www.cidoc-crm.org/cidoc-crm/E15"/>
        <rdfs:range rdf:resource="http://www.cidoc-crm.org/cidoc-crm/E90"/>
        <rdfs:comment xml:lang="en">This property associates the event of assigning an instance of E42 Identifier to an entity, with the instances of E41
            Appellation that were used as elements of the identifier. </rdfs:comment>
        <rdfs:label xml:lang="en">used constituent</rdfs:label>
        <skos:notation rdf:datatype="http://www.w3.org/2001/XMLSchema#string">P142</skos:notation>
    </owl:ObjectProperty>
    


    <!-- http://www.cidoc-crm.org/cidoc-crm/P143 -->

    <owl:ObjectProperty rdf:about="http://www.cidoc-crm.org/cidoc-crm/P143">
        <rdfs:domain rdf:resource="http://www.cidoc-crm.org/cidoc-crm/E85"/>
        <rdfs:range rdf:resource="http://www.cidoc-crm.org/cidoc-crm/E39"/>
        <rdfs:comment xml:lang="en">This property identifies the instance of E39 Actor that becomes member of a E74 Group in an E85 Joining. Joining events allow
            for describing people becoming members of a group with a more detailed path from E74 Group through P144 joined with (gained member by),
            E85 Joining, P143 joined (was joined by) to E39 Actor, compared to the shortcut offered by P107 has current or former member (is current
            or former member of). </rdfs:comment>
        <rdfs:label xml:lang="en">joined</rdfs:label>
        <skos:notation rdf:datatype="http://www.w3.org/2001/XMLSchema#string">P143</skos:notation>
    </owl:ObjectProperty>
    


    <!-- http://www.cidoc-crm.org/cidoc-crm/P144 -->

    <owl:ObjectProperty rdf:about="http://www.cidoc-crm.org/cidoc-crm/P144">
        <rdfs:domain rdf:resource="http://www.cidoc-crm.org/cidoc-crm/E85"/>
        <rdfs:range rdf:resource="http://www.cidoc-crm.org/cidoc-crm/E74"/>
        <rdfs:comment xml:lang="en">This property identifies the instance of E74 Group of which an instance of E39 Actor becomes a member through an instance of E85
            Joining. Although a Joining activity normally concerns only one instance of E74 Group, it is possible to imagine circumstances under which
            becoming member of one Group implies becoming member of another Group as well. Joining events allow for describing people becoming members
            of a group with a more detailed path from E74 Group through P144 joined with (gained member by), E85 Joining, P143 joined (was joined by)
            to E39 Actor, compared to the shortcut offered by P107 has current or former member (is current or former member of). The property P144.1
            kind of member can be used to specify the type of membership or the role the member has in the group. </rdfs:comment>
        <rdfs:label xml:lang="en">joined with</rdfs:label>
        <skos:notation rdf:datatype="http://www.w3.org/2001/XMLSchema#string">P144</skos:notation>
    </owl:ObjectProperty>
    


    <!-- http://www.cidoc-crm.org/cidoc-crm/P145 -->

    <owl:ObjectProperty rdf:about="http://www.cidoc-crm.org/cidoc-crm/P145">
        <rdfs:domain rdf:resource="http://www.cidoc-crm.org/cidoc-crm/E86"/>
        <rdfs:range rdf:resource="http://www.cidoc-crm.org/cidoc-crm/E39"/>
        <rdfs:comment xml:lang="en">This property identifies the instance of E39 Actor that leaves an instance of E74 Group through an instance of E86
            Leaving.</rdfs:comment>
        <rdfs:label xml:lang="en">separated</rdfs:label>
        <skos:notation rdf:datatype="http://www.w3.org/2001/XMLSchema#string">P145</skos:notation>
    </owl:ObjectProperty>
    


    <!-- http://www.cidoc-crm.org/cidoc-crm/P146 -->

    <owl:ObjectProperty rdf:about="http://www.cidoc-crm.org/cidoc-crm/P146">
        <rdfs:domain rdf:resource="http://www.cidoc-crm.org/cidoc-crm/E86"/>
        <rdfs:range rdf:resource="http://www.cidoc-crm.org/cidoc-crm/E74"/>
        <rdfs:comment xml:lang="en">This property identifies the instance of E74 Group an instance of E39 Actor leaves through an instance of E86 Leaving. Although
            a Leaving activity normally concerns only one instance of E74 Group, it is possible to imagine circumstances under which leaving one E74
            Group implies leaving another E74 Group as well. </rdfs:comment>
        <rdfs:label xml:lang="en">separated from</rdfs:label>
        <skos:notation rdf:datatype="http://www.w3.org/2001/XMLSchema#string">P146</skos:notation>
    </owl:ObjectProperty>
    


    <!-- http://www.cidoc-crm.org/cidoc-crm/P147 -->

    <owl:ObjectProperty rdf:about="http://www.cidoc-crm.org/cidoc-crm/P147">
        <rdfs:domain rdf:resource="http://www.cidoc-crm.org/cidoc-crm/E87"/>
        <rdfs:range rdf:resource="http://www.cidoc-crm.org/cidoc-crm/E78"/>
        <rdfs:comment xml:lang="en">This property associates an instance of E87 Curation Activity with the instance of E78 Collection that is subject of that
            curation activity. </rdfs:comment>
        <rdfs:label xml:lang="en">curated</rdfs:label>
        <skos:notation rdf:datatype="http://www.w3.org/2001/XMLSchema#string">P147</skos:notation>
    </owl:ObjectProperty>
    


    <!-- http://www.cidoc-crm.org/cidoc-crm/P148 -->

    <owl:ObjectProperty rdf:about="http://www.cidoc-crm.org/cidoc-crm/P148">
        <rdfs:domain rdf:resource="http://www.cidoc-crm.org/cidoc-crm/E89"/>
        <rdfs:range rdf:resource="http://www.cidoc-crm.org/cidoc-crm/E89"/>
        <rdfs:comment xml:lang="en">This property associates an instance of E89 Propositional Object with a structural part of it that is by itself an instance of
            E89 Propositional Object.</rdfs:comment>
        <rdfs:label xml:lang="en">has component</rdfs:label>
        <skos:notation rdf:datatype="http://www.w3.org/2001/XMLSchema#string">P148</skos:notation>
    </owl:ObjectProperty>
    


    <!-- http://www.cidoc-crm.org/cidoc-crm/P149 -->

    <owl:ObjectProperty rdf:about="http://www.cidoc-crm.org/cidoc-crm/P149">
        <rdfs:domain rdf:resource="http://www.cidoc-crm.org/cidoc-crm/E28"/>
        <rdfs:range rdf:resource="http://www.cidoc-crm.org/cidoc-crm/E75"/>
        <rdfs:comment xml:lang="en">This property identifies an instance of E28 Conceptual Object using an instance of E75 Conceptual Object
            Appellation.</rdfs:comment>
        <rdfs:label xml:lang="en">is identified by</rdfs:label>
        <skos:notation rdf:datatype="http://www.w3.org/2001/XMLSchema#string">P149</skos:notation>
    </owl:ObjectProperty>
    


    <!-- http://www.cidoc-crm.org/cidoc-crm/P15 -->

    <owl:ObjectProperty rdf:about="http://www.cidoc-crm.org/cidoc-crm/P15">
        <rdfs:domain rdf:resource="http://www.cidoc-crm.org/cidoc-crm/E7"/>
        <rdfs:range rdf:resource="http://www.cidoc-crm.org/cidoc-crm/E1"/>
        <rdfs:comment xml:lang="en">This is a high level property, which captures the relationship between an E7 Activity and anything that may have had some
            bearing upon it. The property has more specific sub properties. </rdfs:comment>
        <rdfs:label xml:lang="en">was influenced by</rdfs:label>
        <skos:notation rdf:datatype="http://www.w3.org/2001/XMLSchema#string">P15</skos:notation>
    </owl:ObjectProperty>
    


    <!-- http://www.cidoc-crm.org/cidoc-crm/P150 -->

    <owl:ObjectProperty rdf:about="http://www.cidoc-crm.org/cidoc-crm/P150">
        <rdfs:domain rdf:resource="http://www.cidoc-crm.org/cidoc-crm/E55"/>
        <rdfs:range rdf:resource="http://www.cidoc-crm.org/cidoc-crm/E55"/>
        <rdfs:comment xml:lang="en">The property &quot;broaderPartitive&quot; associates an instance of E55 Type “A” with an instance of E55 Type “B”, when items of type “A”
            typically form part of items of type “B”, such as “car motors” and “cars”. It allows Types to be organised into hierarchies. This is the
            sense of &quot;broader term partitive (BTP)&quot; as defined in ISO 2788 and “broaderPartitive” in SKOS. </rdfs:comment>
        <rdfs:label xml:lang="en">defines typical parts of</rdfs:label>
        <skos:notation rdf:datatype="http://www.w3.org/2001/XMLSchema#string">P150</skos:notation>
    </owl:ObjectProperty>
    


    <!-- http://www.cidoc-crm.org/cidoc-crm/P151 -->

    <owl:ObjectProperty rdf:about="http://www.cidoc-crm.org/cidoc-crm/P151">
        <rdfs:domain rdf:resource="http://www.cidoc-crm.org/cidoc-crm/E66"/>
        <rdfs:range rdf:resource="http://www.cidoc-crm.org/cidoc-crm/E74"/>
        <rdfs:comment xml:lang="en">This property associates an instance of E66 Formation with an instance of E74 Group from which the new group was formed
            preserving a sense of continuity such as in mission, membership or tradition. </rdfs:comment>
        <rdfs:label xml:lang="en">was formed from</rdfs:label>
        <skos:notation rdf:datatype="http://www.w3.org/2001/XMLSchema#string">P151</skos:notation>
    </owl:ObjectProperty>
    


    <!-- http://www.cidoc-crm.org/cidoc-crm/P152 -->

    <owl:ObjectProperty rdf:about="http://www.cidoc-crm.org/cidoc-crm/P152">
        <rdfs:domain rdf:resource="http://www.cidoc-crm.org/cidoc-crm/E21"/>
        <rdfs:range rdf:resource="http://www.cidoc-crm.org/cidoc-crm/E21"/>
        <rdfs:comment xml:lang="en">This property associates an instance of E21 Person with another instance of E21 Person who plays the role of the first instance’s parent, regardless of whether the relationship is biological parenthood, assumed or pretended biological parenthood or an equivalent legal status of rights and obligations obtained by a social or legal act.
This property is, among others, a shortcut of the
            fully developed paths from ‘E21Person’ through ‘P98i was born’, ‘E67 Birth’, ‘P96 by mother’ to ‘E21 Person’, and from ‘E21Person’ through
            ‘P98i was born’, ‘E67 Birth’, ‘P97 from father’ to ‘E21 Person’.</rdfs:comment>
        <rdfs:label xml:lang="en">has parent</rdfs:label>
        <skos:notation rdf:datatype="http://www.w3.org/2001/XMLSchema#string">P152</skos:notation>
    </owl:ObjectProperty>
    


    <!-- http://www.cidoc-crm.org/cidoc-crm/P156 -->

    <owl:ObjectProperty rdf:about="http://www.cidoc-crm.org/cidoc-crm/P156">
        <rdfs:domain rdf:resource="http://www.cidoc-crm.org/cidoc-crm/E18"/>
        <rdfs:range rdf:resource="http://www.cidoc-crm.org/cidoc-crm/E53"/>
        <rdfs:comment xml:lang="en">This property describes the largest volume in space that an instance of E18 Physical Thing has occupied at any time during its
            existence, with respect to the reference space relative to itself. This allows you to describe the thing itself as a place that may
            contain other things, such as a box that may contain coins. In other words, it is the volume that contains all the points which the thing
            has covered at some time during its existence. In the case of an E26 Physical Feature the default reference space is the one in which the
            object that bears the feature or at least the surrounding matter of the feature is at rest. In this case there is a 1:1 relation of E26
            Feature and E53 Place. For simplicity of implementation multiple inheritance (E26 Feature IsA E53 Place) may be a practical approach. For
            instances of E19 Physical Objects the default reference space is the one which is at rest to the object itself, i.e. which moves together
            with the object. We include in the occupied space the space filled by the matter of the physical thing and all its inner spaces. This
            property is a subproperty of P161 has spatial projection because it refers to its own domain as reference space for its range, whereas
            P161 has spatial projection may refer to a place in terms of any reference space. For some instances of E18 Physical Object the relative
            stability of form may not be sufficient to define a useful local reference space, for instance for an amoeba. In such cases the fully
            developed path to an external reference space and using a temporal validity component may be adequate to determine the place they have
            occupied. In contrast to P156 occupies, the property P53 has former or current location identifies an instance of E53 Place at which a
            thing is or has been for some unspecified time span. Further it does not constrain the reference space of the referred instance of P53
            Place. </rdfs:comment>
        <rdfs:label xml:lang="en">occupies</rdfs:label>
        <skos:notation rdf:datatype="http://www.w3.org/2001/XMLSchema#string">P156</skos:notation>
    </owl:ObjectProperty>
    


    <!-- http://www.cidoc-crm.org/cidoc-crm/P157 -->

    <owl:ObjectProperty rdf:about="http://www.cidoc-crm.org/cidoc-crm/P157">
        <rdfs:domain rdf:resource="http://www.cidoc-crm.org/cidoc-crm/E53"/>
        <rdfs:range rdf:resource="http://www.cidoc-crm.org/cidoc-crm/E18"/>
        <rdfs:comment xml:lang="en">This property associates an instance of P53 Place with the instance of E18 Physical Thing that determines a reference space for
            this instance of P53 Place by being at rest with respect to this reference space. The relative stability of form of an E18 Physical Thing
            defines its default reference space. The reference space is not spatially limited to the referred thing. For example, a ship determines a
            reference space in terms of which other ships in its neighbourhood may be described. Larger constellations of matter, such as continental
            plates, may comprise many physical features that are at rest with them and define the same reference space. </rdfs:comment>
        <rdfs:label xml:lang="en">is at rest relative to</rdfs:label>
        <skos:notation rdf:datatype="http://www.w3.org/2001/XMLSchema#string">P157</skos:notation>
    </owl:ObjectProperty>
    


    <!-- http://www.cidoc-crm.org/cidoc-crm/P16 -->

    <owl:ObjectProperty rdf:about="http://www.cidoc-crm.org/cidoc-crm/P16">
        <rdfs:domain rdf:resource="http://www.cidoc-crm.org/cidoc-crm/E7"/>
        <rdfs:range rdf:resource="http://www.cidoc-crm.org/cidoc-crm/E70"/>
        <rdfs:comment xml:lang="en">This property describes the use of material or immaterial things in a way essential to the performance or the outcome of an E7
            Activity. This property typically applies to tools, instruments, moulds, raw materials and items embedded in a product. It implies that
            the presence of the object in question was a necessary condition for the action. For example, the activity of writing this text required
            the use of a computer. An immaterial thing can be used if at least one of its carriers is present. For example, the software tools on a
            computer. Another example is the use of a particular name by a particular group of people over some span to identify a thing, such as a
            settlement. In this case, the physical carriers of this name are at least the people understanding its use. </rdfs:comment>
        <rdfs:label xml:lang="en">used specific object</rdfs:label>
        <skos:notation rdf:datatype="http://www.w3.org/2001/XMLSchema#string">P16</skos:notation>
    </owl:ObjectProperty>
    


    <!-- http://www.cidoc-crm.org/cidoc-crm/P160 -->

    <owl:ObjectProperty rdf:about="http://www.cidoc-crm.org/cidoc-crm/P160">
        <rdfs:domain rdf:resource="http://www.cidoc-crm.org/cidoc-crm/E92"/>
        <rdfs:range rdf:resource="http://www.cidoc-crm.org/cidoc-crm/E52"/>
        <rdfs:comment xml:lang="en">This property describes the temporal projection of an instance of an E92 Spacetime Volume. The property P4 has time-span is the
            same as P160 has temporal projection if it is used to document an instance of E4 Period or any subclass of it. </rdfs:comment>
        <rdfs:label xml:lang="en">has temporal projection</rdfs:label>
        <skos:notation rdf:datatype="http://www.w3.org/2001/XMLSchema#string">P160</skos:notation>
    </owl:ObjectProperty>
    


    <!-- http://www.cidoc-crm.org/cidoc-crm/P161 -->

    <owl:ObjectProperty rdf:about="http://www.cidoc-crm.org/cidoc-crm/P161">
        <rdfs:domain rdf:resource="http://www.cidoc-crm.org/cidoc-crm/E92"/>
        <rdfs:range rdf:resource="http://www.cidoc-crm.org/cidoc-crm/E53"/>
        <rdfs:comment xml:lang="en">This property associates an instance of a E92 Spacetime Volume with an instance of E53 Place that is the result of the spatial
            projection of the instance of a E92 Spacetime Volume on a reference space. In general there can be more than one useful reference space to
            describe the spatial projection of a spacetime volume, such as that of a battle ship versus that of the seafloor. Therefore the projection
            is not unique. This is part of the fully developed path that is shortcut by P7took place at (witnessed).The more fully developed path from
            E4 Period through P161 has spatial projection, E53 Place, P89 falls within (contains) to E53 Place. </rdfs:comment>
        <rdfs:label xml:lang="en">has spatial projection</rdfs:label>
        <skos:notation rdf:datatype="http://www.w3.org/2001/XMLSchema#string">P161</skos:notation>
    </owl:ObjectProperty>
    


    <!-- http://www.cidoc-crm.org/cidoc-crm/P164 -->

    <owl:ObjectProperty rdf:about="http://www.cidoc-crm.org/cidoc-crm/P164">
        <rdfs:domain rdf:resource="http://www.cidoc-crm.org/cidoc-crm/E93"/>
        <rdfs:range rdf:resource="http://www.cidoc-crm.org/cidoc-crm/E52"/>
        <rdfs:comment xml:lang="en">This property relates an E93 Presence with an arbitrary E52 Time-Span that defines the section of the spacetime volume that this
            instance of E93 Presence is related to by P166 was a presence of (had presence) that is concerned by this instance of E93 Presence. </rdfs:comment>
        <rdfs:label xml:lang="en">during</rdfs:label>
        <skos:notation rdf:datatype="http://www.w3.org/2001/XMLSchema#string">P164</skos:notation>
    </owl:ObjectProperty>
    


    <!-- http://www.cidoc-crm.org/cidoc-crm/P165 -->

    <owl:ObjectProperty rdf:about="http://www.cidoc-crm.org/cidoc-crm/P165">
        <rdfs:domain rdf:resource="http://www.cidoc-crm.org/cidoc-crm/E73"/>
        <rdfs:range rdf:resource="http://www.cidoc-crm.org/cidoc-crm/E90"/>
        <rdfs:comment xml:lang="en">This property associates an instance of E73 Information Object with an instance of E90 Symbolic Object (or any of its
            subclasses) that was included in it. This property makes it possible to recognise the autonomous status of the incorporated signs, which
            were created in a distinct context, and can be incorporated in many distinct self-contained expressions, and to highlight the difference
            between structural and accidental whole-part relationships between conceptual entities. It accounts for many cultural facts that are quite
            frequent and significant: the inclusion of a poem in an anthology, the re-use of an operatic aria in a new opera, the use of a
            reproduction of a painting for a book cover or a CD booklet, the integration of textual quotations, the presence of lyrics in a song that
            sets those lyrics to music, the presence of the text of a play in a movie based on that play, etc. In particular, this property allows for
            modelling relationships of different levels of symbolic specificity, such as the natural language words making up a particular text, the
            characters making up the words and punctuation, the choice of fonts and page layout for the characters. A digital photograph of a
            manuscript page incorporates the text of the manuscript page. </rdfs:comment>
        <rdfs:label xml:lang="en">incorporates</rdfs:label>
        <skos:notation rdf:datatype="http://www.w3.org/2001/XMLSchema#string">P165</skos:notation>
    </owl:ObjectProperty>
    


    <!-- http://www.cidoc-crm.org/cidoc-crm/P166 -->

    <owl:ObjectProperty rdf:about="http://www.cidoc-crm.org/cidoc-crm/P166">
        <rdfs:domain rdf:resource="http://www.cidoc-crm.org/cidoc-crm/E93"/>
        <rdfs:range rdf:resource="http://www.cidoc-crm.org/cidoc-crm/E92"/>
        <rdfs:comment xml:lang="en">This property relates an E93 Presence with the STV it is part of… </rdfs:comment>
        <rdfs:label xml:lang="en">was a presence of</rdfs:label>
        <skos:notation rdf:datatype="http://www.w3.org/2001/XMLSchema#string">P166</skos:notation>
    </owl:ObjectProperty>
    


    <!-- http://www.cidoc-crm.org/cidoc-crm/P167 -->

    <owl:ObjectProperty rdf:about="http://www.cidoc-crm.org/cidoc-crm/P167">
        <rdfs:domain rdf:resource="http://www.cidoc-crm.org/cidoc-crm/E93"/>
        <rdfs:range rdf:resource="http://www.cidoc-crm.org/cidoc-crm/E53"/>
        <rdfs:comment xml:lang="en">This property points to a wider area in which my thing /event was… </rdfs:comment>
        <rdfs:label xml:lang="en">was at</rdfs:label>
        <skos:notation rdf:datatype="http://www.w3.org/2001/XMLSchema#string">P167</skos:notation>
    </owl:ObjectProperty>
    


    <!-- http://www.cidoc-crm.org/cidoc-crm/P168 -->

    <owl:ObjectProperty rdf:about="http://www.cidoc-crm.org/cidoc-crm/P168">
        <rdfs:domain rdf:resource="http://www.cidoc-crm.org/cidoc-crm/E53"/>
        <rdfs:range rdf:resource="http://www.cidoc-crm.org/cidoc-crm/E94"/>
        <rdfs:comment xml:lang="en">This property associates an instance of E53 Place with an instance of E94 Space Primitive that defines it. Syntactic variants or
            use of different scripts may result in multiple instances of E94 Space Primitive defining exactly the same place. Transformations between
            different reference systems in general result in new definitions of places approximating each other and not in alternative definitions.
            Note that it is possible for a place to be defined by phenomena causal to it or other forms of identification rather than by an instance
            of E94 Space Primitive. In this case, this property must not be used for approximating the respective instance of E53 Place with an
            instance of E94 Space Primitive. </rdfs:comment>
        <rdfs:label xml:lang="en">place is defined by</rdfs:label>
        <skos:notation rdf:datatype="http://www.w3.org/2001/XMLSchema#string">P168</skos:notation>
    </owl:ObjectProperty>
    


    <!-- http://www.cidoc-crm.org/cidoc-crm/P17 -->

    <owl:ObjectProperty rdf:about="http://www.cidoc-crm.org/cidoc-crm/P17">
        <rdfs:domain rdf:resource="http://www.cidoc-crm.org/cidoc-crm/E7"/>
        <rdfs:range rdf:resource="http://www.cidoc-crm.org/cidoc-crm/E1"/>
        <rdfs:comment xml:lang="en">This property describes an item or items that are regarded as a reason for carrying out the E7 Activity. For example, the
            discovery of a large hoard of treasure may call for a celebration, an order from head quarters can start a military manoeuvre. </rdfs:comment>
        <rdfs:label xml:lang="en">was motivated by</rdfs:label>
        <skos:notation rdf:datatype="http://www.w3.org/2001/XMLSchema#string">P17</skos:notation>
    </owl:ObjectProperty>
    


    <!-- http://www.cidoc-crm.org/cidoc-crm/P180 -->

    <owl:ObjectProperty rdf:about="http://www.cidoc-crm.org/cidoc-crm/P180">
        <rdfs:domain rdf:resource="http://www.cidoc-crm.org/cidoc-crm/E97"/>
        <rdfs:range rdf:resource="http://www.cidoc-crm.org/cidoc-crm/E98"/>
        <rdfs:label xml:lang="en">has currency</rdfs:label>
    </owl:ObjectProperty>
    


    <!-- http://www.cidoc-crm.org/cidoc-crm/P19 -->

    <owl:ObjectProperty rdf:about="http://www.cidoc-crm.org/cidoc-crm/P19">
        <rdfs:domain rdf:resource="http://www.cidoc-crm.org/cidoc-crm/E7"/>
        <rdfs:range rdf:resource="http://www.cidoc-crm.org/cidoc-crm/E71"/>
        <rdfs:comment xml:lang="en">This property relates an E7 Activity with objects created specifically for use in the activity. This is distinct from the
            intended use of an item in some general type of activity such as the book of common prayer which was intended for use in Church of England
            services (see P101 had as general use (was use of)).</rdfs:comment>
        <rdfs:label xml:lang="en">was intended use of</rdfs:label>
        <skos:notation rdf:datatype="http://www.w3.org/2001/XMLSchema#string">P19</skos:notation>
    </owl:ObjectProperty>
    


    <!-- http://www.cidoc-crm.org/cidoc-crm/P2 -->

    <owl:ObjectProperty rdf:about="http://www.cidoc-crm.org/cidoc-crm/P2">
        <rdfs:domain rdf:resource="http://www.cidoc-crm.org/cidoc-crm/E1"/>
        <rdfs:range rdf:resource="http://www.cidoc-crm.org/cidoc-crm/E55"/>
        <rdfs:comment xml:lang="en">This property allows sub typing of CRM entities - a form of specialisation – through the use of a terminological hierarchy, or
            thesaurus. The CRM is intended to focus on the high-level entities and relationships needed to describe data structures. Consequently, it
            does not specialise entities any further than is required for this immediate purpose. However, entities in the isA hierarchy of the CRM
            may by specialised into any number of sub entities, which can be defined in the E55 Type hierarchy. E51 Contact Point, for example, may be
            specialised into “e-mail address”, “telephone number”, “post office box”, “URL” etc. none of which figures explicitly in the CRM
            hierarchy. Sub typing obviously requires consistency between the meaning of the terms assigned and the more general intent of the CRM
            entity in question. </rdfs:comment>
        <rdfs:label xml:lang="en">has type</rdfs:label>
        <skos:notation rdf:datatype="http://www.w3.org/2001/XMLSchema#string">P2</skos:notation>
    </owl:ObjectProperty>
    


    <!-- http://www.cidoc-crm.org/cidoc-crm/P20 -->

    <owl:ObjectProperty rdf:about="http://www.cidoc-crm.org/cidoc-crm/P20">
        <rdfs:domain rdf:resource="http://www.cidoc-crm.org/cidoc-crm/E7"/>
        <rdfs:range rdf:resource="http://www.cidoc-crm.org/cidoc-crm/E5"/>
        <rdfs:comment xml:lang="en">This property identifies the relationship between a preparatory activity and the event it is intended to be preparation for.
            This includes activities, orders and other organisational actions, taken in preparation for other activities or events. P20 had specific
            purpose (was purpose of) implies that an activity succeeded in achieving its aim. If it does not succeed, such as the setting of a trap
            that did not catch anything, one may document the unrealized intention using P21 had general purpose (was purpose of):E55 Type and/or P33
            used specific technique (was used by): E29 Design or Procedure.</rdfs:comment>
        <rdfs:label xml:lang="en">had specific purpose</rdfs:label>
        <skos:notation rdf:datatype="http://www.w3.org/2001/XMLSchema#string">P20</skos:notation>
    </owl:ObjectProperty>
    


    <!-- http://www.cidoc-crm.org/cidoc-crm/P21 -->

    <owl:ObjectProperty rdf:about="http://www.cidoc-crm.org/cidoc-crm/P21">
        <rdfs:domain rdf:resource="http://www.cidoc-crm.org/cidoc-crm/E7"/>
        <rdfs:range rdf:resource="http://www.cidoc-crm.org/cidoc-crm/E55"/>
        <rdfs:comment xml:lang="en">This property describes an intentional relationship between an E7 Activity and some general goal or purpose. This may involve
            activities intended as preparation for some type of activity or event. P21had general purpose (was purpose of) differs from P20 had
            specific purpose (was purpose of) in that no occurrence of an event is implied as the purpose. </rdfs:comment>
        <rdfs:label xml:lang="en">had general purpose</rdfs:label>
        <skos:notation rdf:datatype="http://www.w3.org/2001/XMLSchema#string">P21</skos:notation>
    </owl:ObjectProperty>
    


    <!-- http://www.cidoc-crm.org/cidoc-crm/P22 -->

    <owl:ObjectProperty rdf:about="http://www.cidoc-crm.org/cidoc-crm/P22">
        <rdfs:domain rdf:resource="http://www.cidoc-crm.org/cidoc-crm/E8"/>
        <rdfs:range rdf:resource="http://www.cidoc-crm.org/cidoc-crm/E39"/>
        <rdfs:comment xml:lang="en">This property identifies the E39 Actor that acquires the legal ownership of an object as a result of an E8 Acquisition. The
            property will typically describe an Actor purchasing or otherwise acquiring an object from another Actor. However, title may also be
            acquired, without any corresponding loss of title by another Actor, through legal fieldwork such as hunting, shooting or fishing. In
            reality the title is either transferred to or from someone, or both. </rdfs:comment>
        <rdfs:label xml:lang="en">transferred title to</rdfs:label>
        <skos:notation rdf:datatype="http://www.w3.org/2001/XMLSchema#string">P22</skos:notation>
    </owl:ObjectProperty>
    


    <!-- http://www.cidoc-crm.org/cidoc-crm/P23 -->

    <owl:ObjectProperty rdf:about="http://www.cidoc-crm.org/cidoc-crm/P23">
        <rdfs:domain rdf:resource="http://www.cidoc-crm.org/cidoc-crm/E8"/>
        <rdfs:range rdf:resource="http://www.cidoc-crm.org/cidoc-crm/E39"/>
        <rdfs:comment xml:lang="en">This property identifies the E39 Actor or Actors who relinquish legal ownership as the result of an E8 Acquisition. The property
            will typically be used to describe a person donating or selling an object to a museum. In reality title is either transferred to or from
            someone, or both. </rdfs:comment>
        <rdfs:label xml:lang="en">transferred title from</rdfs:label>
        <skos:notation rdf:datatype="http://www.w3.org/2001/XMLSchema#string">P23</skos:notation>
    </owl:ObjectProperty>
    


    <!-- http://www.cidoc-crm.org/cidoc-crm/P24 -->

    <owl:ObjectProperty rdf:about="http://www.cidoc-crm.org/cidoc-crm/P24">
        <rdfs:domain rdf:resource="http://www.cidoc-crm.org/cidoc-crm/E8"/>
        <rdfs:range rdf:resource="http://www.cidoc-crm.org/cidoc-crm/E18"/>
        <rdfs:comment xml:lang="en">This property identifies the E18 Physical Thing or things involved in an E8 Acquisition. In reality, an acquisition must refer
            to at least one transferred item. </rdfs:comment>
        <rdfs:label xml:lang="en">transferred title of</rdfs:label>
        <skos:notation rdf:datatype="http://www.w3.org/2001/XMLSchema#string">P24</skos:notation>
    </owl:ObjectProperty>
    


    <!-- http://www.cidoc-crm.org/cidoc-crm/P25 -->

    <owl:ObjectProperty rdf:about="http://www.cidoc-crm.org/cidoc-crm/P25">
        <rdfs:domain rdf:resource="http://www.cidoc-crm.org/cidoc-crm/E9"/>
        <rdfs:range rdf:resource="http://www.cidoc-crm.org/cidoc-crm/E19"/>
        <rdfs:comment xml:lang="en">This property identifies an instance of E19 Physical Object that was moved by a move event. A move must concern at least one
            object. The property implies the object&apos;&apos;s passive participation. For example, Monet&apos;&apos;s painting &quot;Impression sunrise&quot; was moved for the
            first Impressionist exhibition in 1874. </rdfs:comment>
        <rdfs:label xml:lang="en">moved</rdfs:label>
        <skos:notation rdf:datatype="http://www.w3.org/2001/XMLSchema#string">P25</skos:notation>
    </owl:ObjectProperty>
    


    <!-- http://www.cidoc-crm.org/cidoc-crm/P26 -->

    <owl:ObjectProperty rdf:about="http://www.cidoc-crm.org/cidoc-crm/P26">
        <rdfs:domain rdf:resource="http://www.cidoc-crm.org/cidoc-crm/E9"/>
        <rdfs:range rdf:resource="http://www.cidoc-crm.org/cidoc-crm/E53"/>
        <rdfs:comment xml:lang="en">This property identifies a destination of a E9 Move. A move will be linked to a destination, such as the move of an artefact
            from storage to display. A move may be linked to many terminal instances of E53 Place by multiple instances of this property. In this case
            the move describes a distribution of a set of objects. The area of the move includes the origin(s), route and destination(s). Therefore
            the described destination is an instance of E53 Place which P89 falls within (contains) the instance of E53 Place the move P7 took place
            at. </rdfs:comment>
        <rdfs:label xml:lang="en">moved to</rdfs:label>
        <skos:notation rdf:datatype="http://www.w3.org/2001/XMLSchema#string">P26</skos:notation>
    </owl:ObjectProperty>
    


    <!-- http://www.cidoc-crm.org/cidoc-crm/P27 -->

    <owl:ObjectProperty rdf:about="http://www.cidoc-crm.org/cidoc-crm/P27">
        <rdfs:domain rdf:resource="http://www.cidoc-crm.org/cidoc-crm/E9"/>
        <rdfs:range rdf:resource="http://www.cidoc-crm.org/cidoc-crm/E53"/>
        <rdfs:comment xml:lang="en">This property identifies a starting E53 Place of an E9 Move. A move will be linked to an origin, such as the move of an artefact
            from storage to display. A move may be linked to many starting instances of E53 Place by multiple instances of this property. In this case
            the move describes the picking up of a set of objects. The area of the move includes the origin(s), route and destination(s). Therefore
            the described origin is an instance of E53 Place which P89 falls within (contains) the instance of E53 Place the move P7 took place at. </rdfs:comment>
        <rdfs:label xml:lang="en">moved from</rdfs:label>
        <skos:notation rdf:datatype="http://www.w3.org/2001/XMLSchema#string">P27</skos:notation>
    </owl:ObjectProperty>
    


    <!-- http://www.cidoc-crm.org/cidoc-crm/P28 -->

    <owl:ObjectProperty rdf:about="http://www.cidoc-crm.org/cidoc-crm/P28">
        <rdfs:domain rdf:resource="http://www.cidoc-crm.org/cidoc-crm/E10"/>
        <rdfs:range rdf:resource="http://www.cidoc-crm.org/cidoc-crm/E39"/>
        <rdfs:comment xml:lang="en">This property identifies the E39 Actor or Actors who surrender custody of an instance of E18 Physical Thing in an E10 Transfer
            of Custody activity. The property will typically describe an Actor surrendering custody of an object when it is handed over to someone
            else’s care. On occasion, physical custody may be surrendered involuntarily – through accident, loss or theft. In reality, custody is
            either transferred to someone or from someone, or both. </rdfs:comment>
        <rdfs:label xml:lang="en">custody surrendered by</rdfs:label>
        <skos:notation rdf:datatype="http://www.w3.org/2001/XMLSchema#string">P28</skos:notation>
    </owl:ObjectProperty>
    


    <!-- http://www.cidoc-crm.org/cidoc-crm/P29 -->

    <owl:ObjectProperty rdf:about="http://www.cidoc-crm.org/cidoc-crm/P29">
        <rdfs:domain rdf:resource="http://www.cidoc-crm.org/cidoc-crm/E10"/>
        <rdfs:range rdf:resource="http://www.cidoc-crm.org/cidoc-crm/E39"/>
        <rdfs:comment xml:lang="en">This property identifies the E39 Actor or Actors who receive custody of an instance of E18 Physical Thing in an E10 Transfer of
            Custody activity. The property will typically describe Actors receiving custody of an object when it is handed over from another Actor’s
            care. On occasion, physical custody may be received involuntarily or illegally – through accident, unsolicited donation, or theft. In
            reality, custody is either transferred to someone or from someone, or both. </rdfs:comment>
        <rdfs:label xml:lang="en">custody received by</rdfs:label>
        <skos:notation rdf:datatype="http://www.w3.org/2001/XMLSchema#string">P29</skos:notation>
    </owl:ObjectProperty>
    


    <!-- http://www.cidoc-crm.org/cidoc-crm/P3 -->

    <owl:ObjectProperty rdf:about="http://www.cidoc-crm.org/cidoc-crm/P3">
        <rdfs:domain rdf:resource="http://www.cidoc-crm.org/cidoc-crm/E1"/>
        <rdfs:range rdf:resource="http://www.cidoc-crm.org/cidoc-crm/E62"/>
    </owl:ObjectProperty>
    


    <!-- http://www.cidoc-crm.org/cidoc-crm/P30 -->

    <owl:ObjectProperty rdf:about="http://www.cidoc-crm.org/cidoc-crm/P30">
        <rdfs:domain rdf:resource="http://www.cidoc-crm.org/cidoc-crm/E10"/>
        <rdfs:range rdf:resource="http://www.cidoc-crm.org/cidoc-crm/E18"/>
        <rdfs:comment xml:lang="en">This property identifies an item or items of E18 Physical Thing concerned in an E10 Transfer of Custody activity. The property
            will typically describe the object that is handed over by an E39 Actor to another Actor’s custody. On occasion, physical custody may be
            transferred involuntarily or illegally – through accident, unsolicited donation, or theft. </rdfs:comment>
        <rdfs:label xml:lang="en">transferred custody of</rdfs:label>
        <skos:notation rdf:datatype="http://www.w3.org/2001/XMLSchema#string">P30</skos:notation>
    </owl:ObjectProperty>
    


    <!-- http://www.cidoc-crm.org/cidoc-crm/P31 -->

    <owl:ObjectProperty rdf:about="http://www.cidoc-crm.org/cidoc-crm/P31">
        <rdfs:domain rdf:resource="http://www.cidoc-crm.org/cidoc-crm/E11"/>
        <rdfs:range rdf:resource="http://www.cidoc-crm.org/cidoc-crm/E24"/>
        <rdfs:comment xml:lang="en">This property identifies the E24 Physical Man-Made Thing modified in an E11 Modification. If a modification is applied to a
            non-man-made object, it is regarded as an E22 Man-Made Object from that time onwards. </rdfs:comment>
        <rdfs:label xml:lang="en">has modified</rdfs:label>
        <skos:notation rdf:datatype="http://www.w3.org/2001/XMLSchema#string">P31</skos:notation>
    </owl:ObjectProperty>
    


    <!-- http://www.cidoc-crm.org/cidoc-crm/P32 -->

    <owl:ObjectProperty rdf:about="http://www.cidoc-crm.org/cidoc-crm/P32">
        <rdfs:domain rdf:resource="http://www.cidoc-crm.org/cidoc-crm/E7"/>
        <rdfs:range rdf:resource="http://www.cidoc-crm.org/cidoc-crm/E55"/>
        <rdfs:comment xml:lang="en">This property identifies the technique or method that was employed in an activity. These techniques should be drawn from an
            external E55 Type hierarchy of consistent terminology of general techniques or methods such as embroidery, oil-painting, carbon dating,
            etc. Specific documented techniques should be described as instances of E29 Design or Procedure. This property identifies the technique
            that was employed in an act of modification. </rdfs:comment>
        <rdfs:label xml:lang="en">used general technique</rdfs:label>
        <skos:notation rdf:datatype="http://www.w3.org/2001/XMLSchema#string">P32</skos:notation>
    </owl:ObjectProperty>
    


    <!-- http://www.cidoc-crm.org/cidoc-crm/P33 -->

    <owl:ObjectProperty rdf:about="http://www.cidoc-crm.org/cidoc-crm/P33">
        <rdfs:domain rdf:resource="http://www.cidoc-crm.org/cidoc-crm/E7"/>
        <rdfs:range rdf:resource="http://www.cidoc-crm.org/cidoc-crm/E29"/>
        <rdfs:comment xml:lang="en">This property identifies a specific instance of E29 Design or Procedure in order to carry out an instance of E7 Activity or
            parts of it. The property differs from P32 used general technique (was technique of) in that P33 refers to an instance of E29 Design or
            Procedure, which is a concrete information object in its own right rather than simply being a term or a method known by tradition. Typical
            examples would include intervention plans for conservation or the construction plans of a building. </rdfs:comment>
        <rdfs:label xml:lang="en">used specific technique</rdfs:label>
        <skos:notation rdf:datatype="http://www.w3.org/2001/XMLSchema#string">P33</skos:notation>
    </owl:ObjectProperty>
    


    <!-- http://www.cidoc-crm.org/cidoc-crm/P34 -->

    <owl:ObjectProperty rdf:about="http://www.cidoc-crm.org/cidoc-crm/P34">
        <rdfs:domain rdf:resource="http://www.cidoc-crm.org/cidoc-crm/E14"/>
        <rdfs:range rdf:resource="http://www.cidoc-crm.org/cidoc-crm/E18"/>
        <rdfs:comment xml:lang="en">This property identifies the E18 Physical Thing that was assessed during an E14 Condition Assessment activity. Conditions may be
            assessed either by direct observation or using recorded evidence. In the latter case the E18 Physical Thing does not need to be present or
            extant. </rdfs:comment>
        <rdfs:label xml:lang="en">concerned</rdfs:label>
        <skos:notation rdf:datatype="http://www.w3.org/2001/XMLSchema#string">P34</skos:notation>
    </owl:ObjectProperty>
    


    <!-- http://www.cidoc-crm.org/cidoc-crm/P35 -->

    <owl:ObjectProperty rdf:about="http://www.cidoc-crm.org/cidoc-crm/P35">
        <rdfs:domain rdf:resource="http://www.cidoc-crm.org/cidoc-crm/E14"/>
        <rdfs:range rdf:resource="http://www.cidoc-crm.org/cidoc-crm/E3"/>
        <rdfs:comment xml:lang="en">This property identifies the E3 Condition State that was observed in an E14 Condition Assessment activity.</rdfs:comment>
        <rdfs:label xml:lang="en">has identified</rdfs:label>
        <skos:notation rdf:datatype="http://www.w3.org/2001/XMLSchema#string">P35</skos:notation>
    </owl:ObjectProperty>
    


    <!-- http://www.cidoc-crm.org/cidoc-crm/P37 -->

    <owl:ObjectProperty rdf:about="http://www.cidoc-crm.org/cidoc-crm/P37">
        <rdfs:domain rdf:resource="http://www.cidoc-crm.org/cidoc-crm/E15"/>
        <rdfs:range rdf:resource="http://www.cidoc-crm.org/cidoc-crm/E42"/>
        <rdfs:comment xml:lang="en">This property records the identifier that was assigned to an item in an Identifier Assignment activity. The same identifier may
            be assigned on more than one occasion. An Identifier might be created prior to an assignment. </rdfs:comment>
        <rdfs:label xml:lang="en">assigned</rdfs:label>
        <skos:notation rdf:datatype="http://www.w3.org/2001/XMLSchema#string">P37</skos:notation>
    </owl:ObjectProperty>
    


    <!-- http://www.cidoc-crm.org/cidoc-crm/P38 -->

    <owl:ObjectProperty rdf:about="http://www.cidoc-crm.org/cidoc-crm/P38">
        <rdfs:domain rdf:resource="http://www.cidoc-crm.org/cidoc-crm/E15"/>
        <rdfs:range rdf:resource="http://www.cidoc-crm.org/cidoc-crm/E42"/>
        <rdfs:comment xml:lang="en">This property records the identifier that was deassigned from an instance of E1 CRM Entity. Deassignment of an identifier may be
            necessary when an item is taken out of an inventory, a new numbering system is introduced or items are merged or split up. The same
            identifier may be deassigned on more than one occasion. </rdfs:comment>
        <rdfs:label xml:lang="en">deassigned</rdfs:label>
        <skos:notation rdf:datatype="http://www.w3.org/2001/XMLSchema#string">P38</skos:notation>
    </owl:ObjectProperty>
    


    <!-- http://www.cidoc-crm.org/cidoc-crm/P39 -->

    <owl:ObjectProperty rdf:about="http://www.cidoc-crm.org/cidoc-crm/P39">
        <rdfs:domain rdf:resource="http://www.cidoc-crm.org/cidoc-crm/E16"/>
        <rdfs:range rdf:resource="http://www.cidoc-crm.org/cidoc-crm/E1"/>
        <rdfs:comment xml:lang="en">This property associates an instance of E16 Measurement with the instance of E1 CRM Entity to which it applied. An instance of
            E1 CRM Entity may be measured more than once. Material and immaterial things and processes may be measured, e.g. the number of words in a
            text, or the duration of an event. </rdfs:comment>
        <rdfs:label xml:lang="en">measured</rdfs:label>
        <skos:notation rdf:datatype="http://www.w3.org/2001/XMLSchema#string">P39</skos:notation>
    </owl:ObjectProperty>
    


    <!-- http://www.cidoc-crm.org/cidoc-crm/P4 -->

    <owl:ObjectProperty rdf:about="http://www.cidoc-crm.org/cidoc-crm/P4">
        <rdfs:domain rdf:resource="http://www.cidoc-crm.org/cidoc-crm/E2"/>
        <rdfs:range rdf:resource="http://www.cidoc-crm.org/cidoc-crm/E52"/>
        <rdfs:comment xml:lang="en">This property describes the temporal confinement of an instance of an E2 Temporal Entity. The related E52 Time-Span is
            understood as the real Time-Span during which the phenomena were active, which make up the temporal entity instance. It does not convey
            any other meaning than a positioning on the “time-line” of chronology. The Time-Span in turn is approximated by a set of dates (E61 Time
            Primitive). A temporal entity can have in reality only one Time-Span, but there may exist alternative opinions about it, which we would
            express by assigning multiple Time-Spans. Related temporal entities may share a Time-Span. Time-Spans may have completely unknown dates
            but other descriptions by which we can infer knowledge. </rdfs:comment>
        <rdfs:label xml:lang="en">has time-span</rdfs:label>
        <skos:notation rdf:datatype="http://www.w3.org/2001/XMLSchema#string">P4</skos:notation>
    </owl:ObjectProperty>
    


    <!-- http://www.cidoc-crm.org/cidoc-crm/P40 -->

    <owl:ObjectProperty rdf:about="http://www.cidoc-crm.org/cidoc-crm/P40">
        <rdfs:domain rdf:resource="http://www.cidoc-crm.org/cidoc-crm/E16"/>
        <rdfs:range rdf:resource="http://www.cidoc-crm.org/cidoc-crm/E54"/>
        <rdfs:comment xml:lang="en">This property records the dimension that was observed in an E16 Measurement Event. E54 Dimension can be any quantifiable aspect
            of E70 Thing. Weight, image colour depth and monetary value are dimensions in this sense. One measurement activity may determine more than
            one dimension of one object. Dimensions may be determined either by direct observation or using recorded evidence. In the latter case the
            measured Thing does not need to be present or extant. Even though knowledge of the value of a dimension requires measurement, the
            dimension may be an object of discourse prior to, or even without, any measurement being made. </rdfs:comment>
        <rdfs:label xml:lang="en">observed dimension</rdfs:label>
        <skos:notation rdf:datatype="http://www.w3.org/2001/XMLSchema#string">P40</skos:notation>
    </owl:ObjectProperty>
    


    <!-- http://www.cidoc-crm.org/cidoc-crm/P41 -->

    <owl:ObjectProperty rdf:about="http://www.cidoc-crm.org/cidoc-crm/P41">
        <rdfs:domain rdf:resource="http://www.cidoc-crm.org/cidoc-crm/E17"/>
        <rdfs:range rdf:resource="http://www.cidoc-crm.org/cidoc-crm/E1"/>
        <rdfs:comment xml:lang="en">This property records the item to which a type was assigned in an E17 Type Assignment activity. Any instance of a CRM entity may
            be assigned a type through type assignment. Type assignment events allow a more detailed path from E1 CRM Entity through P41 classified
            (was classified), E17 Type Assignment, P42 assigned (was assigned by) to E55 Type for assigning types to objects compared to the shortcut
            offered by P2 has type (is type of). </rdfs:comment>
        <rdfs:label xml:lang="en">classified</rdfs:label>
        <skos:notation rdf:datatype="http://www.w3.org/2001/XMLSchema#string">P41</skos:notation>
    </owl:ObjectProperty>
    


    <!-- http://www.cidoc-crm.org/cidoc-crm/P42 -->

    <owl:ObjectProperty rdf:about="http://www.cidoc-crm.org/cidoc-crm/P42">
        <rdfs:domain rdf:resource="http://www.cidoc-crm.org/cidoc-crm/E17"/>
        <rdfs:range rdf:resource="http://www.cidoc-crm.org/cidoc-crm/E55"/>
        <rdfs:comment xml:lang="en">This property records the type that was assigned to an entity by an E17 Type Assignment activity. Type assignment events allow a
            more detailed path from E1 CRM Entity through P41 classified (was classified by), E17 Type Assignment, P42 assigned (was assigned by) to
            E55 Type for assigning types to objects compared to the shortcut offered by P2 has type (is type of). For example, a fragment of an
            antique vessel could be assigned the type “attic red figured belly handled amphora” by expert A. The same fragment could be assigned the
            type “shoulder handled amphora” by expert B. A Type may be intellectually constructed independent from assigning an instance of it. </rdfs:comment>
        <rdfs:label xml:lang="en">assigned</rdfs:label>
        <skos:notation rdf:datatype="http://www.w3.org/2001/XMLSchema#string">P42</skos:notation>
    </owl:ObjectProperty>
    


    <!-- http://www.cidoc-crm.org/cidoc-crm/P43 -->

    <owl:ObjectProperty rdf:about="http://www.cidoc-crm.org/cidoc-crm/P43">
        <rdfs:domain rdf:resource="http://www.cidoc-crm.org/cidoc-crm/E70"/>
        <rdfs:range rdf:resource="http://www.cidoc-crm.org/cidoc-crm/E54"/>
        <rdfs:comment xml:lang="en">This property records a E54 Dimension of some E70 Thing. It is a shortcut of the more fully developed path from E70 Thing
            through P39 measured (was measured by), E16 Measurement P40 observed dimension (was observed in) to E54 Dimension. It offers no
            information about how and when an E54 Dimension was established, nor by whom. An instance of E54 Dimension is specific to an instance of
            E70 Thing. </rdfs:comment>
        <rdfs:label xml:lang="en">has dimension</rdfs:label>
        <skos:notation rdf:datatype="http://www.w3.org/2001/XMLSchema#string">P43</skos:notation>
    </owl:ObjectProperty>
    


    <!-- http://www.cidoc-crm.org/cidoc-crm/P44 -->

    <owl:ObjectProperty rdf:about="http://www.cidoc-crm.org/cidoc-crm/P44">
        <rdfs:domain rdf:resource="http://www.cidoc-crm.org/cidoc-crm/E18"/>
        <rdfs:range rdf:resource="http://www.cidoc-crm.org/cidoc-crm/E3"/>
        <rdfs:comment xml:lang="en">This property records an E3 Condition State for some E18 Physical Thing. It is a shortcut of the more fully developed path from
            E18 Physical Thing through P34 concerned (was assessed by), E14 Condition Assessment P35 has identified (was identified by) to E3
            Condition State. It offers no information about how and when the E3 Condition State was established, nor by whom. An instance of Condition
            State is specific to an instance of Physical Thing. </rdfs:comment>
        <rdfs:label xml:lang="en">has condition</rdfs:label>
        <skos:notation rdf:datatype="http://www.w3.org/2001/XMLSchema#string">P44</skos:notation>
    </owl:ObjectProperty>
    


    <!-- http://www.cidoc-crm.org/cidoc-crm/P45 -->

    <owl:ObjectProperty rdf:about="http://www.cidoc-crm.org/cidoc-crm/P45">
        <rdfs:domain rdf:resource="http://www.cidoc-crm.org/cidoc-crm/E18"/>
        <rdfs:range rdf:resource="http://www.cidoc-crm.org/cidoc-crm/E57"/>
        <rdfs:comment xml:lang="en">This property identifies the instances of E57 Materials of which an instance of E18 Physical Thing is composed. All physical
            things consist of physical materials. P45 consists of (is incorporated in) allows the different Materials to be recorded. P45 consists of
            (is incorporated in) refers here to observed Material as opposed to the consumed raw material. A Material, such as a theoretical alloy,
            may not have any physical instances</rdfs:comment>
        <rdfs:label xml:lang="en">consists of</rdfs:label>
        <skos:notation rdf:datatype="http://www.w3.org/2001/XMLSchema#string">P45</skos:notation>
    </owl:ObjectProperty>
    


    <!-- http://www.cidoc-crm.org/cidoc-crm/P46 -->

    <owl:ObjectProperty rdf:about="http://www.cidoc-crm.org/cidoc-crm/P46">
        <rdfs:domain rdf:resource="http://www.cidoc-crm.org/cidoc-crm/E18"/>
        <rdfs:range rdf:resource="http://www.cidoc-crm.org/cidoc-crm/E18"/>
        <rdfs:comment xml:lang="en">This property allows instances of E18 Physical Thing to be analysed into component elements. Component elements, since they are
            themselves instances of E18 Physical Thing, may be further analysed into sub-components, thereby creating a hierarchy of part
            decomposition. An instance of E18 Physical Thing may be shared between multiple wholes, for example two buildings may share a common wall.
            This property does not specify when and for how long a component element resided in the respective whole. If a component is not part of a
            whole from the beginning of existence or until the end of existence of the whole, the classes E79 Part Addition and E90 Part Removal can
            be used to document when a component became part of a particular whole and/or when it stopped being a part of it. For the time-span of
            being part of the respective whole, the component is completely contained in the place the whole occupies. This property is intended to
            describe specific components that are individually documented, rather than general aspects. Overall descriptions of the structure of an
            instance of E18 Physical Thing are captured by the P3 has note property. The instances of E57 Material of which an item of E18 Physical
            Thing is composed should be documented using P45 consists of (is incorporated in). </rdfs:comment>
        <rdfs:label xml:lang="en">is composed of</rdfs:label>
        <skos:notation rdf:datatype="http://www.w3.org/2001/XMLSchema#string">P46</skos:notation>
    </owl:ObjectProperty>
    


    <!-- http://www.cidoc-crm.org/cidoc-crm/P48 -->

    <owl:ObjectProperty rdf:about="http://www.cidoc-crm.org/cidoc-crm/P48">
        <rdfs:domain rdf:resource="http://www.cidoc-crm.org/cidoc-crm/E1"/>
        <rdfs:range rdf:resource="http://www.cidoc-crm.org/cidoc-crm/E42"/>
        <rdfs:comment xml:lang="en">This property records the preferred E42 Identifier that was used to identify an instance of E1 CRM Entity at the time this
            property was recorded. More than one preferred identifier may have been assigned to an item over time. Use of this property requires an
            external mechanism for assigning temporal validity to the respective CRM instance. P48 has preferred identifier (is preferred identifier
            of), is a shortcut for the path from E1 CRM Entity through P140 assigned attribute to (was attributed by), E15 Identifier Assignment, P37
            assigned (was assigned by) to E42 Identifier. The fact that an identifier is a preferred one for an organisation can be better expressed
            in a context independent form by assigning a suitable E55 Type to the respective instance of E15 Identifier Assignment using the P2 has
            type property. </rdfs:comment>
        <rdfs:label xml:lang="en">has preferred identifier</rdfs:label>
        <skos:notation rdf:datatype="http://www.w3.org/2001/XMLSchema#string">P48</skos:notation>
    </owl:ObjectProperty>
    


    <!-- http://www.cidoc-crm.org/cidoc-crm/P49 -->

    <owl:ObjectProperty rdf:about="http://www.cidoc-crm.org/cidoc-crm/P49">
        <rdfs:domain rdf:resource="http://www.cidoc-crm.org/cidoc-crm/E18"/>
        <rdfs:range rdf:resource="http://www.cidoc-crm.org/cidoc-crm/E39"/>
        <rdfs:comment xml:lang="en">This property identifies the E39 Actor or Actors who have or have had custody of an instance of E18 Physical Thing at some time.
            The distinction with P50 has current keeper (is current keeper of) is that P49 has former or current keeper (is former or current keeper
            of) leaves open the question as to whether the specified keepers are current. P49 has former or current keeper (is former or current
            keeper of) is a shortcut for the more detailed path from E18 Physical Thing through P30 transferred custody of (custody transferred
            through), E10 Transfer of Custody, P28 custody surrendered by (surrendered custody through) or P29 custody received by (received custody
            through) to E39 Actor. </rdfs:comment>
        <rdfs:label xml:lang="en">has former or current keeper</rdfs:label>
        <skos:notation rdf:datatype="http://www.w3.org/2001/XMLSchema#string">P49</skos:notation>
    </owl:ObjectProperty>
    


    <!-- http://www.cidoc-crm.org/cidoc-crm/P5 -->

    <owl:ObjectProperty rdf:about="http://www.cidoc-crm.org/cidoc-crm/P5">
        <rdfs:domain rdf:resource="http://www.cidoc-crm.org/cidoc-crm/E3"/>
        <rdfs:range rdf:resource="http://www.cidoc-crm.org/cidoc-crm/E3"/>
        <rdfs:comment xml:lang="en">This property describes the decomposition of an E3 Condition State into discrete, subsidiary states. It is assumed that the
            sub-states into which the condition state is analysed form a logical whole - although the entire story may not be completely known – and
            that the sub-states are in fact constitutive of the general condition state. For example, a general condition state of “in ruins” may be
            decomposed into the individual stages of decay</rdfs:comment>
        <rdfs:label xml:lang="en">consists of</rdfs:label>
        <skos:notation rdf:datatype="http://www.w3.org/2001/XMLSchema#string">P5</skos:notation>
    </owl:ObjectProperty>
    


    <!-- http://www.cidoc-crm.org/cidoc-crm/P50 -->

    <owl:ObjectProperty rdf:about="http://www.cidoc-crm.org/cidoc-crm/P50">
        <rdfs:domain rdf:resource="http://www.cidoc-crm.org/cidoc-crm/E18"/>
        <rdfs:range rdf:resource="http://www.cidoc-crm.org/cidoc-crm/E39"/>
        <rdfs:comment xml:lang="en">This property identifies the E39 Actor or Actors who had custody of an instance of E18 Physical Thing at the time of validity of
            the record or database containing the statement that uses this property. P50 has current keeper (is current keeper of) is a shortcut for
            the more detailed path from E18 Physical Thing through P30 transferred custody of (custody transferred through), E10 Transfer of Custody,
            P29 custody received by (received custody through) to E39 Actor. </rdfs:comment>
        <rdfs:label xml:lang="en">has current keeper</rdfs:label>
        <skos:notation rdf:datatype="http://www.w3.org/2001/XMLSchema#string">P50</skos:notation>
    </owl:ObjectProperty>
    


    <!-- http://www.cidoc-crm.org/cidoc-crm/P51 -->

    <owl:ObjectProperty rdf:about="http://www.cidoc-crm.org/cidoc-crm/P51">
        <rdfs:domain rdf:resource="http://www.cidoc-crm.org/cidoc-crm/E18"/>
        <rdfs:range rdf:resource="http://www.cidoc-crm.org/cidoc-crm/E39"/>
        <rdfs:comment xml:lang="en">This property identifies the E39 Actor that is or has been the legal owner (i.e. title holder) of an instance of E18 Physical
            Thing at some time. The distinction with P52 has current owner (is current owner of) is that P51 has former or current owner (is former or
            current owner of) does not indicate whether the specified owners are current. P51 has former or current owner (is former or current owner
            of) is a shortcut for the more detailed path from E18 Physical Thing through P24 transferred title of (changed ownership through), E8
            Acquisition, P23 transferred title from (surrendered title through), or P22 transferred title to (acquired title through) to E39 Actor. </rdfs:comment>
        <rdfs:label xml:lang="en">has former or current owner</rdfs:label>
        <skos:notation rdf:datatype="http://www.w3.org/2001/XMLSchema#string">P51</skos:notation>
    </owl:ObjectProperty>
    


    <!-- http://www.cidoc-crm.org/cidoc-crm/P52 -->

    <owl:ObjectProperty rdf:about="http://www.cidoc-crm.org/cidoc-crm/P52">
        <rdfs:domain rdf:resource="http://www.cidoc-crm.org/cidoc-crm/E18"/>
        <rdfs:range rdf:resource="http://www.cidoc-crm.org/cidoc-crm/E39"/>
        <rdfs:comment xml:lang="en">This property identifies the E21 Person, E74 Group or E40 Legal Body that was the owner of an instance of E18 Physical Thing at
            the time of validity of the record or database containing the statement that uses this property. P52 has current owner (is current owner
            of) is a shortcut for the more detailed path from E18 Physical Thing through P24 transferred title of (changed ownership through), E8
            Acquisition, P22 transferred title to (acquired title through) to E39 Actor, if and only if this acquisition event is the most recent. </rdfs:comment>
        <rdfs:label xml:lang="en">has current owner</rdfs:label>
        <skos:notation rdf:datatype="http://www.w3.org/2001/XMLSchema#string">P52</skos:notation>
    </owl:ObjectProperty>
    


    <!-- http://www.cidoc-crm.org/cidoc-crm/P53 -->

    <owl:ObjectProperty rdf:about="http://www.cidoc-crm.org/cidoc-crm/P53">
        <rdfs:domain rdf:resource="http://www.cidoc-crm.org/cidoc-crm/E18"/>
        <rdfs:range rdf:resource="http://www.cidoc-crm.org/cidoc-crm/E53"/>
        <rdfs:comment xml:lang="en">This property allows an instance of E53 Place to be associated as the former or current location of an instance of E18 Physical
            Thing. In the case of E19 Physical Objects, the property does not allow any indication of the Time-Span during which the Physical Object
            was located at this Place, nor if this is the current location. In the case of immobile objects, the Place would normally correspond to
            the Place of creation. P53 has former or current location (is former or current location of) is a shortcut. A more detailed representation
            can make use of the fully developed (i.e. indirect) path from E19 Physical Object through P25 moved (moved by), E9 Move, P26 moved to (was
            destination of) or P27 moved from (was origin of) to E53 Place. </rdfs:comment>
        <rdfs:label xml:lang="en">has former or current location</rdfs:label>
        <skos:notation rdf:datatype="http://www.w3.org/2001/XMLSchema#string">P53</skos:notation>
    </owl:ObjectProperty>
    


    <!-- http://www.cidoc-crm.org/cidoc-crm/P54 -->

    <owl:ObjectProperty rdf:about="http://www.cidoc-crm.org/cidoc-crm/P54">
        <rdfs:domain rdf:resource="http://www.cidoc-crm.org/cidoc-crm/E19"/>
        <rdfs:range rdf:resource="http://www.cidoc-crm.org/cidoc-crm/E53"/>
        <rdfs:comment xml:lang="en">This property records the foreseen permanent location of an instance of E19 Physical Object at the time of validity of the
            record or database containing the statement that uses this property. P54 has current permanent location (is current permanent location of)
            is similar to P55 has current location (currently holds). However, it indicates the E53 Place currently reserved for an object, such as
            the permanent storage location or a permanent exhibit location. The object may be temporarily removed from the permanent location, for
            example when used in temporary exhibitions or loaned to another institution. The object may never actually be located at its permanent
            location. </rdfs:comment>
        <rdfs:label xml:lang="en">has current permanent location</rdfs:label>
        <skos:notation rdf:datatype="http://www.w3.org/2001/XMLSchema#string">P54</skos:notation>
    </owl:ObjectProperty>
    


    <!-- http://www.cidoc-crm.org/cidoc-crm/P55 -->

    <owl:ObjectProperty rdf:about="http://www.cidoc-crm.org/cidoc-crm/P55">
        <rdfs:domain rdf:resource="http://www.cidoc-crm.org/cidoc-crm/E19"/>
        <rdfs:range rdf:resource="http://www.cidoc-crm.org/cidoc-crm/E53"/>
        <rdfs:comment xml:lang="en">This property records the location of an E19 Physical Object at the time of validity of the record or database containing the
            statement that uses this property. This property is a specialisation of P53 has former or current location (is former or current location
            of). It indicates that the E53 Place associated with the E19 Physical Object is the current location of the object. The property does not
            allow any indication of how long the Object has been at the current location. P55 has current location (currently holds) is a shortcut. A
            more detailed representation can make use of the fully developed (i.e. indirect) path from E19 Physical Object through P25 moved (moved
            by), E9 Move P26 moved to (was destination of) to E53 Place if and only if this Move is the most recent. </rdfs:comment>
        <rdfs:label xml:lang="en">has current location</rdfs:label>
        <skos:notation rdf:datatype="http://www.w3.org/2001/XMLSchema#string">P55</skos:notation>
    </owl:ObjectProperty>
    


    <!-- http://www.cidoc-crm.org/cidoc-crm/P56 -->

    <owl:ObjectProperty rdf:about="http://www.cidoc-crm.org/cidoc-crm/P56">
        <rdfs:domain rdf:resource="http://www.cidoc-crm.org/cidoc-crm/E19"/>
        <rdfs:range rdf:resource="http://www.cidoc-crm.org/cidoc-crm/E26"/>
        <rdfs:comment xml:lang="en">This property links an instance of E19 Physical Object to an instance of E26 Physical Feature that it bears. An E26 Physical
            Feature can only exist on one object. One object may bear more than one E26 Physical Feature. An E27 Site should be considered as an E26
            Physical Feature on the surface of the Earth. An instance B of E26 Physical Feature being a detail of the structure of another instance A
            of E26 Physical Feature can be linked to B by use of the property P46 is composed of (forms part of). This implies that the subfeature B
            is P56i found on the same E19 Physical Object as A. P56 bears feature (is found on) is a shortcut. A more detailed representation can make
            use of the fully developed (i.e. indirect) path from E19 Physical Object through P59 has section (is located on or Definition of the CIDOC
            Conceptual Reference Model 149 within), E53 Place, P53 has former or current location (is former or current location of) to E26 Physical
            Feature. </rdfs:comment>
        <rdfs:label xml:lang="en">bears feature</rdfs:label>
        <skos:notation rdf:datatype="http://www.w3.org/2001/XMLSchema#string">P56</skos:notation>
    </owl:ObjectProperty>
    


    <!-- http://www.cidoc-crm.org/cidoc-crm/P57 -->

    <owl:ObjectProperty rdf:about="http://www.cidoc-crm.org/cidoc-crm/P57">
        <rdfs:domain rdf:resource="http://www.cidoc-crm.org/cidoc-crm/E19"/>
        <rdfs:range rdf:resource="http://www.cidoc-crm.org/cidoc-crm/E60"/>
        <rdfs:comment xml:lang="en">This property documents the E60 Number of parts of which an instance of E19 Physical Object is composed. This may be used as a
            method of checking inventory counts with regard to aggregate or collective objects. What constitutes a part or component depends on the
            context and requirements of the documentation. Normally, the parts documented in this way would not be considered as worthy of individual
            attention. For a more complete description, objects may be decomposed into their components and constituents using P46 is composed of
            (forms parts of) and P45 consists of (is incorporated in). This allows each element to be described individually. </rdfs:comment>
        <rdfs:label xml:lang="en">has number of parts</rdfs:label>
        <skos:notation rdf:datatype="http://www.w3.org/2001/XMLSchema#string">P57</skos:notation>
    </owl:ObjectProperty>
    


    <!-- http://www.cidoc-crm.org/cidoc-crm/P58 -->

    <owl:ObjectProperty rdf:about="http://www.cidoc-crm.org/cidoc-crm/P58">
        <rdfs:domain rdf:resource="http://www.cidoc-crm.org/cidoc-crm/E18"/>
        <rdfs:range rdf:resource="http://www.cidoc-crm.org/cidoc-crm/E46"/>
        <rdfs:comment xml:lang="en">This property links an area (section) named by a E46 Section Definition to the instance of E18 Physical Thing upon which it is
            found. The CRM handles sections as locations (instances of E53 Place) within or on E18 Physical Thing that are identified by E46 Section
            Definitions. Sections need not be discrete and separable components or parts of an object. This is part of a more developed path from E18
            Physical Thing through P58, E46 Section Definition, P87 is identified by (identifies) that allows a more precise definition of a location
            found on an object than the shortcut P59 has section (is located on or within). A particular instance of a Section Definition only applies
            to one instance of Physical Thing.</rdfs:comment>
        <rdfs:label xml:lang="en">has section definition</rdfs:label>
        <skos:notation rdf:datatype="http://www.w3.org/2001/XMLSchema#string">P58</skos:notation>
    </owl:ObjectProperty>
    


    <!-- http://www.cidoc-crm.org/cidoc-crm/P59 -->

    <owl:ObjectProperty rdf:about="http://www.cidoc-crm.org/cidoc-crm/P59">
        <rdfs:domain rdf:resource="http://www.cidoc-crm.org/cidoc-crm/E18"/>
        <rdfs:range rdf:resource="http://www.cidoc-crm.org/cidoc-crm/E53"/>
        <rdfs:comment xml:lang="en">This property links an area to the instance of E18 Physical Thing upon which it is found. It is typically used when a named E46
            Section Definition is not appropriate. E18 Physical Thing may be subdivided into arbitrary regions. P59 has section (is located on or
            within) is a shortcut. If the E53 Place is identified by a Section Definition, a more detailed representation can make use of the fully
            developed (i.e. indirect) path from E18 Physical Thing through P58 has section definition (defines section), E46 Section Definition, P87
            is identified by (identifies) to E53 Place. A Place can only be located on or within one Physical Object. </rdfs:comment>
        <rdfs:label xml:lang="en">has section</rdfs:label>
        <skos:notation rdf:datatype="http://www.w3.org/2001/XMLSchema#string">P59</skos:notation>
    </owl:ObjectProperty>
    


    <!-- http://www.cidoc-crm.org/cidoc-crm/P62 -->

    <owl:ObjectProperty rdf:about="http://www.cidoc-crm.org/cidoc-crm/P62">
        <rdfs:domain rdf:resource="http://www.cidoc-crm.org/cidoc-crm/E24"/>
        <rdfs:range rdf:resource="http://www.cidoc-crm.org/cidoc-crm/E1"/>
        <rdfs:comment xml:lang="en">This property identifies something that is depicted by an instance of E24 Physical Man-Made Thing. Depicting is meant in the
            sense that the surface of the E24 Physical Man-Made Thing shows, through its passive optical qualities or form, a representation of the
            entity depicted. It does not pertain to inscriptions or any other information encoding. This property is a shortcut of the more fully
            developed path from E24 Physical Man-Made Thing through P65 shows visual item (is shown by), E36 Visual Item, P138 represents (has
            representation) to E1 CRM Entity. P62.1 mode of depiction allows the nature of the depiction to be refined. </rdfs:comment>
        <rdfs:label xml:lang="en">depicts</rdfs:label>
        <skos:notation rdf:datatype="http://www.w3.org/2001/XMLSchema#string">P62</skos:notation>
    </owl:ObjectProperty>
    


    <!-- http://www.cidoc-crm.org/cidoc-crm/P65 -->

    <owl:ObjectProperty rdf:about="http://www.cidoc-crm.org/cidoc-crm/P65">
        <rdfs:domain rdf:resource="http://www.cidoc-crm.org/cidoc-crm/E24"/>
        <rdfs:range rdf:resource="http://www.cidoc-crm.org/cidoc-crm/E36"/>
        <rdfs:comment xml:lang="en">This property documents an E36 Visual Item shown by an instance of E24 Physical Man-Made Thing. This property is similar to P62
            depicts (is depicted by) in that it associates an item of E24 Physical Man-Made Thing with a visual representation. However, P65 shows
            visual item (is shown by) differs from the P62 depicts (is depicted by) property in that it makes no claims about what the E36 Visual Item
            is deemed to represent. E36 Visual Item identifies a recognisable image or visual symbol, regardless of what this image may or may not
            represent. For example, all recent British coins bear a portrait of Queen Elizabeth II, a fact that is correctly documented using P62
            depicts (is depicted by). Different portraits have been used at different periods, however. P65 shows visual item (is shown by) can be
            used to refer to a particular portrait. P65 shows visual item (is shown by) may also be used for Visual Items such as signs, marks and
            symbols, for example the &apos;&apos;Maltese Cross&apos;&apos; or the &apos;&apos;copyright symbol’ that have no particular representational content. This property is part
            of the fully developed path from E24 Physical Man-Made Thing through P65 shows visual item (is shown by), E36 Visual Item, P138 represents
            (has representation) to E1 CRM Entity which is shortcut by, P62 depicts (is depicted by). </rdfs:comment>
        <rdfs:label xml:lang="en">shows visual item</rdfs:label>
        <skos:notation rdf:datatype="http://www.w3.org/2001/XMLSchema#string">P65</skos:notation>
    </owl:ObjectProperty>
    


    <!-- http://www.cidoc-crm.org/cidoc-crm/P67 -->

    <owl:ObjectProperty rdf:about="http://www.cidoc-crm.org/cidoc-crm/P67">
        <rdfs:domain rdf:resource="http://www.cidoc-crm.org/cidoc-crm/E89"/>
        <rdfs:range rdf:resource="http://www.cidoc-crm.org/cidoc-crm/E1"/>
        <rdfs:comment xml:lang="en">This property documents that an E89 Propositional Object makes a statement about an instance of E1 CRM Entity. P67 refers to (is
            referred to by) has the P67.1 has type link to an instance of E55 Type. This is intended to allow a more detailed description of the type
            of reference. This differs from P129 is about (is subject of), which describes the primary subject or subjects of the E89 Propositional
            Object. </rdfs:comment>
        <rdfs:label xml:lang="en">refers to</rdfs:label>
        <skos:notation rdf:datatype="http://www.w3.org/2001/XMLSchema#string">P67</skos:notation>
    </owl:ObjectProperty>
    


    <!-- http://www.cidoc-crm.org/cidoc-crm/P68 -->

    <owl:ObjectProperty rdf:about="http://www.cidoc-crm.org/cidoc-crm/P68">
        <rdfs:domain rdf:resource="http://www.cidoc-crm.org/cidoc-crm/E29"/>
        <rdfs:range rdf:resource="http://www.cidoc-crm.org/cidoc-crm/E57"/>
        <rdfs:comment xml:lang="en">This property identifies an E57 Material foreseeen to be used by an E29 Design or Procedure. E29 Designs and procedures commonly
            foresee the use of particular E57 Materials. The fabrication of adobe bricks, for example, requires straw, clay and water. This property
            enables this to be documented. This property is not intended for the documentation of E57 Materials that were used on a particular
            occasion when an instance of E29 Design or Procedure was executed. </rdfs:comment>
        <rdfs:label xml:lang="en">foresees use of</rdfs:label>
        <skos:notation rdf:datatype="http://www.w3.org/2001/XMLSchema#string">P68</skos:notation>
    </owl:ObjectProperty>
    


    <!-- http://www.cidoc-crm.org/cidoc-crm/P69 -->

    <owl:ObjectProperty rdf:about="http://www.cidoc-crm.org/cidoc-crm/P69">
        <rdfs:domain rdf:resource="http://www.cidoc-crm.org/cidoc-crm/E29"/>
        <rdfs:range rdf:resource="http://www.cidoc-crm.org/cidoc-crm/E29"/>
        <rdfs:comment xml:lang="en">This property generalises relationships like whole-part, sequence, prerequisite or inspired by between instances of E29 Design
            or Procedure. Any instance of E29 Design or Procedure may be associated with other designs or procedures. The property is considered to be
            symmetrical unless otherwise indicated by P69.1 has type. The P69.1 has type property of P69 has association with allows the nature of the
            association to be specified reading from domain to range; examples of types of association between instances of E29 Design or Procedure
            include: has part, follows, requires, etc. The property can typically be used to model the decomposition of the description of a complete
            workflow into a series of separate procedures. </rdfs:comment>
        <rdfs:label xml:lang="en">has association with</rdfs:label>
        <skos:notation rdf:datatype="http://www.w3.org/2001/XMLSchema#string">P69</skos:notation>
    </owl:ObjectProperty>
    


    <!-- http://www.cidoc-crm.org/cidoc-crm/P7 -->

    <owl:ObjectProperty rdf:about="http://www.cidoc-crm.org/cidoc-crm/P7">
        <rdfs:domain rdf:resource="http://www.cidoc-crm.org/cidoc-crm/E4"/>
        <rdfs:range rdf:resource="http://www.cidoc-crm.org/cidoc-crm/E53"/>
        <rdfs:comment xml:lang="en">This property describes the spatial location of an instance of E4 Period. The related E53 Place should be seen as an
            approximation of the geographical area within which the phenomena that characterise the period in question occurred. P7took place at
            (witnessed) does not convey any meaning other than spatial positioning (generally on the surface of the earth). For example, the period
            &quot;Révolution française&quot; can be said to have taken place in “France”, the “Victorian” period, may be said to have taken place in “Britain”
            and its colonies, as well as other parts of Europe and north America. A period can take place at multiple locations. It is a shortcut of
            the more fully developed path from E4 Period through P161 has spatial projection, E53 Place, P89 falls within (contains) to E53 Place. </rdfs:comment>
        <rdfs:label xml:lang="en">took place at</rdfs:label>
        <skos:notation rdf:datatype="http://www.w3.org/2001/XMLSchema#string">P7</skos:notation>
    </owl:ObjectProperty>
    


    <!-- http://www.cidoc-crm.org/cidoc-crm/P70 -->

    <owl:ObjectProperty rdf:about="http://www.cidoc-crm.org/cidoc-crm/P70">
        <rdfs:domain rdf:resource="http://www.cidoc-crm.org/cidoc-crm/E31"/>
        <rdfs:range rdf:resource="http://www.cidoc-crm.org/cidoc-crm/E1"/>
        <rdfs:comment xml:lang="en">This property describes the CRM Entities documented by instances of E31 Document. Documents may describe any conceivable entity,
            hence the link to the highest-level entity in the CRM hierarchy. This property is intended for cases where a reference is regarded as
            being of a documentary character, in the scholarly or scientific sense. </rdfs:comment>
        <rdfs:label xml:lang="en">documents</rdfs:label>
        <skos:notation rdf:datatype="http://www.w3.org/2001/XMLSchema#string">P70</skos:notation>
    </owl:ObjectProperty>
    


    <!-- http://www.cidoc-crm.org/cidoc-crm/P71 -->

    <owl:ObjectProperty rdf:about="http://www.cidoc-crm.org/cidoc-crm/P71">
        <rdfs:domain rdf:resource="http://www.cidoc-crm.org/cidoc-crm/E32"/>
        <rdfs:range rdf:resource="http://www.cidoc-crm.org/cidoc-crm/E1"/>
        <rdfs:comment xml:lang="en">This property documents a source E32 Authority Document for an instance of an E1 CRM Entity. </rdfs:comment>
        <rdfs:label xml:lang="en">lists</rdfs:label>
        <skos:notation rdf:datatype="http://www.w3.org/2001/XMLSchema#string">P71</skos:notation>
    </owl:ObjectProperty>
    


    <!-- http://www.cidoc-crm.org/cidoc-crm/P72 -->

    <owl:ObjectProperty rdf:about="http://www.cidoc-crm.org/cidoc-crm/P72">
        <rdfs:domain rdf:resource="http://www.cidoc-crm.org/cidoc-crm/E33"/>
        <rdfs:range rdf:resource="http://www.cidoc-crm.org/cidoc-crm/E56"/>
        <rdfs:comment xml:lang="en">This property describes the E56 Language of an E33 Linguistic Object. Linguistic Objects are composed in one or more human
            Languages. This property allows these languages to be documented. </rdfs:comment>
        <rdfs:label xml:lang="en">has language</rdfs:label>
        <skos:notation rdf:datatype="http://www.w3.org/2001/XMLSchema#string">P72</skos:notation>
    </owl:ObjectProperty>
    


    <!-- http://www.cidoc-crm.org/cidoc-crm/P73 -->

    <owl:ObjectProperty rdf:about="http://www.cidoc-crm.org/cidoc-crm/P73">
        <rdfs:domain rdf:resource="http://www.cidoc-crm.org/cidoc-crm/E33"/>
        <rdfs:range rdf:resource="http://www.cidoc-crm.org/cidoc-crm/E33"/>
        <rdfs:comment xml:lang="en">This property describes the source and target of instances of E33Linguistic Object involved in a translation. When a Linguistic
            Object is translated into a new language it becomes a new Linguistic Object, despite being conceptually similar to the source object. </rdfs:comment>
        <rdfs:label xml:lang="en">has translation</rdfs:label>
        <skos:notation rdf:datatype="http://www.w3.org/2001/XMLSchema#string">P73</skos:notation>
    </owl:ObjectProperty>
    


    <!-- http://www.cidoc-crm.org/cidoc-crm/P74 -->

    <owl:ObjectProperty rdf:about="http://www.cidoc-crm.org/cidoc-crm/P74">
        <rdfs:domain rdf:resource="http://www.cidoc-crm.org/cidoc-crm/E39"/>
        <rdfs:range rdf:resource="http://www.cidoc-crm.org/cidoc-crm/E53"/>
        <rdfs:comment xml:lang="en">This property describes the current or former E53 Place of residence of an E39 Actor. The residence may be either the Place
            where the Actor resides, or a legally registered address of any kind. </rdfs:comment>
        <rdfs:label xml:lang="en">has current or former residence</rdfs:label>
        <skos:notation rdf:datatype="http://www.w3.org/2001/XMLSchema#string">P74</skos:notation>
    </owl:ObjectProperty>
    


    <!-- http://www.cidoc-crm.org/cidoc-crm/P75 -->

    <owl:ObjectProperty rdf:about="http://www.cidoc-crm.org/cidoc-crm/P75">
        <rdfs:domain rdf:resource="http://www.cidoc-crm.org/cidoc-crm/E39"/>
        <rdfs:range rdf:resource="http://www.cidoc-crm.org/cidoc-crm/E30"/>
        <rdfs:comment xml:lang="en">This property identifies former or current instances of E30 Rights held by an E39 Actor.</rdfs:comment>
        <rdfs:label xml:lang="en">possesses</rdfs:label>
        <skos:notation rdf:datatype="http://www.w3.org/2001/XMLSchema#string">P75</skos:notation>
    </owl:ObjectProperty>
    


    <!-- http://www.cidoc-crm.org/cidoc-crm/P76 -->

    <owl:ObjectProperty rdf:about="http://www.cidoc-crm.org/cidoc-crm/P76">
        <rdfs:domain rdf:resource="http://www.cidoc-crm.org/cidoc-crm/E39"/>
        <rdfs:range rdf:resource="http://www.cidoc-crm.org/cidoc-crm/E51"/>
        <rdfs:comment xml:lang="en">This property identifies an E51 Contact Point of any type that provides access to an E39 Actor by any communication method, such
            as e-mail or fax. </rdfs:comment>
        <rdfs:label xml:lang="en">has contact point</rdfs:label>
        <skos:notation rdf:datatype="http://www.w3.org/2001/XMLSchema#string">P76</skos:notation>
    </owl:ObjectProperty>
    


    <!-- http://www.cidoc-crm.org/cidoc-crm/P78 -->

    <owl:ObjectProperty rdf:about="http://www.cidoc-crm.org/cidoc-crm/P78">
        <rdfs:domain rdf:resource="http://www.cidoc-crm.org/cidoc-crm/E52"/>
        <rdfs:range rdf:resource="http://www.cidoc-crm.org/cidoc-crm/E49"/>
        <rdfs:comment xml:lang="en">This property identifies an E52 Time-Span using an E49Time Appellation.</rdfs:comment>
        <rdfs:label xml:lang="en">is identified by</rdfs:label>
        <skos:notation rdf:datatype="http://www.w3.org/2001/XMLSchema#string">P78</skos:notation>
    </owl:ObjectProperty>
    


    <!-- http://www.cidoc-crm.org/cidoc-crm/P79 -->

    <owl:ObjectProperty rdf:about="http://www.cidoc-crm.org/cidoc-crm/P79">
        <rdfs:domain rdf:resource="http://www.cidoc-crm.org/cidoc-crm/E52"/>
        <rdfs:range rdf:resource="http://www.cidoc-crm.org/cidoc-crm/E62"/>
        <rdfs:comment xml:lang="en">This property qualifies the beginning of an E52 Time-Span in some way. The nature of the qualification may be certainty,
            precision, source etc. </rdfs:comment>
        <rdfs:label xml:lang="en">beginning is qualified by</rdfs:label>
        <skos:notation rdf:datatype="http://www.w3.org/2001/XMLSchema#string">P79</skos:notation>
    </owl:ObjectProperty>
    


    <!-- http://www.cidoc-crm.org/cidoc-crm/P8 -->

    <owl:ObjectProperty rdf:about="http://www.cidoc-crm.org/cidoc-crm/P8">
        <rdfs:domain rdf:resource="http://www.cidoc-crm.org/cidoc-crm/E4"/>
        <rdfs:range rdf:resource="http://www.cidoc-crm.org/cidoc-crm/E18"/>
        <rdfs:comment xml:lang="en">This property describes the location of an instance of E4 Period with respect to an E19 Physical Object. P8 took place on or
            within (witnessed) is a shortcut of the more fully developed path from E4 Period through P7 took place at, E53 Place, P156 occupies (is
            occupied by) to E18 Physical Thing. It describes a period that can be located with respect to the space defined by an E19 Physical Object
            such as a ship or a building. The precise geographical location of the object during the period in question may be unknown or unimportant.
            For example, the French and German armistice of 22 June 1940 was signed in the same railway carriage as the armistice of 11 November 1918. </rdfs:comment>
        <rdfs:label xml:lang="en">took place on or within</rdfs:label>
        <skos:notation rdf:datatype="http://www.w3.org/2001/XMLSchema#string">P8</skos:notation>
    </owl:ObjectProperty>
    


    <!-- http://www.cidoc-crm.org/cidoc-crm/P80 -->

    <owl:ObjectProperty rdf:about="http://www.cidoc-crm.org/cidoc-crm/P80">
        <rdfs:domain rdf:resource="http://www.cidoc-crm.org/cidoc-crm/E52"/>
        <rdfs:range rdf:resource="http://www.cidoc-crm.org/cidoc-crm/E62"/>
        <rdfs:comment xml:lang="en">This property qualifies the end of an E52 Time-Span in some way. The nature of the qualification may be certainty, precision,
            source etc. </rdfs:comment>
        <rdfs:label xml:lang="en">end is qualified by</rdfs:label>
        <skos:notation rdf:datatype="http://www.w3.org/2001/XMLSchema#string">P80</skos:notation>
    </owl:ObjectProperty>
    


    <!-- http://www.cidoc-crm.org/cidoc-crm/P81 -->

    <owl:ObjectProperty rdf:about="http://www.cidoc-crm.org/cidoc-crm/P81">
        <rdfs:domain rdf:resource="http://www.cidoc-crm.org/cidoc-crm/E52"/>
        <rdfs:range rdf:resource="http://www.cidoc-crm.org/cidoc-crm/E61"/>
        <rdfs:comment xml:lang="en">This property describes the minimum period of time covered by an E52 Time-Span. Since Time-Spans may not have precisely known
            temporal extents, the CRM supports statements about the minimum and maximum temporal extents of Time-Spans. This property allows a
            Time-Span’s minimum temporal extent (i.e. its inner boundary) to be assigned an E61 Time Primitive value. Time Primitives are treated by
            the CRM as application or system specific date intervals, and are not further analysed. </rdfs:comment>
        <rdfs:label xml:lang="en">ongoing throughout</rdfs:label>
        <skos:notation rdf:datatype="http://www.w3.org/2001/XMLSchema#string">P81</skos:notation>
    </owl:ObjectProperty>
    


    <!-- http://www.cidoc-crm.org/cidoc-crm/P81a -->

    <owl:ObjectProperty rdf:about="http://www.cidoc-crm.org/cidoc-crm/P81a">
        <rdfs:domain rdf:resource="http://www.cidoc-crm.org/cidoc-crm/E52"/>
        <rdfs:range rdf:resource="http://www.cidoc-crm.org/cidoc-crm/E61"/>
        <rdfs:comment xml:lang="en">This is defined as the first boundary of the property P81</rdfs:comment>
        <rdfs:label xml:lang="en">end of the begin</rdfs:label>
        <skos:notation rdf:datatype="http://www.w3.org/2001/XMLSchema#string">P81a</skos:notation>
    </owl:ObjectProperty>
    


    <!-- http://www.cidoc-crm.org/cidoc-crm/P81b -->

    <owl:ObjectProperty rdf:about="http://www.cidoc-crm.org/cidoc-crm/P81b">
        <rdfs:domain rdf:resource="http://www.cidoc-crm.org/cidoc-crm/E52"/>
        <rdfs:range rdf:resource="http://www.cidoc-crm.org/cidoc-crm/E61"/>
        <rdfs:comment xml:lang="en">This is defined as the second boundary of the property P81</rdfs:comment>
        <rdfs:label xml:lang="en">begin of the end</rdfs:label>
        <skos:notation rdf:datatype="http://www.w3.org/2001/XMLSchema#string">P81b</skos:notation>
    </owl:ObjectProperty>
    


    <!-- http://www.cidoc-crm.org/cidoc-crm/P82 -->

    <owl:ObjectProperty rdf:about="http://www.cidoc-crm.org/cidoc-crm/P82">
        <rdfs:domain rdf:resource="http://www.cidoc-crm.org/cidoc-crm/E52"/>
        <rdfs:range rdf:resource="http://www.cidoc-crm.org/cidoc-crm/E61"/>
        <rdfs:comment xml:lang="en">This property describes the maximum period of time within which an E52 Time-Span falls. Since Time-Spans may not have precisely
            known temporal extents, the CRM supports statements about the minimum and maximum temporal extents of Time-Spans. This property allows a
            Time-Span’s maximum temporal extent (i.e. its outer boundary) to be assigned an E61 Time Primitive value. Time Primitives are treated by
            the CRM as application or system specific date intervals, and are not further analysed. </rdfs:comment>
        <rdfs:label xml:lang="en">at some time within</rdfs:label>
        <skos:notation rdf:datatype="http://www.w3.org/2001/XMLSchema#string">P82</skos:notation>
    </owl:ObjectProperty>
    


    <!-- http://www.cidoc-crm.org/cidoc-crm/P82a -->

    <owl:ObjectProperty rdf:about="http://www.cidoc-crm.org/cidoc-crm/P82a">
        <rdfs:domain rdf:resource="http://www.cidoc-crm.org/cidoc-crm/E52"/>
        <rdfs:range rdf:resource="http://www.cidoc-crm.org/cidoc-crm/E61"/>
        <rdfs:comment xml:lang="en">This is defined as the first boundary of the property P82</rdfs:comment>
        <rdfs:label xml:lang="en">begin of the begin</rdfs:label>
        <skos:notation rdf:datatype="http://www.w3.org/2001/XMLSchema#string">P82a</skos:notation>
    </owl:ObjectProperty>
    


    <!-- http://www.cidoc-crm.org/cidoc-crm/P82b -->

    <owl:ObjectProperty rdf:about="http://www.cidoc-crm.org/cidoc-crm/P82b">
        <rdfs:domain rdf:resource="http://www.cidoc-crm.org/cidoc-crm/E52"/>
        <rdfs:range rdf:resource="http://www.cidoc-crm.org/cidoc-crm/E61"/>
        <rdfs:comment xml:lang="en">This is defined as the second boundary of the property P82</rdfs:comment>
        <rdfs:label xml:lang="en">end of the end</rdfs:label>
        <skos:notation rdf:datatype="http://www.w3.org/2001/XMLSchema#string">P82b</skos:notation>
    </owl:ObjectProperty>
    


    <!-- http://www.cidoc-crm.org/cidoc-crm/P83 -->

    <owl:ObjectProperty rdf:about="http://www.cidoc-crm.org/cidoc-crm/P83">
        <rdfs:domain rdf:resource="http://www.cidoc-crm.org/cidoc-crm/E52"/>
        <rdfs:range rdf:resource="http://www.cidoc-crm.org/cidoc-crm/E54"/>
        <rdfs:comment xml:lang="en">This property describes the minimum length of time covered by an E52 Time-Span. It allows an E52 Time-Span to be associated with
            an E54 Dimension representing it’s minimum duration (i.e. it’s inner boundary) independent from the actual beginning and end. </rdfs:comment>
        <rdfs:label xml:lang="en">had at least duration</rdfs:label>
        <skos:notation rdf:datatype="http://www.w3.org/2001/XMLSchema#string">P83</skos:notation>
    </owl:ObjectProperty>
    


    <!-- http://www.cidoc-crm.org/cidoc-crm/P84 -->

    <owl:ObjectProperty rdf:about="http://www.cidoc-crm.org/cidoc-crm/P84">
        <rdfs:domain rdf:resource="http://www.cidoc-crm.org/cidoc-crm/E52"/>
        <rdfs:range rdf:resource="http://www.cidoc-crm.org/cidoc-crm/E54"/>
        <rdfs:comment xml:lang="en">This property describes the maximum length of time covered by an E52 Time-Span. It allows an E52 Time-Span to be associated with
            an E54 Dimension representing it’s maximum duration (i.e. it’s outer boundary) independent from the actual beginning and end. </rdfs:comment>
        <rdfs:label xml:lang="en">had at most duration</rdfs:label>
        <skos:notation rdf:datatype="http://www.w3.org/2001/XMLSchema#string">P84</skos:notation>
    </owl:ObjectProperty>
    


    <!-- http://www.cidoc-crm.org/cidoc-crm/P86 -->

    <owl:ObjectProperty rdf:about="http://www.cidoc-crm.org/cidoc-crm/P86">
        <rdfs:domain rdf:resource="http://www.cidoc-crm.org/cidoc-crm/E52"/>
        <rdfs:range rdf:resource="http://www.cidoc-crm.org/cidoc-crm/E52"/>
        <rdfs:comment xml:lang="en">This property describes the inclusion relationship between two instances of E52 Time-Span. This property supports the notion
            that a Time-Span’s temporal extent falls within the temporal extent of another Time-Span. It addresses temporal containment only, and no
            contextual link between the two instances of Time-Span is implied. </rdfs:comment>
        <rdfs:label xml:lang="en">falls within</rdfs:label>
        <skos:notation rdf:datatype="http://www.w3.org/2001/XMLSchema#string">P86</skos:notation>
    </owl:ObjectProperty>
    


    <!-- http://www.cidoc-crm.org/cidoc-crm/P87 -->

    <owl:ObjectProperty rdf:about="http://www.cidoc-crm.org/cidoc-crm/P87">
        <rdfs:domain rdf:resource="http://www.cidoc-crm.org/cidoc-crm/E53"/>
        <rdfs:range rdf:resource="http://www.cidoc-crm.org/cidoc-crm/E44"/>
        <rdfs:comment xml:lang="en">This property identifies an E53 Place using an E44 Place Appellation. Examples of Place Appellations used to identify Places
            include instances of E48 Place Name, addresses, E47 Spatial Coordinates etc. </rdfs:comment>
        <rdfs:label xml:lang="en">is identified by</rdfs:label>
        <skos:notation rdf:datatype="http://www.w3.org/2001/XMLSchema#string">P87</skos:notation>
    </owl:ObjectProperty>
    


    <!-- http://www.cidoc-crm.org/cidoc-crm/P89 -->

    <owl:ObjectProperty rdf:about="http://www.cidoc-crm.org/cidoc-crm/P89">
        <rdfs:domain rdf:resource="http://www.cidoc-crm.org/cidoc-crm/E53"/>
        <rdfs:range rdf:resource="http://www.cidoc-crm.org/cidoc-crm/E53"/>
        <rdfs:comment xml:lang="en">This property identifies an instance of E53 Place that falls wholly within the extent of another E53 Place. It addresses spatial
            containment only, and does not imply any relationship between things or phenomena occupying these places. </rdfs:comment>
        <rdfs:label xml:lang="en">falls within</rdfs:label>
        <skos:notation rdf:datatype="http://www.w3.org/2001/XMLSchema#string">P89</skos:notation>
    </owl:ObjectProperty>
    


    <!-- http://www.cidoc-crm.org/cidoc-crm/P9 -->

    <owl:ObjectProperty rdf:about="http://www.cidoc-crm.org/cidoc-crm/P9">
        <rdfs:domain rdf:resource="http://www.cidoc-crm.org/cidoc-crm/E4"/>
        <rdfs:range rdf:resource="http://www.cidoc-crm.org/cidoc-crm/E4"/>
        <rdfs:comment xml:lang="en">This property associates an instance of E4 Period with another instance of E4 Period that is defined by a subset of the
            phenomena that define the former. Therefore the spacetime volume of the latter must fall within the spacetime volume of the former. </rdfs:comment>
        <rdfs:label xml:lang="en">consists of</rdfs:label>
        <skos:notation rdf:datatype="http://www.w3.org/2001/XMLSchema#string">P9</skos:notation>
    </owl:ObjectProperty>
    


    <!-- http://www.cidoc-crm.org/cidoc-crm/P90 -->

    <owl:ObjectProperty rdf:about="http://www.cidoc-crm.org/cidoc-crm/P90">
        <rdfs:domain rdf:resource="http://www.cidoc-crm.org/cidoc-crm/E54"/>
        <rdfs:range rdf:resource="http://www.cidoc-crm.org/cidoc-crm/E60"/>
        <rdfs:comment xml:lang="en">This property allows an E54 Dimension to be approximated by an E60 Number primitive.</rdfs:comment>
        <rdfs:label xml:lang="en">has value</rdfs:label>
        <skos:notation rdf:datatype="http://www.w3.org/2001/XMLSchema#string">P90</skos:notation>
    </owl:ObjectProperty>
    


    <!-- http://www.cidoc-crm.org/cidoc-crm/P91 -->

    <owl:ObjectProperty rdf:about="http://www.cidoc-crm.org/cidoc-crm/P91">
        <rdfs:domain rdf:resource="http://www.cidoc-crm.org/cidoc-crm/E54"/>
        <rdfs:range rdf:resource="http://www.cidoc-crm.org/cidoc-crm/E58"/>
        <rdfs:comment xml:lang="en">This property shows the type of unit an E54 Dimension was expressed in.</rdfs:comment>
        <rdfs:label xml:lang="en">has unit</rdfs:label>
        <skos:notation rdf:datatype="http://www.w3.org/2001/XMLSchema#string">P91</skos:notation>
    </owl:ObjectProperty>
    


    <!-- http://www.cidoc-crm.org/cidoc-crm/P92 -->

    <owl:ObjectProperty rdf:about="http://www.cidoc-crm.org/cidoc-crm/P92">
        <rdfs:domain rdf:resource="http://www.cidoc-crm.org/cidoc-crm/E63"/>
        <rdfs:range rdf:resource="http://www.cidoc-crm.org/cidoc-crm/E77"/>
        <rdfs:comment xml:lang="en">This property allows an E63 Beginning of Existence event to be linked to the E77 Persistent Item brought into existence by it.
            It allows a “start” to be attached to any Persistent Item being documented i.e. E70 Thing, E72 Legal Object, E39 Actor, E41 Appellation,
            E51 Contact Point and E55 Type</rdfs:comment>
        <rdfs:label xml:lang="en">brought into existence</rdfs:label>
        <skos:notation rdf:datatype="http://www.w3.org/2001/XMLSchema#string">P92</skos:notation>
    </owl:ObjectProperty>
    


    <!-- http://www.cidoc-crm.org/cidoc-crm/P93 -->

    <owl:ObjectProperty rdf:about="http://www.cidoc-crm.org/cidoc-crm/P93">
        <rdfs:domain rdf:resource="http://www.cidoc-crm.org/cidoc-crm/E64"/>
        <rdfs:range rdf:resource="http://www.cidoc-crm.org/cidoc-crm/E77"/>
        <rdfs:comment xml:lang="en">This property allows an E64 End of Existence event to be linked to the E77 Persistent Item taken out of existence by it. In the
            case of immaterial things, the E64 End of Existence is considered to take place with the destruction of the last physical carrier. This
            allows an “end” to be attached to any Persistent Item being documented i.e. E70 Thing, E72 Legal Object, E39 Actor, E41 Appellation, E51
            Contact Point and E55 Type. For many Persistent Items we know the maximum life-span and can infer, that they must have ended to exist. We
            assume in that case an End of Existence, which may be as unnoticeable as forgetting the secret knowledge by the last representative of
            some indigenous nation. </rdfs:comment>
        <rdfs:label xml:lang="en">took out of existence</rdfs:label>
        <skos:notation rdf:datatype="http://www.w3.org/2001/XMLSchema#string">P93</skos:notation>
    </owl:ObjectProperty>
    


    <!-- http://www.cidoc-crm.org/cidoc-crm/P94 -->

    <owl:ObjectProperty rdf:about="http://www.cidoc-crm.org/cidoc-crm/P94">
        <rdfs:domain rdf:resource="http://www.cidoc-crm.org/cidoc-crm/E65"/>
        <rdfs:range rdf:resource="http://www.cidoc-crm.org/cidoc-crm/E28"/>
        <rdfs:comment xml:lang="en">This property allows a conceptual E65 Creation to be linked to the E28 Conceptual Object created by it. It represents the act of
            conceiving the intellectual content of the E28 Conceptual Object. It does not represent the act of creating the first physical carrier of
            the E28 Conceptual Object. As an example, this is the composition of a poem, not its commitment to paper. </rdfs:comment>
        <rdfs:label xml:lang="en">has created</rdfs:label>
        <skos:notation rdf:datatype="http://www.w3.org/2001/XMLSchema#string">P94</skos:notation>
    </owl:ObjectProperty>
    


    <!-- http://www.cidoc-crm.org/cidoc-crm/P95 -->

    <owl:ObjectProperty rdf:about="http://www.cidoc-crm.org/cidoc-crm/P95">
        <rdfs:domain rdf:resource="http://www.cidoc-crm.org/cidoc-crm/E66"/>
        <rdfs:range rdf:resource="http://www.cidoc-crm.org/cidoc-crm/E74"/>
        <rdfs:comment xml:lang="en">This property links the founding or E66 Formation for an E74 Group with the Group itself.</rdfs:comment>
        <rdfs:label xml:lang="en">has formed</rdfs:label>
        <skos:notation rdf:datatype="http://www.w3.org/2001/XMLSchema#string">P95</skos:notation>
    </owl:ObjectProperty>
    


    <!-- http://www.cidoc-crm.org/cidoc-crm/P96 -->

    <owl:ObjectProperty rdf:about="http://www.cidoc-crm.org/cidoc-crm/P96">
        <rdfs:domain rdf:resource="http://www.cidoc-crm.org/cidoc-crm/E67"/>
        <rdfs:range rdf:resource="http://www.cidoc-crm.org/cidoc-crm/E21"/>
        <rdfs:comment xml:lang="en">This property links an E67 Birth event to an E21 Person as a participant in the role of birth-giving mother. Note that
            biological fathers are not necessarily participants in the Birth (see P97 from father (was father for)). The Person being born is linked
            to the Birth with the property P98 brought into life (was born). This is not intended for use with general natural history material, only
            people. There is no explicit method for modelling conception and gestation except by using extensions. This is a sub-property of P11 had
            participant (participated in).</rdfs:comment>
        <rdfs:label xml:lang="en">by mother</rdfs:label>
        <skos:notation rdf:datatype="http://www.w3.org/2001/XMLSchema#string">P96</skos:notation>
    </owl:ObjectProperty>
    


    <!-- http://www.cidoc-crm.org/cidoc-crm/P97 -->

    <owl:ObjectProperty rdf:about="http://www.cidoc-crm.org/cidoc-crm/P97">
        <rdfs:domain rdf:resource="http://www.cidoc-crm.org/cidoc-crm/E67"/>
        <rdfs:range rdf:resource="http://www.cidoc-crm.org/cidoc-crm/E21"/>
        <rdfs:comment xml:lang="en">This property links an E67 Birth event to an E21 Person in the role of biological father. Note that biological fathers are not
            seen as necessary participants in the Birth, whereas birth-giving mothers are (see P96 by mother (gave birth)). The Person being born is
            linked to the Birth with the property P98 brought into life (was born). This is not intended for use with general natural history
            material, only people. There is no explicit method for modelling conception and gestation except by using extensions. A Birth event is
            normally (but not always) associated with one biological father.</rdfs:comment>
        <rdfs:label xml:lang="en">from father</rdfs:label>
        <skos:notation rdf:datatype="http://www.w3.org/2001/XMLSchema#string">P97</skos:notation>
    </owl:ObjectProperty>
    


    <!-- http://www.cidoc-crm.org/cidoc-crm/P98 -->

    <owl:ObjectProperty rdf:about="http://www.cidoc-crm.org/cidoc-crm/P98">
        <rdfs:domain rdf:resource="http://www.cidoc-crm.org/cidoc-crm/E67"/>
        <rdfs:range rdf:resource="http://www.cidoc-crm.org/cidoc-crm/E21"/>
        <rdfs:comment xml:lang="en">This property links an E67Birth event to an E21 Person in the role of offspring. Twins, triplets etc. are brought into life by
            the same Birth event. This is not intended for use with general Natural History material, only people. There is no explicit method for
            modelling conception and gestation except by using extensions. </rdfs:comment>
        <rdfs:label xml:lang="en">brought into life</rdfs:label>
        <skos:notation rdf:datatype="http://www.w3.org/2001/XMLSchema#string">P98</skos:notation>
    </owl:ObjectProperty>
    


    <!-- http://www.cidoc-crm.org/cidoc-crm/P99 -->

    <owl:ObjectProperty rdf:about="http://www.cidoc-crm.org/cidoc-crm/P99">
        <rdfs:domain rdf:resource="http://www.cidoc-crm.org/cidoc-crm/E68"/>
        <rdfs:range rdf:resource="http://www.cidoc-crm.org/cidoc-crm/E74"/>
        <rdfs:comment xml:lang="en">This property links the disbanding or E68 Dissolution of an E74 Group to the Group itself.</rdfs:comment>
        <rdfs:label xml:lang="en">dissolved</rdfs:label>
        <skos:notation rdf:datatype="http://www.w3.org/2001/XMLSchema#string">P99</skos:notation>
    </owl:ObjectProperty>
    


    <!-- https://dataforhistory.org/ontology/maritimehistorycontinued/P10 -->

    <owl:ObjectProperty rdf:about="https://dataforhistory.org/ontology/maritimehistorycontinued/P10">
        <rdfs:domain rdf:resource="http://dataforhistory.org/histdmi-generic-ongoing/class/C4"/>
        <rdfs:range rdf:resource="http://www.cidoc-crm.org/cidoc-crm/E18"/>
        <rdfs:label xml:lang="en">transported</rdfs:label>
    </owl:ObjectProperty>
    


    <!-- https://dataforhistory.org/ontology/maritimehistorycontinued/P11 -->

    <owl:ObjectProperty rdf:about="https://dataforhistory.org/ontology/maritimehistorycontinued/P11">
        <rdfs:domain rdf:resource="http://dataforhistory.org/histsocial-ongoing/class/C7"/>
        <rdfs:range rdf:resource="http://www.cidoc-crm.org/cidoc-crm/E97"/>
        <rdfs:label xml:lang="en">monetary compensation</rdfs:label>
    </owl:ObjectProperty>
    


    <!-- https://dataforhistory.org/ontology/maritimehistorycontinued/P12 -->

    <owl:ObjectProperty rdf:about="https://dataforhistory.org/ontology/maritimehistorycontinued/P12">
        <rdfs:domain rdf:resource="http://www.cidoc-crm.org/cidoc-crm/E70"/>
        <rdfs:range rdf:resource="http://www.cidoc-crm.org/cidoc-crm/E97"/>
        <rdfs:label xml:lang="en">monetary amount</rdfs:label>
    </owl:ObjectProperty>
    


    <!-- https://dataforhistory.org/ontology/maritimehistorycontinued/P19 -->

    <owl:ObjectProperty rdf:about="https://dataforhistory.org/ontology/maritimehistorycontinued/P19">
        <rdfs:domain rdf:resource="http://dataforhistory.org/histsocial-ongoing/class/C7"/>
        <rdfs:range rdf:resource="https://dataforhistory.org/ontology/maritimehistorycontinued/C6"/>
        <rdfs:label xml:lang="en">has responsibility</rdfs:label>
    </owl:ObjectProperty>
    


    <!-- https://dataforhistory.org/ontology/maritimehistorycontinued/P3 -->

    <owl:ObjectProperty rdf:about="https://dataforhistory.org/ontology/maritimehistorycontinued/P3">
        <rdfs:domain rdf:resource="http://www.cidoc-crm.org/cidoc-crm/E40"/>
        <rdfs:range rdf:resource="http://dataforhistory.org/histdmi-generic-ongoing/class/C15"/>
        <rdfs:label xml:lang="en">established in</rdfs:label>
    </owl:ObjectProperty>
    


    <!-- https://dataforhistory.org/ontology/maritimehistorycontinued/P4 -->

    <owl:ObjectProperty rdf:about="https://dataforhistory.org/ontology/maritimehistorycontinued/P4">
        <rdfs:domain rdf:resource="http://www.cidoc-crm.org/cidoc-crm/E39"/>
        <rdfs:range rdf:resource="https://dataforhistory.org/ontology/maritimehistorycontinued/C1"/>
        <rdfs:label xml:lang="en">embarked during</rdfs:label>
    </owl:ObjectProperty>
    


    <!-- https://dataforhistory.org/ontology/maritimehistorycontinued/P5 -->

    <owl:ObjectProperty rdf:about="https://dataforhistory.org/ontology/maritimehistorycontinued/P5">
        <rdfs:domain rdf:resource="http://www.cidoc-crm.org/cidoc-crm/E39"/>
        <rdfs:range rdf:resource="https://dataforhistory.org/ontology/maritimehistorycontinued/C2"/>
        <rdfs:label xml:lang="en">disembarked during</rdfs:label>
    </owl:ObjectProperty>
    


    <!-- https://dataforhistory.org/ontology/maritimehistorycontinued/P6 -->

    <owl:ObjectProperty rdf:about="https://dataforhistory.org/ontology/maritimehistorycontinued/P6">
        <rdfs:domain rdf:resource="http://www.cidoc-crm.org/cidoc-crm/E18"/>
        <rdfs:range rdf:resource="https://dataforhistory.org/ontology/maritimehistorycontinued/C1"/>
        <rdfs:label xml:lang="en">loaded during</rdfs:label>
    </owl:ObjectProperty>
    


    <!-- https://dataforhistory.org/ontology/maritimehistorycontinued/P7 -->

    <owl:ObjectProperty rdf:about="https://dataforhistory.org/ontology/maritimehistorycontinued/P7">
        <rdfs:domain rdf:resource="http://www.cidoc-crm.org/cidoc-crm/E18"/>
        <rdfs:range rdf:resource="https://dataforhistory.org/ontology/maritimehistorycontinued/C2"/>
        <rdfs:label xml:lang="en">unloaded during</rdfs:label>
    </owl:ObjectProperty>
    


    <!-- 
    ///////////////////////////////////////////////////////////////////////////////////////
    //
    // Data properties
    //
    ///////////////////////////////////////////////////////////////////////////////////////
     -->

    


    <!-- http://www.cidoc-crm.org/cidoc-crm/P3 -->

    <owl:DatatypeProperty rdf:about="http://www.cidoc-crm.org/cidoc-crm/P3"/>
    


    <!-- https://dataforhistory.org/ontology/maritimehistorycontinued/P1 -->

    <owl:DatatypeProperty rdf:about="https://dataforhistory.org/ontology/maritimehistorycontinued/P1">
        <rdfs:label xml:lang="en">voy particulars</rdfs:label>
    </owl:DatatypeProperty>
    


    <!-- https://dataforhistory.org/ontology/maritimehistorycontinued/P13 -->

    <owl:DatatypeProperty rdf:about="https://dataforhistory.org/ontology/maritimehistorycontinued/P13">
        <rdfs:label xml:lang="en">place end contract</rdfs:label>
    </owl:DatatypeProperty>
    


    <!-- https://dataforhistory.org/ontology/maritimehistorycontinued/P14 -->

    <owl:DatatypeProperty rdf:about="https://dataforhistory.org/ontology/maritimehistorycontinued/P14">
        <rdfs:subPropertyOf rdf:resource="https://dataforhistory.org/ontology/maritimehistorycontinued/P8"/>
        <rdfs:label rdf:datatype="http://www.w3.org/2001/XMLSchema#string">original vocop</rdfs:label>
    </owl:DatatypeProperty>
    


    <!-- https://dataforhistory.org/ontology/maritimehistorycontinued/P15 -->

    <owl:DatatypeProperty rdf:about="https://dataforhistory.org/ontology/maritimehistorycontinued/P15">
        <rdfs:label xml:lang="en">cargo specification</rdfs:label>
    </owl:DatatypeProperty>
    


    <!-- https://dataforhistory.org/ontology/maritimehistorycontinued/P17 -->

    <owl:DatatypeProperty rdf:about="https://dataforhistory.org/ontology/maritimehistorycontinued/P17">
        <rdfs:subPropertyOf rdf:resource="https://dataforhistory.org/ontology/maritimehistorycontinued/P8"/>
        <rdfs:label xml:lang="en">original place of birth</rdfs:label>
    </owl:DatatypeProperty>
    


    <!-- https://dataforhistory.org/ontology/maritimehistorycontinued/P18 -->

    <owl:DatatypeProperty rdf:about="https://dataforhistory.org/ontology/maritimehistorycontinued/P18">
        <rdfs:subPropertyOf rdf:resource="https://dataforhistory.org/ontology/maritimehistorycontinued/P8"/>
        <rdfs:label xml:lang="en">original rank</rdfs:label>
    </owl:DatatypeProperty>
    


    <!-- https://dataforhistory.org/ontology/maritimehistorycontinued/P2 -->

    <owl:DatatypeProperty rdf:about="https://dataforhistory.org/ontology/maritimehistorycontinued/P2">
        <rdfs:label xml:lang="en">direction of voyage</rdfs:label>
    </owl:DatatypeProperty>
    


    <!-- https://dataforhistory.org/ontology/maritimehistorycontinued/P20 -->

    <owl:DatatypeProperty rdf:about="https://dataforhistory.org/ontology/maritimehistorycontinued/P20">
        <rdfs:domain rdf:resource="http://www.cidoc-crm.org/cidoc-crm/E47"/>
        <rdfs:label xml:lang="en">has WKT</rdfs:label>
    </owl:DatatypeProperty>
    


    <!-- https://dataforhistory.org/ontology/maritimehistorycontinued/P21 -->

    <owl:DatatypeProperty rdf:about="https://dataforhistory.org/ontology/maritimehistorycontinued/P21">
        <rdfs:label xml:lang="en">minimum tonnage</rdfs:label>
    </owl:DatatypeProperty>
    


    <!-- https://dataforhistory.org/ontology/maritimehistorycontinued/P22 -->

    <owl:DatatypeProperty rdf:about="https://dataforhistory.org/ontology/maritimehistorycontinued/P22">
        <rdfs:label xml:lang="en">maximum tonnage</rdfs:label>
    </owl:DatatypeProperty>
    


    <!-- https://dataforhistory.org/ontology/maritimehistorycontinued/P8 -->

    <owl:DatatypeProperty rdf:about="https://dataforhistory.org/ontology/maritimehistorycontinued/P8">
        <rdfs:label xml:lang="en">original appellation</rdfs:label>
    </owl:DatatypeProperty>
    


    <!-- https://dataforhistory.org/ontology/maritimehistorycontinued/P9 -->

    <owl:DatatypeProperty rdf:about="https://dataforhistory.org/ontology/maritimehistorycontinued/P9">
        <rdfs:subPropertyOf rdf:resource="https://dataforhistory.org/ontology/maritimehistorycontinued/P8"/>
        <rdfs:label xml:lang="en">original date</rdfs:label>
    </owl:DatatypeProperty>
    


    <!-- 
    ///////////////////////////////////////////////////////////////////////////////////////
    //
    // Classes
    //
    ///////////////////////////////////////////////////////////////////////////////////////
     -->

    


    <!-- http://dataforhistory.org/histdmi-generic-ongoing/class/C1 -->

    <owl:Class rdf:about="http://dataforhistory.org/histdmi-generic-ongoing/class/C1">
        <rdfs:subClassOf rdf:resource="http://www.cidoc-crm.org/cidoc-crm/E2"/>
        <rdfs:comment rdf:datatype="http://www.w3.org/2001/XMLSchema#string">This class models characteristics, qualities or conditions of persistent items or temporal entities at a given moment or during a time-span. This class is inspired by the perspective of DOLCE qualities which are defined as individualized properties that inhere in particulars: a quality therefore inheres in each class instance and ceases to exist at the end of the life of the instance it inheres to. The quality value or quale (DOLCE) is associated to the entity quality and valid throughout the whole time-span associated to it. The (time-indexed) characteristic or quality (DOLCE) is expressed by the present hist:C1 Entity Quality class and can be further specialized by a suitable quality type or creating subclasses with specific properties.
A characteristic or quality is initiated, influenced and ended by events (crm:E5 Event class) and this is modelled by correspondent properties. In contrast, no generic property is defined to associate any crm:E1 Entity with a quality. As a matter of fact not all subclasses of the hl4hss:C1 Entity Quality class concern the same types of entities and one cannot therefore extend an inheritance of a generic has quality property to all subclasses because this would imply, for example, that a physical object like a rock would virtually have a collective state of mind. In this perspective, the crm:E3 Condition State class can be considered as representig a specialization of the hl4hss:C1 Entity Quality class and the crm:P44 has condition (is condition of) property opportunely associates a physical object with its physical condition or state.</rdfs:comment>
        <rdfs:label xml:lang="en">Entity Quality</rdfs:label>
        <skos:notation rdf:datatype="http://www.w3.org/2001/XMLSchema#string">C1</skos:notation>
    </owl:Class>
    


    <!-- http://dataforhistory.org/histdmi-generic-ongoing/class/C11 -->

    <owl:Class rdf:about="http://dataforhistory.org/histdmi-generic-ongoing/class/C11">
        <rdfs:subClassOf rdf:resource="http://dataforhistory.org/histdmi-generic-ongoing/class/C30"/>
        <rdfs:comment rdf:datatype="http://www.w3.org/2001/XMLSchema#string">This class refers to the fact that an entity (actor, group, concept, etc.) is identified by a group using a specific appellation in a language during a given time span. [social dimension: to be added]
The class does not refer to the activity of continously or repetedly naming an entity with this specific appellation but to the possibility of identifying the entity with the given appellation in a given language.
The appellation is in this sense a property of the entity at given time and for a given language. The FRBRoo class F52_Name_Use_Activity models the activity actually carried out by a person or a group to use a given appellation, which is a distinct phenomenon. F52_Name_Use_Activity is a subclass of activity while the present class is about the given possibility (by use or by law) of using an appellation for identifying a given entity, and is therefore modeled as an entity characteristic.</rdfs:comment>
        <rdfs:label xml:lang="en">Appellation in a language (Temporal Entity)</rdfs:label>
        <skos:notation rdf:datatype="http://www.w3.org/2001/XMLSchema#string">C11</skos:notation>
    </owl:Class>
    


    <!-- http://dataforhistory.org/histdmi-generic-ongoing/class/C12 -->

    <owl:Class rdf:about="http://dataforhistory.org/histdmi-generic-ongoing/class/C12">
        <rdfs:subClassOf rdf:resource="http://www.cidoc-crm.org/cidoc-crm/E55"/>
        <rdfs:comment rdf:datatype="http://www.w3.org/2001/XMLSchema#string">This class comprises concepts denoted by terms from thesauri and controlled vocabularies used to characterize and classify instances of the C7 Appellation in a language (Temporal Entity) class.</rdfs:comment>
        <rdfs:label xml:lang="en">Appellation in a language type</rdfs:label>
        <skos:notation rdf:datatype="http://www.w3.org/2001/XMLSchema#string">C12</skos:notation>
    </owl:Class>
    


    <!-- http://dataforhistory.org/histdmi-generic-ongoing/class/C13 -->

    <owl:Class rdf:about="http://dataforhistory.org/histdmi-generic-ongoing/class/C13">
        <rdfs:subClassOf rdf:resource="http://www.cidoc-crm.org/cidoc-crm/E26"/>
        <rdfs:comment rdf:datatype="http://www.w3.org/2001/XMLSchema#string">This class refers to portions of the surface of the Earth intended as constellations of matter which can be represented by photographs, paintings and maps. The relevant portion of the surface of the Earth can be covered by water (river, sea, ...). The more specific identity of instances of this class is provided by a controlled vocabulary of geographical place types.</rdfs:comment>
        <rdfs:label xml:lang="en">Geographical Place</rdfs:label>
        <skos:notation rdf:datatype="http://www.w3.org/2001/XMLSchema#string">C13</skos:notation>
    </owl:Class>
    


    <!-- http://dataforhistory.org/histdmi-generic-ongoing/class/C14 -->

    <owl:Class rdf:about="http://dataforhistory.org/histdmi-generic-ongoing/class/C14">
        <rdfs:subClassOf rdf:resource="http://www.cidoc-crm.org/cidoc-crm/E55"/>
        <rdfs:comment rdf:datatype="http://www.w3.org/2001/XMLSchema#string">This class comprises concepts denoted by terms from thesauri and controlled vocabularies used to characterize and classify instances of the &apos;hictC8 Geographical place&apos;.</rdfs:comment>
        <rdfs:label xml:lang="en">Geographical Place Type</rdfs:label>
        <skos:notation rdf:datatype="http://www.w3.org/2001/XMLSchema#string">C14</skos:notation>
    </owl:Class>
    


    <!-- http://dataforhistory.org/histdmi-generic-ongoing/class/C15 -->

    <owl:Class rdf:about="http://dataforhistory.org/histdmi-generic-ongoing/class/C15">
        <rdfs:subClassOf rdf:resource="http://dataforhistory.org/histdmi-generic-ongoing/class/C1"/>
        <rdfs:comment rdf:datatype="http://www.w3.org/2001/XMLSchema#string">This class comprises generic geographical locations of persistent items during a given time span.
Given the different ways persistent items are &apos;located&apos; (human beings have legal domiciles but travel around, groups have registered head offices but could also move around, like the Swiss Federal Council having somewhere a meeting, and propositional objects are &apos;located&apos; where their carriers, human or physical, bring them), an opportune typology will allow the different cases to be distinguished. In contrast, the localisation of temporal entities is not modelled with this class.
If the precise location of a persistent item is not known, it can be located in a relative position with respect to another entity whose location is known.</rdfs:comment>
        <rdfs:label xml:lang="en">Geographical Location</rdfs:label>
        <skos:notation rdf:datatype="http://www.w3.org/2001/XMLSchema#string">C15</skos:notation>
    </owl:Class>
    


    <!-- http://dataforhistory.org/histdmi-generic-ongoing/class/C16 -->

    <owl:Class rdf:about="http://dataforhistory.org/histdmi-generic-ongoing/class/C16">
        <rdfs:subClassOf rdf:resource="http://www.cidoc-crm.org/cidoc-crm/E55"/>
        <rdfs:comment rdf:datatype="http://www.w3.org/2001/XMLSchema#string">This class comprises concepts denoted by terms from thesauri and controlled vocabularies used to characterize and classify instances of the &apos;histC2 Geographical localisation&apos;.</rdfs:comment>
        <rdfs:label xml:lang="en">Geographical Location type</rdfs:label>
        <skos:notation rdf:datatype="http://www.w3.org/2001/XMLSchema#string">C16</skos:notation>
    </owl:Class>
    


    <!-- http://dataforhistory.org/histdmi-generic-ongoing/class/C17 -->

    <owl:Class rdf:about="http://dataforhistory.org/histdmi-generic-ongoing/class/C17">
        <rdfs:subClassOf rdf:resource="http://www.cidoc-crm.org/cidoc-crm/E24"/>
        <rdfs:comment rdf:datatype="http://www.w3.org/2001/XMLSchema#string">This class comprises instances of man-made things such as freestanding buildings, components of buildings, and complexes of buildings, but also all man-made parts of infrastructure (roads, lamp post, dams, etc.)</rdfs:comment>
        <rdfs:label xml:lang="en">Built work</rdfs:label>
        <skos:notation rdf:datatype="http://www.w3.org/2001/XMLSchema#string">C17</skos:notation>
    </owl:Class>
    


    <!-- http://dataforhistory.org/histdmi-generic-ongoing/class/C18 -->

    <owl:Class rdf:about="http://dataforhistory.org/histdmi-generic-ongoing/class/C18">
        <rdfs:subClassOf rdf:resource="http://www.cidoc-crm.org/cidoc-crm/E55"/>
        <rdfs:comment rdf:datatype="http://www.w3.org/2001/XMLSchema#string">This class comprises concepts denoted by terms from thesauri and controlled vocabularies used to characterize and classify instances of the &apos;histC11 Built work class&apos;.</rdfs:comment>
        <rdfs:label xml:lang="en">Built work type</rdfs:label>
        <skos:notation rdf:datatype="http://www.w3.org/2001/XMLSchema#string">C18</skos:notation>
    </owl:Class>
    


    <!-- http://dataforhistory.org/histdmi-generic-ongoing/class/C19 -->

    <owl:Class rdf:about="http://dataforhistory.org/histdmi-generic-ongoing/class/C19">
        <rdfs:subClassOf rdf:resource="http://dataforhistory.org/histdmi-generic-ongoing/class/C4"/>
        <rdfs:comment rdf:datatype="http://www.w3.org/2001/XMLSchema#string">This class comprises all the crm:E5 events in which an instance of crm:E77 Persistent Item participates during its life. As a subclass of hist:C4 Phase this class therefore models the phenomenon if the existence or, more precisely, collection of the whole spatio-temporal phenomena related to the existence and life of a persistent item, be this a person, a group, a physical object, etc.
The life of a persistent item is started and ended by events.</rdfs:comment>
        <rdfs:label xml:lang="en">Persistent item life</rdfs:label>
        <skos:notation rdf:datatype="http://www.w3.org/2001/XMLSchema#string">C19</skos:notation>
    </owl:Class>
    


    <!-- http://dataforhistory.org/histdmi-generic-ongoing/class/C2 -->

    <owl:Class rdf:about="http://dataforhistory.org/histdmi-generic-ongoing/class/C2">
        <rdfs:subClassOf rdf:resource="http://dataforhistory.org/histdmi-generic-ongoing/class/C27"/>
        <rdfs:comment rdf:datatype="http://www.w3.org/2001/XMLSchema#string">This class models time-related phenomena (like an election or a marriage) that happen in collective intentionality, effect changes in the social connotation of actors or things and are only perceived in specific social contexts, i.e. persons sharing the same point of view or conceptualization. A social event exists if it P33 satisfies specific social representations, i.e. the conditions that makes it happen in the given society.
Social events, insofar as they happen in the minds of a human collective, do not directly have a projection in geographical space. But as they are always related to sets of human actions (one or more) that provide the setting for the given social events (P43 is setting for) they share with these physical events the geographical location. E.g. a marriage (social event), intended as a transition from being single to being married (in the context of a given society), has the wedding celebration (activity) as its setting.</rdfs:comment>
        <rdfs:label xml:lang="en">Social Event</rdfs:label>
        <skos:notation rdf:datatype="http://www.w3.org/2001/XMLSchema#string">C2</skos:notation>
    </owl:Class>
    


    <!-- http://dataforhistory.org/histdmi-generic-ongoing/class/C20 -->

    <owl:Class rdf:about="http://dataforhistory.org/histdmi-generic-ongoing/class/C20">
        <rdfs:subClassOf rdf:resource="http://www.cidoc-crm.org/cidoc-crm/E55"/>
        <rdfs:comment rdf:datatype="http://www.w3.org/2001/XMLSchema#string">
This class comprises concepts denoted by terms from thesauri and controlled vocabularies used to characterize and classify instances of the C1 Entity Quality class.
</rdfs:comment>
        <rdfs:label xml:lang="en">Entity Quality Type</rdfs:label>
        <skos:notation rdf:datatype="http://www.w3.org/2001/XMLSchema#string">C20</skos:notation>
    </owl:Class>
    


    <!-- http://dataforhistory.org/histdmi-generic-ongoing/class/C21 -->

    <owl:Class rdf:about="http://dataforhistory.org/histdmi-generic-ongoing/class/C21">
        <rdfs:subClassOf rdf:resource="http://dataforhistory.org/histdmi-generic-ongoing/class/C1"/>
        <rdfs:comment rdf:datatype="http://www.w3.org/2001/XMLSchema#string">This class models the ability, based on practical knowledge or know-how, and trained through practice, to do something well. Know-how can be about creating immaterial things, producing physical objects, acting or communicating. The skill is a personal quality, the know-how a shared representation of actions or processes.</rdfs:comment>
        <rdfs:label xml:lang="en">Skill</rdfs:label>
        <skos:notation rdf:datatype="http://www.w3.org/2001/XMLSchema#string">C21</skos:notation>
    </owl:Class>
    


    <!-- http://dataforhistory.org/histdmi-generic-ongoing/class/C22 -->

    <owl:Class rdf:about="http://dataforhistory.org/histdmi-generic-ongoing/class/C22">
        <rdfs:subClassOf rdf:resource="http://dataforhistory.org/histdmi-generic-ongoing/class/C1"/>
        <rdfs:comment rdf:datatype="http://www.w3.org/2001/XMLSchema#string">This class models the composition of instances of E18 Physical Thing out of their component elements and is therefore equivalent to the crm:P46 is composed of property but adds a time-indexed dimension to the composition relation, expressing the presence of parts only during a portion of the lifespan of a physical thing. The crm:P46 property is therefore a shortcut of this class and assumes implicitly that a part is present during the whole life of a physical thing.
This class can be specifically useful for dealing with the belonging of objects to a crm:E78 Collection (the composed, main physical thing) during a particular time-span.
This class is modeled as a subclass of C1 Entity quality (Temporal entity) and therefore instances of the crm:E5 Event class can initiate —P8 effects quality (result from)— or end —P9 ends (is ended by)— a different composition of a physical thing. In the case of instances of crm:E24 Physical Man-Made Thing, instances of E79 Part Addition and E80 Part Removal can be produced.
Component elements, since they are themselves instances of E18 Physical Thing, may be further analysed into sub-components, thereby creating a hierarchy of part decomposition, related to time.</rdfs:comment>
        <rdfs:label xml:lang="en">Composition</rdfs:label>
        <skos:notation rdf:datatype="http://www.w3.org/2001/XMLSchema#string">C22</skos:notation>
    </owl:Class>
    


    <!-- http://dataforhistory.org/histdmi-generic-ongoing/class/C23 -->

    <owl:Class rdf:about="http://dataforhistory.org/histdmi-generic-ongoing/class/C23">
        <rdfs:subClassOf rdf:resource="http://dataforhistory.org/histdmi-generic-ongoing/class/C4"/>
        <rdfs:comment rdf:datatype="http://www.w3.org/2001/XMLSchema#string">This class models the fact that an actor employs something or someone for some purpose for a more or less long period of time. Use is modelled as a phase and therefore includes many actions and activities, as well as possible interruptions, but remains active or at least virtually possible during the indicated period.</rdfs:comment>
        <rdfs:label xml:lang="en">Use</rdfs:label>
        <skos:notation rdf:datatype="http://www.w3.org/2001/XMLSchema#string">C23</skos:notation>
    </owl:Class>
    


    <!-- http://dataforhistory.org/histdmi-generic-ongoing/class/C24 -->

    <owl:Class rdf:about="http://dataforhistory.org/histdmi-generic-ongoing/class/C24">
        <rdfs:subClassOf rdf:resource="http://www.cidoc-crm.org/cidoc-crm/E55"/>
        <rdfs:comment rdf:datatype="http://www.w3.org/2001/XMLSchema#string"> 

This class comprises concepts denoted by terms from thesauri and controlled vocabularies used to characterize and classify instances of the &apos;C23 Use&apos; class.
</rdfs:comment>
        <rdfs:label xml:lang="en">Use type</rdfs:label>
        <skos:notation rdf:datatype="http://www.w3.org/2001/XMLSchema#string">C24</skos:notation>
    </owl:Class>
    


    <!-- http://dataforhistory.org/histdmi-generic-ongoing/class/C25 -->

    <owl:Class rdf:about="http://dataforhistory.org/histdmi-generic-ongoing/class/C25">
        <rdfs:subClassOf rdf:resource="http://www.cidoc-crm.org/cidoc-crm/E77"/>
        <rdfs:comment rdf:datatype="http://www.w3.org/2001/XMLSchema#string">A set of persons sharing the same social representations, i.e. the same point of view or conceptualization on things in the world, or the same know-how and practical attitudes, without acting collectively and therefore without being an identifiable crm:E74 Group, but being generally aware of sharing these conceptualizations with other people and thus having a common social identity based on social representations and collective intentionality.</rdfs:comment>
        <rdfs:label xml:lang="en">Social Collective</rdfs:label>
        <skos:notation rdf:datatype="http://www.w3.org/2001/XMLSchema#string">C25</skos:notation>
    </owl:Class>
    


    <!-- http://dataforhistory.org/histdmi-generic-ongoing/class/C26 -->

    <owl:Class rdf:about="http://dataforhistory.org/histdmi-generic-ongoing/class/C26">
        <rdfs:subClassOf rdf:resource="http://www.cidoc-crm.org/cidoc-crm/E89"/>
        <rdfs:comment rdf:datatype="http://www.w3.org/2001/XMLSchema#string">Social representations, as expression of collective intentionality, are sets of propositional objects and other related abstract objects that are present in human minds as a conceptualization shared by a social collective or social context, i.e. persons sharing the same point of view or conceptualization. These persons do not necessarily act together, and are therefore not a group in the sense of crm:E74 Group but they share the same social representations stemming from education, social context, professional and social engagement, media, etc.
In this perspective, social representations (knowledge, beliefs and practical know-how) are constitutive of human communities and social collectives.</rdfs:comment>
        <rdfs:label xml:lang="en">Social Representation</rdfs:label>
        <skos:notation rdf:datatype="http://www.w3.org/2001/XMLSchema#string">C26</skos:notation>
    </owl:Class>
    


    <!-- http://dataforhistory.org/histdmi-generic-ongoing/class/C27 -->

    <owl:Class rdf:about="http://dataforhistory.org/histdmi-generic-ongoing/class/C27">
        <rdfs:subClassOf rdf:resource="http://www.cidoc-crm.org/cidoc-crm/E2"/>
        <rdfs:comment rdf:datatype="http://www.w3.org/2001/XMLSchema#string">This class models the fact that a community or collective of humans shares or shared instances of hist:C26 Social Representation. The fact of sharing social representations is what constitutes in the most general sense a human intentional collective or social context, besides relations of social power based on acceptance of collective rules. The social collective therefore exists insofar as it shares one or more social representations, be they understood in the sense of beliefs, abstract knowledge or applicable know-how. These are present in a human context at a given moment in time, or time-span, and constitute a social community in the broadest sense.</rdfs:comment>
        <rdfs:label xml:lang="en">Collective State of Mind</rdfs:label>
        <skos:notation rdf:datatype="http://www.w3.org/2001/XMLSchema#string">C27</skos:notation>
    </owl:Class>
    


    <!-- http://dataforhistory.org/histdmi-generic-ongoing/class/C28 -->

    <owl:Class rdf:about="http://dataforhistory.org/histdmi-generic-ongoing/class/C28">
        <rdfs:subClassOf rdf:resource="http://dataforhistory.org/histdmi-generic-ongoing/class/C1"/>
        <rdfs:comment rdf:datatype="http://www.w3.org/2001/XMLSchema#string">This class models the quantifiable information about a quality of an entity.</rdfs:comment>
        <rdfs:label xml:lang="en">Quantifiable Quality</rdfs:label>
        <skos:notation rdf:datatype="http://www.w3.org/2001/XMLSchema#string">C28</skos:notation>
    </owl:Class>
    


    <!-- http://dataforhistory.org/histdmi-generic-ongoing/class/C29 -->

    <owl:Class rdf:about="http://dataforhistory.org/histdmi-generic-ongoing/class/C29">
        <rdfs:subClassOf rdf:resource="http://www.cidoc-crm.org/cidoc-crm/E89"/>
        <rdfs:comment rdf:datatype="http://www.w3.org/2001/XMLSchema#string">This class comprises know-how as practical knowledge, i.e. ​knowledge of how to do something. Experience in doing it is modelled with the hist:C21 Skill as a quality of a person being trained through practice to realize the know-how.</rdfs:comment>
        <rdfs:label xml:lang="en">Know-How</rdfs:label>
        <skos:notation rdf:datatype="http://www.w3.org/2001/XMLSchema#string">C29</skos:notation>
    </owl:Class>
    


    <!-- http://dataforhistory.org/histdmi-generic-ongoing/class/C3 -->

    <owl:Class rdf:about="http://dataforhistory.org/histdmi-generic-ongoing/class/C3">
        <rdfs:subClassOf rdf:resource="http://www.cidoc-crm.org/cidoc-crm/E2"/>
        <rdfs:comment rdf:datatype="http://www.w3.org/2001/XMLSchema#string">This class models time-indexed situations that are known by intentional agents but are not phenomenal in the sense of events (E5 Event), nor occur as expressions of collective intentionality (C3 Social Situation). These are often given under the form of negation, like the known absence of a person at an event or the non-existence of relationships between persons or groups. The correspondent information is available, and attested by sources, but cannot be modelled as a spatial or social phenomenon.</rdfs:comment>
        <rdfs:label xml:lang="en">Epistemic Situation</rdfs:label>
        <skos:notation rdf:datatype="http://www.w3.org/2001/XMLSchema#string">C3</skos:notation>
    </owl:Class>
    


    <!-- http://dataforhistory.org/histdmi-generic-ongoing/class/C30 -->

    <owl:Class rdf:about="http://dataforhistory.org/histdmi-generic-ongoing/class/C30">
        <rdfs:subClassOf rdf:resource="http://dataforhistory.org/histdmi-generic-ongoing/class/C27"/>
        <rdfs:comment rdf:datatype="http://www.w3.org/2001/XMLSchema#string">The Social Connotation class models the integration of an entity into the social representations of a human collective during a given time-span. It provides the entity with a context specific connotation, social quality or characterization: a social collective considers that the adopted connotation, expressed by the propositional content of the collective state of mind, applies to the given entity. The integrated entity can be an actor, a physical or conceptual object, a text, an event, etc. E.g. a celebrated battle is integrated as the founding event of a country&apos;s independence into the representations of its indigenous inhabitants, or a portion of them.
The collective view, perspective or interpretation of the entity, i.e. its social connotation conceived as a shared propositional object concerning it, becomes part of the social representations it is integrated into. As a subclass of hist:C27 Collective state of mind the social connotation is at the same time a quality of the concerned entity and of the social collective sharing the related social representation. Thus it establishes a sort of (intentional) relation between the entity and the collective.
The propositional object providing the connotation or quality of the entity represents the content of the collective state of mind. It is therefore associated to the social quality with the inherited hist:P34 has content property. Furthermore, the hist:P40 has context (is context of) property situates the concerned social quality within the wider context of the social representations it belongs to.</rdfs:comment>
        <rdfs:label xml:lang="en">Social Connotation</rdfs:label>
        <skos:notation rdf:datatype="http://www.w3.org/2001/XMLSchema#string">C30</skos:notation>
    </owl:Class>
    


    <!-- http://dataforhistory.org/histdmi-generic-ongoing/class/C31 -->

    <owl:Class rdf:about="http://dataforhistory.org/histdmi-generic-ongoing/class/C31">
        <rdfs:subClassOf rdf:resource="http://dataforhistory.org/histdmi-generic-ongoing/class/C6"/>
        <rdfs:comment rdf:datatype="http://www.w3.org/2001/XMLSchema#string">This class comprises concepts belonging to social representations used to characterize and classify instances of the hist:C2 Social Event class. These concepts are defined by the communities sharing the said social representations and belong to them.</rdfs:comment>
        <rdfs:label xml:lang="en">Social Event Type</rdfs:label>
        <skos:notation rdf:datatype="http://www.w3.org/2001/XMLSchema#string">C31</skos:notation>
    </owl:Class>
    


    <!-- http://dataforhistory.org/histdmi-generic-ongoing/class/C32 -->

    <owl:Class rdf:about="http://dataforhistory.org/histdmi-generic-ongoing/class/C32">
        <rdfs:subClassOf rdf:resource="http://www.cidoc-crm.org/cidoc-crm/E28"/>
        <rdfs:comment rdf:datatype="http://www.w3.org/2001/XMLSchema#string">This class models individual concepts that are not used to classify or characterize other entities, like instances of crm:E55 Type, but are defined by propositional objects (descriptions in the sense of the DnS ontology) and exist in individual or collective states of mind, or in texts and other information objects. These individuals do not exist in physical reality but just in the intentionality of a person or of a social collective. For example a character in a novel, such as Jean Valjean in Les Misérables by Vicor Hugo, is an abstract individual.
Abstract individuals are created as any other conceptual object by actors in events of type E65 Creation. They are integrated into social representations through C30 Social Connotation, i.e. adoption and integration of these individuals by a collective of humans into their own vision of reality or their fictional world.</rdfs:comment>
        <rdfs:label xml:lang="en">Abstract individual</rdfs:label>
        <skos:notation rdf:datatype="http://www.w3.org/2001/XMLSchema#string">C32</skos:notation>
    </owl:Class>
    


    <!-- http://dataforhistory.org/histdmi-generic-ongoing/class/C33 -->

    <owl:Class rdf:about="http://dataforhistory.org/histdmi-generic-ongoing/class/C33">
        <rdfs:subClassOf rdf:resource="http://www.cidoc-crm.org/cidoc-crm/E5"/>
        <rdfs:comment rdf:datatype="http://www.w3.org/2001/XMLSchema#string">A unitary event takes place in a unit of time, place and action. This definition, that should allow a clear identification of instances of this class, is inspired by the three unities of Greek tragedy: a unitary event should have one principal action (unity of action), it should occur over a limited period of time (no more than 24 hours according to the unity of time in tragedy, but could be longer in real life), and should happen in a single physical location (unity of place). The unitary event is thus defined in contrast to the sdh:C4 Phase class which includes more complex temporalities, being composed of several events, activities or sub-phases, taking place over a longer period, being projected on a space which can be quite vast.</rdfs:comment>
        <rdfs:label xml:lang="en">Unitary Event</rdfs:label>
        <skos:notation rdf:datatype="http://www.w3.org/2001/XMLSchema#string">C33</skos:notation>
    </owl:Class>
    


    <!-- http://dataforhistory.org/histdmi-generic-ongoing/class/C34 -->

    <owl:Class rdf:about="http://dataforhistory.org/histdmi-generic-ongoing/class/C34">
        <rdfs:subClassOf rdf:resource="http://www.cidoc-crm.org/cidoc-crm/E55"/>
        <rdfs:comment rdf:datatype="http://www.w3.org/2001/XMLSchema#string">This class comprises concepts denoted by terms from thesauri and controlled vocabularies used to characterize and classify instances of the sdh:C33 Unitary Event class.</rdfs:comment>
        <rdfs:label xml:lang="en">Unitary Event Type</rdfs:label>
        <skos:notation rdf:datatype="http://www.w3.org/2001/XMLSchema#string">C34</skos:notation>
    </owl:Class>
    


    <!-- http://dataforhistory.org/histdmi-generic-ongoing/class/C4 -->

    <owl:Class rdf:about="http://dataforhistory.org/histdmi-generic-ongoing/class/C4">
        <rdfs:subClassOf rdf:resource="http://www.cidoc-crm.org/cidoc-crm/E5"/>
        <rdfs:comment rdf:datatype="http://www.w3.org/2001/XMLSchema#string">This class models phenomena in time and space that involve one or more persitent items and are conceptualized as homeomeric units that unfold over a period of time: their temporal parts are described, in the intension of the class, by the very expression used for the whole event. E.g. a part of a relationship between two persons is also a relationship between these two persons, and a portion of a travel is also travelling. In the unfolding of time, there can be moments where the phenomena are not actual, but the intended substance of the phenomenon do not change, like a more or less active relationship between persons or the stopping and resting when you go for a long walk. This class is inspired by the DOLCE definition of stative perdurants but adapted to the context of the CIDOC CRM and therefore modelled as a coherent set of spatio-temporal events. This means that a phase can consist of different unitary events, activities or sub-phases (crm:P9 consists of), all of them being intended as components of the phase.
This class is disjoint with the Activity – E7 class, which focus on specific intentional activities, the  Beginning of Existence – E63 or End of Existence – E64 classes which express achievements and models substantially unitary phenomena, and sdh:C33 Unitary Event, that model unity of action, time and place. E63 and E64 instances can start or end phases, but also activities and unitary events.</rdfs:comment>
        <rdfs:label xml:lang="en">Phase</rdfs:label>
        <skos:notation rdf:datatype="http://www.w3.org/2001/XMLSchema#string">C4</skos:notation>
    </owl:Class>
    


    <!-- http://dataforhistory.org/histdmi-generic-ongoing/class/C5 -->

    <owl:Class rdf:about="http://dataforhistory.org/histdmi-generic-ongoing/class/C5">
        <rdfs:comment rdf:datatype="http://www.w3.org/2001/XMLSchema#string">Time span, place, dimension, etc. are all regions in a reference time, space, value range, etc.</rdfs:comment>
        <rdfs:label xml:lang="en">Region</rdfs:label>
        <skos:notation rdf:datatype="http://www.w3.org/2001/XMLSchema#string">C5</skos:notation>
    </owl:Class>
    


    <!-- http://dataforhistory.org/histdmi-generic-ongoing/class/C6 -->

    <owl:Class rdf:about="http://dataforhistory.org/histdmi-generic-ongoing/class/C6">
        <rdfs:subClassOf rdf:resource="http://www.cidoc-crm.org/cidoc-crm/E55"/>
        <rdfs:comment rdf:datatype="http://www.w3.org/2001/XMLSchema#string">This class comprises concepts used to characterize and classify entitites that are defined in and relative to specific social representations. These concepts are conceptualized in specific human groups and considered as valid in their classification and characterization of entities in the physical, intellectual, social and spatio-temporal world.</rdfs:comment>
        <rdfs:label xml:lang="en">Social Type</rdfs:label>
        <skos:notation rdf:datatype="http://www.w3.org/2001/XMLSchema#string">C6</skos:notation>
    </owl:Class>
    


    <!-- http://dataforhistory.org/histdmi-generic-ongoing/class/C7 -->

    <owl:Class rdf:about="http://dataforhistory.org/histdmi-generic-ongoing/class/C7">
        <rdfs:subClassOf rdf:resource="http://dataforhistory.org/histdmi-generic-ongoing/class/C1"/>
        <rdfs:comment rdf:datatype="http://www.w3.org/2001/XMLSchema#string">This class models an opinion, belief, certainty of a person concerning one or more entities. It is modelled as a time-indexed quality inherent to a person, having a propositional object as value.</rdfs:comment>
        <rdfs:label xml:lang="en">Individual State of Mind</rdfs:label>
        <skos:notation rdf:datatype="http://www.w3.org/2001/XMLSchema#string">C7</skos:notation>
    </owl:Class>
    


    <!-- http://dataforhistory.org/histsocial-ongoing/class/C1 -->

    <owl:Class rdf:about="http://dataforhistory.org/histsocial-ongoing/class/C1">
        <rdfs:subClassOf rdf:resource="http://dataforhistory.org/histdmi-generic-ongoing/class/C30"/>
        <rdfs:comment rdf:datatype="http://www.w3.org/2001/XMLSchema#string">Social, professional or political quality of an actor (be it a person or a group), in the sense of a social type and not a specific, legally defined function, limited in time, as it is socially perceived (relatively to a group, the society or a portion of it). The C27 Legal Connotation class, as a subclass of the present class, models clearly defined legal roles and functions and should be reserved for these cases.
 
C13 Social role
 </rdfs:comment>
        <rdfs:label xml:lang="en">Social Quality of an Actor (Temporal entity)</rdfs:label>
        <skos:notation rdf:datatype="http://www.w3.org/2001/XMLSchema#string">C1</skos:notation>
    </owl:Class>
    


    <!-- http://dataforhistory.org/histsocial-ongoing/class/C10 -->

    <owl:Class rdf:about="http://dataforhistory.org/histsocial-ongoing/class/C10">
        <rdfs:subClassOf rdf:resource="http://www.cidoc-crm.org/cidoc-crm/E55"/>
        <rdfs:comment rdf:datatype="http://www.w3.org/2001/XMLSchema#string">This class comprises concepts denoted by terms from thesauri and controlled vocabularies used to characterize and classify instances of the class Union – histC31.</rdfs:comment>
        <rdfs:label xml:lang="en">Type of union</rdfs:label>
        <skos:notation rdf:datatype="http://www.w3.org/2001/XMLSchema#string">C10</skos:notation>
    </owl:Class>
    


    <!-- http://dataforhistory.org/histsocial-ongoing/class/C11 -->

    <owl:Class rdf:about="http://dataforhistory.org/histsocial-ongoing/class/C11">
        <rdfs:subClassOf rdf:resource="http://dataforhistory.org/histsocial-ongoing/class/C2"/>
        <rdfs:comment rdf:datatype="http://www.w3.org/2001/XMLSchema#string">&quot;Gender is the state of being male or female in relation to the social and cultural roles that are considered appropriate for men and women&quot; (Collins).</rdfs:comment>
        <rdfs:label xml:lang="en">Gender</rdfs:label>
        <skos:notation rdf:datatype="http://www.w3.org/2001/XMLSchema#string">C11</skos:notation>
    </owl:Class>
    


    <!-- http://dataforhistory.org/histsocial-ongoing/class/C12 -->

    <owl:Class rdf:about="http://dataforhistory.org/histsocial-ongoing/class/C12">
        <rdfs:subClassOf rdf:resource="http://dataforhistory.org/histdmi-generic-ongoing/class/C32"/>
        <rdfs:comment rdf:datatype="http://www.w3.org/2001/XMLSchema#string">A social actor is an abstract individual to whom social power is conferred, i.e. some rights and duties defining it, like the King, the Republic, the Academy, a Senator as member of the Senate of a State. As individuals existing only in social representations, social actors can only act through their representatives, i.e. the groups or individuals who embody them.
A social actor is an individual and therefore distinct from a concept classifying social roles of people. Il is a collection of specific, more or less precisely defined rights and duties, that is identified by a human society as acting individually. In this specific, individual sense (not classifying other objects) it can be understood as a social role.</rdfs:comment>
        <rdfs:label xml:lang="en">Social actor</rdfs:label>
        <skos:notation rdf:datatype="http://www.w3.org/2001/XMLSchema#string">C12</skos:notation>
    </owl:Class>
    


    <!-- http://dataforhistory.org/histsocial-ongoing/class/C13 -->

    <owl:Class rdf:about="http://dataforhistory.org/histsocial-ongoing/class/C13">
        <rdfs:subClassOf rdf:resource="http://dataforhistory.org/histsocial-ongoing/class/C27"/>
        <rdfs:comment rdf:datatype="http://www.w3.org/2001/XMLSchema#string">The fact of having a more or less formally defined social role or function in a group at a given moment or during a given time-span. The social role is modelled as an embodiment by a (Human) Actor of a Social Actor. It provides the (Human) Actor with prerogatives and rights that are exercised with respect to other persons and groups. It is therefore modelled as a social connotation, i.e. a social qualification of an Actor.</rdfs:comment>
        <rdfs:label xml:lang="en">Social actor embodiment</rdfs:label>
        <skos:notation rdf:datatype="http://www.w3.org/2001/XMLSchema#string">C13</skos:notation>
    </owl:Class>
    


    <!-- http://dataforhistory.org/histsocial-ongoing/class/C14 -->

    <owl:Class rdf:about="http://dataforhistory.org/histsocial-ongoing/class/C14">
        <rdfs:subClassOf rdf:resource="http://dataforhistory.org/histdmi-generic-ongoing/class/C30"/>
        <rdfs:comment rdf:datatype="http://www.w3.org/2001/XMLSchema#string">This class models the fact that during a given time-span a persistent item is considered as subjected to a right (in the widest sense) in the context of the social representations (hist:C26) of a specific social collective (hist:C25).</rdfs:comment>
        <rdfs:label xml:lang="en">Subjection to a Right</rdfs:label>
        <skos:notation rdf:datatype="http://www.w3.org/2001/XMLSchema#string">C14</skos:notation>
    </owl:Class>
    


    <!-- http://dataforhistory.org/histsocial-ongoing/class/C15 -->

    <owl:Class rdf:about="http://dataforhistory.org/histsocial-ongoing/class/C15">
        <rdfs:subClassOf rdf:resource="http://dataforhistory.org/histdmi-generic-ongoing/class/C4"/>
        <rdfs:comment rdf:datatype="http://www.w3.org/2001/XMLSchema#string">This class comprises periods of continuous activity of a person participating in an event, be this a battle, voyage, conference, etc. If the participation involves the exercise of a function or holding of an office or rank this can be associated using the is participation with social character – histP28 Proprety. One or more functions can be associated to the same Participation if their time span is identical. It is otherwise preferable to split consecutive holdins of an office in the same event producing several instances of this class. The time-span of this class is equal to or included in the time-span of the related event.</rdfs:comment>
        <rdfs:label xml:lang="en">Participation</rdfs:label>
        <skos:notation rdf:datatype="http://www.w3.org/2001/XMLSchema#string">C15</skos:notation>
    </owl:Class>
    


    <!-- http://dataforhistory.org/histsocial-ongoing/class/C16 -->

    <owl:Class rdf:about="http://dataforhistory.org/histsocial-ongoing/class/C16">
        <rdfs:subClassOf rdf:resource="http://dataforhistory.org/histdmi-generic-ongoing/class/C30"/>
        <rdfs:comment rdf:datatype="http://www.w3.org/2001/XMLSchema#string">This class models the existence of a legal individual in the social space, i. e. as the expression of collective intentionality considering it as being virtually in force. The existence of the legal individual generally begins with a constitutive social event and ends either with a social event that terminates its existence or with the disappearance of all the people (internal or external to the social collective) who actively considered it as existing.
Knowing that a legal individual existed does not make it legally existingnow: the phenomenon modelled is the virtually being in force, according to active social representations, not the later knowledge of its existence in earlier times.</rdfs:comment>
        <rdfs:label xml:lang="en">Legal Individual Existence</rdfs:label>
        <skos:notation rdf:datatype="http://www.w3.org/2001/XMLSchema#string">C16</skos:notation>
    </owl:Class>
    


    <!-- http://dataforhistory.org/histsocial-ongoing/class/C17 -->

    <owl:Class rdf:about="http://dataforhistory.org/histsocial-ongoing/class/C17">
        <rdfs:subClassOf rdf:resource="http://www.cidoc-crm.org/cidoc-crm/E89"/>
        <rdfs:comment rdf:datatype="http://www.w3.org/2001/XMLSchema#string">Instances of this class are propositional objects that state prerogatives, obligations, rights, powers, etc. of subjects of law (human or legal actors) regarding persistent items.</rdfs:comment>
        <rdfs:label xml:lang="en">Right or obligation</rdfs:label>
        <skos:notation rdf:datatype="http://www.w3.org/2001/XMLSchema#string">C17</skos:notation>
    </owl:Class>
    


    <!-- http://dataforhistory.org/histsocial-ongoing/class/C18 -->

    <owl:Class rdf:about="http://dataforhistory.org/histsocial-ongoing/class/C18">
        <rdfs:subClassOf rdf:resource="http://dataforhistory.org/histdmi-generic-ongoing/class/C4"/>
        <rdfs:comment rdf:datatype="http://www.w3.org/2001/XMLSchema#string">This class models the interaction of persons in time and physical (generally geographical) space. It is disjoint with the C3 Social Relationship class which models the interaction in time and the social space, i.e. the space of a collective state of mind and shared social representations.
The interaction is not restricted to a quantity of persons (a meeting can be modelled with this class) but there must be a unity in time and space for all the participants if the involved persons are more than two. If a person joins the interaction at a later moment than the beginning, the C15 Participation class can be used.
As a subclass of C4 Phase the social interaction can be a collection of different sorts of specific interactions, in space and time, unified by a general view. In this case, the space of the interaction, generally the geographical place, is the maximal projection in space of the whole interaction.</rdfs:comment>
        <rdfs:label xml:lang="en">Persons&apos; Interaction</rdfs:label>
        <skos:notation rdf:datatype="http://www.w3.org/2001/XMLSchema#string">C18</skos:notation>
    </owl:Class>
    


    <!-- http://dataforhistory.org/histsocial-ongoing/class/C19 -->

    <owl:Class rdf:about="http://dataforhistory.org/histsocial-ongoing/class/C19">
        <rdfs:subClassOf rdf:resource="http://dataforhistory.org/histdmi-generic-ongoing/class/C30"/>
        <rdfs:comment rdf:datatype="http://www.w3.org/2001/XMLSchema#string">This class models characteristics associated in collective intentionality to social qualities during a given period of time.</rdfs:comment>
        <rdfs:label xml:lang="en">Legal Individual Characterization (Temporal Entity)</rdfs:label>
        <skos:notation rdf:datatype="http://www.w3.org/2001/XMLSchema#string">C19</skos:notation>
    </owl:Class>
    


    <!-- http://dataforhistory.org/histsocial-ongoing/class/C2 -->

    <owl:Class rdf:about="http://dataforhistory.org/histsocial-ongoing/class/C2">
        <rdfs:subClassOf rdf:resource="http://dataforhistory.org/histdmi-generic-ongoing/class/C6"/>
        <rdfs:comment rdf:datatype="http://www.w3.org/2001/XMLSchema#string">Professional, political, religious or whatever social quality of an actor, be it a person or a group, as it is perceived from the point of view of the representations of a human community. The Social Quality is a socially constructed concept (in the sense of crm:E55 Type) and it is used to socially classify individuals in the perspective of the community. 
This class is not to be confused with the C12 Social role class which models clearly (and often legally) defined social roles and functions of actors and should be exclusively used for these use cases. Social roles are formalisations of social qualities in relation to social actors.</rdfs:comment>
        <rdfs:label xml:lang="en">Social quality</rdfs:label>
        <skos:notation rdf:datatype="http://www.w3.org/2001/XMLSchema#string">C2</skos:notation>
    </owl:Class>
    


    <!-- http://dataforhistory.org/histsocial-ongoing/class/C20 -->

    <owl:Class rdf:about="http://dataforhistory.org/histsocial-ongoing/class/C20">
        <rdfs:subClassOf rdf:resource="http://dataforhistory.org/histdmi-generic-ongoing/class/C30"/>
        <rdfs:comment rdf:datatype="http://www.w3.org/2001/XMLSchema#string">This class models the validity of a right or obligation, i.e. the being in force of a right according to collective intentionalty in the context of specific social representations.</rdfs:comment>
        <rdfs:label xml:lang="en">Right Validity</rdfs:label>
        <skos:notation rdf:datatype="http://www.w3.org/2001/XMLSchema#string">C20</skos:notation>
    </owl:Class>
    


    <!-- http://dataforhistory.org/histsocial-ongoing/class/C21 -->

    <owl:Class rdf:about="http://dataforhistory.org/histsocial-ongoing/class/C21">
        <rdfs:subClassOf rdf:resource="http://www.cidoc-crm.org/cidoc-crm/E55"/>
        <rdfs:comment rdf:datatype="http://www.w3.org/2001/XMLSchema#string">
This class comprises concepts denoted by terms from thesauri and controlled vocabularies used to classify and provide a more specific identity to instances of the Right or obligation class.
</rdfs:comment>
        <rdfs:label xml:lang="en">Right or obligation type</rdfs:label>
        <skos:notation rdf:datatype="http://www.w3.org/2001/XMLSchema#string">C21</skos:notation>
    </owl:Class>
    


    <!-- http://dataforhistory.org/histsocial-ongoing/class/C22 -->

    <owl:Class rdf:about="http://dataforhistory.org/histsocial-ongoing/class/C22">
        <rdfs:subClassOf rdf:resource="http://www.cidoc-crm.org/cidoc-crm/E55"/>
        <rdfs:comment rdf:datatype="http://www.w3.org/2001/XMLSchema#string">This class comprises concepts used to provide a specific identity to instances of the Legal Quality (Temporal entity) class. It should not be confused with the legal quality instance (Abstract Individual) expressed by the C26 Legal quality class, e.g. the legal quality instance is &apos;French nationality&apos; and the legal quality type is &apos;Nationality&apos;.</rdfs:comment>
        <rdfs:label xml:lang="en">Legal Connotation Type</rdfs:label>
        <skos:notation rdf:datatype="http://www.w3.org/2001/XMLSchema#string">C22</skos:notation>
    </owl:Class>
    


    <!-- http://dataforhistory.org/histsocial-ongoing/class/C23 -->

    <owl:Class rdf:about="http://dataforhistory.org/histsocial-ongoing/class/C23">
        <rdfs:subClassOf rdf:resource="http://dataforhistory.org/histsocial-ongoing/class/C1"/>
        <rdfs:comment rdf:datatype="http://www.w3.org/2001/XMLSchema#string">Religious identity of a person in the sense of perception by surrounding society, participation in religious events (e.g. going to church) and contribution to define one&apos; self-concept in the sense of public preference for a specific religion or religious denomination. The official membership in a religious group or Church is not modeled with this class, only the religious social quality of a person.</rdfs:comment>
        <rdfs:label xml:lang="en">Religious identity</rdfs:label>
        <skos:notation rdf:datatype="http://www.w3.org/2001/XMLSchema#string">C23</skos:notation>
    </owl:Class>
    


    <!-- http://dataforhistory.org/histsocial-ongoing/class/C24 -->

    <owl:Class rdf:about="http://dataforhistory.org/histsocial-ongoing/class/C24">
        <rdfs:subClassOf rdf:resource="http://dataforhistory.org/histsocial-ongoing/class/C2"/>
        <rdfs:comment rdf:datatype="http://www.w3.org/2001/XMLSchema#string">This class models religion, in the sense of social sciences, as a type classifying social-cultural systemd of designated behaviors and practices, morals, worldviews, texts, sanctified places, prophecies, ethics, or organizations, that relates humanity to supernatural, transcendental, or spiritual elements (religion) or  is a subgroup within a religion that operates under a common name, tradition, and identity (religious denomination).</rdfs:comment>
        <rdfs:label xml:lang="en">Religion or religious denomination</rdfs:label>
        <skos:notation rdf:datatype="http://www.w3.org/2001/XMLSchema#string">C24</skos:notation>
    </owl:Class>
    


    <!-- http://dataforhistory.org/histsocial-ongoing/class/C25 -->

    <owl:Class rdf:about="http://dataforhistory.org/histsocial-ongoing/class/C25">
        <rdfs:subClassOf rdf:resource="http://dataforhistory.org/histdmi-generic-ongoing/class/C32"/>
        <rdfs:comment rdf:datatype="http://www.w3.org/2001/XMLSchema#string">This class models entities that exist as individuals in legal systems, be they based on oral tradition or written laws.</rdfs:comment>
        <rdfs:label xml:lang="en">Legal individual</rdfs:label>
        <skos:notation rdf:datatype="http://www.w3.org/2001/XMLSchema#string">C25</skos:notation>
    </owl:Class>
    


    <!-- http://dataforhistory.org/histsocial-ongoing/class/C26 -->

    <owl:Class rdf:about="http://dataforhistory.org/histsocial-ongoing/class/C26">
        <rdfs:subClassOf rdf:resource="http://dataforhistory.org/histsocial-ongoing/class/C25"/>
        <rdfs:comment rdf:datatype="http://www.w3.org/2001/XMLSchema#string">A quality of an actor as defined in customary or by written law.</rdfs:comment>
        <rdfs:label xml:lang="en">Actor&apos;s Legal Quality</rdfs:label>
        <skos:notation rdf:datatype="http://www.w3.org/2001/XMLSchema#string">C26</skos:notation>
    </owl:Class>
    


    <!-- http://dataforhistory.org/histsocial-ongoing/class/C27 -->

    <owl:Class rdf:about="http://dataforhistory.org/histsocial-ongoing/class/C27">
        <rdfs:subClassOf rdf:resource="http://dataforhistory.org/histsocial-ongoing/class/C1"/>
        <rdfs:comment rdf:datatype="http://www.w3.org/2001/XMLSchema#string">This class models the fact that an actor (individual or collective) is perceived in society as having a legal quality</rdfs:comment>
        <rdfs:label xml:lang="en">Legal Connotation</rdfs:label>
        <skos:notation rdf:datatype="http://www.w3.org/2001/XMLSchema#string">C27</skos:notation>
    </owl:Class>
    


    <!-- http://dataforhistory.org/histsocial-ongoing/class/C28 -->

    <owl:Class rdf:about="http://dataforhistory.org/histsocial-ongoing/class/C28">
        <rdfs:subClassOf rdf:resource="http://dataforhistory.org/histdmi-generic-ongoing/class/C13"/>
        <rdfs:subClassOf rdf:resource="http://dataforhistory.org/histsocial-ongoing/class/C25"/>
        <rdfs:comment rdf:datatype="http://www.w3.org/2001/XMLSchema#string">The geographical domain under the jurisdiction of a political unit, an organization, etc.</rdfs:comment>
        <rdfs:label xml:lang="en">Territory</rdfs:label>
        <skos:notation rdf:datatype="http://www.w3.org/2001/XMLSchema#string">C28</skos:notation>
    </owl:Class>
    


    <!-- http://dataforhistory.org/histsocial-ongoing/class/C3 -->

    <owl:Class rdf:about="http://dataforhistory.org/histsocial-ongoing/class/C3">
        <rdfs:subClassOf rdf:resource="http://dataforhistory.org/histdmi-generic-ongoing/class/C2"/>
        <rdfs:comment rdf:datatype="http://www.w3.org/2001/XMLSchema#string">This class models the phenomenon of a more or less active social relation between people, groups or countries as it is perceived in the context of specific social representations. In other words, this class does not model a physical interaction of actors in space and time (for persons this interaction is modelled with the C18 Persons&apos; Interaction class) but the perception of a phenomenon like frienship, marriage, apprenticeship, etc. that happens in minds and the social space.
Each relationship generally involves only two instances of one or more classes. If more then two instances are involved (e.g. multilateral political relationships) the unity of time and social space (i.e. the social context) must be given.
If the relationship is symmetrical, the histP32 involves partner property has to be used in order to associate the partners of the relationship. If the relationship is oriented from a source to a target (the partners having a different position in the relationship), the properties histP49 has relationship source and histP50 has relationship target will be used. This generic treatment allows to express a direction of the relationship. The meaning of the direction will be explicitly defined in the controlled vocabulary of relationship types.
Given their different meanings, it is absolutely necessary to avoid mixing the two types of relationships: either use the hist:P32 property or the hist:P49 / hist:P50 – they are disjoint.</rdfs:comment>
        <rdfs:label xml:lang="en">Social Relationship</rdfs:label>
        <skos:notation rdf:datatype="http://www.w3.org/2001/XMLSchema#string">C3</skos:notation>
    </owl:Class>
    


    <!-- http://dataforhistory.org/histsocial-ongoing/class/C4 -->

    <owl:Class rdf:about="http://dataforhistory.org/histsocial-ongoing/class/C4">
        <rdfs:subClassOf rdf:resource="http://www.cidoc-crm.org/cidoc-crm/E55"/>
        <rdfs:comment rdf:datatype="http://www.w3.org/2001/XMLSchema#string">This class comprises concepts denoted by terms from thesauri and controlled vocabularies used to characterize and classify instances of the histC6 Relationship class.
If the relationship is oriented from a source to a target (the partners having a different position in the relationship), the properties histP49 has relationship source and histP50 has relationship target will be used. This generic treatment allows to express a direction of the relationship. The meaning of the direction will be explicitly defined in the definition of the terms in the controlled vocabulary of social relationship types.</rdfs:comment>
        <rdfs:label xml:lang="en">Social Relationship Type</rdfs:label>
        <skos:notation rdf:datatype="http://www.w3.org/2001/XMLSchema#string">C4</skos:notation>
    </owl:Class>
    


    <!-- http://dataforhistory.org/histsocial-ongoing/class/C5 -->

    <owl:Class rdf:about="http://dataforhistory.org/histsocial-ongoing/class/C5">
        <rdfs:subClassOf rdf:resource="http://dataforhistory.org/histsocial-ongoing/class/C1"/>
        <rdfs:comment rdf:datatype="http://www.w3.org/2001/XMLSchema#string">This class models the fact that a person or an organization belongs to a group during a given time span</rdfs:comment>
        <rdfs:label xml:lang="en">Membership</rdfs:label>
        <skos:notation rdf:datatype="http://www.w3.org/2001/XMLSchema#string">C5</skos:notation>
    </owl:Class>
    


    <!-- http://dataforhistory.org/histsocial-ongoing/class/C6 -->

    <owl:Class rdf:about="http://dataforhistory.org/histsocial-ongoing/class/C6">
        <rdfs:subClassOf rdf:resource="http://www.cidoc-crm.org/cidoc-crm/E55"/>
        <rdfs:comment rdf:datatype="http://www.w3.org/2001/XMLSchema#string">This class comprises concepts denoted by terms from thesauri and controlled vocabularies used to characterize and classify instances of C5 Membership.</rdfs:comment>
        <rdfs:label xml:lang="en">Membership type</rdfs:label>
        <skos:notation rdf:datatype="http://www.w3.org/2001/XMLSchema#string">C6</skos:notation>
    </owl:Class>
    


    <!-- http://dataforhistory.org/histsocial-ongoing/class/C7 -->

    <owl:Class rdf:about="http://dataforhistory.org/histsocial-ongoing/class/C7">
        <rdfs:subClassOf rdf:resource="http://dataforhistory.org/histsocial-ongoing/class/C2"/>
        <rdfs:comment rdf:datatype="http://www.w3.org/2001/XMLSchema#string">A job, profession or other activity</rdfs:comment>
        <rdfs:label xml:lang="en">Occupation</rdfs:label>
        <skos:notation rdf:datatype="http://www.w3.org/2001/XMLSchema#string">C7</skos:notation>
    </owl:Class>
    


    <!-- http://dataforhistory.org/histsocial-ongoing/class/C8 -->

    <owl:Class rdf:about="http://dataforhistory.org/histsocial-ongoing/class/C8">
        <rdfs:subClassOf rdf:resource="http://dataforhistory.org/histdmi-generic-ongoing/class/C4"/>
        <rdfs:comment rdf:datatype="http://www.w3.org/2001/XMLSchema#string">Professional or other activity carried out by a person, more or less intensively, over a more or less long period of time. This class does not model a specific activity but a phase during which many specific instances of the same activity are carried out. Each part of having this occupation, e.g. being a merchant or a professor, is having an occupation, therefore this phenomenon is modelled as a phase. During this phase there may be times when the activity is not carried out.</rdfs:comment>
        <rdfs:label xml:lang="en">Occupation (Temporal entity)</rdfs:label>
        <skos:notation rdf:datatype="http://www.w3.org/2001/XMLSchema#string">C8</skos:notation>
    </owl:Class>
    


    <!-- http://dataforhistory.org/histsocial-ongoing/class/C9 -->

    <owl:Class rdf:about="http://dataforhistory.org/histsocial-ongoing/class/C9">
        <rdfs:subClassOf rdf:resource="http://dataforhistory.org/histsocial-ongoing/class/C18"/>
        <rdfs:comment rdf:datatype="http://www.w3.org/2001/XMLSchema#string">[under construction] This class models the fact of the union of two persons for a certain period of time, which may give rise to the birth of children.It is inspired by the GEDCOM modeling used by genealogists (http://fr.wikipedia.org/wiki/Norme_GEDCOM): the &quot;Union&quot; class indicates the existence over time of a couple, to which births, adoptions, etc. can be linked. The class &quot;Union&quot; models all kinds of relationships, regardless of their legal, emotional or social form, and indicates the time span of their duration (start/end date). Same-sex unions are also to be encoded with this class. A type is used to specify the nature of the union (marriage, common-law union, etc.).
[deprecated and to be replaced by characteristic] If a union has several phases, with successive time spans, we create several instances of the class &apos;Union&apos;, with their respective type and time-span, then we associate them to a global union, for the whole duration of the union by using the property is component of (has component) – histP29 .</rdfs:comment>
        <rdfs:label xml:lang="en">Union</rdfs:label>
        <skos:notation rdf:datatype="http://www.w3.org/2001/XMLSchema#string">C9</skos:notation>
    </owl:Class>
    


    <!-- http://dataforhistory.org/maritime-history-ongoing/class/C1 -->

    <owl:Class rdf:about="http://dataforhistory.org/maritime-history-ongoing/class/C1">
        <rdfs:subClassOf rdf:resource="http://dataforhistory.org/histdmi-generic-ongoing/class/C4"/>
        <rdfs:comment rdf:datatype="http://www.w3.org/2001/XMLSchema#string">Used to denote a (long) journey, especially by ship, going from a place of departure to a place of arrival.</rdfs:comment>
        <rdfs:label xml:lang="en">Ship Voyage</rdfs:label>
        <skos:notation rdf:datatype="http://www.w3.org/2001/XMLSchema#string">C1</skos:notation>
    </owl:Class>
    


    <!-- http://dataforhistory.org/maritime-history-ongoing/class/C11 -->

    <owl:Class rdf:about="http://dataforhistory.org/maritime-history-ongoing/class/C11">
        <rdfs:comment rdf:datatype="http://www.w3.org/2001/XMLSchema#string">Used to denote the code of the Historical International Standard Classification of Occupations (HISCO) category that contains the position or profession to which it is linked.</rdfs:comment>
        <rdfs:label xml:lang="en">HISCO category</rdfs:label>
        <skos:notation rdf:datatype="http://www.w3.org/2001/XMLSchema#string">C11</skos:notation>
    </owl:Class>
    


    <!-- http://dataforhistory.org/maritime-history-ongoing/class/C12 -->

    <owl:Class rdf:about="http://dataforhistory.org/maritime-history-ongoing/class/C12">
        <rdfs:subClassOf rdf:resource="http://www.cidoc-crm.org/cidoc-crm/E12"/>
        <rdfs:comment rdf:datatype="http://www.w3.org/2001/XMLSchema#string">This class comprises activities that result in instances of C2 Ship coming into existence.</rdfs:comment>
        <rdfs:label xml:lang="en">Shipbuilding</rdfs:label>
        <skos:notation rdf:datatype="http://www.w3.org/2001/XMLSchema#string">C12</skos:notation>
    </owl:Class>
    


    <!-- http://dataforhistory.org/maritime-history-ongoing/class/C13 -->

    <owl:Class rdf:about="http://dataforhistory.org/maritime-history-ongoing/class/C13">
        <rdfs:subClassOf rdf:resource="http://www.cidoc-crm.org/cidoc-crm/E7"/>
        <rdfs:comment rdf:datatype="http://www.w3.org/2001/XMLSchema#string">This class comprises periods of continuous activity of a person occupying a position during an entire event or part thereof. The time-span of this class is equal to or included to the time-span of the related event.</rdfs:comment>
        <rdfs:label xml:lang="en">[Not in use -reuse]  Participation</rdfs:label>
        <skos:notation rdf:datatype="http://www.w3.org/2001/XMLSchema#string">C13</skos:notation>
    </owl:Class>
    


    <!-- http://dataforhistory.org/maritime-history-ongoing/class/C2 -->

    <owl:Class rdf:about="http://dataforhistory.org/maritime-history-ongoing/class/C2">
        <rdfs:subClassOf rdf:resource="http://www.cidoc-crm.org/cidoc-crm/E22"/>
        <rdfs:comment rdf:datatype="http://www.w3.org/2001/XMLSchema#string">Used to denote a watercraft that travels the world&apos;s oceans and other sufficiently deep waterways, carrying passengers or goods, or in support of specialized missions, such as defense, research and fishing.</rdfs:comment>
        <rdfs:label xml:lang="en">Ship</rdfs:label>
        <skos:notation rdf:datatype="http://www.w3.org/2001/XMLSchema#string">C2</skos:notation>
    </owl:Class>
    


    <!-- http://dataforhistory.org/maritime-history-ongoing/class/C3 -->

    <owl:Class rdf:about="http://dataforhistory.org/maritime-history-ongoing/class/C3">
        <rdfs:subClassOf rdf:resource="http://www.cidoc-crm.org/cidoc-crm/E55"/>
        <rdfs:comment rdf:datatype="http://www.w3.org/2001/XMLSchema#string">Used to denote a specific type of ship.</rdfs:comment>
        <rdfs:label xml:lang="en">Ship Type</rdfs:label>
        <skos:notation rdf:datatype="http://www.w3.org/2001/XMLSchema#string">C3</skos:notation>
    </owl:Class>
    


    <!-- http://dataforhistory.org/maritime-history-ongoing/class/C4 -->

    <owl:Class rdf:about="http://dataforhistory.org/maritime-history-ongoing/class/C4">
        <rdfs:subClassOf rdf:resource="http://www.cidoc-crm.org/cidoc-crm/E40"/>
        <rdfs:comment rdf:datatype="http://www.w3.org/2001/XMLSchema#string">This class includes institutions specializing in shipbuilding.</rdfs:comment>
        <rdfs:label xml:lang="en">Shipyard</rdfs:label>
        <skos:notation rdf:datatype="http://www.w3.org/2001/XMLSchema#string">C4</skos:notation>
    </owl:Class>
    


    <!-- http://dataforhistory.org/maritime-history-ongoing/class/C5 -->

    <owl:Class rdf:about="http://dataforhistory.org/maritime-history-ongoing/class/C5">
        <rdfs:subClassOf rdf:resource="http://www.cidoc-crm.org/cidoc-crm/E19"/>
        <rdfs:comment rdf:datatype="http://www.w3.org/2001/XMLSchema#string">This class comprises instances of physical objects that can be the subject of a commercial activity.
[previous scope note : A commodity or service that satisfies a human need and is the subject of a commercial activity]</rdfs:comment>
        <rdfs:label xml:lang="en">Economic good</rdfs:label>
        <skos:notation rdf:datatype="http://www.w3.org/2001/XMLSchema#string">C5</skos:notation>
    </owl:Class>
    


    <!-- http://dataforhistory.org/maritime-history-ongoing/class/C6 -->

    <owl:Class rdf:about="http://dataforhistory.org/maritime-history-ongoing/class/C6">
        <rdfs:subClassOf rdf:resource="http://www.cidoc-crm.org/cidoc-crm/E7"/>
        <rdfs:comment rdf:datatype="http://www.w3.org/2001/XMLSchema#string"> Activity of carrying goods from one place to another using carriages, trains, ships, etc.</rdfs:comment>
        <rdfs:label xml:lang="en">Transport</rdfs:label>
        <skos:notation rdf:datatype="http://www.w3.org/2001/XMLSchema#string">C6</skos:notation>
    </owl:Class>
    


    <!-- http://dataforhistory.org/maritime-history-ongoing/class/C7 -->

    <owl:Class rdf:about="http://dataforhistory.org/maritime-history-ongoing/class/C7">
        <rdfs:subClassOf rdf:resource="http://www.cidoc-crm.org/cidoc-crm/E5"/>
        <rdfs:comment rdf:datatype="http://www.w3.org/2001/XMLSchema#string">Short stay in a place while on a journey to somewhere else.</rdfs:comment>
        <rdfs:label xml:lang="en">Stopover</rdfs:label>
        <skos:notation rdf:datatype="http://www.w3.org/2001/XMLSchema#string">C7</skos:notation>
    </owl:Class>
    


    <!-- http://dataforhistory.org/maritime-history-ongoing/class/C8 -->

    <owl:Class rdf:about="http://dataforhistory.org/maritime-history-ongoing/class/C8">
        <rdfs:subClassOf rdf:resource="http://www.cidoc-crm.org/cidoc-crm/E40"/>
        <rdfs:comment rdf:datatype="http://www.w3.org/2001/XMLSchema#string">Used to denote a branch of the Dutch East India Company (VOC). There were six semi-independent &apos;chambers&apos; that together formed the VOC: Amsterdam, Zeeland (Middelburg), Enkhuizen, Hoorn, Delft and Rotterdam.</rdfs:comment>
        <rdfs:label xml:lang="en">VOC Chamber</rdfs:label>
        <skos:notation rdf:datatype="http://www.w3.org/2001/XMLSchema#string">C8</skos:notation>
    </owl:Class>
    


    <!-- http://www.cidoc-crm.org/cidoc-crm/E1 -->

    <owl:Class rdf:about="http://www.cidoc-crm.org/cidoc-crm/E1">
        <rdfs:comment rdf:datatype="http://www.w3.org/2001/XMLSchema#string">This class comprises all things in the universe of discourse of the CIDOC Conceptual Reference Model. It is an abstract concept
            providing for three general properties: 1. Identification by name or appellation, and in particular by a preferred identifier 2.
            Classification by type, allowing further refinement of the specific subclass an instance belongs to 3. Attachment of free text for the
            expression of anything not captured by formal properties With the exception of E59 Primitive Value, all other classes within the CRM are
            directly or indirectly specialisations of E1 CRM Entity. </rdfs:comment>
        <rdfs:label xml:lang="en">CRM Entity</rdfs:label>
        <skos:notation rdf:datatype="http://www.w3.org/2001/XMLSchema#string">E1</skos:notation>
    </owl:Class>
    


    <!-- http://www.cidoc-crm.org/cidoc-crm/E10 -->

    <owl:Class rdf:about="http://www.cidoc-crm.org/cidoc-crm/E10">
        <rdfs:subClassOf rdf:resource="http://www.cidoc-crm.org/cidoc-crm/E7"/>
        <rdfs:comment rdf:datatype="http://www.w3.org/2001/XMLSchema#string">This class comprises transfers of physical custody of objects between instances of E39 Actor. The recording of the donor and/or
            recipient is optional. It is possible that in an instance of E10 Transfer of Custody there is either no donor or no recipient. Depending
            on the circumstances it may describe: 1. the beginning of custody 2. the end of custody 3. the transfer of custody 4. the receipt of
            custody from an unknown source 5. the declared loss of an object The distinction between the legal responsibility for custody and the
            actual physical possession of the object should be expressed using the property P2 has type (is type of). A specific case of transfer of
            custody is theft. The interpretation of the museum notion of &quot;accession&quot; differs between institutions. The CRM therefore models legal
            ownership and physical custody separately. Institutions will then model their specific notions of accession and deaccession as
            combinations of these. </rdfs:comment>
        <rdfs:label xml:lang="en">Transfer of Custody</rdfs:label>
        <skos:notation rdf:datatype="http://www.w3.org/2001/XMLSchema#string">E10</skos:notation>
    </owl:Class>
    


    <!-- http://www.cidoc-crm.org/cidoc-crm/E11 -->

    <owl:Class rdf:about="http://www.cidoc-crm.org/cidoc-crm/E11">
        <rdfs:subClassOf rdf:resource="http://www.cidoc-crm.org/cidoc-crm/E7"/>
        <rdfs:comment rdf:datatype="http://www.w3.org/2001/XMLSchema#string">This class comprises all instances of E7 Activity that create, alter or change E24 Physical Man-Made Thing. This class includes the
            production of an item from raw materials, and other so far undocumented objects, and the preventive treatment or restoration of an object
            for conservation. Since the distinction between modification and production is not always clear, modification is regarded as the more
            generally applicable concept. This implies that some items may be consumed or destroyed in a Modification, and that others may be produced
            as a result of it. An event should also be documented using E81 Transformation if it results in the destruction of one or more objects and
            the simultaneous production of others using parts or material from the originals. In this case, the new items have separate identities. If
            the instance of the E29 Design or Procedure utilized for the modification prescribes the use of specific materials, they should be
            documented using property P68 foresees use of (use foreseen by): E57 Material of E29 Design or Procedure, rather than via P126 employed
            (was employed in): E57 Material. </rdfs:comment>
        <rdfs:label xml:lang="en">Modification</rdfs:label>
        <skos:notation rdf:datatype="http://www.w3.org/2001/XMLSchema#string">E11</skos:notation>
    </owl:Class>
    


    <!-- http://www.cidoc-crm.org/cidoc-crm/E12 -->

    <owl:Class rdf:about="http://www.cidoc-crm.org/cidoc-crm/E12">
        <rdfs:subClassOf rdf:resource="http://www.cidoc-crm.org/cidoc-crm/E11"/>
        <rdfs:subClassOf rdf:resource="http://www.cidoc-crm.org/cidoc-crm/E63"/>
        <rdfs:comment rdf:datatype="http://www.w3.org/2001/XMLSchema#string">This class comprises activities that are designed to, and succeed in, creating one or more new items. It specializes the notion of
            modification into production. The decision as to whether or not an object is regarded as new is context sensitive. Normally, items are
            considered “new” if there is no obvious overall similarity between them and the consumed items and material used in their production. In
            other cases, an item is considered “new” because it becomes relevant to documentation by a modification. For example, the scribbling of a
            name on a potsherd may make it a voting token. The original potsherd may not be worth documenting, in contrast to the inscribed one. This
            entity can be collective: the printing of a thousand books, for example, would normally be considered a single event. An event should also
            be documented using E81 Transformation if it results in the destruction of one or more objects and the simultaneous production of others
            using parts or material from the originals. In this case, the new items have separate identities and matter is preserved, but identity is
            not. </rdfs:comment>
        <rdfs:label xml:lang="en">Production</rdfs:label>
        <skos:notation rdf:datatype="http://www.w3.org/2001/XMLSchema#string">E12</skos:notation>
    </owl:Class>
    


    <!-- http://www.cidoc-crm.org/cidoc-crm/E13 -->

    <owl:Class rdf:about="http://www.cidoc-crm.org/cidoc-crm/E13">
        <rdfs:subClassOf rdf:resource="http://www.cidoc-crm.org/cidoc-crm/E7"/>
        <rdfs:comment rdf:datatype="http://www.w3.org/2001/XMLSchema#string">This class comprises the actions of making assertions about properties of an object or any relation between two items or concepts.
            This class allows the documentation of how the respective assignment came about, and whose opinion it was. All the attributes or
            properties assigned in such an action can also be seen as directly attached to the respective item or concept, possibly as a collection of
            contradictory values. All cases of properties in this model that are also described indirectly through an action are characterised as
            &quot;short cuts&quot; of this action. This redundant modelling of two alternative views is preferred because many implementations may have good
            reasons to model either the action or the short cut, and the relation between both alternatives can be captured by simple rules. In
            particular, the class describes the actions of people making propositions and statements during certain museum procedures, e.g. the person
            and date when a condition statement was made, an identifier was assigned, the museum object was measured, etc. Which kinds of such
            assignments and statements need to be documented explicitly in structures of a schema rather than free text, depends on if this
            information should be accessible by structured queries. </rdfs:comment>
        <rdfs:label xml:lang="en">Attribute Assignment</rdfs:label>
        <skos:notation rdf:datatype="http://www.w3.org/2001/XMLSchema#string">E13</skos:notation>
    </owl:Class>
    


    <!-- http://www.cidoc-crm.org/cidoc-crm/E14 -->

    <owl:Class rdf:about="http://www.cidoc-crm.org/cidoc-crm/E14">
        <rdfs:subClassOf rdf:resource="http://www.cidoc-crm.org/cidoc-crm/E13"/>
        <rdfs:comment rdf:datatype="http://www.w3.org/2001/XMLSchema#string">This class describes the act of assessing the state of preservation of an object during a particular period. The condition assessment
            may be carried out by inspection, measurement or through historical research. This class is used to document circumstances of the
            respective assessment that may be relevant to interpret its quality at a later stage, or to continue research on related documents. </rdfs:comment>
        <rdfs:label xml:lang="en">Condition Assessment</rdfs:label>
        <skos:notation rdf:datatype="http://www.w3.org/2001/XMLSchema#string">E14</skos:notation>
    </owl:Class>
    


    <!-- http://www.cidoc-crm.org/cidoc-crm/E15 -->

    <owl:Class rdf:about="http://www.cidoc-crm.org/cidoc-crm/E15">
        <rdfs:subClassOf rdf:resource="http://www.cidoc-crm.org/cidoc-crm/E13"/>
        <rdfs:comment rdf:datatype="http://www.w3.org/2001/XMLSchema#string">This class comprises activities that result in the allocation of an identifier to an instance of E1 CRM Entity. An E15 Identifier
            Assignment may include the creation of the identifier from multiple constituents, which themselves may be instances of E41 Appellation.
            The syntax and kinds of constituents to be used may be declared in a rule constituting an instance of E29 Design or Procedure. Examples of
            such identifiers include Find Numbers, Inventory Numbers, uniform titles in the sense of librarianship and Digital Object Identifiers
            (DOI). Documenting the act of identifier assignment and deassignment is especially useful when objects change custody or the
            identification system of an organization is changed. In order to keep track of the identity of things in such cases, it is important to
            document by whom, when and for what purpose an identifier is assigned to an item. The fact that an identifier is a preferred one for an
            organisation can be expressed by using the property E1 CRM Entity. P48 has preferred identifier (is preferred identifier of): E42
            Identifier. It can better be expressed in a context independent form by assigning a suitable E55 Type, such as “preferred identifier
            assignment”, to the respective instance of E15 Identifier Assignment via the P2 has type property. </rdfs:comment>
        <rdfs:label xml:lang="en">Identifier Assignment</rdfs:label>
        <skos:notation rdf:datatype="http://www.w3.org/2001/XMLSchema#string">E15</skos:notation>
    </owl:Class>
    


    <!-- http://www.cidoc-crm.org/cidoc-crm/E16 -->

    <owl:Class rdf:about="http://www.cidoc-crm.org/cidoc-crm/E16">
        <rdfs:subClassOf rdf:resource="http://www.cidoc-crm.org/cidoc-crm/E13"/>
        <rdfs:comment rdf:datatype="http://www.w3.org/2001/XMLSchema#string">This class comprises actions measuring physical properties and other values that can be determined by a systematic procedure.
            Examples include measuring the monetary value of a collection of coins or the running time of a specific video cassette. The E16
            Measurement may use simple counting or tools, such as yardsticks or radiation detection devices. The interest is in the method and care
            applied, so that the reliability of the result may be judged at a later stage, or research continued on the associated documents. The date
            of the event is important for dimensions, which may change value over time, such as the length of an object subject to shrinkage. Details
            of methods and devices are best handled as free text, whereas basic techniques such as &quot;carbon 14 dating&quot; should be encoded using P2 has
            type (is type of:) E55 Type. </rdfs:comment>
        <rdfs:label xml:lang="en">Measurement</rdfs:label>
        <skos:notation rdf:datatype="http://www.w3.org/2001/XMLSchema#string">E16</skos:notation>
    </owl:Class>
    


    <!-- http://www.cidoc-crm.org/cidoc-crm/E17 -->

    <owl:Class rdf:about="http://www.cidoc-crm.org/cidoc-crm/E17">
        <rdfs:subClassOf rdf:resource="http://www.cidoc-crm.org/cidoc-crm/E13"/>
        <rdfs:comment rdf:datatype="http://www.w3.org/2001/XMLSchema#string">This class comprises the actions of classifying items of whatever kind. Such items include objects, specimens, people, actions and
            concepts. This class allows for the documentation of the context of classification acts in cases where the value of the classification
            depends on the personal opinion of the classifier, and the date that the classification was made. This class also encompasses the notion
            of &quot;determination,&quot; i.e. the systematic and molecular identification of a specimen in biology. </rdfs:comment>
        <rdfs:label xml:lang="en">Type Assignment</rdfs:label>
        <skos:notation rdf:datatype="http://www.w3.org/2001/XMLSchema#string">E17</skos:notation>
    </owl:Class>
    


    <!-- http://www.cidoc-crm.org/cidoc-crm/E18 -->

    <owl:Class rdf:about="http://www.cidoc-crm.org/cidoc-crm/E18">
        <rdfs:subClassOf rdf:resource="http://www.cidoc-crm.org/cidoc-crm/E72"/>
        <rdfs:subClassOf rdf:resource="http://www.cidoc-crm.org/cidoc-crm/E92"/>
        <rdfs:comment rdf:datatype="http://www.w3.org/2001/XMLSchema#string">This class comprises all persistent physical items with a relatively stable form, man-made or natural. Depending on the existence of
            natural boundaries of such things, the CRM distinguishes the instances of E19 Physical Object from instances of E26 Physical Feature, such
            as holes, rivers, pieces of land etc. Most instances of E19 Physical Object can be moved (if not too heavy), whereas features are integral
            to the surrounding matter. An instance of E18 Physical Thing occupies not only a particular geometric space, but in the course of its
            existence it also forms a trajectory through spacetime, which occupies a real, that is phenomenal, volume in spacetime. We include in the
            occupied space the space filled by the matter of the physical thing and all its inner spaces, such as the interior of a box. Physical
            things consisting of aggregations of physically unconnected objects, such as a set of chessmen, occupy a number of individually contiguous
            spacetime volumes equal to the number of unconnected objects that constitute the set. We model E18 Physical Thing to be a subclass of E72
            Legal Object and of E92 Spacetime volume. The latter is intended as a phenomenal spacetime volume as defined in CRMgeo (Doerr and Hiebel
            2013). By virtue of this multiple inheritance we can discuss the physical extent of an E18 Physical Thing without representing each
            instance of it together with an instance of its associated spacetime volume. This model combines two quite different kinds of substance:
            an instance of E18 Physical Thing is matter while a spacetime volume is an aggregation of points in spacetime. However, the real
            spatiotemporal extent of an instance of E18 Physical Thing is regarded to be unique to it, due to all its details and fuzziness; its
            identity and existence depends uniquely on the identity of the instance of E18 Physical Thing. Therefore this multiple inheritance is
            unambiguous and effective and furthermore corresponds to the intuitions of natural language. The CIDOC CRM is generally not concerned with
            amounts of matter in fluid or gaseous states. </rdfs:comment>
        <rdfs:label xml:lang="en">Physical Thing</rdfs:label>
        <skos:notation rdf:datatype="http://www.w3.org/2001/XMLSchema#string">E18</skos:notation>
    </owl:Class>
    


    <!-- http://www.cidoc-crm.org/cidoc-crm/E19 -->

    <owl:Class rdf:about="http://www.cidoc-crm.org/cidoc-crm/E19">
        <rdfs:subClassOf rdf:resource="http://www.cidoc-crm.org/cidoc-crm/E18"/>
        <rdfs:comment rdf:datatype="http://www.w3.org/2001/XMLSchema#string">This class comprises items of a material nature that are units for documentation and have physical boundaries that separate them
            completely in an objective way from other objects. The class also includes all aggregates of objects made for functional purposes of
            whatever kind, independent of physical coherence, such as a set of chessmen. Typically, instances of E19 Physical Object can be moved (if
            not too heavy). In some contexts, such objects, except for aggregates, are also called “bona fide objects” (Smith   Varzi, 2000,
            pp.401-420), i.e. naturally defined objects. The decision as to what is documented as a complete item, rather than by its parts or
            components, may be a purely administrative decision or may be a result of the order in which the item was acquired. </rdfs:comment>
        <rdfs:label xml:lang="en">Physical Object</rdfs:label>
        <skos:notation rdf:datatype="http://www.w3.org/2001/XMLSchema#string">E19</skos:notation>
    </owl:Class>
    


    <!-- http://www.cidoc-crm.org/cidoc-crm/E2 -->

    <owl:Class rdf:about="http://www.cidoc-crm.org/cidoc-crm/E2">
        <rdfs:subClassOf rdf:resource="http://www.cidoc-crm.org/cidoc-crm/E1"/>
        <rdfs:comment rdf:datatype="http://www.w3.org/2001/XMLSchema#string">This class comprises all phenomena, such as the instances of E4 Periods, E5 Events and states, which happen over a limited extent in
            time. In some contexts, these are also called perdurants. This class is disjoint from E77 Persistent Item. This is an abstract class and
            has no direct instances. E2 Temporal Entity is specialized into E4 Period, which applies to a particular geographic area (defined with a
            greater or lesser degree of precision), and E3 Condition State, which applies to instances of E18 Physical Thing. </rdfs:comment>
        <rdfs:label xml:lang="en">Temporal Entity</rdfs:label>
        <skos:notation rdf:datatype="http://www.w3.org/2001/XMLSchema#string">E2</skos:notation>
    </owl:Class>
    


    <!-- http://www.cidoc-crm.org/cidoc-crm/E20 -->

    <owl:Class rdf:about="http://www.cidoc-crm.org/cidoc-crm/E20">
        <rdfs:subClassOf rdf:resource="http://www.cidoc-crm.org/cidoc-crm/E19"/>
        <rdfs:comment rdf:datatype="http://www.w3.org/2001/XMLSchema#string">This class comprises individual items of a material nature, which live, have lived or are natural products of or from living
            organisms. Artificial objects that incorporate biological elements, such as Victorian butterfly frames, can be documented as both
            instances of E20 Biological Object and E22 Man-Made Object. </rdfs:comment>
        <rdfs:label xml:lang="en">Biological Object</rdfs:label>
        <skos:notation rdf:datatype="http://www.w3.org/2001/XMLSchema#string">E20</skos:notation>
    </owl:Class>
    


    <!-- http://www.cidoc-crm.org/cidoc-crm/E21 -->

    <owl:Class rdf:about="http://www.cidoc-crm.org/cidoc-crm/E21">
        <rdfs:subClassOf rdf:resource="http://www.cidoc-crm.org/cidoc-crm/E20"/>
        <rdfs:subClassOf rdf:resource="http://www.cidoc-crm.org/cidoc-crm/E39"/>
        <rdfs:comment rdf:datatype="http://www.w3.org/2001/XMLSchema#string">This class comprises real persons who live or are assumed to have lived. Legendary figures that may have existed, such as Ulysses and
            King Arthur, fall into this class if the documentation refers to them as historical figures. In cases where doubt exists as to whether
            several persons are in fact identical, multiple instances can be created and linked to indicate their relationship. The CRM does not
            propose a specific form to support reasoning about possible identity. </rdfs:comment>
        <rdfs:label xml:lang="en">Person</rdfs:label>
        <skos:notation rdf:datatype="http://www.w3.org/2001/XMLSchema#string">E21</skos:notation>
    </owl:Class>
    


    <!-- http://www.cidoc-crm.org/cidoc-crm/E22 -->

    <owl:Class rdf:about="http://www.cidoc-crm.org/cidoc-crm/E22">
        <rdfs:subClassOf rdf:resource="http://www.cidoc-crm.org/cidoc-crm/E19"/>
        <rdfs:subClassOf rdf:resource="http://www.cidoc-crm.org/cidoc-crm/E24"/>
        <rdfs:comment rdf:datatype="http://www.w3.org/2001/XMLSchema#string">This class comprises physical objects purposely created by human activity. No assumptions are made as to the extent of modification
            required to justify regarding an object as man-made. For example, an inscribed piece of rock or a preserved butterfly are both regarded as
            instances of E22 Man-Made Object. </rdfs:comment>
        <rdfs:label xml:lang="en">Man-Made Object</rdfs:label>
        <skos:notation rdf:datatype="http://www.w3.org/2001/XMLSchema#string">E22</skos:notation>
    </owl:Class>
    


    <!-- http://www.cidoc-crm.org/cidoc-crm/E24 -->

    <owl:Class rdf:about="http://www.cidoc-crm.org/cidoc-crm/E24">
        <rdfs:subClassOf rdf:resource="http://www.cidoc-crm.org/cidoc-crm/E18"/>
        <rdfs:subClassOf rdf:resource="http://www.cidoc-crm.org/cidoc-crm/E71"/>
        <rdfs:comment rdf:datatype="http://www.w3.org/2001/XMLSchema#string">This class comprises all persistent physical items that are purposely created by human activity. This class comprises man-made
            objects, such as a swords, and man-made features, such as rock art. No assumptions are made as to the extent of modification required to
            justify regarding an object as man-made. For example, a “cup and ring” carving on bedrock is regarded as instance of E24 Physical Man-Made
            Thing. </rdfs:comment>
        <rdfs:label xml:lang="en">Physical Man-Made Thing</rdfs:label>
        <skos:notation rdf:datatype="http://www.w3.org/2001/XMLSchema#string">E24</skos:notation>
    </owl:Class>
    


    <!-- http://www.cidoc-crm.org/cidoc-crm/E25 -->

    <owl:Class rdf:about="http://www.cidoc-crm.org/cidoc-crm/E25">
        <rdfs:subClassOf rdf:resource="http://www.cidoc-crm.org/cidoc-crm/E24"/>
        <rdfs:subClassOf rdf:resource="http://www.cidoc-crm.org/cidoc-crm/E26"/>
        <rdfs:comment rdf:datatype="http://www.w3.org/2001/XMLSchema#string">This class comprises physical features that are purposely created by human activity, such as scratches, artificial caves, artificial
            water channels, etc. No assumptions are made as to the extent of modification required to justify regarding a feature as man-made. For
            example, rock art or even “cup and ring” carvings on bedrock a regarded as types of E25 Man-Made Feature. </rdfs:comment>
        <rdfs:label xml:lang="en">Man-Made Feature</rdfs:label>
        <skos:notation rdf:datatype="http://www.w3.org/2001/XMLSchema#string">E25</skos:notation>
    </owl:Class>
    


    <!-- http://www.cidoc-crm.org/cidoc-crm/E26 -->

    <owl:Class rdf:about="http://www.cidoc-crm.org/cidoc-crm/E26">
        <rdfs:subClassOf rdf:resource="http://www.cidoc-crm.org/cidoc-crm/E18"/>
        <rdfs:comment rdf:datatype="http://www.w3.org/2001/XMLSchema#string">This class comprises identifiable features that are physically attached in an integral way to particular physical objects. Instances
            of E26 Physical Feature share many of the attributes of instances of E19 Physical Object. They may have a one-, two- or three-dimensional
            geometric extent, but there are no natural borders that separate them completely in an objective way from the carrier objects. For
            example, a doorway is a feature but the door itself, being attached by hinges, is not. Instances of E26 Physical Feature can be features
            in a narrower sense, such as scratches, holes, reliefs, surface colours, reflection zones in an opal crystal or a density change in a
            piece of wood. In the wider sense, they are portions of particular objects with partially imaginary borders, such as the core of the
            Earth, an area of property on the surface of the Earth, a landscape or the head of a contiguous marble statue. They can be measured and
            dated, and it is sometimes possible to state who or what is or was responsible for them. They cannot be separated from the carrier object,
            but a segment of the carrier object may be identified (or sometimes removed) carrying the complete feature. This definition coincides with
            the definition of &quot;fiat objects&quot; (Smith   Varzi, 2000, pp.401-420), with the exception of aggregates of “bona fide objects”. </rdfs:comment>
        <rdfs:label xml:lang="en">Physical Feature</rdfs:label>
        <skos:notation rdf:datatype="http://www.w3.org/2001/XMLSchema#string">E26</skos:notation>
    </owl:Class>
    


    <!-- http://www.cidoc-crm.org/cidoc-crm/E27 -->

    <owl:Class rdf:about="http://www.cidoc-crm.org/cidoc-crm/E27">
        <rdfs:subClassOf rdf:resource="http://www.cidoc-crm.org/cidoc-crm/E26"/>
        <rdfs:comment rdf:datatype="http://www.w3.org/2001/XMLSchema#string">This class comprises pieces of land or sea floor. In contrast to the purely geometric notion of E53 Place, this class describes
            constellations of matter on the surface of the Earth or other celestial body, which can be represented by photographs, paintings and maps.
            Instances of E27 Site are composed of relatively immobile material items and features in a particular configuration at a particular
            location</rdfs:comment>
        <rdfs:label xml:lang="en">Site</rdfs:label>
        <skos:notation rdf:datatype="http://www.w3.org/2001/XMLSchema#string">E27</skos:notation>
    </owl:Class>
    


    <!-- http://www.cidoc-crm.org/cidoc-crm/E28 -->

    <owl:Class rdf:about="http://www.cidoc-crm.org/cidoc-crm/E28">
        <rdfs:subClassOf rdf:resource="http://www.cidoc-crm.org/cidoc-crm/E71"/>
        <rdfs:comment rdf:datatype="http://www.w3.org/2001/XMLSchema#string">This class comprises non-material products of our minds and other human produced data that have become objects of a discourse about
            their identity, circumstances of creation or historical implication. The production of such information may have been supported by the use
            of technical devices such as cameras or computers. Characteristically, instances of this class are created, invented or thought by
            someone, and then may be documented or communicated between persons. Instances of E28 Conceptual Object have the ability to exist on more
            than one particular carrier at the same time, such as paper, electronic signals, marks, audio media, paintings, photos, human memories,
            etc. They cannot be destroyed. They exist as long as they can be found on at least one carrier or in at least one human memory. Their
            existence ends when the last carrier and the last memory are lost. </rdfs:comment>
        <rdfs:label xml:lang="en">Conceptual Object</rdfs:label>
        <skos:notation rdf:datatype="http://www.w3.org/2001/XMLSchema#string">E28</skos:notation>
    </owl:Class>
    


    <!-- http://www.cidoc-crm.org/cidoc-crm/E29 -->

    <owl:Class rdf:about="http://www.cidoc-crm.org/cidoc-crm/E29">
        <rdfs:subClassOf rdf:resource="http://www.cidoc-crm.org/cidoc-crm/E73"/>
        <rdfs:comment rdf:datatype="http://www.w3.org/2001/XMLSchema#string">This class comprises documented plans for the execution of actions in order to achieve a result of a specific quality, form or contents. In particular it comprises plans for deliberate human activities that may result in the modification or production of instances of E24 Physical Thing.
Instances of E29 Design or Procedure can be structured in parts and sequences or depend on others. This is modelled using P69 has association with (is associated with).
Designs or procedures can be seen as one of the following:
1. A schema for the activities it describes2. A schema of the products that result from their application.3. An independent intellectual product that may have never been applied, such as Leonardo da Vinci’s famous plans for flying machines.
Because designs or procedures may never be applied or only partially executed, the CRM models a loose relationship between the plan and the respective product.</rdfs:comment>
        <rdfs:label xml:lang="en">Design or Procedure</rdfs:label>
        <skos:notation rdf:datatype="http://www.w3.org/2001/XMLSchema#string">E29</skos:notation>
    </owl:Class>
    


    <!-- http://www.cidoc-crm.org/cidoc-crm/E3 -->

    <owl:Class rdf:about="http://www.cidoc-crm.org/cidoc-crm/E3">
        <rdfs:subClassOf rdf:resource="http://www.cidoc-crm.org/cidoc-crm/E2"/>
        <rdfs:comment rdf:datatype="http://www.w3.org/2001/XMLSchema#string">This class comprises the states of objects characterised by a certain condition over a time-span. An instance of this class describes
            the prevailing physical condition of any material object or feature during a specific E52 Time Span. In general, the time-span for which a
            certain condition can be asserted may be shorter than the real time-span, for which this condition held. The nature of that condition can
            be described using P2 has type. For example, the E3 Condition State “condition of the SS Great Britain between 22 September 1846 and 27
            August 1847” can be characterized as E55 Type “wrecked”. </rdfs:comment>
        <rdfs:label xml:lang="en">Condition State</rdfs:label>
        <skos:notation rdf:datatype="http://www.w3.org/2001/XMLSchema#string">E3</skos:notation>
    </owl:Class>
    


    <!-- http://www.cidoc-crm.org/cidoc-crm/E30 -->

    <owl:Class rdf:about="http://www.cidoc-crm.org/cidoc-crm/E30">
        <rdfs:subClassOf rdf:resource="http://www.cidoc-crm.org/cidoc-crm/E89"/>
        <rdfs:comment rdf:datatype="http://www.w3.org/2001/XMLSchema#string">This class comprises legal privileges concerning material and immaterial things or their derivatives. These include reproduction and
            property rights</rdfs:comment>
        <rdfs:label xml:lang="en">Right</rdfs:label>
        <skos:notation rdf:datatype="http://www.w3.org/2001/XMLSchema#string">E30</skos:notation>
    </owl:Class>
    


    <!-- http://www.cidoc-crm.org/cidoc-crm/E31 -->

    <owl:Class rdf:about="http://www.cidoc-crm.org/cidoc-crm/E31">
        <rdfs:subClassOf rdf:resource="http://www.cidoc-crm.org/cidoc-crm/E73"/>
        <rdfs:comment rdf:datatype="http://www.w3.org/2001/XMLSchema#string">This class comprises identifiable immaterial items that make propositions about reality. These propositions may be expressed in text,
            graphics, images, audiograms, videograms or by other similar means. Documentation databases are regarded as a special case of E31
            Document. This class should not be confused with the term “document” in Information Technology, which is compatible with E73 Information
            Object. </rdfs:comment>
        <rdfs:label xml:lang="en">Document</rdfs:label>
        <skos:notation rdf:datatype="http://www.w3.org/2001/XMLSchema#string">E31</skos:notation>
    </owl:Class>
    


    <!-- http://www.cidoc-crm.org/cidoc-crm/E32 -->

    <owl:Class rdf:about="http://www.cidoc-crm.org/cidoc-crm/E32">
        <rdfs:subClassOf rdf:resource="http://www.cidoc-crm.org/cidoc-crm/E31"/>
        <rdfs:comment rdf:datatype="http://www.w3.org/2001/XMLSchema#string">This class comprises encyclopaedia, thesauri, authority lists and other documents that define terminology or conceptual systems for
            consistent use. </rdfs:comment>
        <rdfs:label xml:lang="en">Authority Document</rdfs:label>
        <skos:notation rdf:datatype="http://www.w3.org/2001/XMLSchema#string">E32</skos:notation>
    </owl:Class>
    


    <!-- http://www.cidoc-crm.org/cidoc-crm/E33 -->

    <owl:Class rdf:about="http://www.cidoc-crm.org/cidoc-crm/E33">
        <rdfs:subClassOf rdf:resource="http://www.cidoc-crm.org/cidoc-crm/E73"/>
        <rdfs:comment rdf:datatype="http://www.w3.org/2001/XMLSchema#string">This class comprises identifiable expressions in natural language or languages. Instances of E33 Linguistic Object can be expressed
            in many ways: e.g. as written texts, recorded speech or sign language. However, the CRM treats instances of E33 Linguistic Object
            independently from the medium or method by which they are expressed. Expressions in formal languages, such as computer code or
            mathematical formulae, are not treated as instances of E33 Linguistic Object by the CRM. These should be modelled as instances of E73
            Information Object. The text of an instance of E33 Linguistic Object can be documented in a note by P3 has note: E62 String </rdfs:comment>
        <rdfs:label xml:lang="en">Linguistic Object</rdfs:label>
        <skos:notation rdf:datatype="http://www.w3.org/2001/XMLSchema#string">E33</skos:notation>
    </owl:Class>
    


    <!-- http://www.cidoc-crm.org/cidoc-crm/E34 -->

    <owl:Class rdf:about="http://www.cidoc-crm.org/cidoc-crm/E34">
        <rdfs:subClassOf rdf:resource="http://www.cidoc-crm.org/cidoc-crm/E33"/>
        <rdfs:subClassOf rdf:resource="http://www.cidoc-crm.org/cidoc-crm/E37"/>
        <rdfs:comment rdf:datatype="http://www.w3.org/2001/XMLSchema#string">This class comprises recognisable, short texts attached to instances of E24 Physical Man-Made Thing. The transcription of the text
            can be documented in a note by P3 has note: E62 String. The alphabet used can be documented by P2 has type: E55 Type. This class does not
            intend to describe the idiosyncratic characteristics of an individual physical embodiment of an inscription, but the underlying prototype.
            The physical embodiment is modelled in the CRM as E24 Physical Man-Made Thing. The relationship of a physical copy of a book to the text
            it contains is modelled using E84 Information Carrier. P128 carries (is carried by): E33 Linguistic Object. </rdfs:comment>
        <rdfs:label xml:lang="en">Inscription</rdfs:label>
        <skos:notation rdf:datatype="http://www.w3.org/2001/XMLSchema#string">E34</skos:notation>
    </owl:Class>
    


    <!-- http://www.cidoc-crm.org/cidoc-crm/E35 -->

    <owl:Class rdf:about="http://www.cidoc-crm.org/cidoc-crm/E35">
        <rdfs:subClassOf rdf:resource="http://www.cidoc-crm.org/cidoc-crm/E33"/>
        <rdfs:subClassOf rdf:resource="http://www.cidoc-crm.org/cidoc-crm/E41"/>
        <rdfs:comment rdf:datatype="http://www.w3.org/2001/XMLSchema#string">This class comprises the names assigned to works, such as texts, artworks or pieces of music. Titles are proper noun phrases or
            verbal phrases, and should not be confused with generic object names such as “chair”, “painting” or “book” (the latter are common nouns
            that stand for instances of E55 Type). Titles may be assigned by the creator of the work itself, or by a social group. This class also
            comprises the translations of titles that are used as surrogates for the original titles in different social contexts. </rdfs:comment>
        <rdfs:label xml:lang="en">Title</rdfs:label>
        <skos:notation rdf:datatype="http://www.w3.org/2001/XMLSchema#string">E35</skos:notation>
    </owl:Class>
    


    <!-- http://www.cidoc-crm.org/cidoc-crm/E36 -->

    <owl:Class rdf:about="http://www.cidoc-crm.org/cidoc-crm/E36">
        <rdfs:subClassOf rdf:resource="http://www.cidoc-crm.org/cidoc-crm/E73"/>
        <rdfs:comment rdf:datatype="http://www.w3.org/2001/XMLSchema#string">This class comprises the intellectual or conceptual aspects of recognisable marks and images. This class does not intend to describe
            the idiosyncratic characteristics of an individual physical embodiment of a visual item, but the underlying prototype. For example, a mark
            such as the ICOM logo is generally considered to be the same logo when used on any number of publications. The size, orientation and
            colour may change, but the logo remains uniquely identifiable. The same is true of images that are reproduced many times. This means that
            visual items are independent of their physical support. The class E36 Visual Item provides a means of identifying and linking together
            instances of E24 Physical Man-Made Thing that carry the same visual symbols, marks or images etc. The property P62 depicts (is depicted
            by) between E24 Physical Man-Made Thing and depicted subjects (E1 CRM Entity) can be regarded as a short-cut of the more fully developed
            path from E24 Physical Man-Made Thing through P65 shows visual item (is shown by), E36 Visual Item, P138 represents (has representation)
            to E1CRM Entity, which in addition captures the optical features of the depiction. </rdfs:comment>
        <rdfs:label xml:lang="en">Visual Item</rdfs:label>
        <skos:notation rdf:datatype="http://www.w3.org/2001/XMLSchema#string">E36</skos:notation>
    </owl:Class>
    


    <!-- http://www.cidoc-crm.org/cidoc-crm/E37 -->

    <owl:Class rdf:about="http://www.cidoc-crm.org/cidoc-crm/E37">
        <rdfs:subClassOf rdf:resource="http://www.cidoc-crm.org/cidoc-crm/E36"/>
        <rdfs:comment rdf:datatype="http://www.w3.org/2001/XMLSchema#string">This class comprises symbols, signs, signatures or short texts applied to instances of E24 Physical Man-Made Thing by arbitrary
            techniques in order to indicate the creator, owner, dedications, purpose, etc. This class specifically excludes features that have no
            semantic significance, such as scratches or tool marks. These should be documented as instances of E25 Man-Made Feature. </rdfs:comment>
        <rdfs:label xml:lang="en">Mark</rdfs:label>
        <skos:notation rdf:datatype="http://www.w3.org/2001/XMLSchema#string">E37</skos:notation>
    </owl:Class>
    


    <!-- http://www.cidoc-crm.org/cidoc-crm/E38 -->

    <owl:Class rdf:about="http://www.cidoc-crm.org/cidoc-crm/E38">
        <rdfs:subClassOf rdf:resource="http://www.cidoc-crm.org/cidoc-crm/E36"/>
        <rdfs:comment rdf:datatype="http://www.w3.org/2001/XMLSchema#string">This class comprises distributions of form, tone and colour that may be found on surfaces such as photos, paintings, prints and
            sculptures or directly on electronic media. The degree to which variations in the distribution of form and colour affect the identity of
            an instance of E38 Image depends on a given purpose. The original painting of the Mona Lisa in the Louvre may be said to bear the same
            instance of E38 Image as reproductions in the form of transparencies, postcards, posters or T-shirts, even though they may differ in size
            and carrier and may vary in tone and colour. The images in a “spot the difference” competition are not the same with respect to their
            context, however similar they may at first appear. </rdfs:comment>
        <rdfs:label xml:lang="en">Image</rdfs:label>
        <skos:notation rdf:datatype="http://www.w3.org/2001/XMLSchema#string">E38</skos:notation>
    </owl:Class>
    


    <!-- http://www.cidoc-crm.org/cidoc-crm/E39 -->

    <owl:Class rdf:about="http://www.cidoc-crm.org/cidoc-crm/E39">
        <rdfs:subClassOf rdf:resource="http://www.cidoc-crm.org/cidoc-crm/E77"/>
        <rdfs:comment rdf:datatype="http://www.w3.org/2001/XMLSchema#string">This class comprises people, either individually or in groups, who have the potential to perform intentional actions of kinds for
            which someone may be held responsible. The CRM does not attempt to model the inadvertent actions of such actors. Individual people should
            be documented as instances of E21 Person, whereas groups should be documented as instances of either E74 Group or its subclass E40 Legal
            Body. </rdfs:comment>
        <rdfs:label xml:lang="en">Actor</rdfs:label>
        <skos:notation rdf:datatype="http://www.w3.org/2001/XMLSchema#string">E39</skos:notation>
    </owl:Class>
    


    <!-- http://www.cidoc-crm.org/cidoc-crm/E4 -->

    <owl:Class rdf:about="http://www.cidoc-crm.org/cidoc-crm/E4">
        <rdfs:subClassOf rdf:resource="http://www.cidoc-crm.org/cidoc-crm/E2"/>
        <rdfs:subClassOf rdf:resource="http://www.cidoc-crm.org/cidoc-crm/E92"/>
        <rdfs:comment rdf:datatype="http://www.w3.org/2001/XMLSchema#string">This class comprises sets of coherent phenomena or cultural manifestations occurring in time and space. It is the social or physical
            coherence of these phenomena that identify an E4 Period and not the associated spatiotemporal extent. This extent is only the &quot;ground&quot; or
            space in an abstract physical sense that the actual process of growth, spread and retreat has covered. Consequently, different periods can
            overlap and coexist in time and space, such as when a nomadic culture exists in the same area and time as a sedentary culture. This also
            means that overlapping land use rights, common among first nations, amounts to overlapping periods. Often, this class is used to describe
            prehistoric or historic periods such as the &quot;Neolithic Period&quot;, the &quot;Ming Dynasty&quot; or the &quot;McCarthy Era&quot;, but also geopolitical units and
            activities of settlements are regarded as special cases of E4 Period. However, there are no assumptions about the scale of the associated
            phenomena. In particular all events are seen as synthetic processes consisting of coherent phenomena. Therefore E4 Period is a superclass
            of E5 Event. For example, a modern clinical E67 Birth can be seen as both an atomic E5 Event and as an E4 Period that consists of multiple
            activities performed by multiple instances of E39 Actor. As the actual extent of an E4 Period in spacetime we regard the trajectories of
            the participating physical things during their participation in an instance of E4 Period. This includes the open spaces via which these
            things have interacted and the spaces by which they had the potential to interact during that period or event in the way defined by the
            type of the respective period or event. Examples include the air in a meeting room transferring the voices of the participants. Since
            these phenomena are fuzzy, we assume the spatiotemporal extent to be contiguous, except for cases of phenomena spreading out over islands
            or other separated areas, including geopolitical units distributed over disconnected areas such as islands or colonies. Whether the
            trajectories necessary for participants to travel between these areas are regarded as part of the spatiotemporal extent or not has to be
            decided in each case based on a concrete analysis, taking use of the sea for other purposes than travel, such as fishing, into
            consideration. One may also argue that the activities to govern disconnected areas imply travelling through spaces connecting them and
            that these areas hence are spatially connected in a way, but it appears counterintuitive to consider for instance travel routes in
            international waters as extensions of geopolitical units. Consequently, an instance of E4 Period may occupy a number of disjoint spacetime
            volumes, however there must not be a discontinuity in the timespan covered by these spacetime volumes. This means that an instance of E4
            Period must be contiguous in time. If it has ended in all areas, it has ended as a whole. However it may end in one area before another,
            such as in the Polynesian migration, and it continues as long as it is ongoing in at least one area. We model E4 Period as a subclass of
            E2 Temporal Entity and of E92 Spacetime volume. The latter is intended as a phenomenal spacetime volume as defined in CRMgeo (Doerr and
            Hiebel 2013). By virtue of this multiple inheritance we can discuss the physical extent of an E4 Period without representing each instance
            of it together with an instance of its associated spacetime volume. This model combines two quite different kinds of substance: an
            instance of E4 Period is a phenomena while a space-time volume is an aggregation of points in spacetime. However, the real spatiotemporal
            extent of an instance of E4 Period is regarded to be unique to it due to all its details and fuzziness; its identity and existence depends
            uniquely on the identity of the instance of E4 Period. Therefore this multiple inheritance is unambiguous and effective and furthermore
            corresponds to the intuitions of natural language. There are two different conceptualisations of &apos;artistic style&apos;, defined either by
            physical features or by historical context. For example, “Impressionism” can be viewed as a period lasting from approximately 1870 to 1905
            during which paintings with particular characteristics were produced by a group of artists that included (among others) Monet, Renoir,
            Pissarro, Sisley and Degas. Alternatively, it can be regarded as a style applicable to all paintings sharing the characteristics of the
            works produced by the Impressionist painters, regardless of historical context. The first interpretation is an instance of E4 Period, and
            the second defines morphological object types that fall under E55 Type. Another specific case of an E4 Period is the set of activities and
            phenomena associated with a settlement, such as the populated period of Nineveh. </rdfs:comment>
        <rdfs:label xml:lang="en">Period</rdfs:label>
        <skos:notation rdf:datatype="http://www.w3.org/2001/XMLSchema#string">E4</skos:notation>
    </owl:Class>
    


    <!-- http://www.cidoc-crm.org/cidoc-crm/E40 -->

    <owl:Class rdf:about="http://www.cidoc-crm.org/cidoc-crm/E40">
        <rdfs:subClassOf rdf:resource="http://www.cidoc-crm.org/cidoc-crm/E74"/>
        <rdfs:comment rdf:datatype="http://www.w3.org/2001/XMLSchema#string">This class comprises institutions or groups of people that have obtained a legal recognition as a group and can act collectively as
            agents. This means that they can perform actions, own property, create or destroy things and can be held collectively responsible for
            their actions like individual people. The term &apos;personne morale&apos; is often used for this in French. </rdfs:comment>
        <rdfs:label xml:lang="en">Legal Body</rdfs:label>
        <skos:notation rdf:datatype="http://www.w3.org/2001/XMLSchema#string">E40</skos:notation>
    </owl:Class>
    


    <!-- http://www.cidoc-crm.org/cidoc-crm/E41 -->

    <owl:Class rdf:about="http://www.cidoc-crm.org/cidoc-crm/E41">
        <rdfs:subClassOf rdf:resource="http://www.cidoc-crm.org/cidoc-crm/E90"/>
        <rdfs:comment rdf:datatype="http://www.w3.org/2001/XMLSchema#string">This class comprises signs, either meaningful or not, or arrangements of signs following a specific syntax, that are used or can be
            used to refer to and identify a specific instance of some class or category within a certain context. Instances of E41 Appellation do not
            identify things by their meaning, even if they happen to have one, but instead by convention, tradition, or agreement. Instances of E41
            Appellation are cultural constructs; as such, they have a context, a history, and a use in time and space by some group of users. A given
            instance of E41 Appellation can have alternative forms, i.e., other instances of E41 Appellation that are always regarded as equivalent
            independent from the thing it denotes. Specific subclasses of E41 Appellation should be used when instances of E41 Appellation of a
            characteristic form are used for particular objects. Instances of E49 Time Appellation, for example, which take the form of instances of
            E50 Date, can be easily recognised. E41 Appellation should not be confused with the act of naming something. Cf. E15 Identifier Assignment </rdfs:comment>
        <rdfs:label xml:lang="en">Appellation</rdfs:label>
        <skos:notation rdf:datatype="http://www.w3.org/2001/XMLSchema#string">E41</skos:notation>
    </owl:Class>
    


    <!-- http://www.cidoc-crm.org/cidoc-crm/E42 -->

    <owl:Class rdf:about="http://www.cidoc-crm.org/cidoc-crm/E42">
        <rdfs:subClassOf rdf:resource="http://www.cidoc-crm.org/cidoc-crm/E41"/>
        <rdfs:comment rdf:datatype="http://www.w3.org/2001/XMLSchema#string">This class comprises strings or codes assigned to instances of E1 CRM Entity in order to identify them uniquely and permanently
            within the context of one or more organisations. Such codes are often known as inventory numbers, registration codes, etc. and are
            typically composed of alphanumeric sequences. The class E42 Identifier is not normally used for machine-generated identifiers used for
            automated processing unless these are also used by human agents.</rdfs:comment>
        <rdfs:label xml:lang="en">Identifier</rdfs:label>
        <skos:notation rdf:datatype="http://www.w3.org/2001/XMLSchema#string">E42</skos:notation>
    </owl:Class>
    


    <!-- http://www.cidoc-crm.org/cidoc-crm/E44 -->

    <owl:Class rdf:about="http://www.cidoc-crm.org/cidoc-crm/E44">
        <rdfs:subClassOf rdf:resource="http://www.cidoc-crm.org/cidoc-crm/E41"/>
        <rdfs:comment rdf:datatype="http://www.w3.org/2001/XMLSchema#string">This class comprises any sort of identifier characteristically used to refer to an E53 Place. Instances of E44 Place Appellation may
            vary in their degree of precision and their meaning may vary over time - the same instance of E44 Place Appellation may be used to refer
            to several places, either because of cultural shifts, or because objects used as reference points have moved around. Instances of E44
            Place Appellation can be extremely varied in form: postal addresses, instances of E47 Spatial Coordinate, and parts of buildings can all
            be considered as instances of E44 Place Appellation. </rdfs:comment>
        <rdfs:label xml:lang="en">Place Appellation</rdfs:label>
        <skos:notation rdf:datatype="http://www.w3.org/2001/XMLSchema#string">E44</skos:notation>
    </owl:Class>
    


    <!-- http://www.cidoc-crm.org/cidoc-crm/E45 -->

    <owl:Class rdf:about="http://www.cidoc-crm.org/cidoc-crm/E45">
        <rdfs:subClassOf rdf:resource="http://www.cidoc-crm.org/cidoc-crm/E44"/>
        <rdfs:subClassOf rdf:resource="http://www.cidoc-crm.org/cidoc-crm/E51"/>
        <rdfs:comment rdf:datatype="http://www.w3.org/2001/XMLSchema#string">This class comprises identifiers expressed in coding systems for places, such as postal addresses used for mailing. An E45 Address
            can be considered both as the name of an E53 Place and as an E51 Contact Point for an E39 Actor. This dual aspect is reflected in the
            multiple inheritance. However, some forms of mailing addresses, such as a postal box, are only instances of E51 Contact Point, since they
            do not identify any particular Place. These should not be documented as instances of E45 Address. </rdfs:comment>
        <rdfs:label xml:lang="en">Address</rdfs:label>
        <skos:notation rdf:datatype="http://www.w3.org/2001/XMLSchema#string">E45</skos:notation>
    </owl:Class>
    


    <!-- http://www.cidoc-crm.org/cidoc-crm/E46 -->

    <owl:Class rdf:about="http://www.cidoc-crm.org/cidoc-crm/E46">
        <rdfs:subClassOf rdf:resource="http://www.cidoc-crm.org/cidoc-crm/E44"/>
        <rdfs:comment rdf:datatype="http://www.w3.org/2001/XMLSchema#string">This class comprises areas of objects referred to in terms specific to the general geometry or structure of its kind. The &apos;prow&apos; of
            the boat, the &apos;frame&apos; of the picture, the &apos;front&apos; of the building are all instances of E46 Section Definition. The class highlights the
            fact that parts of objects can be treated as locations. This holds in particular for features without natural boundaries, such as the
            “head” of a marble statue made out of one block (cf. E53 Place). In answer to the question &apos;where is the signature?&apos; one might reply &apos;on
            the lower left corner&apos;. (Section Definition is closely related to the term “segment” in Gerstl, P.  Pribbenow, S, 1996 “ A conceptual
            theory of part – whole relations and its applications”, Data   Knowledge Engineering 20 305-322, North Holland- Elsevier ). </rdfs:comment>
        <rdfs:label xml:lang="en">Section Definition</rdfs:label>
        <skos:notation rdf:datatype="http://www.w3.org/2001/XMLSchema#string">E46</skos:notation>
    </owl:Class>
    


    <!-- http://www.cidoc-crm.org/cidoc-crm/E47 -->

    <owl:Class rdf:about="http://www.cidoc-crm.org/cidoc-crm/E47">
        <rdfs:subClassOf rdf:resource="http://www.cidoc-crm.org/cidoc-crm/E44"/>
        <rdfs:comment rdf:datatype="http://www.w3.org/2001/XMLSchema#string">This class comprises the textual or numeric information required to locate specific instances of E53 Place within schemes of spatial
            identification. Coordinates are a specific form of E44 Place Appellation, that is, a means of referring to a particular E53 Place.
            Coordinates are not restricted to longitude, latitude and altitude. Any regular system of reference that maps onto an E19 Physical Object
            can be used to generate coordinates. </rdfs:comment>
        <rdfs:label xml:lang="en">Spatial Coordinates</rdfs:label>
        <skos:notation rdf:datatype="http://www.w3.org/2001/XMLSchema#string">E47</skos:notation>
    </owl:Class>
    


    <!-- http://www.cidoc-crm.org/cidoc-crm/E48 -->

    <owl:Class rdf:about="http://www.cidoc-crm.org/cidoc-crm/E48">
        <rdfs:subClassOf rdf:resource="http://www.cidoc-crm.org/cidoc-crm/E44"/>
        <rdfs:comment rdf:datatype="http://www.w3.org/2001/XMLSchema#string">This class comprises particular and common forms of E44 Place Appellation. Place Names may change their application over time: the
            name of an E53 Place may change, and a name may be reused for a different E53 Place. Instances of E48 Place Name are typically subject to
            place name gazetteers.</rdfs:comment>
        <rdfs:label xml:lang="en">Place Name</rdfs:label>
        <skos:notation rdf:datatype="http://www.w3.org/2001/XMLSchema#string">E48</skos:notation>
    </owl:Class>
    


    <!-- http://www.cidoc-crm.org/cidoc-crm/E49 -->

    <owl:Class rdf:about="http://www.cidoc-crm.org/cidoc-crm/E49">
        <rdfs:subClassOf rdf:resource="http://www.cidoc-crm.org/cidoc-crm/E41"/>
        <rdfs:comment rdf:datatype="http://www.w3.org/2001/XMLSchema#string">This class comprises all forms of names or codes, such as historical periods, and dates, which are characteristically used to refer
            to a specific E52 Time-Span. The instances of E49 Time Appellation may vary in their degree of precision, and they may be relative to
            other time frames, “Before Christ” for example. Instances of E52 Time-Span are often defined by reference to a cultural period or an event
            e.g. ‘the duration of the Ming Dynasty’.</rdfs:comment>
        <rdfs:label xml:lang="en">Time Appellation</rdfs:label>
        <skos:notation rdf:datatype="http://www.w3.org/2001/XMLSchema#string">E49</skos:notation>
    </owl:Class>
    


    <!-- http://www.cidoc-crm.org/cidoc-crm/E5 -->

    <owl:Class rdf:about="http://www.cidoc-crm.org/cidoc-crm/E5">
        <rdfs:subClassOf rdf:resource="http://www.cidoc-crm.org/cidoc-crm/E4"/>
        <rdfs:comment rdf:datatype="http://www.w3.org/2001/XMLSchema#string">This class comprises changes of states in cultural, social or physical systems, regardless of scale, brought about by a series or
            group of coherent physical, cultural, technological or legal phenomena. Such changes of state will affect instances of E77 Persistent Item
            or its subclasses. The distinction between an E5 Event and an E4 Period is partly a question of the scale of observation. Viewed at a
            coarse level of detail, an E5 Event is an ‘instantaneous’ change of state. At a fine level, the E5 Event can be analysed into its
            component phenomena within a space and time frame, and as such can be seen as an E4 Period. The reverse is not necessarily the case: not
            all instances of E4 Period give rise to a noteworthy change of state. </rdfs:comment>
        <rdfs:label xml:lang="en">Event</rdfs:label>
        <skos:notation rdf:datatype="http://www.w3.org/2001/XMLSchema#string">E5</skos:notation>
    </owl:Class>
    


    <!-- http://www.cidoc-crm.org/cidoc-crm/E50 -->

    <owl:Class rdf:about="http://www.cidoc-crm.org/cidoc-crm/E50">
        <rdfs:subClassOf rdf:resource="http://www.cidoc-crm.org/cidoc-crm/E49"/>
        <rdfs:comment rdf:datatype="http://www.w3.org/2001/XMLSchema#string">This class comprises specific forms of E49 Time Appellation.</rdfs:comment>
        <rdfs:label xml:lang="en">Date</rdfs:label>
        <skos:notation rdf:datatype="http://www.w3.org/2001/XMLSchema#string">E50</skos:notation>
    </owl:Class>
    


    <!-- http://www.cidoc-crm.org/cidoc-crm/E51 -->

    <owl:Class rdf:about="http://www.cidoc-crm.org/cidoc-crm/E51">
        <rdfs:subClassOf rdf:resource="http://www.cidoc-crm.org/cidoc-crm/E41"/>
        <rdfs:comment rdf:datatype="http://www.w3.org/2001/XMLSchema#string">This class comprises identifiers employed, or understood, by communication services to direct communications to an instance of E39
            Actor. These include E-mail addresses, telephone numbers, post office boxes, Fax numbers, URLs etc. Most postal addresses can be
            considered both as instances of E44 Place Appellation and E51 Contact Point. In such cases the subclass E45 Address should be used. URLs
            are addresses used by machines to access another machine through an http request. Since the accessed machine acts on behalf of the E39
            Actor providing the machine, URLs are considered as instances of E51 Contact Point to that E39 Actor. </rdfs:comment>
        <rdfs:label xml:lang="en">Contact Point</rdfs:label>
        <skos:notation rdf:datatype="http://www.w3.org/2001/XMLSchema#string">E51</skos:notation>
    </owl:Class>
    


    <!-- http://www.cidoc-crm.org/cidoc-crm/E52 -->

    <owl:Class rdf:about="http://www.cidoc-crm.org/cidoc-crm/E52">
        <rdfs:subClassOf rdf:resource="http://www.cidoc-crm.org/cidoc-crm/E1"/>
        <rdfs:comment rdf:datatype="http://www.w3.org/2001/XMLSchema#string">This class comprises abstract temporal extents, in the sense of Galilean physics, having a beginning, an end and a duration. Time
            Span has no other semantic connotations. Time-Spans are used to define the temporal extent of instances of E4 Period, E5 Event and any
            other phenomena valid for a certain time. An E52 Time-Span may be identified by one or more instances of E49 Time Appellation. Since our
            knowledge of history is imperfect, instances of E52 Time-Span can best be considered as approximations of the actual Time-Spans of
            temporal entities. The properties of E52 Time-Span are intended to allow these approximations to be expressed precisely. An extreme case
            of approximation, might, for example, define an E52 Time-Span having unknown beginning, end and duration. Used as a common E52 Time-Span
            for two events, it would nevertheless define them as being simultaneous, even if nothing else was known. Automatic processing and querying
            of instances of E52 Time-Span is facilitated if data can be parsed into an E61 Time Primitive. </rdfs:comment>
        <rdfs:label xml:lang="en">Time-Span</rdfs:label>
        <skos:notation rdf:datatype="http://www.w3.org/2001/XMLSchema#string">E52</skos:notation>
    </owl:Class>
    


    <!-- http://www.cidoc-crm.org/cidoc-crm/E53 -->

    <owl:Class rdf:about="http://www.cidoc-crm.org/cidoc-crm/E53">
        <rdfs:subClassOf rdf:resource="http://www.cidoc-crm.org/cidoc-crm/E1"/>
        <rdfs:comment rdf:datatype="http://www.w3.org/2001/XMLSchema#string">This class comprises extents in space, in particular on the surface of the earth, in the pure sense of physics: independent from
            temporal phenomena and matter. The instances of E53 Place are usually determined by reference to the position of “immobile” objects such
            as buildings, cities, mountains, rivers, or dedicated geodetic marks. A Place can be determined by combining a frame of reference and a
            location with respect to this frame. It may be identified by one or more instances of E44 Place Appellation. It is sometimes argued that
            instances of E53 Place are best identified by global coordinates or absolute reference systems. However, relative references are often
            more relevant in the context of cultural documentation and tend to be more precise. In particular, we are often interested in position in
            relation to large, mobile objects, such as ships. For example, the Place at which Nelson died is known with reference to a large mobile
            object – H.M.S Victory. A resolution of this Place in terms of absolute coordinates would require knowledge of the movements of the vessel
            and the precise time of death, either of which may be revised, and the result would lack historical and cultural relevance. Any object can
            serve as a frame of reference for E53 Place determination. The model foresees the notion of a &quot;section&quot; of an E19 Physical Object as a
            valid E53 Place determination.</rdfs:comment>
        <rdfs:label xml:lang="en">Place</rdfs:label>
        <skos:notation rdf:datatype="http://www.w3.org/2001/XMLSchema#string">E53</skos:notation>
    </owl:Class>
    


    <!-- http://www.cidoc-crm.org/cidoc-crm/E54 -->

    <owl:Class rdf:about="http://www.cidoc-crm.org/cidoc-crm/E54">
        <rdfs:subClassOf rdf:resource="http://www.cidoc-crm.org/cidoc-crm/E1"/>
        <rdfs:comment rdf:datatype="http://www.w3.org/2001/XMLSchema#string">This class comprises quantifiable properties that can be measured by some calibrated means and can be approximated by values, i.e.
            points or regions in a mathematical or conceptual space, such as natural or real numbers, RGB values etc. An instance of E54 Dimension
            represents the true quantity, independent from its numerical approximation, e.g. in inches or in cm. The properties of the class E54
            Dimension allow for expressing the numerical approximation of the values of an instance of E54 Dimension. If the true values belong to a
            non-discrete space, such as spatial distances, it is recommended to record them as approximations by intervals or regions of indeterminacy
            enclosing the assumed true values. For instance, a length of 5 cm may be recorded as 4.5-5.5 cm, according to the precision of the
            respective observation. Note, that interoperability of values described in different units depends critically on the representation as
            value regions. Numerical approximations in archaic instances of E58 Measurement Unit used in historical records should be preserved.
            Equivalents corresponding to current knowledge should be recorded as additional instances of E54 Dimension as appropriate. </rdfs:comment>
        <rdfs:label xml:lang="en">Dimension</rdfs:label>
        <skos:notation rdf:datatype="http://www.w3.org/2001/XMLSchema#string">E54</skos:notation>
    </owl:Class>
    


    <!-- http://www.cidoc-crm.org/cidoc-crm/E55 -->

    <owl:Class rdf:about="http://www.cidoc-crm.org/cidoc-crm/E55">
        <rdfs:subClassOf rdf:resource="http://www.cidoc-crm.org/cidoc-crm/E28"/>
        <rdfs:comment rdf:datatype="http://www.w3.org/2001/XMLSchema#string">This class comprises concepts denoted by terms from thesauri and controlled vocabularies used to characterize and classify instances
            of CRM classes. Instances of E55 Type represent concepts in contrast to instances of E41 Appellation which are used to name instances of
            CRM classes. E55 Type is the CRM’s interface to domain specific ontologies and thesauri. These can be represented in the CRM as subclasses
            of E55 Type, forming hierarchies of terms, i.e. instances of E55 Type linked via P127 has broader term (has narrower term). Such
            hierarchies may be extended with additional properties. </rdfs:comment>
        <rdfs:label xml:lang="en">Type</rdfs:label>
        <skos:notation rdf:datatype="http://www.w3.org/2001/XMLSchema#string">E55</skos:notation>
    </owl:Class>
    


    <!-- http://www.cidoc-crm.org/cidoc-crm/E56 -->

    <owl:Class rdf:about="http://www.cidoc-crm.org/cidoc-crm/E56">
        <rdfs:subClassOf rdf:resource="http://www.cidoc-crm.org/cidoc-crm/E55"/>
        <rdfs:comment rdf:datatype="http://www.w3.org/2001/XMLSchema#string">This class is a specialization of E55 Type and comprises the natural languages in the sense of concepts. This type is used
            categorically in the model without reference to instances of it, i.e. the Model does not foresee the description of instances of instances
            of E56 Language, e.g.: “instances of Mandarin Chinese”. It is recommended that internationally or nationally agreed codes and terminology
            are used to denote instances of E56 Language, such as those defined in ISO 639:1988. </rdfs:comment>
        <rdfs:label xml:lang="en">Language</rdfs:label>
        <skos:notation rdf:datatype="http://www.w3.org/2001/XMLSchema#string">E56</skos:notation>
    </owl:Class>
    


    <!-- http://www.cidoc-crm.org/cidoc-crm/E57 -->

    <owl:Class rdf:about="http://www.cidoc-crm.org/cidoc-crm/E57">
        <rdfs:subClassOf rdf:resource="http://www.cidoc-crm.org/cidoc-crm/E55"/>
        <rdfs:comment rdf:datatype="http://www.w3.org/2001/XMLSchema#string">This class is a specialization of E55 Type and comprises the concepts of materials. Instances of E57 Material may denote properties
            of matter before its use, during its use, and as incorporated in an object, such as ultramarine powder, tempera paste, reinforced
            concrete. Discrete pieces of raw-materials kept in museums, such as bricks, sheets of fabric, pieces of metal, should be modelled
            individually in the same way as other objects. Discrete used or processed pieces, such as the stones from Nefer Titi&apos;s temple, should be
            modelled as parts (cf. P46 is composed of). This type is used categorically in the model without reference to instances of it, i.e. the
            Model does not foresee the description of instances of instances of E57 Material, e.g.: “instances of gold”. It is recommended that
            internationally or nationally agreed codes and terminology are used.</rdfs:comment>
        <rdfs:label xml:lang="en">Material</rdfs:label>
        <skos:notation rdf:datatype="http://www.w3.org/2001/XMLSchema#string">E57</skos:notation>
    </owl:Class>
    


    <!-- http://www.cidoc-crm.org/cidoc-crm/E58 -->

    <owl:Class rdf:about="http://www.cidoc-crm.org/cidoc-crm/E58">
        <rdfs:subClassOf rdf:resource="http://www.cidoc-crm.org/cidoc-crm/E55"/>
        <rdfs:comment rdf:datatype="http://www.w3.org/2001/XMLSchema#string">This class is a specialization of E55 Type and comprises the types of measurement units: feet, inches, centimetres, litres, lumens, etc. This type is used categorically in the model without reference to instances of it, i.e. the Model does not foresee the description of instances of instances of E58 Measurement Unit, e.g.: “instances of cm”. Système International (SI) units or internationally recognized non-SI terms should be used whenever possible. (ISO 1000:1992). Archaic Measurement Units used in historical records should be preserved.</rdfs:comment>
        <rdfs:label xml:lang="en">Measurement Unit</rdfs:label>
        <skos:notation rdf:datatype="http://www.w3.org/2001/XMLSchema#string">E58</skos:notation>
    </owl:Class>
    


    <!-- http://www.cidoc-crm.org/cidoc-crm/E59 -->

    <owl:Class rdf:about="http://www.cidoc-crm.org/cidoc-crm/E59">
        <rdfs:comment rdf:datatype="http://www.w3.org/2001/XMLSchema#string">This class comprises primitive values used as documentation elements, which are not further
elaborated upon within the model.
As such they are not considered as elements within our universe of discourse. No specific
implementation recommendations are made. It is recommended that the primitive value system
from the implementation platform be used to substitute for this class and its subclasses.</rdfs:comment>
        <rdfs:label xml:lang="en">Primitive Value</rdfs:label>
        <skos:notation rdf:datatype="http://www.w3.org/2001/XMLSchema#string">E59</skos:notation>
    </owl:Class>
    


    <!-- http://www.cidoc-crm.org/cidoc-crm/E6 -->

    <owl:Class rdf:about="http://www.cidoc-crm.org/cidoc-crm/E6">
        <rdfs:subClassOf rdf:resource="http://www.cidoc-crm.org/cidoc-crm/E64"/>
        <rdfs:comment rdf:datatype="http://www.w3.org/2001/XMLSchema#string">This class comprises events that destroy one or more instances of E18 Physical Thing such that they lose their identity as the
            subjects of documentation. Some destruction events are intentional, while others are independent of human activity. Intentional
            destruction may be documented by classifying the event as both an E6 Destruction and E7 Activity. The decision to document an object as
            destroyed, transformed or modified is context sensitive: 1. If the matter remaining from the destruction is not documented, the event is
            modelled solely as E6 Destruction. 2. An event should also be documented using E81 Transformation if it results in the destruction of one
            or more objects and the simultaneous production of others using parts or material from the original. In this case, the new items have
            separate identities. Matter is preserved, but identity is not. 3. When the initial identity of the changed instance of E18 Physical Thing
            is preserved, the event should be documented as E11 Modification. </rdfs:comment>
        <rdfs:label xml:lang="en">Destruction</rdfs:label>
        <skos:notation rdf:datatype="http://www.w3.org/2001/XMLSchema#string">E6</skos:notation>
    </owl:Class>
    


    <!-- http://www.cidoc-crm.org/cidoc-crm/E60 -->

    <owl:Class rdf:about="http://www.cidoc-crm.org/cidoc-crm/E60">
        <rdfs:subClassOf rdf:resource="http://www.cidoc-crm.org/cidoc-crm/E59"/>
        <rdfs:comment rdf:datatype="http://www.w3.org/2001/XMLSchema#string">This class comprises any encoding of computable (algebraic) values such as integers, real numbers,
complex numbers, vectors, tensors etc., including intervals of these values to express limited precision.
Numbers are fundamentally distinct from identifiers in continua, such as instances of E50 Date and E47 Spatial Coordinate, even though their encoding may be similar. Instances of E60 Number can be
combined with each other in algebraic operations to yield other instances of E60 Number, e.g., 1+1=2. Identifiers in continua may be combined with numbers expressing distances to yield new identifiers, e.g., 1924-01-31 + 2 days = 1924-02-02. Cf. E54 Dimension</rdfs:comment>
        <rdfs:label xml:lang="en">Number</rdfs:label>
        <skos:notation rdf:datatype="http://www.w3.org/2001/XMLSchema#string">E60</skos:notation>
    </owl:Class>
    


    <!-- http://www.cidoc-crm.org/cidoc-crm/E61 -->

    <owl:Class rdf:about="http://www.cidoc-crm.org/cidoc-crm/E61">
        <rdfs:subClassOf rdf:resource="http://www.cidoc-crm.org/cidoc-crm/E59"/>
        <rdfs:comment rdf:datatype="http://www.w3.org/2001/XMLSchema#string">This class comprises instances of E59 Primitive Value for time that should be implemented with appropriate validation, precision and interval logic to express date ranges relevant to cultural documentation. 
 
E61 Time Primitive is not further elaborated upon within the model.</rdfs:comment>
        <rdfs:label xml:lang="en">Time Primitive</rdfs:label>
        <skos:notation rdf:datatype="http://www.w3.org/2001/XMLSchema#string">E61</skos:notation>
    </owl:Class>
    


    <!-- http://www.cidoc-crm.org/cidoc-crm/E62 -->

    <owl:Class rdf:about="http://www.cidoc-crm.org/cidoc-crm/E62">
        <rdfs:subClassOf rdf:resource="http://www.cidoc-crm.org/cidoc-crm/E59"/>
        <rdfs:comment rdf:datatype="http://www.w3.org/2001/XMLSchema#string">This class comprises the instances of E59 Primitive Values used for documentation such as free text
strings, bitmaps, vector graphics, etc.</rdfs:comment>
        <rdfs:label xml:lang="en">String</rdfs:label>
        <skos:notation rdf:datatype="http://www.w3.org/2001/XMLSchema#string">E62</skos:notation>
    </owl:Class>
    


    <!-- http://www.cidoc-crm.org/cidoc-crm/E63 -->

    <owl:Class rdf:about="http://www.cidoc-crm.org/cidoc-crm/E63">
        <rdfs:subClassOf rdf:resource="http://www.cidoc-crm.org/cidoc-crm/E5"/>
        <rdfs:comment rdf:datatype="http://www.w3.org/2001/XMLSchema#string">This class comprises events that bring into existence any E77 Persistent Item. It may be used for temporal reasoning about things
            (intellectual products, physical items, groups of people, living beings) beginning to exist; it serves as a hook for determination of a
            terminus post quem and ante quem. </rdfs:comment>
        <rdfs:label xml:lang="en">Beginning of Existence</rdfs:label>
        <skos:notation rdf:datatype="http://www.w3.org/2001/XMLSchema#string">E63</skos:notation>
    </owl:Class>
    


    <!-- http://www.cidoc-crm.org/cidoc-crm/E64 -->

    <owl:Class rdf:about="http://www.cidoc-crm.org/cidoc-crm/E64">
        <rdfs:subClassOf rdf:resource="http://www.cidoc-crm.org/cidoc-crm/E5"/>
        <rdfs:comment rdf:datatype="http://www.w3.org/2001/XMLSchema#string">This class comprises events that end the existence of any E77 Persistent Item. It may be used for temporal reasoning about things
            (physical items, groups of people, living beings) ceasing to exist; it serves as a hook for determination of a terminus postquem and
            antequem. In cases where substance from a Persistent Item continues to exist in a new form, the process would be documented by E81
            Transformation. </rdfs:comment>
        <rdfs:label xml:lang="en">End of Existence</rdfs:label>
        <skos:notation rdf:datatype="http://www.w3.org/2001/XMLSchema#string">E64</skos:notation>
    </owl:Class>
    


    <!-- http://www.cidoc-crm.org/cidoc-crm/E65 -->

    <owl:Class rdf:about="http://www.cidoc-crm.org/cidoc-crm/E65">
        <rdfs:subClassOf rdf:resource="http://www.cidoc-crm.org/cidoc-crm/E63"/>
        <rdfs:subClassOf rdf:resource="http://www.cidoc-crm.org/cidoc-crm/E7"/>
        <rdfs:comment rdf:datatype="http://www.w3.org/2001/XMLSchema#string">This class comprises events that result in the creation of conceptual items or immaterial products, such as legends, poems, texts,
            music, images, movies, laws, types etc. </rdfs:comment>
        <rdfs:label xml:lang="en">Creation</rdfs:label>
        <skos:notation rdf:datatype="http://www.w3.org/2001/XMLSchema#string">E65</skos:notation>
    </owl:Class>
    


    <!-- http://www.cidoc-crm.org/cidoc-crm/E66 -->

    <owl:Class rdf:about="http://www.cidoc-crm.org/cidoc-crm/E66">
        <rdfs:subClassOf rdf:resource="http://www.cidoc-crm.org/cidoc-crm/E63"/>
        <rdfs:subClassOf rdf:resource="http://www.cidoc-crm.org/cidoc-crm/E7"/>
        <rdfs:comment rdf:datatype="http://www.w3.org/2001/XMLSchema#string">This class comprises events that result in the formation of a formal or informal E74 Group of people, such as a club, society,
            association, corporation or nation. E66 Formation does not include the arbitrary aggregation of people who do not act as a collective. The
            formation of an instance of E74 Group does not require that the group is populated with members at the time of formation. In order to
            express the joining of members at the time of formation, the respective activity should be simultaneously an instance of both E66
            Formation and E85 Joining. </rdfs:comment>
        <rdfs:label xml:lang="en">Formation</rdfs:label>
        <skos:notation rdf:datatype="http://www.w3.org/2001/XMLSchema#string">E66</skos:notation>
    </owl:Class>
    


    <!-- http://www.cidoc-crm.org/cidoc-crm/E67 -->

    <owl:Class rdf:about="http://www.cidoc-crm.org/cidoc-crm/E67">
        <rdfs:subClassOf rdf:resource="http://www.cidoc-crm.org/cidoc-crm/E63"/>
        <rdfs:comment rdf:datatype="http://www.w3.org/2001/XMLSchema#string">This class comprises the births of human beings. E67 Birth is a biological event focussing on the context of people coming into life.
            (E63 Beginning of Existence comprises the coming into life of any living beings). Twins, triplets etc. are brought into life by the same
            E67 Birth event. The introduction of the E67 Birth event as a documentation element allows the description of a range of family
            relationships in a simple model. Suitable extensions may describe more details and the complexity of motherhood with the intervention of
            modern medicine. In this model, the biological father is not seen as a necessary participant in the E67 Birth event. </rdfs:comment>
        <rdfs:label xml:lang="en">Birth</rdfs:label>
        <skos:notation rdf:datatype="http://www.w3.org/2001/XMLSchema#string">E67</skos:notation>
    </owl:Class>
    


    <!-- http://www.cidoc-crm.org/cidoc-crm/E68 -->

    <owl:Class rdf:about="http://www.cidoc-crm.org/cidoc-crm/E68">
        <rdfs:subClassOf rdf:resource="http://www.cidoc-crm.org/cidoc-crm/E64"/>
        <rdfs:comment rdf:datatype="http://www.w3.org/2001/XMLSchema#string">This class comprises the events that result in the formal or informal termination of an E74 Group of people. If the dissolution was
            deliberate, the Dissolution event should also be instantiated as an E7 Activity. </rdfs:comment>
        <rdfs:label xml:lang="en">Dissolution</rdfs:label>
        <skos:notation rdf:datatype="http://www.w3.org/2001/XMLSchema#string">E68</skos:notation>
    </owl:Class>
    


    <!-- http://www.cidoc-crm.org/cidoc-crm/E69 -->

    <owl:Class rdf:about="http://www.cidoc-crm.org/cidoc-crm/E69">
        <rdfs:subClassOf rdf:resource="http://www.cidoc-crm.org/cidoc-crm/E64"/>
        <rdfs:comment rdf:datatype="http://www.w3.org/2001/XMLSchema#string">This class comprises the deaths of human beings. If a person is killed, their death should be instantiated as E69 Death and as E7
            Activity. The death or perishing of other living beings should be documented using E64 End of Existence. </rdfs:comment>
        <rdfs:label xml:lang="en">Death</rdfs:label>
        <skos:notation rdf:datatype="http://www.w3.org/2001/XMLSchema#string">E69</skos:notation>
    </owl:Class>
    


    <!-- http://www.cidoc-crm.org/cidoc-crm/E7 -->

    <owl:Class rdf:about="http://www.cidoc-crm.org/cidoc-crm/E7">
        <rdfs:subClassOf rdf:resource="http://www.cidoc-crm.org/cidoc-crm/E5"/>
        <rdfs:comment rdf:datatype="http://www.w3.org/2001/XMLSchema#string">This class comprises actions intentionally carried out by instances of E39 Actor that result in changes of state in the cultural,
            social, or physical systems documented. This notion includes complex, composite and long-lasting actions such as the building of a
            settlement or a war, as well as simple, short-lived actions such as the opening of a door. </rdfs:comment>
        <rdfs:label xml:lang="en">Activity</rdfs:label>
        <skos:notation rdf:datatype="http://www.w3.org/2001/XMLSchema#string">E7</skos:notation>
    </owl:Class>
    


    <!-- http://www.cidoc-crm.org/cidoc-crm/E70 -->

    <owl:Class rdf:about="http://www.cidoc-crm.org/cidoc-crm/E70">
        <rdfs:subClassOf rdf:resource="http://www.cidoc-crm.org/cidoc-crm/E77"/>
        <rdfs:comment rdf:datatype="http://www.w3.org/2001/XMLSchema#string">This general class comprises discrete, identifiable, instances of E77 Persistent Item that are documented as single units, that
            either consist of matter or depend on being carried by matter and are characterized by relative stability. They may be intellectual
            products or physical things. They may for instance have a solid physical form, an electronic encoding, or they may be a logical concept or
            structure. </rdfs:comment>
        <rdfs:label xml:lang="en">Thing</rdfs:label>
        <skos:notation rdf:datatype="http://www.w3.org/2001/XMLSchema#string">E70</skos:notation>
    </owl:Class>
    


    <!-- http://www.cidoc-crm.org/cidoc-crm/E71 -->

    <owl:Class rdf:about="http://www.cidoc-crm.org/cidoc-crm/E71">
        <rdfs:subClassOf rdf:resource="http://www.cidoc-crm.org/cidoc-crm/E70"/>
        <rdfs:comment rdf:datatype="http://www.w3.org/2001/XMLSchema#string">This class comprises discrete, identifiable man-made items that are documented as single units. These items are either intellectual
            products or man-made physical things, and are characterized by relative stability. They may for instance have a solid physical form, an
            electronic encoding, or they may be logical concepts or structures. </rdfs:comment>
        <rdfs:label xml:lang="en">Man-Made Thing</rdfs:label>
        <skos:notation rdf:datatype="http://www.w3.org/2001/XMLSchema#string">E71</skos:notation>
    </owl:Class>
    


    <!-- http://www.cidoc-crm.org/cidoc-crm/E72 -->

    <owl:Class rdf:about="http://www.cidoc-crm.org/cidoc-crm/E72">
        <rdfs:subClassOf rdf:resource="http://www.cidoc-crm.org/cidoc-crm/E70"/>
        <rdfs:comment rdf:datatype="http://www.w3.org/2001/XMLSchema#string">This class comprises those material or immaterial items to which instances of E30 Right, such as the right of ownership or use, can
            be applied. This is true for all E18 Physical Thing. In the case of instances of E28 Conceptual Object, however, the identity of the E28
            Conceptual Object or the method of its use may be too ambiguous to reliably establish instances of E30 Right, as in the case of taxa and
            inspirations. Ownership of corporations is currently regarded as out of scope of the CRM. </rdfs:comment>
        <rdfs:label xml:lang="en">Legal Object</rdfs:label>
        <skos:notation rdf:datatype="http://www.w3.org/2001/XMLSchema#string">E72</skos:notation>
    </owl:Class>
    


    <!-- http://www.cidoc-crm.org/cidoc-crm/E73 -->

    <owl:Class rdf:about="http://www.cidoc-crm.org/cidoc-crm/E73">
        <rdfs:subClassOf rdf:resource="http://www.cidoc-crm.org/cidoc-crm/E89"/>
        <rdfs:subClassOf rdf:resource="http://www.cidoc-crm.org/cidoc-crm/E90"/>
        <rdfs:comment rdf:datatype="http://www.w3.org/2001/XMLSchema#string">This class comprises identifiable immaterial items, such as a poems, jokes, data sets, images, texts, multimedia objects, procedural
            prescriptions, computer program code, algorithm or mathematical formulae, that have an objectively recognizable structure and are
            documented as single units. The encoding structure known as a &quot;named graph&quot; also falls under this class, so that each &quot;named graph&quot; is an
            instance of an E73 Information Object. An E73 Information Object does not depend on a specific physical carrier, which can include human
            memory, and it can exist on one or more carriers simultaneously. Instances of E73 Information Object of a linguistic nature should be
            declared as instances of the E33 Linguistic Object subclass. Instances of E73 Information Object of a documentary nature should be
            declared as instances of the E31 Document subclass. Conceptual items such as types and classes are not instances of E73 Information
            Object, nor are ideas without a reproducible expression. </rdfs:comment>
        <rdfs:label xml:lang="en">Information Object</rdfs:label>
        <skos:notation rdf:datatype="http://www.w3.org/2001/XMLSchema#string">E73</skos:notation>
    </owl:Class>
    


    <!-- http://www.cidoc-crm.org/cidoc-crm/E74 -->

    <owl:Class rdf:about="http://www.cidoc-crm.org/cidoc-crm/E74">
        <rdfs:subClassOf rdf:resource="http://www.cidoc-crm.org/cidoc-crm/E39"/>
        <rdfs:comment rdf:datatype="http://www.w3.org/2001/XMLSchema#string">This class comprises any gatherings or organizations of E39 Actors that act collectively or in a similar way due to any form of
            unifying relationship. In the wider sense this class also comprises official positions which used to be regarded in certain contexts as
            one actor, independent of the current holder of the office, such as the president of a country. In such cases, it may happen that the
            Group never had more than one member. A joint pseudonym (i.e., a name that seems indicative of an individual but that is actually used as
            a persona by two or more people) is a particular case of E74 Group. A gathering of people becomes an E74 Group when it exhibits
            organizational characteristics usually typified by a set of ideas or beliefs held in common, or actions performed together. These might be
            communication, creating some common artifact, a common purpose such as study, worship, business, sports, etc. Nationality can be modeled
            as membership in an E74 Group (cf. HumanML markup). Married couples and other concepts of family are regarded as particular examples of
            E74 Group. </rdfs:comment>
        <rdfs:label xml:lang="en">Group</rdfs:label>
        <skos:notation rdf:datatype="http://www.w3.org/2001/XMLSchema#string">E74</skos:notation>
    </owl:Class>
    


    <!-- http://www.cidoc-crm.org/cidoc-crm/E75 -->

    <owl:Class rdf:about="http://www.cidoc-crm.org/cidoc-crm/E75">
        <rdfs:subClassOf rdf:resource="http://www.cidoc-crm.org/cidoc-crm/E41"/>
        <rdfs:comment rdf:datatype="http://www.w3.org/2001/XMLSchema#string">This class comprises appellations that are by their form or syntax specific to identifying instances of E28 Conceptual Object, such
            as intellectual products, standardized patterns etc.</rdfs:comment>
        <rdfs:label xml:lang="en">Conceptual Object Appellation</rdfs:label>
        <skos:notation rdf:datatype="http://www.w3.org/2001/XMLSchema#string">E75</skos:notation>
    </owl:Class>
    


    <!-- http://www.cidoc-crm.org/cidoc-crm/E77 -->

    <owl:Class rdf:about="http://www.cidoc-crm.org/cidoc-crm/E77">
        <rdfs:subClassOf rdf:resource="http://www.cidoc-crm.org/cidoc-crm/E1"/>
        <rdfs:comment rdf:datatype="http://www.w3.org/2001/XMLSchema#string">This class comprises items that have a persistent identity, sometimes known as “endurants” in philosophy. They can be repeatedly
            recognized within the duration of their existence by identity criteria rather than by continuity or observation. Persistent Items can be
            either physical entities, such as people, animals or things, or conceptual entities such as ideas, concepts, products of the imagination
            or common names. The criteria that determine the identity of an item are often difficult to establish -; the decision depends largely on
            the judgement of the observer. For example, a building is regarded as no longer existing if it is dismantled and the materials reused in a
            different configuration. On the other hand, human beings go through radical and profound changes during their life-span, affecting both
            material composition and form, yet preserve their identity by other criteria. Similarly, inanimate objects may be subject to exchange of
            parts and matter. The class E77 Persistent Item does not take any position about the nature of the applicable identity criteria and if
            actual knowledge about identity of an instance of this class exists. There may be cases, where the identity of an E77 Persistent Item is
            not decidable by a certain state of knowledge. The main classes of objects that fall outside the scope the E77 Persistent Item class are
            temporal objects such as periods, events and acts, and descriptive properties. </rdfs:comment>
        <rdfs:label xml:lang="en">Persistent Item</rdfs:label>
        <skos:notation rdf:datatype="http://www.w3.org/2001/XMLSchema#string">E77</skos:notation>
    </owl:Class>
    


    <!-- http://www.cidoc-crm.org/cidoc-crm/E78 -->

    <owl:Class rdf:about="http://www.cidoc-crm.org/cidoc-crm/E78">
        <rdfs:subClassOf rdf:resource="http://www.cidoc-crm.org/cidoc-crm/E24"/>
        <rdfs:comment rdf:datatype="http://www.w3.org/2001/XMLSchema#string">This class comprises aggregations of instances of E18 Physical Thing that are assembled and maintained (&quot;curated&quot; and &quot;preserved&quot;, in
            museological terminology) by one or more instances of E39 Actor over time for a specific purpose and audience, and according to a
            particular collection development plan. Items may be added or removed from an E78 Collection in pursuit of this plan. This class should
            not be confused with the E39 Actor maintaining the E78 Collection often referred to with the name of the E78 Collection (e.g. “The Wallace
            Collection decided…”). Collective objects in the general sense, like a tomb full of gifts, a folder with stamps or a set of chessmen,
            should be documented as instances of E19 Physical Object, and not as instances of E78 Collection. This is because they form wholes either
            because they are physically bound together or because they are kept together for their functionality. </rdfs:comment>
        <rdfs:label xml:lang="en">Collection</rdfs:label>
        <skos:notation rdf:datatype="http://www.w3.org/2001/XMLSchema#string">E78</skos:notation>
    </owl:Class>
    


    <!-- http://www.cidoc-crm.org/cidoc-crm/E79 -->

    <owl:Class rdf:about="http://www.cidoc-crm.org/cidoc-crm/E79">
        <rdfs:subClassOf rdf:resource="http://www.cidoc-crm.org/cidoc-crm/E11"/>
        <rdfs:comment rdf:datatype="http://www.w3.org/2001/XMLSchema#string">This class comprises activities that result in an instance of E24 Physical Man-Made Thing being increased, enlarged or augmented by
            the addition of a part. Typical scenarios include the attachment of an accessory, the integration of a component, the addition of an
            element to an aggregate object, or the accessioning of an object into a curated E78 Collection. Objects to which parts are added are, by
            definition, man-made, since the addition of a part implies a human activity. Following the addition of parts, the resulting man-made
            assemblages are treated objectively as single identifiable wholes, made up of constituent or component parts bound together either
            physically (for example the engine becoming a part of the car), or by sharing a common purpose (such as the 32 chess pieces that make up a
            chess set). This class of activities forms a basis for reasoning about the history and continuity of identity of objects that are
            integrated into other objects over time, such as precious gemstones being repeatedly incorporated into different items of jewellery, or
            cultural artifacts being added to different museum instances of E78 Collection over their lifespan. </rdfs:comment>
        <rdfs:label xml:lang="en">Part Addition</rdfs:label>
        <skos:notation rdf:datatype="http://www.w3.org/2001/XMLSchema#string">E79</skos:notation>
    </owl:Class>
    


    <!-- http://www.cidoc-crm.org/cidoc-crm/E8 -->

    <owl:Class rdf:about="http://www.cidoc-crm.org/cidoc-crm/E8">
        <rdfs:subClassOf rdf:resource="http://www.cidoc-crm.org/cidoc-crm/E7"/>
        <rdfs:comment rdf:datatype="http://www.w3.org/2001/XMLSchema#string">This class comprises transfers of legal ownership from one or more instances of E39 Actor to one or more other instances of E39
            Actor. The class also applies to the establishment or loss of ownership of instances of E18 Physical Thing. It does not, however, imply
            changes of any other kinds of right. The recording of the donor and/or recipient is optional. It is possible that in an instance of E8
            Acquisition there is either no donor or no recipient. Depending on the circumstances, it may describe: 1) the beginning of ownership 
2) the end of ownership  3) the transfer of ownership
 4) the acquisition from an unknown source 
5) the loss of title due to destruction of the item It may also describe events where a collector appropriates legal title, for example by annexation or field collection. The
            interpretation of the museum notion of &quot;accession&quot; differs between institutions. The CRM therefore models legal ownership (E8 Acquisition)
            and physical custody (E10 Transfer of Custody) separately. Institutions will then model their specific notions of accession and
            deaccession as combinations of these.</rdfs:comment>
        <rdfs:label xml:lang="en">Acquisition</rdfs:label>
        <skos:notation rdf:datatype="http://www.w3.org/2001/XMLSchema#string">E8</skos:notation>
    </owl:Class>
    


    <!-- http://www.cidoc-crm.org/cidoc-crm/E80 -->

    <owl:Class rdf:about="http://www.cidoc-crm.org/cidoc-crm/E80">
        <rdfs:subClassOf rdf:resource="http://www.cidoc-crm.org/cidoc-crm/E11"/>
        <rdfs:comment rdf:datatype="http://www.w3.org/2001/XMLSchema#string">This class comprises the activities that result in an instance of E18 Physical Thing being decreased by the removal of a part.
            Typical scenarios include the detachment of an accessory, the removal of a component or part of a composite object, or the deaccessioning
            of an object from a curated E78 Collection. If the E80 Part Removal results in the total decomposition of the original object into pieces,
            such that the whole ceases to exist, the activity should instead be modelled as an E81 Transformation, i.e. a simultaneous destruction and
            production. In cases where the part removed has no discernible identity prior to its removal but does have an identity subsequent to its
            removal, the activity should be regarded as both E80 Part Removal and E12 Production. This class of activities forms a basis for reasoning
            about the history, and continuity of identity over time, of objects that are removed from other objects, such as precious gemstones being
            extracted from different items of jewelry, or cultural artifacts being deaccessioned from different museum collections over their
            lifespan. </rdfs:comment>
        <rdfs:label xml:lang="en">Part Removal</rdfs:label>
        <skos:notation rdf:datatype="http://www.w3.org/2001/XMLSchema#string">E80</skos:notation>
    </owl:Class>
    


    <!-- http://www.cidoc-crm.org/cidoc-crm/E81 -->

    <owl:Class rdf:about="http://www.cidoc-crm.org/cidoc-crm/E81">
        <rdfs:subClassOf rdf:resource="http://www.cidoc-crm.org/cidoc-crm/E63"/>
        <rdfs:subClassOf rdf:resource="http://www.cidoc-crm.org/cidoc-crm/E64"/>
        <rdfs:comment rdf:datatype="http://www.w3.org/2001/XMLSchema#string">This class comprises the events that result in the simultaneous destruction of one or more than one E77 Persistent Item and the
            creation of one or more than one E77 Persistent Item that preserves recognizable substance from the first one(s) but has fundamentally
            different nature and identity. Although the old and the new instances of E77 Persistent Item are treated as discrete entities having
            separate, unique identities, they are causally connected through the E81 Transformation; the destruction of the old E77 Persistent Item(s)
            directly causes the creation of the new one(s) using or preserving some relevant substance. Instances of E81 Transformation are therefore
            distinct from re-classifications (documented using E17 Type Assignment) or modifications (documented using E11 Modification) of objects
            that do not fundamentally change their nature or identity. Characteristic cases are reconstructions and repurposing of historical
            buildings or ruins, fires leaving buildings in ruins, taxidermy of specimen in natural history and the reorganization of a corporate body
            into a new one. </rdfs:comment>
        <rdfs:label xml:lang="en">Transformation</rdfs:label>
        <skos:notation rdf:datatype="http://www.w3.org/2001/XMLSchema#string">E81</skos:notation>
    </owl:Class>
    


    <!-- http://www.cidoc-crm.org/cidoc-crm/E82 -->

    <owl:Class rdf:about="http://www.cidoc-crm.org/cidoc-crm/E82">
        <rdfs:subClassOf rdf:resource="http://www.cidoc-crm.org/cidoc-crm/E41"/>
        <rdfs:comment rdf:datatype="http://www.w3.org/2001/XMLSchema#string">This class comprises any sort of name, number, code or symbol characteristically used to identify an E39 Actor. An E39 Actor will
            typically have more than one E82 Actor Appellation, and instances of E82 Actor Appellation in turn may have alternative representations.
            The distinction between corporate and personal names, which is particularly important in library applications, should be made by
            explicitly linking the E82 Actor Appellation to an instance of either E21 Person or E74 Group/E40 Legal Body. If this is not possible, the
            distinction can be made through the use of the P2 has type mechanism. </rdfs:comment>
        <rdfs:label xml:lang="en">Actor Appellation</rdfs:label>
        <skos:notation rdf:datatype="http://www.w3.org/2001/XMLSchema#string">E82</skos:notation>
    </owl:Class>
    


    <!-- http://www.cidoc-crm.org/cidoc-crm/E83 -->

    <owl:Class rdf:about="http://www.cidoc-crm.org/cidoc-crm/E83">
        <rdfs:subClassOf rdf:resource="http://www.cidoc-crm.org/cidoc-crm/E65"/>
        <rdfs:comment rdf:datatype="http://www.w3.org/2001/XMLSchema#string">This class comprises activities formally defining new types of items. It is typically a rigorous scholarly or scientific process that
            ensures a type is exhaustively described and appropriately named. In some cases, particularly in archaeology and the life sciences, E83
            Type Creation requires the identification of an exemplary specimen and the publication of the type definition in an appropriate scholarly
            forum. The activity of E83 Type Creation is central to research in the life sciences, where a type would be referred to as a “taxon,” the
            type description as a “protologue,” and the exemplary specimens as “orgininal element” or “holotype”. </rdfs:comment>
        <rdfs:label xml:lang="en">Type Creation</rdfs:label>
        <skos:notation rdf:datatype="http://www.w3.org/2001/XMLSchema#string">E83</skos:notation>
    </owl:Class>
    


    <!-- http://www.cidoc-crm.org/cidoc-crm/E84 -->

    <owl:Class rdf:about="http://www.cidoc-crm.org/cidoc-crm/E84">
        <rdfs:subClassOf rdf:resource="http://www.cidoc-crm.org/cidoc-crm/E22"/>
        <rdfs:comment rdf:datatype="http://www.w3.org/2001/XMLSchema#string">This class comprises all instances of E22 Man-Made Object that are explicitly designed to act as persistent physical carriers for
            instances of E73 Information Object. An E84 Information Carrier may or may not contain information, e.g., a diskette. Note that any E18
            Physical Thing may carry information, such as an E34 Inscription. However, unless it was specifically designed for this purpose, it is not
            an Information Carrier. Therefore the property P128 carries (is carried by) applies to E18 Physical Thing in general. </rdfs:comment>
        <rdfs:label xml:lang="en">Information Carrier</rdfs:label>
        <skos:notation rdf:datatype="http://www.w3.org/2001/XMLSchema#string">E84</skos:notation>
    </owl:Class>
    


    <!-- http://www.cidoc-crm.org/cidoc-crm/E85 -->

    <owl:Class rdf:about="http://www.cidoc-crm.org/cidoc-crm/E85">
        <rdfs:subClassOf rdf:resource="http://www.cidoc-crm.org/cidoc-crm/E7"/>
        <rdfs:comment rdf:datatype="http://www.w3.org/2001/XMLSchema#string">This class comprises the activities that result in an instance of E39 Actor becoming a member of an instance of E74 Group. This class
            does not imply initiative by either party. It may be the initiative of a third party. Typical scenarios include becoming a member of a
            social organisation, becoming employee of a company, marriage, the adoption of a child by a family and the inauguration of somebody into
            an official position. </rdfs:comment>
        <rdfs:label xml:lang="en">Joining</rdfs:label>
        <skos:notation rdf:datatype="http://www.w3.org/2001/XMLSchema#string">E85</skos:notation>
    </owl:Class>
    


    <!-- http://www.cidoc-crm.org/cidoc-crm/E86 -->

    <owl:Class rdf:about="http://www.cidoc-crm.org/cidoc-crm/E86">
        <rdfs:subClassOf rdf:resource="http://www.cidoc-crm.org/cidoc-crm/E7"/>
        <rdfs:comment rdf:datatype="http://www.w3.org/2001/XMLSchema#string">This class comprises the activities that result in an instance of E39 Actor to be disassociated from an instance of E74 Group. This
            class does not imply initiative by either party. It may be the initiative of a third party. Typical scenarios include the termination of
            membership in a social organisation, ending the employment at a company, divorce, and the end of tenure of somebody in an official
            position.</rdfs:comment>
        <rdfs:label xml:lang="en">Leaving</rdfs:label>
        <skos:notation rdf:datatype="http://www.w3.org/2001/XMLSchema#string">E86</skos:notation>
    </owl:Class>
    


    <!-- http://www.cidoc-crm.org/cidoc-crm/E87 -->

    <owl:Class rdf:about="http://www.cidoc-crm.org/cidoc-crm/E87">
        <rdfs:subClassOf rdf:resource="http://www.cidoc-crm.org/cidoc-crm/E7"/>
        <rdfs:comment rdf:datatype="http://www.w3.org/2001/XMLSchema#string">This class comprises the activities that result in the continuity of management and the preservation and evolution of instances of
            E78 Collection, following an implicit or explicit curation plan. It specializes the notion of activity into the curation of a collection
            and allows the history of curation to be recorded. Items are accumulated and organized following criteria like subject, chronological
            period, material type, style of art etc. and can be added or removed from an E78 Collection for a specific purpose and/or audience. The
            initial aggregation of items of a collection is regarded as an instance of E12 Production Event while the activity of evolving, preserving
            and promoting a collection is regarded as an instance of E87 Curation Activity. </rdfs:comment>
        <rdfs:label xml:lang="en">Curation Activity</rdfs:label>
        <skos:notation rdf:datatype="http://www.w3.org/2001/XMLSchema#string">E87</skos:notation>
    </owl:Class>
    


    <!-- http://www.cidoc-crm.org/cidoc-crm/E89 -->

    <owl:Class rdf:about="http://www.cidoc-crm.org/cidoc-crm/E89">
        <rdfs:subClassOf rdf:resource="http://www.cidoc-crm.org/cidoc-crm/E28"/>
        <rdfs:comment rdf:datatype="http://www.w3.org/2001/XMLSchema#string">This class comprises immaterial items, including but not limited to stories, plots, procedural prescriptions, algorithms, laws of
            physics or images that are, or represent in some sense, sets of propositions about real or imaginary things and that are documented as
            single units or serve as topics of discourse. This class also comprises items that are “about” something in the sense of a subject. In the
            wider sense, this class includes expressions of psychological value such as non-figural art and musical themes. However, conceptual items
            such as types and classes are not instances of E89 Propositional Object. This should not be confused with the definition of a type, which
            is indeed an instance of E89 Propositional Object. </rdfs:comment>
        <rdfs:label xml:lang="en">Propositional Object</rdfs:label>
        <skos:notation rdf:datatype="http://www.w3.org/2001/XMLSchema#string">E89</skos:notation>
    </owl:Class>
    


    <!-- http://www.cidoc-crm.org/cidoc-crm/E9 -->

    <owl:Class rdf:about="http://www.cidoc-crm.org/cidoc-crm/E9">
        <rdfs:subClassOf rdf:resource="http://www.cidoc-crm.org/cidoc-crm/E7"/>
        <rdfs:comment rdf:datatype="http://www.w3.org/2001/XMLSchema#string">This class comprises changes of the physical location of the instances of E19 Physical Object. Note, that the class E9 Move inherits
            the property P7 took place at (witnessed): E53 Place. This property should be used to describe the trajectory or a larger area within
            which a move takes place, whereas the properties P26 moved to (was destination of), P27 moved from (was origin of) describe the start and
            end points only. Moves may also be documented to consist of other moves (via P9 consists of (forms part of)), in order to describe
            intermediate stages on a trajectory. In that case, start and end points of the partial moves should match appropriately between each other
            and with the overall event. </rdfs:comment>
        <rdfs:label xml:lang="en">Move</rdfs:label>
        <skos:notation rdf:datatype="http://www.w3.org/2001/XMLSchema#string">E9</skos:notation>
    </owl:Class>
    


    <!-- http://www.cidoc-crm.org/cidoc-crm/E90 -->

    <owl:Class rdf:about="http://www.cidoc-crm.org/cidoc-crm/E90">
        <rdfs:subClassOf rdf:resource="http://www.cidoc-crm.org/cidoc-crm/E28"/>
        <rdfs:subClassOf rdf:resource="http://www.cidoc-crm.org/cidoc-crm/E72"/>
        <rdfs:comment rdf:datatype="http://www.w3.org/2001/XMLSchema#string">This class comprises identifiable symbols and any aggregation of symbols, such as characters, identifiers, traffic signs, emblems,
            texts, data sets, images, musical scores, multimedia objects, computer program code or mathematical formulae that have an objectively
            recognizable structure and that are documented as single units. It includes sets of signs of any nature, which may serve to designate
            something, or to communicate some propositional content. An instance of E90 Symbolic Object does not depend on a specific physical
            carrier, which can include human memory, and it can exist on one or more carriers simultaneously. An instance of E90 Symbolic Object may
            or may not have a specific meaning, for example an arbitrary character string. In some cases, the content of an instance of E90 Symbolic
            Object may completely be represented by a serialized content model, such.. as the property P3 has note allows for describing this content
            model…P3.1 has type: E55 Type to specify the encoding.. </rdfs:comment>
        <rdfs:label xml:lang="en">Symbolic Object</rdfs:label>
        <skos:notation rdf:datatype="http://www.w3.org/2001/XMLSchema#string">E90</skos:notation>
    </owl:Class>
    


    <!-- http://www.cidoc-crm.org/cidoc-crm/E92 -->

    <owl:Class rdf:about="http://www.cidoc-crm.org/cidoc-crm/E92">
        <rdfs:subClassOf rdf:resource="http://www.cidoc-crm.org/cidoc-crm/E1"/>
        <rdfs:comment rdf:datatype="http://www.w3.org/2001/XMLSchema#string">This class comprises 4 dimensional point sets (volumes) in physical spacetime regardless its true geometric form. They may derive
            their identity from being the extent of a material phenomenon or from being the interpretation of an expression defining an extent in
            spacetime. Intersections of instances of E92 Spacetime Volume, Place and Timespan are also regarded as instances of E92 Spacetime Volume.
            An instance of E92 Spacetime Volume is either contiguous or composed of a finite number of contiguous subsets. Its boundaries may be fuzzy
            due to the properties of the phenomena it derives from or due to the limited precision up to which defining expression can be identified
            with a real extent in spacetime. The duration of existence of an instance of a spacetime volume is trivially its projection on time. </rdfs:comment>
        <rdfs:label xml:lang="en">Spacetime Volume</rdfs:label>
        <skos:notation rdf:datatype="http://www.w3.org/2001/XMLSchema#string">E92</skos:notation>
    </owl:Class>
    


    <!-- http://www.cidoc-crm.org/cidoc-crm/E93 -->

    <owl:Class rdf:about="http://www.cidoc-crm.org/cidoc-crm/E93">
        <rdfs:subClassOf rdf:resource="http://www.cidoc-crm.org/cidoc-crm/E92"/>
        <rdfs:comment rdf:datatype="http://www.w3.org/2001/XMLSchema#string">This class comprises instances of E92 Spacetime Volume that result from intersection of instances of E92 Spacetime Volume with an
            instance of E52 Time-Span. The identity of an instance of this class is determined by the identities of the constituing spacetime volume
            and the time-span. This class can be used to define temporal snapshots at a particular time-span, such as the extent of the Roman Empire
            at 33 B.C., or the extent occupied by a museum object at rest in an exhibit. In particular, it can be used to define the spatial
            projection of a spacetime volume during a particular time-span, such as the maximal spatial extent of a flood at some particular hour, or
            all areas covered by the Poland within the 20th century AD. </rdfs:comment>
        <rdfs:label xml:lang="en">Presence</rdfs:label>
        <skos:notation rdf:datatype="http://www.w3.org/2001/XMLSchema#string">E93</skos:notation>
    </owl:Class>
    


    <!-- http://www.cidoc-crm.org/cidoc-crm/E94 -->

    <owl:Class rdf:about="http://www.cidoc-crm.org/cidoc-crm/E94">
        <rdfs:subClassOf rdf:resource="http://www.cidoc-crm.org/cidoc-crm/E59"/>
        <rdfs:comment rdf:datatype="http://www.w3.org/2001/XMLSchema#string">This property associates an instance of E53 Place with an instance of E94 Space Primitive that defines it. Syntactic variants or use of different scripts may result in multiple instances of E94 Space Primitive defining exactly the same place. Transformations between different reference systems in general result in new definitions of places approximating each other and not in alternative definitions. Note that it is possible for a place to be defined by phenomena causal to it or other forms of identification rather than by an instance of E94 Space Primitive. In this case, this property must not be used for approximating the respective instance of E53 Place with an instance of E94 Space Primitive.</rdfs:comment>
        <rdfs:label xml:lang="en">Space Primitive</rdfs:label>
        <skos:notation rdf:datatype="http://www.w3.org/2001/XMLSchema#string">E94</skos:notation>
    </owl:Class>
    


    <!-- http://www.cidoc-crm.org/cidoc-crm/E97 -->

    <owl:Class rdf:about="http://www.cidoc-crm.org/cidoc-crm/E97">
        <rdfs:subClassOf rdf:resource="http://www.cidoc-crm.org/cidoc-crm/E54"/>
        <rdfs:label xml:lang="en">Monetary Amount</rdfs:label>
    </owl:Class>
    


    <!-- http://www.cidoc-crm.org/cidoc-crm/E98 -->

    <owl:Class rdf:about="http://www.cidoc-crm.org/cidoc-crm/E98">
        <rdfs:subClassOf rdf:resource="http://www.cidoc-crm.org/cidoc-crm/E58"/>
        <rdfs:label xml:lang="en">Currency</rdfs:label>
    </owl:Class>
    


    <!-- https://dataforhistory.org/ontology/maritimehistorycontinued/C1 -->

    <owl:Class rdf:about="https://dataforhistory.org/ontology/maritimehistorycontinued/C1">
        <rdfs:subClassOf rdf:resource="http://dataforhistory.org/histdmi-generic-ongoing/class/C33"/>
        <rdfs:label xml:lang="en">Departing</rdfs:label>
    </owl:Class>
    


    <!-- https://dataforhistory.org/ontology/maritimehistorycontinued/C2 -->

    <owl:Class rdf:about="https://dataforhistory.org/ontology/maritimehistorycontinued/C2">
        <rdfs:subClassOf rdf:resource="http://dataforhistory.org/histdmi-generic-ongoing/class/C33"/>
        <rdfs:label xml:lang="en">Arriving</rdfs:label>
    </owl:Class>
    


    <!-- https://dataforhistory.org/ontology/maritimehistorycontinued/C3 -->

    <owl:Class rdf:about="https://dataforhistory.org/ontology/maritimehistorycontinued/C3">
        <rdfs:subClassOf rdf:resource="http://dataforhistory.org/histdmi-generic-ongoing/class/C4"/>
        <rdfs:label xml:lang="en">Leg</rdfs:label>
    </owl:Class>
    


    <!-- https://dataforhistory.org/ontology/maritimehistorycontinued/C4 -->

    <owl:Class rdf:about="https://dataforhistory.org/ontology/maritimehistorycontinued/C4">
        <rdfs:subClassOf rdf:resource="http://www.cidoc-crm.org/cidoc-crm/E55"/>
        <rdfs:label xml:lang="en">Product Type</rdfs:label>
    </owl:Class>
    


    <!-- https://dataforhistory.org/ontology/maritimehistorycontinued/C5 -->

    <owl:Class rdf:about="https://dataforhistory.org/ontology/maritimehistorycontinued/C5">
        <rdfs:subClassOf rdf:resource="http://dataforhistory.org/histsocial-ongoing/class/C7"/>
        <rdfs:label xml:lang="en">Rank</rdfs:label>
    </owl:Class>
    


    <!-- https://dataforhistory.org/ontology/maritimehistorycontinued/C6 -->

    <owl:Class rdf:about="https://dataforhistory.org/ontology/maritimehistorycontinued/C6">
        <rdfs:subClassOf rdf:resource="http://www.cidoc-crm.org/cidoc-crm/E89"/>
        <rdfs:label xml:lang="en">Occupational Responsibility</rdfs:label>
    </owl:Class>
    


    <!-- 
    ///////////////////////////////////////////////////////////////////////////////////////
    //
    // Annotations
    //
    ///////////////////////////////////////////////////////////////////////////////////////
     -->

    <rdf:Description rdf:about="http://www.cidoc-crm.org/cidoc-crm/P3">
        <skos:notation rdf:datatype="http://www.w3.org/2001/XMLSchema#string">P3</skos:notation>
        <rdfs:label xml:lang="en">has note</rdfs:label>
        <rdfs:comment xml:lang="en">This property is a container for all informal descriptions about an object that have not been expressed in terms of CRM
            constructs. In particular it captures the characterisation of the item itself, its internal structures, appearance etc. Like property P2
            has type (is type of), this property is a consequence of the restricted focus of the CRM. The aim is not to capture, in a structured form,
            everything that can be said about an item; indeed, the CRM formalism is not regarded as sufficient to express everything that can be said.
            Good practice requires use of distinct note fields for different aspects of a characterisation. The P3.1 has type property of P3 has note
            allows differentiation of specific notes, e.g. “construction”, “decoration” etc. An item may have many notes, but a note is attached to a
            specific item. </rdfs:comment>
    </rdf:Description>
</rdf:RDF>



<!-- Generated by the OWL API (version 4.5.9.2019-02-01T07:24:44Z) https://github.com/owlcs/owlapi -->

